@prefix : <https://w3id.org/crmrp#> .
@prefix dc: <http://purl.org/dc/elements/1.1/> .
@prefix dct: <http://purl.org/dc/terms/> .
@prefix owl: <http://www.w3.org/2002/07/owl#> .
@prefix rdf: <http://www.w3.org/1999/02/22-rdf-syntax-ns#> .
@prefix xml: <http://www.w3.org/XML/1998/namespace> .
@prefix xsd: <http://www.w3.org/2001/XMLSchema#> .
@prefix rdfs: <http://www.w3.org/2000/01/rdf-schema#> .
@prefix skos: <http://www.w3.org/2004/02/skos/core#> .
@prefix crmrp: <https://w3id.org/crmrp#> .
@prefix grddl: <http://www.w3.org/2003/g/data-view#> .
@base <https://w3id.org/crmrp> .

<https://w3id.org/crmrp> rdf:type owl:Ontology ;
                          owl:imports <http://www.cidoc-crm.org/cidoc-crm/> ,
                                      <http://www.cidoc-crm.org/extensions/crmsci/>,
 				      <http://www.cidoc-crm.org/extensions/crmdig/> .

#################################################################
#    Annotation properties
#################################################################

###  http://www.cidoc-crm.org/extensions/crmsci/O16_observed_value
<http://www.cidoc-crm.org/extensions/crmsci/O16_observed_value> rdfs:range <http://www.cidoc-crm.org/cidoc-crm/E54_Dimension> ,
                                                                           <http://www.cidoc-crm.org/cidoc-crm/E73_Information_Object> .


###  http://www.w3.org/2004/02/skos/core#altLabel
skos:altLabel rdf:type owl:AnnotationProperty ;
              rdfs:subPropertyOf rdfs:label .


###  http://www.w3.org/2004/02/skos/core#broader
skos:broader rdf:type owl:AnnotationProperty .


###  http://www.w3.org/2004/02/skos/core#closeMatc
skos:closeMatc rdf:type owl:AnnotationProperty .


###  http://www.w3.org/2004/02/skos/core#closeMatch
skos:closeMatch rdf:type owl:AnnotationProperty .


###  http://www.w3.org/2004/02/skos/core#definition
skos:definition rdf:type owl:AnnotationProperty ;
                rdfs:subPropertyOf rdfs:label .


###  http://www.w3.org/2004/02/skos/core#defintion
skos:defintion rdf:type owl:AnnotationProperty .


###  http://www.w3.org/2004/02/skos/core#editorialNote
skos:editorialNote rdf:type owl:AnnotationProperty ;
                   rdfs:subPropertyOf rdfs:label .


###  http://www.w3.org/2004/02/skos/core#exactMatch
skos:exactMatch rdf:type owl:AnnotationProperty .


###  http://www.w3.org/2004/02/skos/core#inScheme
skos:inScheme rdf:type owl:AnnotationProperty .


###  http://www.w3.org/2004/02/skos/core#note
skos:note rdf:type owl:AnnotationProperty .


###  http://www.w3.org/2004/02/skos/core#prefLabel
skos:prefLabel rdf:type owl:AnnotationProperty ;
               rdfs:subPropertyOf rdfs:label .


###  http://www.w3.org/2004/02/skos/core#source
skos:source rdf:type owl:AnnotationProperty .


###  http://www.w3.org/2004/02/skos/core#topConceptOf
skos:topConceptOf rdf:type owl:AnnotationProperty .


#################################################################
#    Object Properties
#################################################################

###  http://www.cidoc-crm.org/cidoc-crm/P108i_was_produced_by
<http://www.cidoc-crm.org/cidoc-crm/P108i_was_produced_by> rdfs:domain crmrp:R1_Restoration_Object;

rdfs:range <http://www.cidoc-crm.org/cidoc-crm/E73_Exectution_Technique> .

###  http://www.cidoc-crm.org/cidoc-crm/P165_incorporates
<http://www.cidoc-crm.org/cidoc-crm/P165_incorporates> rdfs:domain crmrp:R2_Audio_Documentation ,
                                                                   crmrp:R3_Graphic_Documentation ,
                                                                   crmrp:R4_Photographic_Documentation ,
                                                                   crmrp:R5_Source_and_Document ,
                                                                   crmrp:R6_Video_Documentation ;
                                                       rdfs:range <http://www.cidoc-crm.org/cidoc-crm/E73_Information_Object> .


###  http://www.cidoc-crm.org/cidoc-crm/P2_has_type
<http://www.cidoc-crm.org/cidoc-crm/P2_has_type> rdfs:domain <http://www.cidoc-crm.org/cidoc-crm/R13_Execution_Technique> ,                                                     
                                                             <http://www.cidoc-crm.org/extensions/crmsci/S18_Alteration> ,
                                                             crmrp:R10_Sign_of_Workmanship ,
                                                             crmrp:R11_Non-invasive_archaeometric_and_diagnostic_analysis ,
                                                             crmrp:R12_Invasive_archaeometric_and_diagnostic_analysis ,
                                                             crmrp:R1_Restoration_Object ,
                                                             crmrp:R5_Source_and_Document ,
                                                             crmrp:R8_Intervention;
							rdfs:range <http://www.cidoc-crm.org/cidoc-crm/E55_Type>.


###  http://www.cidoc-crm.org/extensions/crmsci/O24i_was_measured_by
<http://www.cidoc-crm.org/cidoc-crm/P39i_was_measured_by> rdfs:domain <http://www.cidoc-crm.org/extensions/crmsci/S18_Alteration> ,
                                                                      crmrp:R1_Restoration_Object ;
                                                          rdfs:range crmrp:R11_Non-invasive_archaeometric_and_diagnostic_analysis ,
                                                                     crmrp:R12_Invasive_archaeometric_and_diagnostic_analysis .


###  http://www.cidoc-crm.org/cidoc-crm/P45_consists_of
<http://www.cidoc-crm.org/cidoc-crm/P45_consists_of> rdfs:domain crmrp:R1_Restoration_Object ;
							rdfs:range <http://www.cidoc-crm.org/cidoc-crm/E57_Material>.


###  http://www.cidoc-crm.org/cidoc-crm/P4_has_time-span
<http://www.cidoc-crm.org/cidoc-crm/P4_has_time-span> rdfs:domain crmrp:R7_Restoration_Project ,
                                                                  crmrp:R8_Intervention ;
							rdfs:range <http://www.cidoc-crm.org/cidoc-crm/E52_Time-Span>.


###  http://www.cidoc-crm.org/cidoc-crm/P56_bears_feature
<http://www.cidoc-crm.org/cidoc-crm/P56_bears_feature> rdfs:domain crmrp:R1_Restoration_Object ;
                                                       rdfs:range crmrp:R10_Sign_of_Workmanship .


###  http://www.cidoc-crm.org/cidoc-crm/P70i_is_documented_in
<http://www.cidoc-crm.org/cidoc-crm/P70i_is_documented_in> rdfs:domain crmrp:R7_Restoration_Project ;
							rdfs:range <http://www.cidoc-crm.org/cidoc-crm/E31_Document>.


###  http://www.cidoc-crm.org/extensions/crmsci/O16_observed_value
<http://www.cidoc-crm.org/extensions/crmsci/O16_observed_value> rdfs:domain crmrp:R11_Non-invasive_archaeometric_and_diagnostic_analysis ,
                                                                            crmrp:R12_Invasive_archaeometric_and_diagnostic_analysis ;
									rdfs:range <http://www.cidoc-crm.org/cidoc-crm/E73_Information_Object>.


###  http://www.cidoc-crm.org/extensions/crmsci/O18i_was_altered_by
<http://www.cidoc-crm.org/extensions/crmsci/O18i_was_altered_by> rdfs:domain crmrp:R1_Restoration_Object ;
							rdfs:range <http://www.cidoc-crm.org/extensions/crmsci/S18_Alteration>.


###  http://www.cidoc-crm.org/extensions/crmsci/O24_measured
<http://www.cidoc-crm.org/extensions/crmsci/O24_measured> rdfs:domain crmrp:R11_Non-invasive_archaeometric_and_diagnostic_analysis,
								crmrp:R12_Invasive_archaeometric_and_diagnostic_analysis;
                                                          rdfs:range <http://www.cidoc-crm.org/extensions/crmsci/S18_Alteration> .


###  https://w3id.org/crmrp#RP1_intervents_on
crmrp:RP1_intervents_on rdf:type owl:ObjectProperty ;
                        owl:inverseOf crmrp:RP1i_needed_intervention ;
                        rdfs:domain crmrp:R7_Restoration_Project ,
                                    crmrp:R8_Intervention ;
                        rdfs:range <http://www.cidoc-crm.org/extensions/crmsci/S18_Alteration> ,
                                   crmrp:R1_Restoration_Object ;
                        rdfs:comment """This property links R1 Restoration Object and R7 Restoration Project
This property RP1 intervents on (needed intervention) allows you to indicate which artwork the restoration project refers to.""" ;
                        rdfs:label "intervents on"@en .


###  https://w3id.org/crmrp#RP1i_needed_intervention
crmrp:RP1i_needed_intervention rdf:type owl:ObjectProperty ;
                               rdfs:domain <http://www.cidoc-crm.org/extensions/crmsci/S18_Alteration> ,
                                           crmrp:R1_Restoration_Object ;
                               rdfs:range crmrp:R7_Restoration_Project ,
                                          crmrp:R8_Intervention ;
                               rdfs:comment """This property links R1 Restoration Object and R7 Restoration Project
This property RP1 intervents on (needed intervention) allows you to indicate which artwork the restoration project refers to.""" ;
                               rdfs:label "needed intervention"@en .


###  https://w3id.org/crmrp#RP2_targets
crmrp:RP2_targets rdf:type owl:ObjectProperty ;
                  rdfs:domain <http://www.cidoc-crm.org/extensions/crmsci/S18_Alteration> ,
                              crmrp:R8_Intervention ;
                  rdfs:range crmrp:R9_Altered_Area ;
                  rdfs:label "targets"@en .


###  https://w3id.org/crmrp#RP3_has_intervention
crmrp:RP3_has_intervention rdf:type owl:ObjectProperty ;
                           rdfs:domain crmrp:R7_Restoration_Project ;
                           rdfs:range crmrp:R8_Intervention ;
                           rdfs:comment """This property links R7 Restoration Project to R8 Intervention.
This property allows you to specify which operations (or interventions) were performed during the restoration.""" ;
                           rdfs:label "has intervention"@en .


###  https://w3id.org/crmrp#RP4_is_pre-restoration
crmrp:RP4_is_pre-restoration rdf:type owl:ObjectProperty ;
                             rdfs:domain crmrp:R11_Non-invasive_archaeometric_and_diagnostic_analysis ,
                                         crmrp:R12_Invasive_archaeometric_and_diagnostic_analysis ;
                             rdfs:range crmrp:R7_Restoration_Project ;
                             rdfs:comment """This property links Invasive archaeometric and diagnostic analysis and Non-invasive achaeometric and diagnostic analysis to Restoration Project.
Indeed, some archaeometric and diagnostic analyses are sometimes repeated before and after the restoration."""@en ;
                             rdfs:label "is pre-restoration"@en .


###  https://w3id.org/crmrp#RP5_is_post-restoration
crmrp:RP5_is_post-restoration rdf:type owl:ObjectProperty ;
                              rdfs:domain crmrp:R11_Non-invasive_archaeometric_and_diagnostic_analysis ,
                                          crmrp:R12_Invasive_archaeometric_and_diagnostic_analysis ;
                              rdfs:range crmrp:R7_Restoration_Project ;
                              rdfs:comment """This property links Invasive archaeometric and diagnostic analysis and Non-invasive achaeometric and diagnostic analysis to Restoration Project.
Indeed, some archaeometric and diagnostic analyses are sometimes repeated before and after the restoration."""@en ;
                              rdfs:label "is post-restoration"@en .


###  https://w3id.org/crmrp#RP6_is_pre-intervention
crmrp:RP6_is_pre-intervention rdf:type owl:ObjectProperty ;
                              rdfs:domain crmrp:R11_Non-invasive_archaeometric_and_diagnostic_analysis ,
                                          crmrp:R12_Invasive_archaeometric_and_diagnostic_analysis ;
                              rdfs:range crmrp:R8_Intervention ;
                              rdfs:comment """This property links Invasive archaeometric and diagnostic analysis and Non-invasive achaeometric and diagnostic analysis to Intervention.
Indeed, some archaeometric and diagnostic analyses are sometimes repeated before and after specific interventions."""@en ;
                              rdfs:label "is pre-intervention"@en .


###  https://w3id.org/crmrp#RP7_is_post-intervention
crmrp:RP7_is_post-intervention rdf:type owl:ObjectProperty ;
                               rdfs:domain crmrp:R11_Non-invasive_archaeometric_and_diagnostic_analysis ,
                                           crmrp:R12_Invasive_archaeometric_and_diagnostic_analysis ;
                               rdfs:range crmrp:R8_Intervention ;
                               rdfs:comment """This property links Invasive archaeometric and diagnostic analysis and Non-invasive achaeometric and diagnostic analysis to Intervention.
Indeed, some archaeometric and diagnostic analyses are sometimes repeated before and after specific interventions."""@en ;
                               rdfs:label "is post-intervention"@en .


#################################################################
#    Classes
#################################################################

###  http://www.w3.org/2004/02/skos/core#Concept
skos:Concept rdf:type owl:Class .


###  http://www.w3.org/2004/02/skos/core#ConceptScheme
skos:ConceptScheme rdf:type owl:Class .


###  https://w3id.org/crmrp#R10_Sign_of_Workmanship
crmrp:R10_Sign_of_Workmanship rdf:type owl:Class ;
                              rdfs:subClassOf <http://www.cidoc-crm.org/cidoc-crm/E25_Human-Made_Feature> ;
                              rdfs:comment """This class describe the signs of workmanship visible on an artwork.
These may be grooves left on the surface by tools or marks indicative of the execution technique used by the artist."""@en ;
                              rdfs:label "Sign of Workmanship"@en .


###  https://w3id.org/crmrp#R11_Non-invasive_archaeometric_and_diagnostic_analysis
crmrp:R11_Non-invasive_archaeometric_and_diagnostic_analysis rdf:type owl:Class ;
                                                             rdfs:subClassOf <http://www.cidoc-crm.org/extensions/crmsci/S21_Measurement>  ;
                                                             rdfs:comment """This class describe the non-invasive archaeometric and diagnostic analysis.
Non-invasive investigations are those that do not require a sample to be taken from the artwork."""@en ;
                                                             rdfs:label "Non-invasive archaeometric and diagnostic analysis"@en .


###  https://w3id.org/crmrp#R12_Invasive_archaeometric_and_diagnostic_analysis
crmrp:R12_Invasive_archaeometric_and_diagnostic_analysis rdf:type owl:Class ;
                                                         rdfs:subClassOf <http://www.cidoc-crm.org/extensions/crmsci/S3_Measurement_by_Sampling>;
                                                         rdfs:comment """This class describes the invasive investigations.
To get very specific results, it is sometimes necessary to choose invasive invesstigations."""@en ;
                                                         rdfs:label "Invasive archaeometric and diagnostic analysis"@en .


###  https://w3id.org/crmrp#R13_Execution_Technique
crmrp:R13_Execution_Technique rdf:type owl:Class ;
                              rdfs:subClassOf <http://www.cidoc-crm.org/cidoc-crm/E12_Production> ;
                              rdfs:comment "The purpose of this class is to indicate the execution techniques used in the creation of a work of art."@en ;
                              rdfs:label "Execution Technique" .


###  https://w3id.org/crmrp#R1_Restoration_Object
crmrp:R1_Restoration_Object rdf:type owl:Class ;
                            rdfs:subClassOf <http://www.cidoc-crm.org/cidoc-crm/E22_Human-Made_Object> ;
                            rdfs:comment """This class is the core concept of the schema and denotes the artefact to be (or that has been) restored. 
As C. Brandi states in Theory of Restoration: \"restoration constitutes the methodological moment of recognition of an artwork\". This implies that an artefact must first be recognised as an object of cultural interest to be passed on to the future in order to be considered restorable. Hence, a \"Restoration object\" is a \"Cultural Object\", and as such, it has been catalogued, and its catalogue sheet provides all the principal historical and artistic information. This is also the case for composite artworks and for their individual components, such as a painted panel of a polyptych, or a painting that is part of a cycle."""@en ;
                            rdfs:label "Restoration Object"@en .


###  https://w3id.org/crmrp#R2_Audio_Documentation
crmrp:R2_Audio_Documentation rdf:type owl:Class ;
                             rdfs:subClassOf <http://www.cidoc-crm.org/cidoc-crm/E31_Document> ;
                             rdfs:comment """This class represents the audio documentation of an object.
In the case of contemporary art, it is possible to find a few recorded interviews of the artist and to understand the execution techniques or the artist's idea about the restoration of their works.
Furthermore, it might be possible to rediscover the sound of an ancient instrument that is currently too fragile to be played."""@en ;
                             rdfs:label "Audio Documentation"@en .


###  https://w3id.org/crmrp#R3_Graphic_Documentation
crmrp:R3_Graphic_Documentation rdf:type owl:Class ;
                               rdfs:subClassOf <http://www.cidoc-crm.org/cidoc-crm/E31_Document> ;
                               rdfs:comment """This class represents the graphic or cartographic documentation of an object.
Before and during restoration work, it is necessary to produce graphical representations of the conservation state of the artifact before the restoration, showing all alterations and their extent, as well as illustrating the interventions carried out and their area. This can help clients to understand the restoration and restorers to calculate the value of their work."""@en ;
                               rdfs:label "Graphic Documentation"@en .


###  https://w3id.org/crmrp#R4_Photographic_Documentation
crmrp:R4_Photographic_Documentation rdf:type owl:Class ;
                                    rdfs:subClassOf <http://www.cidoc-crm.org/cidoc-crm/E31_Document> ;
                                    rdfs:comment """This class represents the photographic documentation of an object.
Before and during restoration work, it is necessary to know more about the history of artefacts, so sometimes a few photos from the past can help restorers better understand the artworks and how they looked in the past."""@en ;
                                    rdfs:label "Photographic Documentation"@en .


###  https://w3id.org/crmrp#R5_Source_and_Document
crmrp:R5_Source_and_Document rdf:type owl:Class ;
                             rdfs:subClassOf <http://www.cidoc-crm.org/cidoc-crm/E31_Document> ;
                             rdfs:comment """This class represents source and document related to an object.
Every restoration is accompanied by a huge amount of documents, such as projects or reports. Most of these are required by the Superintendencies to evaluate if the restoration works has been carried out with the respect for the artifacts and their history.
These documents can also help future restorers to know how restorations were carried out in the past or to understand how to operate on artworks with similar characteristics (such as materials or execution techniques)."""@en ;
                             rdfs:label "Source and Document"@en .


###  https://w3id.org/crmrp#R6_Video_Documentation
crmrp:R6_Video_Documentation rdf:type owl:Class ;
                             rdfs:subClassOf <http://www.cidoc-crm.org/cidoc-crm/E31_Document> ;
                             rdfs:comment """This class represents the video documentation of an object.
In particular, in the case of contemporary art, it is possible to find a few recorded interviews of the artist and to understand the execution techniques or the artist's idea about the restoration of their works."""@en ;
                             rdfs:label "Video Documentation"@en .


###  https://w3id.org/crmrp#R7_Restoration_Project
crmrp:R7_Restoration_Project rdf:type owl:Class ;
                             rdfs:subClassOf <http://www.cidoc-crm.org/cidoc-crm/E5_Event> ;
                             rdfs:comment """This class is about the overall view of a restoration project.
It refers to the entire restoration process, including the various operations that have taken place in an artwork. The purpose of this class is not only to group a series of operations, but also to be able to indicate the time frame required to complete each operation and the entire restoration site."""@en ;
                             rdfs:label "Restoration Project"@en .


###  https://w3id.org/crmrp#R8_Intervention
crmrp:R8_Intervention rdf:type owl:Class ;
                      rdfs:subClassOf <http://www.cidoc-crm.org/cidoc-crm/E7_Activity> ;
                      rdfs:comment """This class indicates the individual intervention of restoration."""@en ;
                      rdfs:label "Intervention"@en .


###  https://w3id.org/crmrp#R9_Altered_Area
crmrp:R9_Altered_Area rdf:type owl:Class ;
                      rdfs:subClassOf <http://www.cidoc-crm.org/extensions/crmdig/D35_Area> ;
                      rdfs:comment """This class indicates the area altered by an alteration event or an intervention.
It is useful to know where an alteration form is found on an artwork because this fact can help restorers to understand the cause of the alteration or the way to resolve it and, moreover, to prevent it in the future."""@en ;
                      rdfs:label "Altered Area"@en .


#################################################################
#    Individuals
#################################################################

###  https://w3id.org/crmrp#Alteration
crmrp:Alteration rdf:type owl:NamedIndividual ,
                                  skos:ConceptScheme ;
 			skos:definition "Change in condition, beneficial or not, intentional or not."@en ;
                         skos:note "Uni Cen/Ts 17135:2021 - Conservation of cultural heritage. General terms and definitions"@en ;
                         skos:prefLabel "Alteration"@en , "Alterazione"@it ;
 			skos:altLabel "Conservation state"@en, "Stato di conservazione"@it .




###  https://w3id.org/crmrp#Restoration_Object
crmrp:Restoration_Object rdf:type owl:NamedIndividual ,
                               skos:ConceptScheme ;
                         skos:note "International references could not be found"@en ;
                         skos:prefLabel "Restoration object"@en , "Bene (culturale)"@it .


###  https://w3id.org/crmrp#Documentation
crmrp:Documentation rdf:type owl:NamedIndividual ,
                             skos:ConceptScheme ;
                    skos:definition "Set of information recorded, created, collected, stored and updated for the purpose of facilitating present and future preservation. Is as reference material. Examples: X-rays, drawings, photographs, written reports, digital files, photogrammetry, laser scans, etc."@en ;
                    skos:editorialNote "Uni En 15898:2019 Conservazione del patrimonio culturale - Termini generali e definizioni"@en ;
                    skos:note "International references could not be found"@en ;
                    skos:prefLabel "Documentation"@en , "Documentazione"@it .


###  https://w3id.org/crmrp#Material
crmrp:Material rdf:type owl:NamedIndividual ,
                        skos:ConceptScheme ;
               skos:note "International references could not be found"@en ;
               skos:prefLabel "Material"@en , "Materia"@it .


###  https://w3id.org/crmrp#Intervention
crmrp:Intervention rdf:type owl:NamedIndividual , 
                           skos:ConceptScheme ;
                  skos:definition "Actions performed on an object under stable or stabilised conditions, aimed at improving its appreciation, understanding and/or enjoyment, respecting and/or highlighting its cultural relevance, materials and techniques used."@en ;
                  skos:editorialNote "Uni En 15898:2019 Conservazione del patrimonio culturale - Termini generali e definizioni"@en ;
                  skos:note "International references could not be found"@en ;
 		skos:prefLabel "Intervention"@en, "Intervento"@it ;
                  skos:altLabel "Restoration"@en , "Restauro"@it .

 
 

###  https://w3id.org/crmrp#Execution_Technique
crmrp:Execution_Technique rdf:type owl:NamedIndividual ,                
                         skos:ConceptScheme ;
                skos:prefLabel "Execution Technique"@en , "Tecnica esecutiva"@it .


###  https://w3id.org/crmrp#Archeometric_and_Diagnostic_Analysis
crmrp:Archeometric_and_Diagnostic_Analysis 
                 rdf:type owl:NamedIndividual ,                
                         skos:ConceptScheme; 
                 skos:note "International references could not be found"@en ;
                skos:prefLabel "Archaeometric and diagnostic analysis"@en , "Indagine archeometrica e diagnostica"@it .


###  https://w3id.org/crmrp#c_00213896
crmrp:c_00213896 rdf:type owl:NamedIndividual ,
                          skos:Concept ;
                 rdfs:label "Satin finishing"@en ;
                 skos:broader :c_757ed6ec ;
                 skos:definition "The final appearance is half-veined and can be achieved by passing the agate stone over the bolus before the leaf is applied."@en ;
                 skos:editorialNote "G. Pignolo, “Effetti d’oro - Storia e tecnica della doratura nell’arte”, Editrice Compositori, Bologna, 2002"@it ;
			     skos:inScheme :Execution_Technique;
                 skos:topConceptOf :Execution_Technique ;
                 skos:note "International references could not be found"@en ;
                 skos:prefLabel "Satin finishing"@en , "Satinatura"@it .


###  https://w3id.org/crmrp#c_003d58ac
crmrp:c_003d58ac rdf:type owl:NamedIndividual ,
                          skos:Concept ;
                 rdfs:label "Secco"@en ;
                 skos:altLabel "Fresco secco"@en ;
                 skos:broader :c_6626f18c ;
                 skos:closeMatch <http://vocab.getty.edu/page/aat/300053374> ;
                 skos:definition "A wall painting technique where pigments mixed with an organic binder and /or lime are applied onto a dry plaster."@en ;
                 skos:editorialNote "A. Weyer et al., “EwaGlos - European Illustrated Glossary of conservation terms for wall paintings and architectural surfaces”, Michael Imhof Verlag, Petersberg, Germany"@en ,
                                    "Getty AAT http://vocab.getty.edu/page/aat/300053374"@en ;
                 skos:inScheme :Execution_Technique ;
skos:topConceptOf :Execution_Technique ;
                 skos:note "The preferred editorial note and the definition closest to the meaning is EwaGlos - European Illustrated Glossary of conservation terms for wall paintings and architectural surfaces"@en ;
                 skos:prefLabel "Secco"@en , "A secco"@it .


###  https://w3id.org/crmrp#c_00c8100f
crmrp:c_00c8100f rdf:type owl:NamedIndividual ,
                          skos:Concept ;
                 rdfs:label "Crust"@en ;
                 skos:closeMatch <http://vocab.getty.edu/page/aat/300220976> ;
                 skos:definition "Distinct outer layer more or less adherent to the surface of an object"@en ;
                 skos:editorialNote "Getty AAT http://vocab.getty.edu/page/aat/300220976"@en ,
                                    "Uni Cen/Ts 17135:2021 - Conservation of cultural heritage. General terms and definitions"@en ,
                                    "Verg`es-Belmin et al., ICOMOS-ISCS: Illustrated glossary on stone deterioration patterns, vol. XV. Icomos International Council on Monuments and Sites, 2008"@en ;
                 skos:note "The preferred editorial note and the definition closest to the meaning is Uni Cen/Ts 17135:2021"@en ;
				 skos:prefLabel "Crust"@en , "Crosta"@it ;
				 skos:inScheme :Alteration ;
                 skos:topConceptOf :Alteration .


###  https://w3id.org/crmrp#c_0143a1d7
crmrp:c_0143a1d7 rdf:type owl:NamedIndividual ,
                          skos:Concept ;
                 rdfs:label "Hairline crack"@en ;
                 skos:broader :c_8c762c3e ;
                 skos:definition "Depending on the shape, size and number of cracks a specific term as hairline crack"@en ;
                 skos:editorialNote "Uni Cen/Ts 17135:2021 - Conservation of cultural heritage. General terms and definitions"@en ;
                 skos:inScheme :Alteration ;
skos:topConceptOf :Alteration ;
                 skos:prefLabel "Hairline crack"@en , "Cavillatura"@it .


###  https://w3id.org/crmrp#c_0146af00
crmrp:c_0146af00 rdf:type owl:NamedIndividual ,
                          skos:Concept ;
                 rdfs:label "Tempera"@en ;
                 skos:broader :c_051209b3 ;
                 skos:definition "Paint formed of an emulsion of fatty and watery constituents. The standard emulsion is usually created with egg yolk and water, with variants of man-made emulsions created with whole egg, linseed oil, casein glue, gum, or wax."@en ;
                 skos:editorialNote "Getty AAT http://vocab.getty.edu/page/aat/300015062"@en ;
                 skos:exactMatch <http://vocab.getty.edu/page/aat/300015062> ;
                 skos:inScheme :Execution_Technique ;
skos:topConceptOf :Execution_Technique ;
                 skos:prefLabel "Tempera"@en, "Tempera"@it .


###  https://w3id.org/crmrp#c_01bba8b4
crmrp:c_01bba8b4 rdf:type owl:NamedIndividual ,
                          skos:Concept ;
                 rdfs:label "Opus vermiculatum"@en ;
                 skos:broader :c_b9a6a1c8 ;
                 skos:definition "Type of opus tessellatum made of tesserae of very small dimensions (generally less than 4 mm wide). A small mosaic panel (usually less than a square meter) made in opus vermiculatum and inserted in a mosaic pavement (or sometimes on a vertical surface) is called an emblema. It is generally made separately on a stone slab or large ceramic tile in a workshop prior to the making of the mosaic into which it is inserted. This type of mosaic was also made as a portable work of art, independent from any building."@en ;
                 skos:editorialNote "C. Fiori “Teoria e tecniche per la conservazione del mosaico”, Il Prato, Padova, 2002"@en ,
                                    "Getty Conservation Institute “Illustrated Glossary - Technician Training for the Maintenance of In Situ Mosaics”, Los Angeles, 2013"@en ;
                 skos:inScheme :Execution_Technique ;
skos:topConceptOf :Execution_Technique ;
                 skos:prefLabel "Opus vermiculatum"@en , "Opus vermiculatum"@it .


###  https://w3id.org/crmrp#c_01fedc05
crmrp:c_01fedc05 rdf:type owl:NamedIndividual ,
                          skos:Concept ;
                 rdfs:label "Bronze"@en ;
                 skos:broader :c_6407466f ;
                 skos:definition "Refers to a broad range of alloys of copper, specifically any non-ferrous alloy of copper, tin, and zinc or other trace metals. Bronze was made before 3,000 BCE -- possibly as early as 10,000 BCE, although its common use in tools and decorative items is dated only in later artifacts. The proportions of copper and tin vary widely, from 70 to 95 percent copper in surviving ancient artifacts. Because of the copper base, bronze may be very malleable and easy to work. By the Middle Ages in Europe, it was recognized that using the metals in certain proportions could yield specific properties. Some modern bronzes contain no tin at all, substituting other metals such as aluminum, manganese, and even zinc. Historically, the term was used interchangeably with latten. U.S. standard bronze is composed of 90% copper, 7% tin and 3% zinc. Ancient bronze alloys sometimes contained up to 14% tin. "@en ;
                 skos:editorialNote "Getty AAT http://vocab.getty.edu/page/aat/300010957"@en ;
                 skos:exactMatch <http://vocab.getty.edu/page/aat/300010957> ;
                 skos:inScheme :Material ;
		 skos:topConceptOf :Material ;
                 skos:prefLabel "Bronze"@en , "Bronzo"@it .


###  https://w3id.org/crmrp#c_044b6056
crmrp:c_044b6056 rdf:type owl:NamedIndividual ,
                          skos:Concept ;
                 rdfs:label "Paper technique"@en ;
                 skos:definition "Indicates the differences in types of paper art techniques"@en ;
                 skos:note "International references could not be found"@en ;
                 skos:prefLabel "Paper technique"@en , "Tecnica su carta"@it ;
		 skos:inScheme :Execution_Technique ;
                 skos:topConceptOf :Execution_Technique .


###  https://w3id.org/crmrp#c_051209b3
crmrp:c_051209b3 rdf:type owl:NamedIndividual ,
                          skos:Concept ;
                 rdfs:label "Panel painting technique"@en ;
                 skos:closeMatch <http://vocab.getty.edu/page/aat/300033656> ;
                 skos:definition "Refers to paintings on wooden supports, including smaller portable paintings and medium-sized paintings, such as altarpieces, for which several planks of wood were joined to form a larger panel. The term is typically used to refer to paintings on a wooden support in Western art, generally dating from ancient Greece and Rome through the Renaissance, after which time canvas became the standard support for paintings in this size range. Panel paintings are still common today in Greek and Russian Orthodox icons."@en ;
                 skos:editorialNote "Getty AAT http://vocab.getty.edu/page/aat/300033656"@en ;
                 skos:prefLabel "Panel painting technique"@en , "Tecnica su tavola"@it ;
		 skos:inScheme :Execution_Technique ;
                 skos:topConceptOf :Execution_Technique .


###  https://w3id.org/crmrp#c_05163919
crmrp:c_05163919 rdf:type owl:NamedIndividual ,
                          skos:Concept ;
                 rdfs:label "Scientific instruments"@en ;
                 skos:definition "Crafted instruments used for scientific purposes and research, in all branches of science."@en ;
                 skos:editorialNote "Getty AAT http://vocab.getty.edu/page/aat/300122283"@en ;
                 skos:exactMatch <http://vocab.getty.edu/page/aat/300122283> ;
                 skos:prefLabel "Scientific instruments"@en , "Scientifico-tecnologico"@it ;
		 skos:inScheme :Restoration_Object ;
                 skos:topConceptOf :Restoration_Object .


###  https://w3id.org/crmrp#c_05e03365
crmrp:c_05e03365 rdf:type owl:NamedIndividual ,
                          skos:Concept ;
                 rdfs:label "Orthophoto"@en ;
                 skos:broader :c_773e0829 ;
                 skos:definition "Orthophoto is an image obtained after photo-rectification (also known as photogrammetric straightening). It is an image that has undergone treatment, scaled and geometrically, in order to become an orthogonal projection and thus be measurable."@en ;
                 skos:inScheme :Documentation ;
		 skos:topConceptOf :Documentation ;
                 skos:note "International references could not be found"@en ;
                 skos:prefLabel "Orthophoto"@en , "Ortofoto"@it .


###  https://w3id.org/crmrp#c_062492de
crmrp:c_062492de rdf:type owl:NamedIndividual ,
                          skos:Concept ;
                 rdfs:label "Pointillism"@en ;
                 skos:broader :c_326da7e4 ;
                 skos:definition "The colour – and not necessarily the shape – of the damage or lacuna is reconstructed using a dense application of dots (wherever possible in pure colours)."@en ;
                 skos:editorialNote "A. Weyer et al., “EwaGlos - European Illustrated Glossary of conservation terms for wall paintings and architectural surfaces”, Michael Imhof Verlag, Petersberg, Germany"@en ;
                 skos:inScheme :Intervention ;
		 skos:topConceptOf :Intervention ;
                 skos:prefLabel "Pointillism"@en , "Punteggiato"@it .


###  https://w3id.org/crmrp#c_06f56dce
crmrp:c_06f56dce rdf:type owl:NamedIndividual ,
                          skos:Concept ;
                 rdfs:label "Rising damp"@en ;
                 skos:broader :c_61d92422 ;
                 skos:definition "Dampness in the lower part of buildings resulting from capillary rise of ground water."@en ;
                 skos:editorialNote "A. Weyer et al., “EwaGlos - European Illustrated Glossary of conservation terms for wall paintings and architectural surfaces”, Michael Imhof Verlag, Petersberg, Germany"@en ,
                                    "Getty AAT http://vocab.getty.edu/page/aat/30022016"@en ;
                 skos:exactMatch <http://vocab.getty.edu/page/aat/300220162> ;
                 skos:inScheme :Alteration ;
		 skos:topConceptOf :Alteration;
                 skos:note "The preferred editorial note and the definition closest to the meaning is EwaGlos - European Illustrated Glossary of conservation terms for wall paintings and architectural surfaces"@en ;
                 skos:prefLabel "Rising damp"@en , "Risalita"@it .


###  https://w3id.org/crmrp#c_07895c25
crmrp:c_07895c25 rdf:type owl:NamedIndividual ,
                          skos:Concept ;
                 rdfs:label "Engraving"@en ;
                 skos:broader :c_757ed6ec ;
                 skos:closeMatch <http://vocab.getty.edu/page/aat/300053829> ;
                 skos:definition "Creating marks on the surface of a hard material, such as metal or glass, by incising with a sharp tool, when the designs or images created are for their own sake and not to be printed from."@en ;
                 skos:editorialNote "Getty AAT http://vocab.getty.edu/page/aat/300053829"@en ;
                 skos:inScheme :Execution_Technique ;
		 skos:topConceptOf :Execution_Technique ;
                 skos:prefLabel "Engraving"@en , "Bulinatura"@it .


###  https://w3id.org/crmrp#c_07ae8f41
crmrp:c_07ae8f41 rdf:type owl:NamedIndividual ,
                          skos:Concept ;
                 rdfs:label "Mosaics"@en ;
                 skos:definition "Images or patterns composed of small, regularly shaped pieces of durable material, usually stone or colored glass."@en ;
                 skos:editorialNote "Getty AAT http://vocab.getty.edu/page/aat/300015342"@en ;
                 skos:exactMatch <http://vocab.getty.edu/page/aat/300015342> ;
                 skos:prefLabel "Mosaics"@en , "Mosaico"@it ;
		 skos:inScheme :Restoration_Object ;
                 skos:topConceptOf :Restoration_Object .


###  https://w3id.org/crmrp#c_07e518a1
crmrp:c_07e518a1 rdf:type owl:NamedIndividual ,
                          skos:Concept ;
                 rdfs:label "Textile materials"@en ;
                 skos:definition "Materials produced by weaving, felting, knotting, twining, or otherwise processing natural or synthetic fibers so that they cohere into a form or unit; traditionally excludes fiberboard, paper, papier-mâché, and papyrus, which, though also fiber products, are considered as separate types of material."@en ;
                 skos:editorialNote "Getty AAT http://vocab.getty.edu/page/aat/300231565"@en ;
                 skos:exactMatch <http://vocab.getty.edu/page/aat/300231565> ;
                 skos:prefLabel "Textile materials"@en , "Tessile"@it ;
		 skos:inScheme :Material ;
                 skos:topConceptOf :Material .


###  https://w3id.org/crmrp#c_088ec8d4
crmrp:c_088ec8d4 rdf:type owl:NamedIndividual ,
                          skos:Concept ;
                 rdfs:label "Earthenware"@en ;
                 skos:broader :c_bd34e984 ;
                 skos:closeMatch <http://vocab.getty.edu/page/aat/300010662> ;
                 skos:definition "Pottery with a porous body, fired below 1200 degrees Centigrade. It is not vitrified, and must be glazed to render it nonporous"@en ;
                 skos:editorialNote "Getty AAT http://vocab.getty.edu/page/aat/300010662"@en ;
                 skos:inScheme :Material ;
		 skos:topConceptOf :Material ;
                 skos:prefLabel "Earthenware"@en , "Terraglia"@it .


###  https://w3id.org/crmrp#c_0a209790
crmrp:c_0a209790 rdf:type owl:NamedIndividual ,
                          skos:Concept ;
                 rdfs:label "Glass"@en ;
                 skos:definition "An amorphous, inorganic substance made by fusing silica (silicon dioxide) with a basic oxide; generally transparent but often translucent or opaque. Its characteristic properties are its hardness and rigidity at ordinary temperatures, its capacity for plastic working at elevated temperatures, and its resistance to weathering and to most chemicals except hydrofluoric acid. Used for both utilitarian and decorative purposes, it can be formed into various shapes, colored or decorated. Glass originated as a glaze in Mesopotamia in about 3500 BCE and the first objects made wholly of glass date to about 2500 BCE."@en ;
                 skos:editorialNote "Getty AAT http://vocab.getty.edu/page/aat/300010797"@en ;
                 skos:exactMatch <http://vocab.getty.edu/page/aat/300010797> ;
                 skos:prefLabel "Glass"@en , "Vetro"@it ;
		 skos:inScheme :Material ;
                 skos:topConceptOf :Material .


###  https://w3id.org/crmrp#c_0a9f4d42
crmrp:c_0a9f4d42 rdf:type owl:NamedIndividual ,
                          skos:Concept ;
                 rdfs:label "Founding"@en ;
                 skos:closeMatch <http://vocab.getty.edu/page/aat/300054038> ;
                 skos:definition "Process of melting and pouring materials, such as metal or glass, into a mold; for glass also includes fusing."@en ;
                 skos:editorialNote "A.Giuffredi “Formatura e fonderia”, Alinea editrice, Firenze, 2010"@it ,
                                    "Getty AAT http://vocab.getty.edu/page/aat/300054038"@en ;
                 skos:prefLabel "Founding"@en , "Tecnica di fonderia"@it ;
		 skos:inScheme :Execution_Technique ;
                 skos:topConceptOf :Execution_Technique .


###  https://w3id.org/crmrp#c_0b943779
crmrp:c_0b943779 rdf:type owl:NamedIndividual ,
                          skos:Concept ;
                 rdfs:label "Opus spicatum"@en ;
                 skos:broader :c_b9a6a1c8 ;
                 skos:definition "Pavement made of ceramic elements, usually of the same size and rectangular shape, arranged in a herringbone pattern."@en ;
                 skos:editorialNote "Getty Conservation Institute “Illustrated Glossary - Technician Training for the Maintenance of In Situ Mosaics”, Los Angeles, 2013"@en ;
                 skos:inScheme :Execution_Technique ;
		 skos:topConceptOf :Execution_Technique ;
                 skos:prefLabel "Opus spicatum"@en , "Opus spicatum"@it .


###  https://w3id.org/crmrp#c_0be4284c
crmrp:c_0be4284c rdf:type owl:NamedIndividual ,
                          skos:Concept ;
                 rdfs:label "Yellowed"@en ;
                 skos:broader :c_df05cb61 ;
                 skos:editorialNote "A. Weyer et al., “EwaGlos - European Illustrated Glossary of conservation terms for wall paintings and architectural surfaces”, Michael Imhof Verlag, Petersberg, Germany"@en ,
                                    "Uni Cen/Ts 17135:2021 - Conservation of cultural heritage. General terms and definitions"@en ;
                 skos:inScheme :Alteration ;
		 skos:topConceptOf :Alteration ;
                 skos:note "The preferred editorial note and the definition closest to the meaning is Uni Cen/Ts 17135:2021"@en ;
                 skos:prefLabel "Yellowed"@en , "Ingiallimento"@it .


###  https://w3id.org/crmrp#c_0ca4ad6d
crmrp:c_0ca4ad6d rdf:type owl:NamedIndividual ,
                          skos:Concept ;
                 rdfs:label "Paper"@en ;
                 skos:definition "Refers generally to all types of thin matted or felted sheets or webs of fiber formed and dried on a fine screen from a pulpy water suspension. The fibers may be animal, such as hair, silk or wool, or mineral, such as asbestos, or synthetic. However most paper is made from cellulosic plant fiber, such as from wood pulp, grass, cotton, linen, and straw."@en ;
                 skos:editorialNote "Getty AAT http://vocab.getty.edu/page/aat/300014109"@en ;
                 skos:exactMatch <http://vocab.getty.edu/page/aat/300014109> ;
                 skos:prefLabel "Paper"@en , "Carta"@it ;
		 skos:inScheme :Material ;
                 skos:topConceptOf :Material .


###  https://w3id.org/crmrp#c_0ddda1a6
crmrp:c_0ddda1a6 rdf:type owl:NamedIndividual ,
                          skos:Concept ;
                 rdfs:label "Mezzo fresco"@en ;
                 skos:broader :c_6626f18c ;
                 skos:definition "Technique where the painting is executed on a lime plaster surface which is in a state of advanced carbonation."@en ;
                 skos:editorialNote "A. Weyer et al., “EwaGlos - European Illustrated Glossary of conservation terms for wall paintings and architectural surfaces”, Michael Imhof Verlag, Petersberg, Germany"@en ,
                                    "Getty AAT http://vocab.getty.edu/page/aat/300053364"@en ;
                 skos:exactMatch <http://vocab.getty.edu/page/aat/300053364> ;
                 skos:inScheme :Execution_Technique ;
		 skos:topConceptOf :Execution_Technique ;
                 skos:note "The preferred editorial note and the most complete definition is in EwaGlos - European Illustrated Glossary of conservation terms for wall paintings and architectural surfaces"@en ;
                 skos:prefLabel "Mezzo fresco"@en , "Mezzo fresco"@it .


###  https://w3id.org/crmrp#c_0e594482
crmrp:c_0e594482 rdf:type owl:NamedIndividual ,
                          skos:Concept ;
                 rdfs:label "Electrochemical analysis"@en ;
                 skos:broader :c_abed88a5 ;
                 skos:definition "Electrochemical analysis is based on the use of conductive probes or electrodes connected to electronic devices capable of measuring the electrical parameters generated by the oxidation-reduction reaction of species in solution."@en ;
                 skos:inScheme :Archeometric_and_Diagnostic_Analysis ;
		 skos:topConceptOf :Archeometric_and_Diagnostic_Analysis ;
                 skos:prefLabel "Electrochemical analysis"@en , "Analisi elettrochimica"@it .


###  https://w3id.org/crmrp#c_0f7eacd7
crmrp:c_0f7eacd7 rdf:type owl:NamedIndividual ,
                          skos:Concept ;
                 rdfs:label "Reintegration"@en ;
                 skos:definition "Restoration action consisting in the addition of material for the reconstruction of appearance (e.g. pictorial retouching, insertion, repainting, filling, etc.)"@en ;
                 skos:editorialNote "A. Weyer et al., “EwaGlos - European Illustrated Glossary of conservation terms for wall paintings and architectural surfaces”, Michael Imhof Verlag, Petersberg, Germany"@en ,
                                    "Uni En 15898:2019 Conservazione del patrimonio culturale - Termini generali e definizioni"@it ;
                 skos:note "The preferred editorial note and the definition closest to the meaning is Uni En 15898:2019"@en ;
                 skos:prefLabel "Reintegration"@en , "Reintegrazione"@it ;
		 skos:inScheme :Intervention ;
                 skos:topConceptOf :Intervention .


###  https://w3id.org/crmrp#c_0f7fe37e
crmrp:c_0f7fe37e rdf:type owl:NamedIndividual ,
                          skos:Concept ;
                 rdfs:label "Mass Spectrometry Matrix-Assisted Laser Desorption/Ionization (MALDI-MS)"@en ;
                 skos:broader :c_789c3e32 ;
                 skos:definition "Method of ionizing samples for use in mass spectrometry allowing the analysis of fragile biomolecules and organic molecules which fragment when ionized by other methods. The analyte is prepared in or on an organic matrix that is coated on a surface which is then irradiated by laser photons, removing the analyte from the surface and ionizing it for analysis."@en ;
                 skos:editorialNote "Getty AAT http://vocab.getty.edu/page/aat/300390518"@en ;
                 skos:exactMatch <http://vocab.getty.edu/page/aat/300390518> ;
                 skos:inScheme :Archeometric_and_Diagnostic_Analysis ;
		 skos:topConceptOf :Archeometric_and_Diagnostic_Analysis ;
                 skos:prefLabel "Mass Spectrometry Matrix-Assisted Laser Desorption/Ionization (MALDI-MS)"@en , "Spettrometria di massa  Matrix-Assisted Laser Desorption/Ionization (MALDI-MS)"@it .


###  https://w3id.org/crmrp#c_101f9b20
crmrp:c_101f9b20 rdf:type owl:NamedIndividual ,
                          skos:Concept ;
                 rdfs:label "Arching"@en ;
                 skos:broader :c_13f3ce9e ;
                 skos:definition "Deformation of sawn wood. In panel paintings, it causes movement or disruption in the overlying imprimitura and colour."@en ;
                 skos:editorialNote "C. Giannini, “Dizionario del restauro - Tecniche diagnostica conservazione”, Nardini Editore, Firenze, 2010"@en ;
                 skos:inScheme :Alteration ;
		 skos:topConceptOf :Alteration ;
                 skos:note "International references could not be found"@en ;
                 skos:prefLabel "Arching"@en , "Arcuatura"@it .


###  https://w3id.org/crmrp#c_11153277
crmrp:c_11153277 rdf:type owl:NamedIndividual ,
                          skos:Concept ;
                 rdfs:label "Infrared thermography"@en ;
                 skos:broader :c_1fd6102e ;
                 skos:closeMatch <http://vocab.getty.edu/page/aat/300379531> ;
                 skos:definition "A technique that measures variations in temperature of an area, object, or organism by creating infrared images (thermograms) to detect discontinuities such as voids in solid structures, deteriorations in frescoes, biotic infestations of a surface, or tumors in human tissue."@en ;
                 skos:editorialNote "Getty AAT http://vocab.getty.edu/page/aat/300379531"@en ;
                 skos:inScheme :Archeometric_and_Diagnostic_Analysis ;
		 skos:topConceptOf :Archeometric_and_Diagnostic_Analysis ;
                 skos:prefLabel "Infrared thermography"@en , "Termografia"@it .


###  https://w3id.org/crmrp#c_11b3f32e
crmrp:c_11b3f32e rdf:type owl:NamedIndividual ,
                          skos:Concept ;
                 rdfs:label "Bowing"@en ;
                 skos:broader :c_13f3ce9e ;
                 skos:closeMatch <http://vocab.getty.edu/page/aat/300389996> ;
                 skos:definition "A type of warping usually associated with wood when one face of a length of lumber shrinks more than the other, resulting in a bowed curvature. Less commonly this process may occur in stone such as marble, due to residual stresses, anisotropic thermal expansion of calcitic grains, variation of fluid contents, and dissolution processes."@en ;
                 skos:editorialNote "Getty AAT http://vocab.getty.edu/page/aat/300389996"@en ;
                 skos:inScheme :Alteration ;
 		 skos:topConceptOf :Alteration ;
                 skos:prefLabel "Bowing"@en , "Imbarcamento"@it .


###  https://w3id.org/crmrp#c_1283fc77
crmrp:c_1283fc77 rdf:type owl:NamedIndividual ,
                          skos:Concept ;
                 rdfs:label "Sculpture technique"@en ;
                 skos:closeMatch <http://vocab.getty.edu/page/aat/300053618> ;
                 skos:definition "Describes techniques for creating three-dimensional objects with malleable or hard materials, such as clay, wood, stone, bronze, ivory, and found objects."@en ;
                 skos:editorialNote "Getty AAt http://vocab.getty.edu/page/aat/300053618"@en ;
                 skos:prefLabel "Sculpture technique"@en , "Tecnica del marmo e delle pietre dure"@it ;
		 skos:inScheme :Execution_Technique ;
                 skos:topConceptOf :Execution_Technique .


###  https://w3id.org/crmrp#c_1285fa71
crmrp:c_1285fa71 rdf:type owl:NamedIndividual ,
                          skos:Concept ;
                 rdfs:label "Reflectography"@en ;
                 skos:broader :c_1fd6102e ;
                 skos:definition "It is a non-invasive technique that does not damage the works and allows the underlying layers of paintings on canvas, panel or paper to be revealed"@en ;
                 skos:editorialNote "C. Giannini, “Dizionario del restauro - Tecniche diagnostica conservazione”, Nardini Editore, Firenze, 2010"@it ;
                 skos:inScheme :Archeometric_and_Diagnostic_Analysis ;
		 skos:topConceptOf :Archeometric_and_Diagnostic_Analysis ;
                 skos:note "International references could not be found"@en ;
                 skos:prefLabel "Reflectography"@en , "Riflettografia"@it .


###  https://w3id.org/crmrp#c_1381790a
crmrp:c_1381790a rdf:type owl:NamedIndividual ,
                          skos:Concept ;
                 rdfs:label "Faience"@en ;
                 skos:broader :c_bd34e984 ;
                 skos:closeMatch <http://vocab.getty.edu/page/aat/30026518> ;
                 skos:definition "A composite material consisting of a body of sintered quartz coupled with an alkaline glaze surface, and used for decorating beads, amulets, figurines, and other small objects. It was invented in Mesopotamia or Iran ca. 4500 BCE, and produced through the mid-7th century CE."@en ;
                 skos:editorialNote "Getty AAT http://vocab.getty.edu/page/aat/300265183"@en ;
                 skos:inScheme :Material ;
				 skos:topConceptOf :Material ;
                 skos:prefLabel "Faience"@en , "Faience"@it .


###  https://w3id.org/crmrp#c_13f3ce9e
crmrp:c_13f3ce9e rdf:type owl:NamedIndividual ,
                          skos:Concept ;
                 rdfs:label "Deformation"@en ;
                 skos:definition "Change, without a break, of the form and/or dimensions of an object"@en ;
                 skos:editorialNote "A. Weyer et al., “EwaGlos - European Illustrated Glossary of conservation terms for wall paintings and architectural surfaces”, Michael Imhof Verlag, Petersberg, Germany"@en ,
                                    "Getty AAT http://vocab.getty.edu/page/aat/300072976"@en ,
                                    "Uni Cen/Ts 17135:2021 - Conservation of cultural heritage. General terms and definitions"@en ;
                 skos:exactMatch <http://vocab.getty.edu/page/aat/300072976> ;
                 skos:note "The preferred editorial note and the definition closest to the meaning is Uni Cen/Ts 17135:2021"@en ;
                 skos:prefLabel "Deformation"@en , "Deformazione"@it ;
		 skos:inScheme :Alteration ;
                 skos:topConceptOf :Alteration .


###  https://w3id.org/crmrp#c_143349b9
crmrp:c_143349b9 rdf:type owl:NamedIndividual ,
                          skos:Concept ;
                 rdfs:label "Canvas painting technique"@en ;
                 skos:definition "Painting for which canvas is the support, typically using canvas stretched over stretcher bars or another secondary support."@en ;
                 skos:editorialNote "Getty AAT http://vocab.getty.edu/page/aat/300410350"@en ;
                 skos:exactMatch <http://vocab.getty.edu/page/aat/300410350> ;
                 skos:prefLabel "Canvas painting technique"@en , "Tecnica dipinto su tela"@it ;
		 skos:inScheme :Execution_Technique ;
                 skos:topConceptOf :Execution_Technique .


###  https://w3id.org/crmrp#c_1440c4b3
crmrp:c_1440c4b3 rdf:type owl:NamedIndividual ,
                          skos:Concept ;
                 rdfs:label "Fixing"@en ;
                 skos:closeMatch <http://vocab.getty.edu/page/aat/300053097> ;
                 skos:definition "Application of an adhesive product able to join together layers of plaster, renders or painting layers and fill voids or gaps in between."@en ;
                 skos:editorialNote "A. Weyer et al., “EwaGlos - European Illustrated Glossary of conservation terms for wall paintings and architectural surfaces”, Michael Imhof Verlag, Petersberg, Germany"@en ,
                                    "Getty AAT http://vocab.getty.edu/page/aat/300053097"@en ,
                                    "etty Conservation Institute “Illustrated Glossary - Definitions of terms used for the graphic documentation of in situ floor mosaics”, “Mosaics In Situ Project”, Los Angeles, 2003"@en ;
                 skos:note "The preferred editorial note and the definition closest to the meaning is A. Weyer et al., “EwaGlos - European Illustrated Glossary of conservation terms for wall paintings and architectural surfaces”, Michael Imhof Verlag, Petersberg, Germany"@en ;
                 skos:prefLabel "Fixing"@en , "Riadesione"@it ;
		 skos:inScheme :Intervention ;
                 skos:topConceptOf :Intervention .


###  https://w3id.org/crmrp#c_150915f4
crmrp:c_150915f4 rdf:type owl:NamedIndividual ,
                          skos:Concept ;
                 rdfs:label "Enzymes"@en ;
                 skos:broader :c_5a83cd16 ;
                 skos:definition "Enzymes make it possible to remove the protein films that often form on the surface of works of art. There are essentially two enzymes used in restoration: proteases and lipases. The former are capable of breaking down protein molecules. Lipases are capable of dissolving fats (or lipids), catalysing the hydrolysis of triglycerides, the basic components of oils (e.g. linseed oil)"@en ;
                 skos:editorialNote "P.Cremonesi, E. Signorini, “Un approccio alla pulitura dei dipinti mobili”, Il Prato, Padova, 2016"@it ;
                 skos:inScheme :Intervention ;
		 skos:TopConceptOf :Intervention ;
                 skos:note "International references could not be found"@en ;
                 skos:prefLabel "Enzymes"@en , "Enzimi"@it .


###  https://w3id.org/crmrp#c_160c713a
crmrp:c_160c713a rdf:type owl:NamedIndividual ,
                          skos:Concept ;
                 rdfs:label "Sculpture"@en ;
                 skos:definition "Three-dimensional works of art in which images and forms are produced in relief, in intaglio, or in the round. The term refers particularly to art works created by carving or engraving a hard material, by molding or casting a malleable material (which usually then hardens), or by assembling parts to create a three-dimensional object. It is typically used to refer to large or medium-sized objects made of stone, wood, bronze, or another metal."@en ;
                 skos:editorialNote "Getty AAT http://vocab.getty.edu/page/aat/300047090"@en ;
                 skos:exactMatch <http://vocab.getty.edu/page/aat/300047090> ;
                 skos:inScheme :Restoration_Object ;
                 skos:prefLabel "Sculpture"@en , "Scultura"@it ;
                 skos:topConceptOf :Restoration_Object .


###  https://w3id.org/crmrp#c_17157ccd
crmrp:c_17157ccd rdf:type owl:NamedIndividual ,
                          skos:Concept ;
                 rdfs:label "Moulding / Casting technique"@en ;
                 skos:closeMatch <http://vocab.getty.edu/page/aat/300053104> , <http://vocab.getty.edu/page/aat/300053134> ;
                 skos:definition "Giving form to something by use of a mold; usually refers to pressing a material into the mold, as distinct from pouring liquid material into the mold, for which prefer casting."@en ,
                                 "The act or process of making casts or of shaping in a mold; usually refers to pouring liquid material into a mold, as distinguished from pressing a material into a mold, for which prefer molding."@en ;
                 skos:editorialNote "A.Giuffredi, “Formatura e fonderia”, Alinea editrice, Firenze, 2010"@it ,
                                    "Getty AAT http://vocab.getty.edu/page/aat/300053104"@en ,
                                    "Getty AAT http://vocab.getty.edu/page/aat/300053134"@en ;
                 skos:inScheme :Execution_Technique ;
                 skos:prefLabel "Moulding / Casting technique"@en , "Tecnica di fonderia"@it ;
                 skos:topConceptOf :Execution_Technique .


###  https://w3id.org/crmrp#c_17ef6a5b
crmrp:c_17ef6a5b rdf:type owl:NamedIndividual ,
                          skos:Concept ;
                 rdfs:label "False-colour infrared photography"@en ;
                 skos:broader :c_1fd6102e ;
                 skos:defintion "Infrared photography technique commonly applied to a variety of techniques including aerial photography and art examination. False color infrared is preferred for vegetative and hydrologic studies. False color infrared film is sensitive to ultraviolet, visible and infrared radiation to approximately 900 nm. When the film is exposed with a yellow filter, the emulsion layers become sensitive to only green, red and infrared wavelengths. Blue radiation is absorbed by the filter; hence, the greater haze penetration ability of infrared film. In art conservation, the resulting false color images can be used as a noninvasive means of identifying the pigments that have been used in a painting or underdrawing."@en ;
                 skos:editorialNote "Getty AAT http://vocab.getty.edu/page/aat/300391245"@en ;
                 skos:exactMatch <http://vocab.getty.edu/page/aat/300391245> ;
                 skos:inScheme :Archeometric_and_Diagnostic_Analysis ;
 		 skos:topConceptOf :Archeometric_and_Diagnostic_Analysis ;
                 skos:prefLabel "False-colour infrared photography"@en , "Falso colore"@it .


###  https://w3id.org/crmrp#c_18db1b80
crmrp:c_18db1b80 rdf:type owl:NamedIndividual ,
                          skos:Concept ;
                 rdfs:label "Selezione cromatica"@en ;
                 skos:broader :c_326da7e4 ;
                 skos:definition "The lacuna is reintegrated with short parallel lines in pure colours on a light background, which follow the shapes and contours of the original alongside them."@en ;
                 skos:editorialNote "A. Weyer et al., “EwaGlos - European Illustrated Glossary of conservation terms for wall paintings and architectural surfaces”, Michael Imhof Verlag, Petersberg, Germany"@en ;
                 skos:inScheme :Intervention ;
		 skos:topConceptOf :Intervention ;
                 skos:prefLabel "Selezione cromatica"@en , "Selezione cromatica"@it .


###  https://w3id.org/crmrp#c_18e54874
crmrp:c_18e54874 rdf:type owl:NamedIndividual ,
                          skos:Concept ;
                 rdfs:label "Mechanical cleaning"@en ;
                 skos:broader :c_830e6744 ;
                 skos:definition "Removal of all surface impurities (dust, insect droppings, micro-organism spores, etc.) using brushes, scalpels. laser and/or soft rubbers, often without the use of water or other solvents. This term comprises the dry cleaning techniques."@en ;
                 skos:editorialNote "G. Botticelli, “Lezioni di restauro - Le pitture murali”, Centro Di Editore, Firenze, 2012"@en ;
                 skos:inScheme :Intervention;
		 skos:topConceptOf :Intervention ;
                 skos:note "International references could not be found"@en ;
                 skos:prefLabel "Mechanical cleaning"@en , "Pulitura meccanica"@it .


###  https://w3id.org/crmrp#c_18fdda7b
crmrp:c_18fdda7b rdf:type owl:NamedIndividual ,
                          skos:Concept ;
                 rdfs:label "Lithography"@en ;
                 skos:broader :c_aee6a805 ;
                 skos:closeMatch <http://vocab.getty.edu/page/aat/300053271> ;
                 skos:definition "Planographic printing process in which a design is deposited on a stone or plate with a greasy substance and the surface is chemically treated to accept ink only in the greasy areas."@en ;
                 skos:editorialNote "Getty AAT http://vocab.getty.edu/page/aat/300053271"@en ;
                 skos:inScheme :Execution_Technique ;
		 skos:topConceptOf :Execution_Technique ;
                 skos:prefLabel "Lithography"@en , "Litografia"@it .


###  https://w3id.org/crmrp#c_1931dc9b
crmrp:c_1931dc9b rdf:type owl:NamedIndividual ,
                          skos:Concept ;
                 rdfs:label "Forma persa"@en ;
                 skos:broader :c_17157ccd ;
                 skos:definition "Plaster mould made on clay, plasticine or wax models that makes it possible to obtain a single plaster model, as for its extraction the form must be destroyed"@en ;
                 skos:editorialNote "P. Clérin, “Manuale di scultura - Tecniche, materiali, realizzazioni”, Sovera editore, Roma, 1995"@it ;
                 skos:inScheme :Execution_Technique ;
		 skos:topConceptOf :Execution_Technique ;
                 skos:note "It was decided not to proceed with the English translation in order to avoid possible lexical errors and misunderstandings."@en ;
                 skos:prefLabel "Forma persa"@en , "Forma persa"@it .


###  https://w3id.org/crmrp#c_19d7c1db
crmrp:c_19d7c1db rdf:type owl:NamedIndividual ,
                          skos:Concept ;
                 rdfs:label "Sgraffito (graffito)"@en ;
                 skos:broader :c_6626f18c ;
                 skos:definition "Multi-layer decoration technique executed by scratching the upper plaster layer to reveal parts of the underlying (e.g. dark plaster) layer."@en ;
                 skos:editorialNote "A. Weyer et al., “EwaGlos - European Illustrated Glossary of conservation terms for wall paintings and architectural surfaces”, Michael Imhof Verlag, Petersberg, Germany"@en ,
                                    "Getty AAT http://vocab.getty.edu/page/aat/300266416"@en ;
                 skos:exactMatch <http://vocab.getty.edu/page/aat/300266416> ;
                 skos:inScheme :Execution_Technique ;
		 skos:topConceptOf :Execution_Technique ;
                 skos:note "The preferred editorial note and the definition closest to the meaning is EwaGlos - European Illustrated Glossary of conservation terms for wall paintings and architectural surfaces"@en ;
                 skos:prefLabel "Sgraffito (graffito)"@en , "Sgraffito (graffito)"@it .


###  https://w3id.org/crmrp#c_1b40d0c6
crmrp:c_1b40d0c6 rdf:type owl:NamedIndividual ,
                          skos:Concept ;
                 rdfs:label "Relief"@en ;
                 skos:broader :c_160c713a ;
                 skos:closeMatch <http://vocab.getty.edu/page/aat/300053622> ;
                 skos:definition "Use to describe a surface that has been carved, molded, or stamped so that an image or design projects from or is sunk into a continuous surface."@en ;
                 skos:editorialNote "Getty AAT http://vocab.getty.edu/page/aat/300053622"@en ;
                 skos:inScheme :Restoration_Object ;
		 skos:topConceptOf :Restoration_Object ;
                 skos:prefLabel "Relief"@en , "Rilievo"@it .


###  https://w3id.org/crmrp#c_1b678edf
crmrp:c_1b678edf rdf:type owl:NamedIndividual ,
                          skos:Concept ;
                 rdfs:label "Erosion"@en ;
                 skos:altLabel "Eroded"@en ;
                 skos:definition "Gradual loss of surface material due to external factors."@en ;
                 skos:editorialNote "Getty AAT http://vocab.getty.edu/page/aat/300054116"@en ,
                                    "Getty Conservation Institute “Illustrated Glossary - Definitions of terms used for the graphic documentation of in situ floor mosaics”, “Mosaics In Situ Project”, Los Angeles, 2003"@en ,
                                    "Uni Cen/Ts 17135:2021 - Conservation of cultural heritage. General terms and definitions"@en ,
                                    "Verg`es-Belmin et al., ICOMOS-ISCS: Illustrated glossary on stone deterioration patterns, vol. XV. Icomos International Council on Monuments and Sites, 2008"@en ;
                 skos:exactMatch <http://vocab.getty.edu/page/aat/300054116> ;
                 skos:inScheme :Alteration ;
                 skos:note "The preferred editorial note and the closest definition to the meaning is Uni Cen/Ts 17135:2021"@en ;
                 skos:prefLabel "Erosion"@en , "Erosione"@it ;
                 skos:topConceptOf :Alteration .


###  https://w3id.org/crmrp#c_1d7e9880
crmrp:c_1d7e9880 rdf:type owl:NamedIndividual ,
                          skos:Concept ;
                 rdfs:label "Alveolisation"@en ;
                 skos:altLabel "Alveolization"@en ;
                 skos:definition "The formation of numerous cavities of various shapes and sizes on stone."@en ;
                 skos:editorialNote "Uni Cen/Ts 17135:2021 - Conservation of cultural heritage. General terms and definitions"@en ,
                                    "Verg`es-Belmin et al., ICOMOS-ISCS: Illustrated glossary on stone deterioration patterns, vol. XV. Icomos International Council on Monuments and Sites, 2008"@en ;
                 skos:inScheme :Alteration ;
                 skos:note "The preferred editorial note and the closest definition to the meaning is Uni Cen/Ts 17135:2021"@en ;
                 skos:prefLabel "Alveolisation"@en , "Alveolizzazione"@it ;
                 skos:topConceptOf :Alteration .


###  https://w3id.org/crmrp#c_1e25ce8c
crmrp:c_1e25ce8c rdf:type owl:NamedIndividual ,
                          skos:Concept ;
                 rdfs:label "Reconstruction"@en ;
                 skos:broader :c_24cc76d5 ;
                 skos:definition "Restoration of an object to an inferred previous form using existing and/or replacement material"@en ;
                 skos:editorialNote "Uni En 15898:2019 Conservazione del patrimonio culturale - Termini generali e definizioni"@it ;
                 skos:inScheme :Intervention ;
		 skos:topConceptOf :Intervention ;
                 skos:prefLabel "Reconstruction"@en , "Ricostruzione"@it .


###  https://w3id.org/crmrp#c_1e84806e
crmrp:c_1e84806e rdf:type owl:NamedIndividual ,
                          skos:Concept ;
                 rdfs:label "Woodworking"@en ;
                 skos:closeMatch <http://vocab.getty.edu/page/aat/300054083> ;
                 skos:definition "Refers broadly to the activity of fashioning in wood. For the art of making fine furniture and intricate woodwork, see cabinetmaking. See the narrower carpentry for constructing buildings and other structures with wood, including the installation of floors, windows, and other trim work."@en ;
                 skos:editorialNote "Getty AAT http://vocab.getty.edu/page/aat/300054083"@en ;
                 skos:inScheme :Execution_Technique ;
                 skos:prefLabel "Woodworking"@en , "Tecnica di lavorazione del legno"@it ;
                 skos:topConceptOf :Execution_Technique .


###  https://w3id.org/crmrp#c_1f7aff6a
crmrp:c_1f7aff6a rdf:type owl:NamedIndividual ,
                          skos:Concept ;
                 rdfs:label "X-ray fluorescence (XRF)"@en ;
                 skos:broader :c_1fd6102e ;
                 skos:definition "XRF is an X-ray emission spectroscopy technique that allows the identification of chemical elements that are present in, or make up, the sample"@en ;
                 skos:editorialNote "C. Giannini, “Dizionario del restauro - Tecniche diagnostica conservazione”, Nardini Editore, Firenze, 2010"@it ,
                                    "M.Ceroni, G.Elia, “Diagnostica per i beni culturali”, Alinea editrice, Firenze, 2008"@it ,
                                    "S. Volpin e L. Appolonia “Le analisi di laboratorio applicate ai beni artistici policromi”, Il Prato, Padova, 1999"@it ;
                 skos:inScheme :Archeometric_and_Diagnostic_Analysis ;
 		 skos:topConceptOf :Archeometric_and_Diagnostic_Analysis ;
                 skos:note "International references could not be found"@en ;
                 skos:prefLabel "X-ray fluorescence (XRF)"@en , "Fluorescenza ai raggi X (XRF)"@it .


###  https://w3id.org/crmrp#c_1fd6102e
crmrp:c_1fd6102e rdf:type owl:NamedIndividual ,
                          skos:Concept ;
                 rdfs:label "Non-invasive investigation"@en ;
                 skos:altLabel "Noninvasive testing"@en ;
                 skos:definition "The gathering of information on site using techniques that do not modify or damage the material at the contact point between the instrument or the beam emitted by the instrument and the object surface."@en ;
                 skos:editorialNote "A. Weyer et al., “EwaGlos - European Illustrated Glossary of conservation terms for wall paintings and architectural surfaces”, Michael Imhof Verlag, Petersberg, Germany"@en ,
                                    "Getty AAT http://vocab.getty.edu/page/aat/300389952"@en ;
                 skos:exactMatch <http://vocab.getty.edu/page/aat/300389952> ;
                 skos:inScheme :Archeometric_and_Diagnostic_Analysis ;
		 skos:topConceptOf :Archeometric_and_Diagnostic_Analysis ;
                 skos:note "The preferred editorial note and the definition closest to the meaning is EwaGlos - European Illustrated Glossary of conservation terms for wall paintings and architectural surfaces"@en ;
                 skos:prefLabel "Non-invasive investigation"@en , "Indagine non invasiva"@it .



###  https://w3id.org/crmrp#c_21ebd5c7
crmrp:c_21ebd5c7 rdf:type owl:NamedIndividual ,
                          skos:Concept ;
                 rdfs:label "Solvent"@en ;
                 skos:broader :c_5a83cd16 ;
                 skos:definition "Any material, usually liquid, having the power of dissolving another material."@en ;
                 skos:editorialNote "Getty AAT http://vocab.getty.edu/page/aat/300015217"@en ;
                 skos:exactMatch <http://vocab.getty.edu/page/aat/300015217> ;
                 skos:inScheme :Intervention ;
		 skos:topConceptOf :Intervention ;
                 skos:prefLabel "Solvent"@en , "Solvente"@it .


###  https://w3id.org/crmrp#c_227577b2
crmrp:c_227577b2 rdf:type owl:NamedIndividual ,
                          skos:Concept ;
                 rdfs:label "Faded"@en ;
                 skos:broader :c_df05cb61 ;
                 skos:closeMatch <http://vocab.getty.edu/page/aat/300053048> ;
                 skos:definition "Exhibiting reduced chroma"@en ;
                 skos:editorialNote "A. Weyer et al., “EwaGlos - European Illustrated Glossary of conservation terms for wall paintings and architectural surfaces”, Michael Imhof Verlag, Petersberg, Germany"@en ,
                                    "Getty AAT http://vocab.getty.edu/page/aat/300053048"@en ,
                                    "Uni Cen/Ts 17135:2021 - Conservation of cultural heritage. General terms and definitions"@en ;
                 skos:inScheme :Alteration ;
 		 skos:topConceptOf :Alteration ;
                 skos:note "The preferred editorial note and the definition closest to the meaning is Uni Cen/Ts 17135:2021"@en ;
                 skos:prefLabel "Faded"@en , "Sbiadimento"@it .


###  https://w3id.org/crmrp#c_2471b55e
crmrp:c_2471b55e rdf:type owl:NamedIndividual ,
                          skos:Concept ;
                 rdfs:label "Thermoluminescence"@en ;
                 skos:broader :c_abed88a5 ;
                 skos:closeMatch <http://vocab.getty.edu/page/aat/300056215> ;
                 skos:definition "The glow or emission of light produced by the application of heat."@en ;
                 skos:editorialNote "Getty ATT http://vocab.getty.edu/page/aat/300056215"@en ;
                 skos:inScheme :Archeometric_and_Diagnostic_Analysis ;
		 skos:topConceptOf :Archeometric_and_Diagnostic_Analysis ;
                 skos:prefLabel "Thermoluminescence"@en , "Termoluminescenza"@it .


###  https://w3id.org/crmrp#c_249b3e7c
crmrp:c_249b3e7c rdf:type owl:NamedIndividual ,
                          skos:Concept ;
                 rdfs:label "Furniture"@en ;
                 skos:broader :Restoration_Object ;
                 skos:definition "Movable or fixed objects or equipment, which may be either functional or ornamental, particularly objects for sitting, reclining, or storage, such as chairs, beds, tables, cabinets, etc., in a dwelling, business, or public space."@en ;
                 skos:editorialNote "Getty AAT http://vocab.getty.edu/page/aat/300037680"@en ;
                 skos:exactMatch <http://vocab.getty.edu/page/aat/300037680> ;
                 skos:inScheme :Restoration_Object ;
 		 skos:topConceptOf :Restoration_Object ;
                 skos:prefLabel "Furniture"@en , "Arredo"@it ;
                 skos:topConceptOf :Restoration_Object .


###  https://w3id.org/crmrp#c_24a7d5f2
crmrp:c_24a7d5f2 rdf:type owl:NamedIndividual ,
                          skos:Concept ;
                 rdfs:label "Gas chromatography (GC)"@en ;
                 skos:broader :c_2d5cde83 ;
                 skos:definition "Chromatography of volatile substances existing in or converted to a vapor state."@en ;
                 skos:editorialNote "Getty AAT http://vocab.getty.edu/page/aat/300223948"@en ;
                 skos:exactMatch <http://vocab.getty.edu/page/aat/300223948> ;
                 skos:inScheme :Archeometric_and_Diagnostic_Analysis ;
		 skos:topConceptOf :Archeometric_and_Diagnostic_Analysis ;
                 skos:prefLabel "Gas chromatography (GC)"@en ,"Gas cromatografia (GC)"@it .


###  https://w3id.org/crmrp#c_24cc76d5
crmrp:c_24cc76d5 rdf:type owl:NamedIndividual ,
                          skos:Concept ;
                 rdfs:label "Materic Integration"@en ;
                 skos:broader :c_0f7eacd7 ;
                 skos:definition "integrative intervention often indispensable to restore legibility to heavily degraded artefacts."@en ;
                 skos:editorialNote "C. Giannini, “Dizionario del restauro - Tecniche diagnostica  conservazione”, Nardini Editore, Firenze, 2010"@it ;
                 skos:inScheme :Intervention ;
		 skos:topConceptOf :Intervention ;
                 skos:prefLabel "Materic Integration"@en , "Reintegrazione materica"@it .


###  https://w3id.org/crmrp#c_251b286b
crmrp:c_251b286b rdf:type owl:NamedIndividual ,
                          skos:Concept ;
                 rdfs:label "Photographic technique"@en ;
                 skos:closeMatch <http://vocab.getty.edu/page/aat/300134334> ;
                 skos:definition "Use with regard to specialized procedures related to how a photograph is taken or composed, or is manipulated during or after processing. Use photographic processes for the procedures by which light-sensitive materials are made to produce an image."@en ;
                 skos:editorialNote "Getty AAT http://vocab.getty.edu/page/aat/300134334"@en ;
                 skos:inScheme :Execution_Technique ;
                 skos:prefLabel "Photographic technique"@en , "Tecnica fotografica"@it ;
                 skos:topConceptOf :Execution_Technique .


###  https://w3id.org/crmrp#c_25bbe064
crmrp:c_25bbe064 rdf:type owl:NamedIndividual ,
                          skos:Concept ;
                 rdfs:label "Determination of water absorption by capillarity"@en ;
                 skos:broader :c_1fd6102e ;
                 skos:definition "Capillary water absorption is the determination of the amount of water absorbed per unit area, as a function of time, at ambient pressure and temperature, by a sample having its base surface in contact with deionised water."@en ;
                 skos:editorialNote "UNI EN 15801:2010 Conservazione dei beni culturali - Metodi di prova - Determinazione dell'assorbimento dell'acqua per capillarità"@it ;
                 skos:inScheme :Archeometric_and_Diagnostic_Analysis ;
		 skos:topConceptOf :Archeometric_and_Diagnostic_Analysis ;
                 skos:note "International references could not be found"@en ;
                 skos:prefLabel "Determination of water absorption by capillarity"@en , "Determinazione dell'assorbimento d'acqua per capillarità"@it .


###  https://w3id.org/crmrp#c_25d4058b
crmrp:c_25d4058b rdf:type owl:NamedIndividual ,
                          skos:Concept ;
                 rdfs:label "Weighting method humidity measurement"@en ;
                 skos:broader :c_abed88a5 ;
                 skos:definition "The weighing method involves taking dust samples from bricks or mortar by drilling, in order to calculate the weight humidity in the wall"@en ;
                 skos:editorialNote "UNI 11085:2003 Beni culturali - Materiali lapidei naturali ed artificiali - Determinazione del contenuto d'acqua: Metodo ponderale"@it ;
                 skos:inScheme :Archeometric_and_Diagnostic_Analysis ;
		 skos:topConceptOf :Archeometric_and_Diagnostic_Analysis ;
                 skos:note "International references could not be found"@en ;
                 skos:prefLabel "Weighting method humidity measurement"@en , "Misura ponderale umidità nelle murature"@it .


###  https://w3id.org/crmrp#c_269dfecc
crmrp:c_269dfecc rdf:type owl:NamedIndividual ,
                          skos:Concept ;
                 rdfs:label "Typography"@en ;
                 skos:broader :c_aee6a805 ;
                 skos:closeMatch <http://vocab.getty.edu/page/aat/300195853> ;
                 skos:definition "Various processes performed with type and typefaces, including setting type and creating layouts with type for printing. For the process of designing type used in the practice of typography, use type design."@en ;
                 skos:editorialNote "Getty AAT http://vocab.getty.edu/page/aat/300195853"@en ;
                 skos:inScheme :Execution_Technique ;
 		 skos:topConceptOf :Execution_Technique ;
                 skos:prefLabel "Typography"@en , "Tipografia"@it .


###  https://w3id.org/crmrp#c_272b9517
crmrp:c_272b9517 rdf:type owl:NamedIndividual ,
                          skos:Concept ;
                 rdfs:label "Sciacquo"@en ;
                 skos:broader :c_17157ccd ;
                 skos:definition "Moulding technique implemented during the 19th century that allows hollow models to be obtained by pouring liquid plaster into the mould in several pours"@en ;
                 skos:editorialNote "A.Giuffredi, “Formatura e fonderia”, Alinea editrice, Firenze, 2010"@it ;
                 skos:inScheme :Execution_Technique ;
		 skos:topConceptOf :Execution_Technique ;
                 skos:note "It was decided not to proceed with the English translation in order to avoid possible lexical errors and misunderstandings."@en ;
                 skos:prefLabel "Sciacquo"@en , "Sciacquo"@it .


###  https://w3id.org/crmrp#c_27b869ee
crmrp:c_27b869ee rdf:type owl:NamedIndividual ,
                          skos:Concept ;
                 rdfs:label "Gold"@en ;
                 skos:broader :c_6407466f ;
                 skos:definition "Pure metallic element having symbol Au and atomic number 79; a soft, inert, shiny reddish yellow metal that is very malleable and ductile. Gold has been highly valued and found in artifacts dating to before 5000 BCE. Native gold, found in quartz veins (vein gold) and alluvial deposits (placer gold), generally contains some silver and copper. Gold is purified by dissolution in mercury or cyanide solutions, by melting, or by electrodeposition. The purity of commercial gold is expressed in karats which is the number of parts of gold in 24 parts of the alloy. Today gold is primarily used for monetary systems and for jewelry."@en ;
                 skos:editorialNote "Getty AAT http://vocab.getty.edu/page/aat/300011021"@en ;
                 skos:exactMatch <http://vocab.getty.edu/page/aat/300011021> ;
                 skos:inScheme :Material ;
		 skos:topConceptOf :Material ;
                 skos:prefLabel "Gold"@en , "Oro"@it .


###  https://w3id.org/crmrp#c_287887a9
crmrp:c_287887a9 rdf:type owl:NamedIndividual ,
                          skos:Concept ;
                 rdfs:label "Mapping"@en ;
                 skos:broader :c_f383c4d3 ;
                 skos:definition "Graphical representation of a single or several patterns on an object."@en ;
                 skos:editorialNote "A. Weyer et al., “EwaGlos - European Illustrated Glossary of conservation terms for wall paintings and architectural surfaces”, Michael Imhof Verlag, Petersberg, Germany"@en ;
                 skos:inScheme :Documentation ;
		 skos:topConceptOf :Documentation ;
                 skos:prefLabel "Mapping"@en , "CAD 2D"@it .


###  https://w3id.org/crmrp#c_2a4faa96
crmrp:c_2a4faa96 rdf:type owl:NamedIndividual ,
                          skos:Concept ;
                 rdfs:label "Opus scutulatum"@en ;
                 skos:broader :c_b9a6a1c8 ;
                 skos:definition "Pavement combining an opus tessellatum background, frequently monochrome, and small stone slabs, often in fragments, generally aligned in rows. The slabs are of different forms, colors, and dimensions."@en ;
                 skos:editorialNote "C. Fiori “Teoria e tecniche per la conservazione del mosaico”, Il Prato, Padova, 2002"@it ,
                                    "Getty Conservation Institute “Illustrated Glossary - Technician Training for the Maintenance of In Situ Mosaics”, Los Angeles, 2013"@en ;
                 skos:inScheme :Execution_Technique ;
		 skos:topConceptOf :Execution_Technique ;
                 skos:prefLabel "Opus scutulatum"@en , "Opus scutulatum"@it .


###  https://w3id.org/crmrp#c_2ce35f2b
crmrp:c_2ce35f2b rdf:type owl:NamedIndividual ,
                          skos:Concept ;
                 rdfs:label "Determination of the static contact angle"@en ;
                 skos:broader :c_1fd6102e ;
                 skos:definition "The contact angle, θ (theta), is a quantitative measure of the wettability of a solid by a liquid"@en ;
                 skos:editorialNote "UNI EN 15802:2010 Conservazione dei beni culturali - Metodi di prova - Determinazione dell'angolo di contatto statico"@it ;
                 skos:inScheme :Archeometric_and_Diagnostic_Analysis ;
		 skos:topConceptOf :Archeometric_and_Diagnostic_Analysis ;
                 skos:note "International references could not be found"@en ;
                 skos:prefLabel "Determination of the static contact angle"@en , "Determinazione dell'angolo di contatto"@it .


###  https://w3id.org/crmrp#c_2d586e2e
crmrp:c_2d586e2e rdf:type owl:NamedIndividual ,
                          skos:Concept ;
                 rdfs:label "Contact sponge"@en ;
                 skos:broader :c_1fd6102e ;
                 skos:definition "The contact sponge method is a test of water absorption by the material under test, which can also be carried out in situ. A sponge of a predetermined type and size is loaded with a quantity of water such that, when kept in contact with constant pressure and for a short time, it does not drip. A circular plastic plate is used to facilitate and maintain adhesion of the sponge to the surface. The amount of water absorbed by the surface is calculated by difference, weighing the sponge before and after application using an analytical balance."@en ;
                 skos:editorialNote "UNI 11432:2011 Beni culturali - Materiali lapidei naturali ed artificiali - Misura della capacità di assorbimento di acqua mediante spugna di contatto"@it ;
                 skos:inScheme :Archeometric_and_Diagnostic_Analysis ;
		 skos:topConceptOf :Archeometric_and_Diagnostic_Analysis ;
                 skos:note "International references could not be found"@en ;
                 skos:prefLabel "Contact sponge"@en , "Misura della capacità di assorbimento di acqua mediante spugna di contatto"@it .


###  https://w3id.org/crmrp#c_2d5cde83
crmrp:c_2d5cde83 rdf:type owl:NamedIndividual ,
                          skos:Concept ;
                 rdfs:label "Chromatography"@en ;
                 skos:broader :c_abed88a5 ;
                 skos:closeMatch <http://vocab.getty.edu/page/aat/300214721> ;
                 skos:definition "The separation of chemical substances by making use of differences in the rates at which the substances travel through or along a stationary medium."@en ;
                 skos:editorialNote "Getty AAT http://vocab.getty.edu/page/aat/300214721"@en ;
                 skos:inScheme :Archeometric_and_Diagnostic_Analysis ;
		 skos:topConceptOf :Archeometric_and_Diagnostic_Analysis ;
		 skos:prefLabel "Chromatography"@en , "Cromatografia"@it .


###  https://w3id.org/crmrp#c_2ff31b40
crmrp:c_2ff31b40 rdf:type owl:NamedIndividual ,
                          skos:Concept ;
                 rdfs:label "Opus segmentatum"@en ;
                 skos:broader :c_b9a6a1c8 ;
                 skos:definition "Pavement made of stone slab fragments, most commonly marble, of different colors, cut in irregular shapes and placed side by side without creating any geometric or figurative motif."@en ;
                 skos:editorialNote "C. Fiori “Teoria e tecniche per la conservazione del mosaico”, Il Prato, Padova, 2002"@it ,
                                    "Getty Conservation Institute “Illustrated Glossary - Technician Training for the Maintenance of In Situ Mosaics”, Los Angeles, 2013"@en ;
                 skos:inScheme :Execution_Technique ;
		 skos:topConceptOf :Execution_Technique ;
                 skos:prefLabel "Opus segmentatum"@en , "Opus segmentatum"@it .


###  https://w3id.org/crmrp#c_326da7e4
crmrp:c_326da7e4 rdf:type owl:NamedIndividual ,
                          skos:Concept ;
                 rdfs:label "Inpainting"@en ;
                 skos:altLabel "Pictorial retouching"@en ,
                               "Retouching"@en ;
                 skos:broader :c_0f7eacd7 ;
                 skos:closeMatch <http://vocab.getty.edu/page/aat/300053723> ;
                 skos:definition " In the conservation of paintings, the introduction of new paint into and limited to areas of loss in the original paint layer in order to restore design continuity."@en ;
                 skos:editorialNote "Getty AAT http://vocab.getty.edu/page/aat/300053723"@en ;
                 skos:inScheme :Intervention ;
 		 skos:topConceptOf :Intervention ;
                 skos:prefLabel "Inpainting"@en , "Reintegrazione pittorica"@it .


###  https://w3id.org/crmrp#c_33147d64
crmrp:c_33147d64 rdf:type owl:NamedIndividual ,
                          skos:Concept ;
                 rdfs:label "Miniature"@en ;
                 skos:altLabel "Illuminations"@en ;
                 skos:broader :c_044b6056 ;
                 skos:closeMatch <http://vocab.getty.edu/page/aat/300033936> ;
                 skos:definition "Paintings on a very small scale. The term is often applied specifically to small scenes in illuminated manuscripts or to portraits on vellum or ivory that were popular in Europe and America from the Renaissance into the 19th century. For paintings in manuscripts, the term illuminations may also be appropriate."@en ;
                 skos:editorialNote "Getty AAT http://vocab.getty.edu/page/aat/300033936"@en ;
                 skos:inScheme :Execution_Technique ;
		 skos:topConceptOf :Execution_Technique ;
                 skos:prefLabel "Miniature"@en , "Miniatura"@it .


###  https://w3id.org/crmrp#c_33b4c491
crmrp:c_33b4c491 rdf:type owl:NamedIndividual ,
                          skos:Concept ;
                 rdfs:label "Shrinkage"@en ;
                 skos:broader :c_13f3ce9e ;
                 skos:definition "Decrease in dimensions."@en ;
                 skos:editorialNote "Getty AAT http://vocab.getty.edu/page/aat/300054120"@en ,
                                    "Uni Cen/Ts 17135:2021 - Conservation of cultural heritage. General terms and definitions"@en ;
                 skos:exactMatch <http://vocab.getty.edu/page/aat/300054120> ;
                 skos:inScheme :Alteration ;
		 skos:topConceptOf :Alteration ;
                 skos:note "The preferred editorial note and the definition closest to the meaning is Uni Cen/Ts 17135:2021"@en ;
                 skos:prefLabel "Shrinkage"@en , "Ristringimento"@it .


###  https://w3id.org/crmrp#c_33e199bc
crmrp:c_33e199bc rdf:type owl:NamedIndividual ,
                          skos:Concept ;
                 rdfs:label "Thin layer chromatography (TLC)"@en ;
                 skos:broader :c_2d5cde83 ;
                 skos:closeMatch <http://vocab.getty.edu/page/aat/300214726> ;
                 skos:definition "Chromatography in which glass plates coated with thin layers of alumina, silica gel, or cellulose are used as an adsorbent."@en ;
                 skos:editorialNote "Getty AAT http://vocab.getty.edu/page/aat/300214726"@en ;
                 skos:inScheme :Archeometric_and_Diagnostic_Analysis ;
		 skos:topConceptOf :Archeometric_and_Diagnostic_Analysis ;
                 skos:prefLabel "Thin layer chromatography (TLC)"@en , "Cromatografia su strato sottile (TLC)"@it .


###  https://w3id.org/crmrp#c_342e7fe6
crmrp:c_342e7fe6 rdf:type owl:NamedIndividual ,
                          skos:Concept ;
                 rdfs:label "Sagging"@en ;
                 skos:broader :c_13f3ce9e ;
                 skos:definition "Deformation of tapestries, canvases and large paper supports due to the prolonged action of their own weight."@en ;
                 skos:editorialNote "C. Giannini, “Dizionario del restauro - Tecniche diagnostica conservazione”, Nardini Editore, Firenze, 2010"@it ;
                 skos:inScheme :Alteration ;
		 skos:topConceptOf :Alteration ;
                 skos:note "International references could not be found"@en ;
                 skos:prefLabel "Sagging"@en , "Afflosciamento"@it .


###  https://w3id.org/crmrp#c_34d8fe56
crmrp:c_34d8fe56 rdf:type owl:NamedIndividual ,
                          skos:Concept ;
                 rdfs:label "Stone"@en ;
                 skos:closeMatch <http://vocab.getty.edu/page/aat/300011176> ;
                 skos:definition "General term for rock that has been cut, shaped, crushed, or otherwise formed for use in construction or other purposes. Includes the specific archaeological and anthropological sense of individual stones which may be decorated or ornamented and which may be used in ritual contexts. These are usually not carved or dressed, and so differ from sculptures made from stone."@en ;
                 skos:editorialNote "Getty AAT http://vocab.getty.edu/page/aat/300011176"@en ;
                 skos:inScheme :Material ;
                 skos:prefLabel "Stone"@en , "Lapideo"@it ;
                 skos:topConceptOf :Material .


###  https://w3id.org/crmrp#c_3523110e
crmrp:c_3523110e rdf:type owl:NamedIndividual ,
                          skos:Concept ;
                 rdfs:label "Low pressure karsten tube"@en ;
                 skos:broader :c_1fd6102e ;
                 skos:definition "The low-pressure water absorption method is performed to determine the volume of water absorbed at low pressure by a given surface of material, after a set time."@en ;
                 skos:editorialNote "UNI EN 16302:2013 Conservazione dei Beni Culturali - Metodi di prova - Misura dell'assorbimento di acqua con il metodo della pipetta"@it ;
                 skos:inScheme :Archeometric_and_Diagnostic_Analysis ;
		 skos:topConceptOf :Archeometric_and_Diagnostic_Analysis ;
                 skos:note "International references could not be found"@en ;
                 skos:prefLabel "Low pressure karsten tube"@en , "Misura dell'assorbimento di acqua con il metodo della pipetta"@it .


###  https://w3id.org/crmrp#c_3639e649
crmrp:c_3639e649 rdf:type owl:NamedIndividual ,
                          skos:Concept ;
                 rdfs:label "Scratch"@en ;
                 skos:altLabel "Cut"@en ;
                 skos:definition "Line of loss or displacement of material caused by sharp edge."@en ;
                 skos:editorialNote "Uni Cen/Ts 17135:2021 - Conservation of cultural heritage. General terms and definitions"@en ,
                                    "Verg`es-Belmin et al., ICOMOS-ISCS: Illustrated glossary on stone deterioration patterns, vol. XV. Icomos International Council on Monuments and Sites, 2008"@en ;
                 skos:inScheme :Alteration ;
                 skos:note "The preferred editorial note and the closest definition  to the meaning is Uni Cen/Ts 17135:2021"@en ;
                 skos:prefLabel "Scratch"@en , "Graffio"@it ;
                 skos:topConceptOf :Alteration .


###  https://w3id.org/crmrp#c_37bf4517
crmrp:c_37bf4517 rdf:type owl:NamedIndividual ,
                          skos:Concept ;
                 rdfs:label "Fusion with ceramic coating"@en ;
                 skos:broader :c_0a9f4d42 ;
                 skos:definition "This type of technique is used for the production of mechanical parts, especially in the weapons industry. The advantages of ceramic casting are precision and fidelity in the reproduction of the smallest details. The limitations are mainly the small dimensions that can be achieved."@en ;
                 skos:editorialNote "A.Giuffredi “Formatura e fonderia”, Alinea editrice, Firenze, 2010"@it ;
                 skos:inScheme :Execution_Technique ;
 		 skos:topConceptOf :Execution_Technique ;
                 skos:note "International references could not be found"@en ;
                 skos:prefLabel "Fusion with ceramic coating"@en , "Fusione a rivestimento ceramico"@it .


###  https://w3id.org/crmrp#c_380df6b8
crmrp:c_380df6b8 rdf:type owl:NamedIndividual ,
                          skos:Concept ;
                 rdfs:label "Conservation report"@en ;
                 skos:broader :c_5b7fce15 ;
                 skos:definition "A document which gives brief information concerning the history of the building, the wall painting, conservation and past restoration campaigns and results arising from tests and scientific studies, as well as environmental aspects, mapping, building and site surveys etc."@en ;
                 skos:editorialNote "A. Weyer et al., “EwaGlos - European Illustrated Glossary of conservation terms for wall paintings and architectural surfaces”, Michael Imhof Verlag, Petersberg, Germany"@en ;
                 skos:inScheme :Documentation ;
		 skos:topConceptOf :Documentation ;
                 skos:prefLabel "Conservation report"@en , "Relazione tecnico-scientifica"@it .


###  https://w3id.org/crmrp#c_390901fa
crmrp:c_390901fa rdf:type owl:NamedIndividual ,
                          skos:Concept ;
                 rdfs:label "X-ray diffraction (XRD)"@en ;
                 skos:broader :c_789c3e32 ;
                 skos:definition "Diffraction of x-rays by the regularly spaced atoms of a substance, useful for determining the arrangement of atoms and thereby the nature or composition of a substance"@en ;
                 skos:editorialNote "Getty AAT http://vocab.getty.edu/page/aat/300233218"@en ;
                 skos:exactMatch <http://vocab.getty.edu/page/aat/300233218> ;
                 skos:inScheme :Archeometric_and_Diagnostic_Analysis ;
		 skos:topConceptOf :Archeometric_and_Diagnostic_Analysis ;
                 skos:prefLabel "X-ray diffraction (XRD)"@en , "Diffrazione ai raggi X (XRD)"@it .


###  https://w3id.org/crmrp#c_3b191842
crmrp:c_3b191842 rdf:type owl:NamedIndividual ,
                          skos:Concept ;
                 rdfs:label "Blister"@en ;
                 skos:altLabel "Bulge"@en ;
                 skos:broader :c_13f3ce9e ;
                 skos:definition "Domed surface with a cavity beneath."@en ;
                 skos:editorialNote " A. Weyer et al., “EwaGlos - European Illustrated Glossary of conservation terms for wall paintings and architectural surfaces”, Michael Imhof Verlag, Petersberg, Germany"@en ,
                                    "Uni Cen/Ts 17135:2021 - Conservation of cultural heritage. General terms and definitions"@en ;
                 skos:inScheme :Alteration ;
 		 skos:topConceptOf :Alteration ;
                 skos:note "The preferred editorial note and the definition closest to the meaning is Uni Cen/Ts 17135:2021"@en ;
                 skos:prefLabel "Blister"@en , "Sbollatura"@it .


###  https://w3id.org/crmrp#c_3b7b721f
crmrp:c_3b7b721f rdf:type owl:NamedIndividual ,
                          skos:Concept ;
                 rdfs:label "Tonal adjustment"@en ;
                 skos:altLabel "Glazing"@en ;
                 skos:broader :c_326da7e4 ;
                 skos:definition "Small losses in the paint layer, in the preparatory layer or in the final layer, caused by wear/use, abrasion or other damage, are reintegrated by means of reducing the tone with transparent glazes (applied using watercolours or any other compatible and adequate binding media)."@en ;
                 skos:editorialNote "A. Weyer et al., “EwaGlos - European Illustrated Glossary of conservation terms for wall paintings and architectural surfaces”, Michael Imhof Verlag, Petersberg, Germany"@en ;
                 skos:inScheme :Intervention ;
 		 skos:topConceptOf :Intervention ;
                 skos:prefLabel "Tonal adjustment"@en , "Abbassamento tonale"@it .


###  https://w3id.org/crmrp#c_3b8e5779
crmrp:c_3b8e5779 rdf:type owl:NamedIndividual ,
                          skos:Concept ;
                 rdfs:label "Scagliola"@en ;
                 skos:broader :c_17157ccd ;
                 skos:editorialNote "A. Weyer et al., “EwaGlos - European Illustrated Glossary of conservation terms for wall paintings and architectural surfaces”, Michael Imhof Verlag, Petersberg, Germany"@en ,
                                    "Getty AAT http://vocab.getty.edu/page/aat/300014963"@en ;
                 skos:exactMatch <http://vocab.getty.edu/page/aat/300014963> ;
                 skos:inScheme :Execution_Technique ;
		 skos:topConceptOf :Execution_Technique ;
                 skos:prefLabel "Scagliola"@en , "Scagliola"@it .


###  https://w3id.org/crmrp#c_3ba05aa7
crmrp:c_3ba05aa7 rdf:type owl:NamedIndividual ,
                          skos:Concept ;
                 rdfs:label "Resistography"@en ;
                 skos:broader :c_abed88a5 ;
                 skos:definition "Resistographic analysis allows field diagnosis and visualisation of density variations in timber structures"@en ;
                 skos:editorialNote "M.Ceroni, G.Elia, “Diagnostica per i beni culturali”, Alinea editrice, Firenze, 2008"@it ;
                 skos:inScheme :Archeometric_and_Diagnostic_Analysis ;
		 skos:topConceptOf :Archeometric_and_Diagnostic_Analysis ;
                 skos:note "International references could not be found"@en ;
                 skos:prefLabel "Resistography"@en , "Resistografia"@it .


###  https://w3id.org/crmrp#c_3cbfcf7b
crmrp:c_3cbfcf7b rdf:type owl:NamedIndividual ,
                          skos:Concept ;
                 rdfs:label "Raman spectroscopy"@en ;
                 skos:broader :c_789c3e32 ;
                 skos:definition "Technique of scattering a monochromatic light, such as a laser, changing the vibrational, rotational, or electronic energy of a sample, the results of which help determine its molecular structure. Discovered by Indian physicist Sir Chandrasekhara Venkata Raman (1888-1970)."@en ;
                 skos:editorialNote "Getty AAT http://vocab.getty.edu/page/aat/300266192"@en ;
                 skos:exactMatch <http://vocab.getty.edu/page/aat/300266192> ;
                 skos:inScheme :Archeometric_and_Diagnostic_Analysis ;
		 skos:topConceptOf :Archeometric_and_Diagnostic_Analysis ;
                 skos:prefLabel "Raman spectroscopy"@en , "Spettrofotometria Raman"@it .


###  https://w3id.org/crmrp#c_3de3f55a
crmrp:c_3de3f55a rdf:type owl:NamedIndividual ,
                          skos:Concept ;
                 rdfs:label "Metallisation"@en ;
                 skos:broader :c_f1c689bb ;
                 skos:definition "Metallisation is a fundamental process in surface finishing, especially of steel and iron. This metal coating protects the underlying material from oxidation and corrosion, extending durability and strength over time."@en ;
                 skos:editorialNote "C. Giannini, “Dizionario del restauro - Tecniche diagnostica conservazione”, Nardini Editore, Firenze, 2010"@it ,
                                    "T. Turco, “Il doratore”, Hoepli, Milano, 2017"@it ;
                 skos:inScheme :Execution_Technique ;
 		 skos:topConceptOf :Execution_Technique ;
                 skos:note "International references could not be found"@en ;
                 skos:prefLabel "Metallisation"@en , "Metalizzazione"@it .


###  https://w3id.org/crmrp#c_3edabaad
crmrp:c_3edabaad rdf:type owl:NamedIndividual ,
                          skos:Concept ;
                 rdfs:label "Polishing"@en ;
                 skos:broader :c_757ed6ec ;
                 skos:definition "Process of rubbing a surface to make it smooth or shiny."@en ;
                 skos:editorialNote "Getty AAT http://vocab.getty.edu/page/aat/300053867"@en ;
                 skos:exactMatch <http://vocab.getty.edu/page/aat/300053867> ;
                 skos:inScheme :Execution_Technique ;
 		 skos:topConceptOf :Execution_Technique ;
                 skos:prefLabel "Polishing"@en , "Brunitura"@it .


###  https://w3id.org/crmrp#c_3ef20257
crmrp:c_3ef20257 rdf:type owl:NamedIndividual ,
                          skos:Concept ;
                 rdfs:label "Biological colonisation"@en ;
                 skos:altLabel "Biodegradation"@en ,
                               "Biodeterioration"@en ,
                               "Biological growth"@en ,
                               "Microbiological organisms"@en ;
                 skos:closeMatch <http://vocab.getty.edu/page/aat/300219639> ,
                                 <http://vocab.getty.edu/page/aat/300419379> ;
                 skos:definition "Growth of organisms on or within an object. Example: lichen, moss, plant, animals, microorganisms."@en ;
                 skos:editorialNote " A. Weyer et al., “EwaGlos - European Illustrated Glossary of conservation terms for wall paintings and architectural surfaces”, Michael Imhof Verlag, Petersberg, Germany"@en ,
                                    "Getty AAT http://vocab.getty.edu/page/aat/300219639"@en ,
                                    "Getty AAT http://vocab.getty.edu/page/aat/300419379"@en ,
                                    "Getty Conservation Institute “Illustrated Glossary - Definitions of terms used for the graphic documentation of in situ floor mosaics”, “Mosaics In Situ Project”, Los Angeles, 2003"@en ,
                                    "Uni Cen/Ts 17135:2021 - Conservation of cultural heritage. General terms and definitions"@en ,
                                    "Verg`es-Belmin et al., ICOMOS-ISCS: Illustrated glossary on stone deterioration patterns, vol. XV. Icomos International Council on Monuments and Sites, 2008"@en ;
                 skos:inScheme :Alteration ;
                 skos:note "The preferred editorial note and the definition closest to the meaning is Uni Cen/Ts 17135:2021"@en ;
                 skos:prefLabel "Biological colonisation"@en , "Colonizzazione biologica"@it ;
                 skos:topConceptOf :Alteration .


###  https://w3id.org/crmrp#c_3fa9cd31
crmrp:c_3fa9cd31 rdf:type owl:NamedIndividual ,
                          skos:Concept ;
                 rdfs:label "Polymer paint"@en ;
                 skos:broader :c_143349b9 ;
                 skos:definition "Paint with a base that is polymer, which is compound formed by the combination of two or more molecules of the same substance to produce a new compound with the same empirical formula but with higher molecular weight. It is typically made from pigments in an acrylic resin or vinyl resin, which are polymers, or a combination of both resins. It is water based, spreads out in a layer, and forms a continuous, flexible, and waterproof film of plastic when the water evaporates."@en ;
                 skos:editorialNote "Getty AAT http://vocab.getty.edu/page/aat/300015055"@en ;
                 skos:exactMatch <http://vocab.getty.edu/page/aat/300147678> ;
                 skos:inScheme :Execution_Technique ;
		 skos:topConceptOf :Execution_Technique ;
                 skos:prefLabel "Polymer paint"@en , "Polimero sintetico"@it .


###  https://w3id.org/crmrp#c_404ba9c8
crmrp:c_404ba9c8 rdf:type owl:NamedIndividual ,
                          skos:Concept ;
                 rdfs:label "Excrement"@en ;
                 skos:broader :c_3ef20257 ;
                 skos:closeMatch <http://vocab.getty.edu/page/aat/300191590> ;
                 skos:definition "Waste matter discharged from the body."@en ;
                 skos:editorialNote "Getty AAT http://vocab.getty.edu/page/aat/300191590"@en ;
                 skos:inScheme :Alteration ;
		 skos:topConceptOf :Alteration ;
                 skos:prefLabel "Excrement"@en , "Guano"@it .


###  https://w3id.org/crmrp#c_4064717d
crmrp:c_4064717d rdf:type owl:NamedIndividual ,
                          skos:Concept ;
                 rdfs:label "Stereomicroscope"@en ;
                 skos:broader :c_abed88a5 ;
                 skos:definition "The stereoscopic microscope, also known as stereomicroscope, microstereoscope or dissector, is a type of optical microscope designed to produce a stereoscopic view of an object."@en ;
                 skos:editorialNote "M.Ceroni, G.Elia, “Diagnostica per i beni culturali”, Alinea editrice, Firenze, 2008"@en ;
                 skos:inScheme :Archeometric_and_Diagnostic_Analysis ;
		 skos:topConceptOf :Archeometric_and_Diagnostic_Analysis ;
                 skos:note "International references could not be found"@en ;
                 skos:prefLabel "Stereomicroscope"@en , "Stereomicroscopio"@it .


###  https://w3id.org/crmrp#c_40a6d4b1
crmrp:c_40a6d4b1 rdf:type owl:NamedIndividual ,
                          skos:Concept ;
                 rdfs:label "Steel"@en ;
                 skos:broader :c_6407466f ;
                 skos:closeMatch <http://vocab.getty.edu/page/aat/300133751> ;
                 skos:definition "Any of various hard, strong, durable, malleable alloys of iron and carbon, often with other elements such as manganese, chromium, nickel, molybdenum, copper, tungsten, cobalt, or silicon; widely used as a structural material."@en ;
                 skos:editorialNote "Getty AAT http://vocab.getty.edu/page/aat/300133751"@en ;
                 skos:inScheme :Material ;
		 skos:topConceptOf :Material ;
                 skos:prefLabel "Steel"@en , "Acciao"@it .


###  https://w3id.org/crmrp#c_41624a1a
crmrp:c_41624a1a rdf:type owl:NamedIndividual ,
                          skos:Concept ;
                 rdfs:label "Palaentological"@en ;
                 skos:altLabel "remains (object genre)"@en ;
                 skos:closeMatch <http://vocab.getty.edu/page/aat/300265420> ;
                 skos:definition "Materials or items left of a thing or things after other parts have been removed, used, or destroyed. Examples include substances of organic origin that are entirely or partially preserved, often in the earth, in a conserved or fossilized condition, including what is left of a person or animal when life is extinct. May also include artifacts, ruins, and other remanants of a person or civilization."@en ;
                 skos:editorialNote "Getty AAT http://vocab.getty.edu/page/aat/300265420"@en ;
                 skos:inScheme :Restoration_Object ;
                 skos:prefLabel "Palaentological"@en , "Paleontologico"@it ;
                 skos:topConceptOf :Restoration_Object .


###  https://w3id.org/crmrp#c_41bb39c8
crmrp:c_41bb39c8 rdf:type owl:NamedIndividual ,
                          skos:Concept ;
                 rdfs:label "Authorisation"@en ;
                 skos:broader :c_5b7fce15 ;
                 skos:definition "Confirmation by the competent state bodies of the relevance of projects, reports or work carried out directly on works of art."@en ;
                 skos:inScheme :Documentation ;
  		 skos:topConceptOf :Documentation ;
                 skos:note "International references could not be found"@en ;
                 skos:prefLabel "Authorisation"@en , "Autorizzazione"@it .


###  https://w3id.org/crmrp#c_42b93bd2
crmrp:c_42b93bd2 rdf:type owl:NamedIndividual ,
                          skos:Concept ;
                 rdfs:label "Infra-red reflectography"@en ;
                 skos:broader :c_1285fa71 ;
                 skos:definition "Infrared reflectography is a digital imaging technique that allows study of layers beneath the surface of a painting by capturing absorption/emission characteristics of reflected infrared radiation. A complementary technique to x-radiography, IRR uncovers somewhat different information.The longer wavelengths of infrared radiation penetrate most surface pigments and reveal charcoal or graphite underdrawings, the underlying initial stages of a composition"@en ;
                 skos:editorialNote "Getty AAT http://vocab.getty.edu/page/aat/300379538"@en ;
                 skos:exactMatch <http://vocab.getty.edu/page/aat/300379538> ;
                 skos:inScheme :Archeometric_and_Diagnostic_Analysis ;
   		 skos:topConceptOf :Archeometric_and_Diagnostic_Analysis ;
                 skos:prefLabel "Infra-red reflectography"@en , "Riflettografia infrarossa"@it .


###  https://w3id.org/crmrp#c_42f16f05
crmrp:c_42f16f05 rdf:type owl:NamedIndividual ,
                          skos:Concept ;
                 rdfs:label "RTI (Reflectance Transformation Imaging)"@en ;
                 skos:broader :c_1fd6102e ;
                 skos:definition "Reflectance Transformation Imaging (RTI) is a new imaging technique that creates hyper-realistic digital surrogates that are interactively controlled by the viewer. This new method is based upon the synthesis of multiple digital images of a subject in a fixed position collected from a fixed camera position."@en ;
                 skos:inScheme :Archeometric_and_Diagnostic_Analysis ;
		 skos:topConceptOf :Archeometric_and_Diagnostic_Analysis ;
                 skos:note "International references could not be found."@en ;
                 skos:prefLabel "RTI (Reflectance Transformation Imaging)"@en , "RTI (Reflectance Transformation Imaging)"@it .


###  https://w3id.org/crmrp#c_446c8061
crmrp:c_446c8061 rdf:type owl:NamedIndividual ,
                          skos:Concept ;
                 rdfs:label "Stain"@en ;
                 skos:closeMatch <http://vocab.getty.edu/page/aat/300379497> ;
                 skos:definition "Area of change of colour."@en ;
                 skos:editorialNote "Getty AAT http://vocab.getty.edu/page/aat/300379497"@en ,
                                    "Uni Cen/Ts 17135:2021 - Conservation of cultural heritage. General terms and definitions"@en ;
                 skos:inScheme :Alteration ;
                 skos:note "The preferred editorial note and the definition closest to the meaning is Uni Cen/Ts 17135:2021"@en ;
                 skos:prefLabel "Stain"@en , "Macchia"@it ;
                 skos:topConceptOf :Alteration .


###  https://w3id.org/crmrp#c_46b47593
crmrp:c_46b47593 rdf:type owl:NamedIndividual ,
                          skos:Concept ;
                 rdfs:label "Dendrochronology"@en ;
                 skos:broader :c_abed88a5 ;
                 skos:definition " The technique of dating events, intervals of time, and variations in environment understood by studying the sequence of and differences between rings of growth in trees and aged wood."@en ;
                 skos:editorialNote "Getty AAT http://vocab.getty.edu/page/aat/300054715"@en ;
                 skos:exactMatch <http://vocab.getty.edu/page/aat/300054715> ;
                 skos:inScheme :Archeometric_and_Diagnostic_Analysis ;
		 skos:topConceptOf :Archeometric_and_Diagnostic_Analysis ;
                 skos:prefLabel "Dendrochronology"@en , "Dendrocronologia"@it .


###  https://w3id.org/crmrp#c_46fa5a86
crmrp:c_46fa5a86 rdf:type owl:NamedIndividual ,
                          skos:Concept ;
                 rdfs:label "Cast iron"@en ;
                 skos:broader :c_6407466f ;
                 skos:closeMatch <http://vocab.getty.edu/page/aat/300011004> ;
                 skos:definition "An iron alloy containing about 2 to 4% carbon and 1 to 3% silicon, having a high compressive strength but low tensile strength. Cast iron is manufactured by melting scrap iron or pig iron in a cupola that is in contact with the coal fuel, then casting the molten iron into a mold. A large range of building and decorative items are made of cast iron by pouring the molten metal into sand molds and then machining. It is inexpensive and easy to make. It was made in China by at least the 3rd century BCE; the technique for its production did not reach Europe until medieval times."@en ;
                 skos:inScheme :Material ;
		 skos:topConceptOf :Material ;
                 skos:prefLabel "Cast iron"@en , "Ghisa"@it ;
                 skos:source "Getty AAT http://vocab.getty.edu/page/aat/300011004"@en .


###  https://w3id.org/crmrp#c_4823a051
crmrp:c_4823a051 rdf:type owl:NamedIndividual ,
                          skos:Concept ;
                 rdfs:label "Revowen"@en ;
                 skos:broader :c_24cc76d5 ;
                 skos:definition "integrative restoration of the gaps in the tapestries that can be combined with the principle of abstraction or colour selection."@en ;
                 skos:editorialNote "C. Giannini, “Dizionario del restauro - Tecniche diagnostica  conservazione”, Nardini Editore, Firenze, 2010"@it ;
                 skos:inScheme :Intervention ;
   		 skos:topConceptOf :Intervention ;
                 skos:note "International references could not be found"@en ;
                 skos:prefLabel "Revowen"@en , "Ritessitura"@it .


###  https://w3id.org/crmrp#c_4973d8ba
crmrp:c_4973d8ba rdf:type owl:NamedIndividual ,
                          skos:Concept ;
                 rdfs:label "Biofilm"@en ;
                 skos:broader :c_3ef20257 ;
                 skos:definition "Film consisting of an aggregation of microorganisms adhering to a surface."@en ;
                 skos:editorialNote "Getty AAT http://vocab.getty.edu/page/aat/300379570"@en ,
                                    "Uni Cen/Ts 17135:2021 - Conservation of cultural heritage. General terms and definitions"@en ;
                 skos:exactMatch <http://vocab.getty.edu/page/aat/300379570> ;
                 skos:inScheme :Alteration ;
		 skos:topConceptOf :Alteration ;
                 skos:note "The preferred editorial note and the definition closest to the meaning is Uni Cen/Ts 17135:2021"@en ;
                 skos:prefLabel "Biofilm"@en , "Biofilm"@it .


###  https://w3id.org/crmrp#c_49988b8d
crmrp:c_49988b8d rdf:type owl:NamedIndividual ,
                          skos:Concept ;
                 rdfs:label "Xylophagous attack"@en ;
                 skos:broader :c_3ef20257 ;
                 skos:definition "A category of insects belonging to numerous orders and families (Lepidoptera Cossidae, Bostricidae beetles, Scolytidae, Cerambidae, Buprestidae, Hymenoptera Siricidae); they feed on wood even after the plant has been felled and are one of the causes of the degradation of the substrates of wooden artefacts, in which they dig tunnels tunnels that make the material porous and fragile, destructuring it."@en ;
                 skos:inScheme :Alteration ;
 		 skos:topConceptOf :Alteration ;
                 skos:note "International references could not be found"@en ;
                 skos:prefLabel "Xylophagous attack"@en , "Attacco xilofago"@it .


###  https://w3id.org/crmrp#c_49aa1adb
crmrp:c_49aa1adb rdf:type owl:NamedIndividual ,
                          skos:Concept ;
                 rdfs:label "Dosing of soluble salts"@en ;
                 skos:broader :c_abed88a5 ;
                 skos:defintion "The test is conducted in order to determine the presence of specific soluble salts (qualitative analysis) and to detect a range within which the concentration of the detected salts can be found"@en ;
                 skos:editorialNote "UNI 11087:2003 Beni culturali - Materiali lapidei naturali ed artificiali - Determinazione del contenuto di sali solubili"@it ;
                 skos:inScheme :Archeometric_and_Diagnostic_Analysis ;
 		 skos:topConceptOf :Archeometric_and_Diagnostic_Analysis ;
                 skos:note "International references could not be found"@en ;
                 skos:prefLabel "Dosing of soluble salts"@en , "Dosaggio sali solubili"@it .


###  https://w3id.org/crmrp#c_49fed917
crmrp:c_49fed917 rdf:type owl:NamedIndividual ,
                          skos:Concept ;
                 rdfs:label "Aquarelle"@en ;
                 skos:altLabel "Watercolour"@en ;
                 skos:broader :c_044b6056 ;
                 skos:definition "Watercolor painting done in transparent washes of color as distinguished from the opaque method using gouache"@en ;
                 skos:editorialNote "Getty AAT http://vocab.getty.edu/page/aat/300053363"@en ;
                 skos:exactMatch <http://vocab.getty.edu/page/aat/300053363> ;
                 skos:inScheme :Execution_Technique ;
		 skos:topConceptOf :Execution_Technique ;
                 skos:prefLabel "Aquarelle"@en , "Acquerello"@it .


###  https://w3id.org/crmrp#c_4a72d11e
crmrp:c_4a72d11e rdf:type owl:NamedIndividual ,
                          skos:Concept ;
                 rdfs:label "Abrasion"@en ;
                 skos:definition "loss of material from a surface due to frictional forces."@en ;
                 skos:editorialNote " A. Weyer et al., “EwaGlos - European Illustrated Glossary of conservation terms for wall paintings and architectural surfaces”, Michael Imhof Verlag, Petersberg, Germany"@en ,
                                    "Getty AAT http://vocab.getty.edu/page/aat/300053077"@en ,
                                    "Uni Cen/Ts 17135:2021 - Conservation of cultural heritage. General terms and definitions"@en ,
                                    "Verg`es-Belmin et al., ICOMOS-ISCS: Illustrated glossary on stone deterioration patterns, vol. XV. Icomos International Council on Monuments and Sites, 2008"@en ;
                 skos:exactMatch <http://vocab.getty.edu/page/aat/300053077> ;
                 skos:inScheme :Alteration ;
                 skos:note "The preferred editorial note and the definition closest to the meaning is Uni Cen/Ts 17135:2021"@en ;
                 skos:prefLabel "Abrasion"@en , "Abrasione"@it ;
                 skos:topConceptOf :Alteration .


###  https://w3id.org/crmrp#c_4ad9e448
crmrp:c_4ad9e448 rdf:type owl:NamedIndividual ,
                          skos:Concept ;
                 rdfs:label "Incision"@en ;
                 skos:altLabel "Engraving"@en;
                 skos:definition "Separation with sharply defined edges limited to a part of the thickness of the material"@en ;
                 skos:editorialNote "Uni Cen/Ts 17135:2021 - Conservation of cultural heritage. General terms and definitions"@en ,
                                    "Verg`es-Belmin et al., ICOMOS-ISCS: Illustrated glossary on stone deterioration patterns, vol. XV. Icomos International Council on Monuments and Sites, 2008"@en ;
                 skos:inScheme :Alteration ;
                 skos:note "The preferred editorial note and the definition closest to the meaning is Uni Cen/Ts 17135:2021"@en ;
                 skos:prefLabel "Incision"@en , "Incisione"@it ;
                 skos:topConceptOf :Alteration .


###  https://w3id.org/crmrp#c_4b4e8dc7
crmrp:c_4b4e8dc7 rdf:type owl:NamedIndividual ,
                          skos:Concept ;
                 rdfs:label "Specular light"@en ;
                 skos:broader :c_1fd6102e ;
                 skos:definition "Specular light is light reflected from a surface on which a single ray is reflected in a single direction."@en ;
                 skos:inScheme :Archeometric_and_Diagnostic_Analysis ;
 		 skos:topConceptOf :Archeometric_and_Diagnostic_Analysis ;
                 skos:note "International references could not be found"@en ;
                 skos:prefLabel "Specular light"@en , "Fotografia a luce speculare"@it .


###  https://w3id.org/crmrp#c_4cd02f85
crmrp:c_4cd02f85 rdf:type owl:NamedIndividual ,
                          skos:Concept ;
                 rdfs:label "Scanning electronic microscope (SEM) equipped with electronic micro wave (EDS)"@en ;
                 skos:broader :c_7ee727f3 ;
                 skos:closeMatch <http://vocab.getty.edu/page/aat/300343819> ;
                 skos:definition "Electron microscopes designed for directly studying the surfaces of solid objects, utilizing a beam of focused electrons of relatively low energy as an electron probe that is scanned in a regular manner over the specimen. An electrical signal is obtained by collecting and amplifying secondary electrons emitted by the specimen and is applied to a cathode-ray tube scanned in synchronism with the electron beam."@en ;
                 skos:editorialNote "Getty AAT http://vocab.getty.edu/page/aat/300343819"@en ;
                 skos:inScheme :Archeometric_and_Diagnostic_Analysis ;
		 skos:topConceptOf :Archeometric_and_Diagnostic_Analysis ;
                 skos:prefLabel "Scanning electronic microscope (SEM) equipped with electronic micro wave (EDS)"@en , "Microscopia elettronica a scansione (SEM) corredata di microsonda elettronica (EDS)"@it .


###  https://w3id.org/crmrp#c_4d471b17
crmrp:c_4d471b17 rdf:type owl:NamedIndividual ,
                          skos:Concept ;
                 rdfs:label "Size gilding"@en ;
                 skos:broader :c_8af455cd ;
                 skos:definition "Mission gilding is a definitive gilding because an irreversible adhesive is used as a leaf adhesive. The preparation of the object is the same as for gouache gilding, right down to the bolus preparation. Oil mission is more resistant than water mission and is used for objects placed outdoors."@en ;
                 skos:editorialNote "C. Giannini, “Dizionario del restauro - Tecniche diagnostica conservazione”, Nardini Editore, Firenze, 2010"@it ,
                                    "G. Pignolo, “Effetti d’oro - Storia e tecnica della doratura nell’arte”, Editrice Compositori, Bologna, 2002"@it ;
                 skos:inScheme :Execution_Technique ;
		 skos:topConceptOf :Execution_Technique ;
                 skos:note "International references could not be found, but the preferred editorial note and the definition closest to the meaning is Effetti d’oro - Storia e tecnica della doratura nell’arte"@en ;
                 skos:prefLabel "Size gilding"@en , "A missione"@it .


###  https://w3id.org/crmrp#c_4d9c61a1
crmrp:c_4d9c61a1 rdf:type owl:NamedIndividual ,
                          skos:Concept ;
                 rdfs:label "Chelator"@en ;
                 skos:broader :c_5a83cd16 ;
                 skos:definition "Chelants are substances that can be used to remove metal ions. From an application point of view, this can result in different operations, depending on the type of work being worked on."@en ;
                 skos:editorialNote "P.Cremonesi, E. Signorini, “Un approccio alla pulitura dei dipinti mobili”, Il Prato, Padova, 2016"@en ;
                 skos:inScheme :Intervention ;
 		 skos:topConceptOf :Intervention ;
                 skos:note "International references could not be found"@en ;
                 skos:prefLabel "Chelator"@en , "Chelante"@it .


###  https://w3id.org/crmrp#c_4ed58c32
crmrp:c_4ed58c32 rdf:type owl:NamedIndividual ,
                          skos:Concept ;
                 rdfs:label "Etchings"@en ;
                 skos:broader :c_aee6a805 ;
                 skos:closeMatch <http://vocab.getty.edu/page/aat/300041365> ;
                 skos:definition "Prints made from an etched printing plate, which is a metal plate on which a design is made by coating the plate with an acid-resistant substance, creating a design in the coating, and then exposing the plate to acid, which etches the plate where the metal is exposed. For designs incised directly into a copper plate using a burin or graver, use engravings (prints)."@en ;
                 skos:editorialNote "Getty AAT http://vocab.getty.edu/page/aat/300041365"@en ;
                 skos:inScheme :Execution_Technique ;
		 skos:topConceptOf :Execution_Technique ;
                 skos:prefLabel "Etchings"@en , "Acquaforte"@it .


###  https://w3id.org/crmrp#c_4f621a84
crmrp:c_4f621a84 rdf:type owl:NamedIndividual ,
                          skos:Concept ;
                 rdfs:label "Fungus"@en ;
                 skos:broader :c_3ef20257 ;
                 skos:definition "A micro-organism that usually develops as a result of moisture and attacks mainly canvas, paper, natural and artificial stone surfaces; it forms black, greenish or yellow colonies preferably in the presence of glues and on painted parts that are then altered. Mycological studies have demonstrated the great ability of fungal species to adapt to different microclimates, confirming their harmfulness to various types of artistic artefacts."@en ;
                 skos:editorialNote "C. Giannini, “Dizionario del restauro - Tecniche diagnostica conservazione”, Nardini Editore, Firenze, 2010"@it ;
                 skos:inScheme :Alteration ;
 		 skos:topConceptOf :Alteration ;
                 skos:note "International references could not be found"@en ;
                 skos:prefLabel "Fungus"@en , "Fungo"@it .


###  https://w3id.org/crmrp#c_4fe4d308
crmrp:c_4fe4d308 rdf:type owl:NamedIndividual ,
                          skos:Concept ;
                 rdfs:label "Detachment"@en ;
                 skos:altLabel "Detaching"@en ;
                 skos:definition "Removal of a wall painting by separating the paint layer, with or without intonaco, arriccio and part of the wall support. It is done when there are problems in the supporting structure, or when the painting needs to be moved. This operation is usually carried out on murals but can also be developed in artworks with different media"@en ;
                 skos:editorialNote "A. Weyer et al., “EwaGlos - European Illustrated Glossary of conservation terms for wall paintings and architectural surfaces”, Michael Imhof Verlag, Petersberg, Germany"@en ,
                                    "Getty AAT http://vocab.getty.edu/page/aat/300264843"@en ;
                 skos:inScheme :Intervention ;
                 skos:note "The preferred editorial note and the definition closest to the meaning is EwaGlos - European Illustrated Glossary of conservation terms for wall paintings and architectural surfaces"@en ;
                 skos:prefLabel "Detachment"@en , "Trasporto"@it ;
                 skos:topConceptOf :Intervention .


###  https://w3id.org/crmrp#c_502e151f
crmrp:c_502e151f rdf:type owl:NamedIndividual ,
                          skos:Concept ;
                 rdfs:label "Fusione all'osso di seppia"@en ;
                 skos:broader :c_0a9f4d42 ;
                 skos:definition "Cuttlebone casting exploits the special characteristics of these types of bones: workability and resistance to molten metal. Two cuttlefish bones are taken and flattened on the softer side, thus creating two matching surfaces on which the negative can be cast."@en ;
                 skos:editorialNote "A.Giuffredi “Formatura e fonderia”, Alinea editrice, Firenze, 2010"@it ;
                 skos:inScheme :Execution_Technique ;
		 skos:topConceptOf :Execution_Technique ;
                 skos:note "International references could not be found"@en ;
                 skos:prefLabel "Fusione all'osso di seppia"@en , "Fusione all'osso di seppia"@it .


###  https://w3id.org/crmrp#c_51f2e48a
crmrp:c_51f2e48a rdf:type owl:NamedIndividual ,
                          skos:Concept ;
                 rdfs:label "Photographs"@en ;
                 skos:definition "Refers to still images produced from radiation-sensitive materials (sensitive to light, electron beams, or nuclear radiation), generally by means of the chemical action of light on a sensitive film, paper, glass, or metal. Photographs may be positive or negative, opaque or transparent. The concept does not include reproductive prints of documents and technical drawings. The concept may include photographs made by digital means."@en ;
                 skos:editorialNote "Getty AAT http://vocab.getty.edu/page/aat/300046300"@en ;
                 skos:exactMatch <http://vocab.getty.edu/page/aat/300046300> ;
                 skos:inScheme :Restoration_Object ;
                 skos:prefLabel "Photographs"@en , "Fotografia"@it ;
                 skos:topConceptOf :Restoration_Object .


###  https://w3id.org/crmrp#c_52e9c866
crmrp:c_52e9c866 rdf:type owl:NamedIndividual ,
                          skos:Concept ;
                 rdfs:label "Pastille gilding"@en ;
                 skos:broader :c_4d471b17 ;
                 skos:definition "A technique used by ancient decorators to reproduce friezes and high reliefs on different supports. The mixture consists of plaster, scagliola and starch glue."@en ;
                 skos:editorialNote "C. Giannini, “Dizionario del restauro - Tecniche diagnostica conservazione”, Nardini Editore, Firenze, 2010"@it ,
                                    "G. Pignolo, “Effetti d’oro - Storia e tecnica della doratura nell’arte”, Editrice Compositori, Bologna, 2002"@it ;
                 skos:inScheme :Execution_Technique ;
   		 skos:topConceptOf :Execution_Technique ;
                 skos:note "International references could not be found"@en ;
  		 skos:prefLabel "Pastille gilding"@en , "Pastiglia"@it .


###  https://w3id.org/crmrp#c_5422ce57
crmrp:c_5422ce57 rdf:type owl:NamedIndividual ,
                          skos:Concept ;
                 rdfs:label "Lead"@en ;
                 skos:broader :c_6407466f ;
                 skos:definition "Pure metallic element having symbol Pb and atomic number 82; soft, dense ductile metal of a dull gray color, shiny when freshly cut, occuring naturally most often as a sulfide in the mineral galena. Other lead minerals include anglesite (lead sulfate) and cerussite (lead carbonate). Native metallic lead was found and used from about 3600-2600 BCE when the technique for obtaining lead from roasting the sulfide ore (galena) was discovered. Lead was used to make small cast items such as coins and statuettes, plumbing pipes, spires, statues, cisterns, gargoyles, pigments (lead white, litharge, orange mineral, etc.), as a component in pottery glazes, for roofing, flashing, stained glass windows, as a soft solder, and as radiation shielding."@en ;
                 skos:editorialNote "Getty AAT http://vocab.getty.edu/page/aat/300011022"@en ;
                 skos:exactMatch <http://vocab.getty.edu/page/aat/300011022> ;
                 skos:inScheme :Material ;
		 skos:topConceptOf :Material ;
                 skos:prefLabel "Lead"@en , "Piombo"@it .


###  https://w3id.org/crmrp#c_54648e63
crmrp:c_54648e63 rdf:type owl:NamedIndividual ,
                          skos:Concept ;
                 rdfs:label "Colorimetry"@en ;
                 skos:broader :c_1fd6102e ;
                 skos:closeMatch <http://vocab.getty.edu/page/aat/300053579> ;
                 skos:defintion "The process of determining and specifying colors."@en ;
                 skos:editorialNote "Getty AAT http://vocab.getty.edu/page/aat/300053579"@en ;
                 skos:inScheme :Archeometric_and_Diagnostic_Analysis ;
     		 skos:topConceptOf :Archeometric_and_Diagnostic_Analysis ;
                 skos:prefLabel "Colorimetry"@en , "Analisi colorimetrica"@it .


###  https://w3id.org/crmrp#c_547cec21
crmrp:c_547cec21 rdf:type owl:NamedIndividual ,
                          skos:Concept ;
                 rdfs:label "Disgregation"@en ;
                 skos:altLabel "Chalking"@en ,
                               "Powdering"@en , "Polverizzazione"@it ;
                 skos:closeMatch <http://vocab.getty.edu/page/aat/300379824> ;
                 skos:definition "Detachment of single grains or aggregates of grains."@en ;
                 skos:editorialNote "A. Weyer et al., “EwaGlos - European Illustrated Glossary of conservation terms for wall paintings and architectural surfaces”, Michael Imhof Verlag, Petersberg, Germany"@en ,
                                    "Getty AAT http://vocab.getty.edu/page/aat/300379824"@en ,
                                    "Getty Conservation Institute “Illustrated Glossary - Definitions of terms used for the graphic documentation of in situ floor mosaics”, “Mosaics In Situ Project”, Los Angeles, 2003"@en ,
                                    "Verg`es-Belmin et al., ICOMOS-ISCS: Illustrated glossary on stone deterioration patterns, vol. XV. Icomos International Council on Monuments and Sites, 2008"@en ;
                 skos:inScheme :Alteration ;
                 skos:note "The preferred editorial note and the definition closest to the meaning is ICOMOS-ISCS: Illustrated glossary on stone deterioration patterns"@en ;
                 skos:prefLabel "Disgregation"@en , "Disgregazione"@it ;
                 skos:topConceptOf :Alteration .


###  https://w3id.org/crmrp#c_560a9552
crmrp:c_560a9552 rdf:type owl:NamedIndividual ,
                          skos:Concept ;
                 rdfs:label "Satin finishing"@en ;
                 skos:broader :c_4d471b17 ;
                 skos:definition "The final appearance is half-veined and can be achieved by passing the agate stone over the bolus before the leaf is applied."@en ;
                 skos:editorialNote "G. Pignolo, “Effetti d’oro - Storia e tecnica della doratura nell’arte”, Editrice Compositori, Bologna, 2002"@it ;
                 skos:inScheme :Execution_Technique ;
skos:topConceptOf :Execution_Technique ;
                 skos:note "International references could not be found"@en ;
                 skos:prefLabel "Satin finishing"@en , "Satinatura"@it .


###  https://w3id.org/crmrp#c_564ad901
crmrp:c_564ad901 rdf:type owl:NamedIndividual ,
                          skos:Concept ;
                 rdfs:label "Ultraviolet fluorescence"@en ;
                 skos:broader :c_1fd6102e ;
                 skos:closeMatch <http://vocab.getty.edu/page/aat/300379552> ;
                 skos:definition "Visible fluorescence emitted by materials in paintings and other objects exposed to ultraviolet radiation"@en ;
                 skos:editorialNote "Getty AAT http://vocab.getty.edu/page/aat/300379552"@en ;
                 skos:inScheme :Archeometric_and_Diagnostic_Analysis ;
		 skos:topConceptOf :Archeometric_and_Diagnostic_Analysis ;
                 skos:prefLabel "Ultraviolet fluorescence"@en , "Fluorescenza ultravioletta"@it .


###  https://w3id.org/crmrp#c_56afc892
crmrp:c_56afc892 rdf:type owl:NamedIndividual ,
                          skos:Concept ;
                 rdfs:label "Stucco"@en ;
                 skos:broader :c_34d8fe56 ;
                 skos:closeMatch "Stucco"@en ;
                 skos:definition "The plastic moulding of all kinds of mortars on architectural surfaces for decorative purposes."@en ;
                 skos:editorialNote "A. Weyer et al., “EwaGlos - European Illustrated Glossary of conservation terms for wall paintings and architectural surfaces”, Michael Imhof Verlag, Petersberg, Germany"@en ;
                 skos:inScheme :Material ;
                 skos:topConceptOf :Material ;
                 skos:prefLabel "Stucco"@en , "Stucco"@it .


###  https://w3id.org/crmrp#c_570dee40
crmrp:c_570dee40 rdf:type owl:NamedIndividual ,
                          skos:Concept ;
                 rdfs:label "Raking light"@en ;
                 skos:broader :c_1fd6102e ;
                 skos:definition "The surface is lit, preferably using daylight-spots at a specific angle, in order to show the relief through shadow effects."@en ;
                 skos:editorialNote "A. Weyer et al., “EwaGlos - European Illustrated Glossary of conservation terms for wall paintings and architectural surfaces”, Michael Imhof Verlag, Petersberg, Germany"@en ;
                 skos:inScheme :Archeometric_and_Diagnostic_Analysis ;
                 skos:topConceptOf :Archeometric_and_Diagnostic_Analysis ;
                 skos:prefLabel "Raking light"@en , "Fotografia a luce radente"@it .


###  https://w3id.org/crmrp#c_575a314b
crmrp:c_575a314b rdf:type owl:NamedIndividual ,
                          skos:Concept ;
                 rdfs:label "Drawing"@en ;
                 skos:definition "Visual works produced by drawing, which is the application of lines on a surface, often paper, by using a pencil, pen, chalk, or some other tracing instrument to focus on the delineation of form rather than the application of color. This term is often defined broadly to refer to computer-generated images as well."@en ;
                 skos:editorialNote "Getty AAT http://vocab.getty.edu/page/aat/300033973"@en ;
                 skos:exactMatch <http://vocab.getty.edu/page/aat/300033973> ;
                 skos:inScheme :Restoration_Object ;
                 skos:prefLabel "Drawing"@en , "Disegno"@it ;
                 skos:topConceptOf :Restoration_Object .


###  https://w3id.org/crmrp#c_584a7943
crmrp:c_584a7943 rdf:type owl:NamedIndividual ,
                          skos:Concept ;
                 rdfs:label "Microscopes"@en ;
                 skos:broader :c_1fd6102e ;
                 skos:closeMatch <http://vocab.getty.edu/page/aat/300024594> ;
                 skos:definition "Optical instruments consisting of a lens or combination of lenses that allow the viewing of objects that are too small to be seen with the naked, unaided eye. The term may also be used for various types of instruments that use a stream of electrons (electron microscope), electromagnetic radiation (x-ray microscope), or other means other than light and lenses to magnify images of small objects."@en ;
                 skos:editorialNote "Getty AAT http://vocab.getty.edu/page/aat/300024594"@en ;
                 skos:inScheme :Archeometric_and_Diagnostic_Analysis ;
                 skos:topConceptOf :Archeometric_and_Diagnostic_Analysis ;
                 skos:prefLabel "Microscopes"@en , "Microscopia"@it .


###  https://w3id.org/crmrp#c_5885a25d
crmrp:c_5885a25d rdf:type owl:NamedIndividual ,
                          skos:Concept ;
                 rdfs:label "Deposit"@en ;
		 skos:closeMatch <http://vocab.getty.edu/page/aat/300264846> ;
                 skos:definition "Exogenic substance on the surface of an object."@en ;
                 skos:editorialNote "Getty AAT http://vocab.getty.edu/page/aat/300264846"@en ,
                                    "Getty Conservation Institute “Illustrated Glossary - Definitions of terms used for the graphic documentation of in situ floor mosaics”, “Mosaics In Situ Project”, Los Angeles, 2003"@en ,
                                    "Uni Cen/Ts 17135:2021 - Conservation of cultural heritage. General terms and definitions"@en ,
                                    "Verg`es-Belmin et al., ICOMOS-ISCS: Illustrated glossary on stone deterioration patterns, vol. XV. Icomos International Council on Monuments and Sites, 2008"@en ;
                 skos:inScheme :Alteration ;
                 skos:note "The preferred editorial note and the definition closest to the meaning is Uni Cen/Ts 17135:2021"@en ;
                 skos:prefLabel "Deposit"@en , "Deposito superficiale"@it ;
                 skos:topConceptOf :Alteration .


###  https://w3id.org/crmrp#c_58e9ad7f
crmrp:c_58e9ad7f rdf:type owl:NamedIndividual ,
                          skos:Concept ;
                 rdfs:label "Infill"@en ;
                 skos:altLabel "Filling"@en ;
                 skos:broader :c_24cc76d5 ;
                 skos:definition "Definition: To re-establish continuity between layers reinstating their structural and aesthetic properties."@en ;
                 skos:editorialNote "A. Weyer et al., “EwaGlos - European Illustrated Glossary of conservation terms for wall paintings and architectural surfaces”, Michael Imhof Verlag, Petersberg, Germany"@en ,
                                    "Getty AAT http://vocab.getty.edu/page/aat/300264840"@en ,
                                    "Getty Conservation Institute “Illustrated Glossary - Definitions of terms used for the graphic documentation of in situ floor mosaics”, “Mosaics In Situ Project”, Los Angeles, 2003"@en ;
                 skos:exactMatch <http://vocab.getty.edu/page/aat/30026484> ;
                 skos:inScheme :Intervention ;
                 skos:topConceptOf :Intervention ;
                 skos:note "The preferred editorial note and the definition closest to the meaning is EwaGlos - European Illustrated Glossary of conservation terms for wall paintings and architectural surfaces"@en ;
                 skos:prefLabel "Infill"@en , "Stuccatura"@it .


###  https://w3id.org/crmrp#c_5a83cd16
crmrp:c_5a83cd16 rdf:type owl:NamedIndividual ,
                          skos:Concept ;
                 rdfs:label "Chemical cleaning"@en ;
                 skos:broader :c_830e6744 ;
                 skos:definition "Physico-chemical cleaning aims to dissolve the materials to be removed by means of organic solvents, water and/or chemical reagents."@en ;
                 skos:editorialNote "Getty Conservation Institute “Illustrated Glossary - Technician Training for the Maintenance of In Situ Mosaics”, Los Angeles, 2013"@en ;
                 skos:inScheme :Intervention ;
                 skos:topConceptOf :Intervention ;
                 skos:prefLabel "Chemical cleaning"@en , "Pulitura chimico-fisica"@it .


###  https://w3id.org/crmrp#c_5b39b8a8
crmrp:c_5b39b8a8 rdf:type owl:NamedIndividual ,
                          skos:Concept ;
                 rdfs:label "Mecca gilding"@en ;
                 skos:broader :c_757ed6ec ;
                 skos:definition "Technique of applying paint known as mecha on tin or silver surfaces to achieve an optical effect similar to gilding"@en ;
                 skos:editorialNote "C. Giannini, “Dizionario del restauro - Tecniche diagnostica conservazione”, Nardini Editore, Firenze, 2010"@it ;
                 skos:inScheme :Execution_Technique ;
                 skos:topConceptOf :Execution_Technique ;
                 skos:note "International references could not be found"@en ;
                 skos:prefLabel "Mecca gilding"@en , "Meccatura"@it .


###  https://w3id.org/crmrp#c_5b7fce15
crmrp:c_5b7fce15 rdf:type owl:NamedIndividual ,
                          skos:Concept ;
                 rdfs:label "Sources and documents"@en ;
                 skos:definition "It comprise technical and scientific reports produced before and after each restoration. Moreover, restoration is a moment of recognition and in-depth study of an artwork, so it is not uncommon to review additional resources to broaden the knowledge of it, from historical and conservation perspective."@en ;
                 skos:inScheme :Documentation ;
                 skos:note "International references could not be found"@en ;
                 skos:prefLabel "Sources and documents"@en , "Fonti e documenti"@it ;
                 skos:topConceptOf :Documentation .


###  https://w3id.org/crmrp#c_5b84d202
crmrp:c_5b84d202 rdf:type owl:NamedIndividual ,
                          skos:Concept ;
                 rdfs:label "Transillumination"@en ;
                 skos:broader :c_1fd6102e ;
                 skos:definition "Technique of observation in the visible where the is placed between the illumination source and the observer. Transillumination can only be used only on materials that are partially or fully transparent to visible radiation"@en ;
                 skos:editorialNote "A. Aldrovandi, M. Picollo “Metodi di documentazione indagini non invasive sui dipinti”, Il Prato, Padova"@it ,
                                    "C. Giannini, “Dizionario del restauro - Tecniche diagnostica conservazione”, Nardini Editore, Firenze, 2010"@it ,
                                    "M.Ceroni, G.Elia, “Diagnostica per i beni culturali”, Alinea editrice, Firenze, 2008"@it ,
                                    "P.Cremonesi, E. Signorini, “Un approccio alla pulitura dei dipinti mobili”, Il Prato, Padova, 2016"@it ;
                 skos:inScheme :Archeometric_and_Diagnostic_Analysis ;
                 skos:topConceptOf :Archeometric_and_Diagnostic_Analysis ;
                 skos:note "International references could not be found, but the preferred editorial note and the definition closest to the meaning is Dizionario del restauro - Tecniche diagnostica conservazione"@en ;
                 skos:prefLabel "Transillumination"@en , "Transilluminazione"@it .


###  https://w3id.org/crmrp#c_5ca7c66b
crmrp:c_5ca7c66b rdf:type owl:NamedIndividual ,
                          skos:Concept ;
                 rdfs:label "Surface active agent"@en ;
                 skos:broader :c_5a83cd16 ;
                 skos:definition "Compound able to reduce the surface tension of liquid to which it is added."@en ;
                 skos:editorialNote "Getty AAT http://vocab.getty.edu/page/aat/300015321"@en ;
                 skos:exactMatch <http://vocab.getty.edu/page/aat/300015321> ;
                 skos:inScheme :Intervention ;
                 skos:topConceptOf :Intervention ;
                 skos:prefLabel "Surface active agent"@en , "Tensioattivo"@it .


###  https://w3id.org/crmrp#c_5cbafe21
crmrp:c_5cbafe21 rdf:type owl:NamedIndividual ,
                          skos:Concept ;
                 rdfs:label "Bloom"@en ;
                 skos:broader :c_df05cb61 ;
                 skos:definition "Haze on a surface"@en ;
                 skos:editorialNote "Getty AAT http://vocab.getty.edu/page/aat/300186215"@en ,
                                    "Uni Cen/Ts 17135:2021 - Conservation of cultural heritage. General terms and definitions"@en ;
                 skos:exactMatch <http://vocab.getty.edu/page/aat/300186215> ;
                 skos:inScheme :Alteration ;
                 skos:topConceptOf :Alteration ;
                 skos:note "The preferred editorial note and the definition closest to the meaning is Uni Cen/Ts 17135:2021"@en ;
                 skos:prefLabel "Bloom"@en , "Sbiancamento"@it .


###  https://w3id.org/crmrp#c_5d7824f1
crmrp:c_5d7824f1 rdf:type owl:NamedIndividual ,
                          skos:Concept ;
                 rdfs:label "Installations"@en ;
                 skos:definition "Works dating from the 1960s or later that use their exhibition space as part of their design. Demanding a viewer's active engagement, installations are often created by artists in direct opposition to the notion of permanent artwork, or art as a commodity."@en ;
                 skos:editorialNote "Getty AAT http://vocab.getty.edu/page/aat/300047896"@en ;
                 skos:exactMatch <http://vocab.getty.edu/page/aat/300047896> ;
                 skos:inScheme :Restoration_Object ;
                 skos:prefLabel "Installations"@en , "Installazione"@it ;
                 skos:topConceptOf :Restoration_Object .


###  https://w3id.org/crmrp#c_5e406e4a
crmrp:c_5e406e4a rdf:type owl:NamedIndividual ,
                          skos:Concept ;
                 rdfs:label "Charcoal"@en ;
                 skos:broader :c_044b6056 ;
                 skos:closeMatch <http://vocab.getty.edu/page/aat/300012862> ;
                 skos:definition "A black, porous carbonaceous material comprising the carbon-containing residue from burned wood (e.g., willow, maple, beech, linden or plum) or other organic containing materials such as bone, plants or animals. It is used as a drawing material, for filtering liquids or air, and for other purposes."@en ;
                 skos:editorialNote "Getty AAt http://vocab.getty.edu/page/aat/300012862"@en ;
                 skos:inScheme :Execution_Technique ;
                 skos:topConceptOf :Execution_Technique ;
                 skos:prefLabel "Charcoal"@en , "Carboncino"@it .


###  https://w3id.org/crmrp#c_5f3ffc3c
crmrp:c_5f3ffc3c rdf:type owl:NamedIndividual ,
                          skos:Concept ;
                 rdfs:label "Pitting"@en ;
                 skos:closeMatc <http://vocab.getty.edu/page/aat/300054130> ;
                 skos:definition "Numerous, densely packed shallow cavities on a surface."@en ;
                 skos:editorialNote "Getty AAT http://vocab.getty.edu/page/aat/300054130"@en ,
                                    "Getty Conservation Institute “Illustrated Glossary - Definitions of terms used for the graphic documentation of in situ floor mosaics”, “Mosaics In Situ Project”, Los Angeles, 2003"@en ,
                                    "Uni Cen/Ts 17135:2021 - Conservation of cultural heritage. General terms and definitions"@en ,
                                    "Verg`es-Belmin et al., ICOMOS-ISCS: Illustrated glossary on stone deterioration patterns, vol. XV. Icomos International Council on Monuments and Sites, 2008"@en ;
                 skos:inScheme :Alteration ;
                 skos:note "The preferred editorial note and the definition closest to the meaning is Uni Cen/Ts 17135:2021"@en ;
                 skos:prefLabel "Pitting"@en , "Pitting"@it ;
                 skos:topConceptOf :Alteration .


###  https://w3id.org/crmrp#c_5f7995a8
crmrp:c_5f7995a8 rdf:type owl:NamedIndividual ,
                          skos:Concept ;
                 rdfs:label "Wedge"@en ;
                 skos:broader :c_e8592f3b ;
                 skos:definition "A wooden element used in the restoration of painted or sculpted boards to restore cracks or splits in the support, or to give renewed stability and flatness to bent boards."@en ;
                 skos:editorialNote "C. Giannini, “Dizionario del restauro - Tecniche diagnostica conservazione”, Nardini Editore, Firenze, 2010"@it ;
                 skos:inScheme :Intervention ;
                 skos:topConceptOf :Intervention ;
                 skos:note "International references could not be found"@en ;
                 skos:prefLabel "Wedge"@en , "Cuneo"@it .


###  https://w3id.org/crmrp#c_602a357d
crmrp:c_602a357d rdf:type owl:NamedIndividual ,
                          skos:Concept ;
                 rdfs:label "Visible diffuse light"@en ;
                 skos:broader :c_1fd6102e ;
                 skos:definition "Photographs obtained by recreating, even artificially, lighting conditions that make the composition and its colour values most readable."@en ;
                 skos:editorialNote "A. Aldrovandi, M. Picollo “Metodi di documentazione indagini non invasive sui dipinti”, Il Prato, Padova, 1999"@it ,
                                    "V. Marcovaz, “Indagine e diagnostica fotografica per i beni culturali”, Isiaurbino, Trieste, 2016"@it ;
                 skos:inScheme :Archeometric_and_Diagnostic_Analysis ;
                 skos:topConceptOf :Archeometric_and_Diagnostic_Analysis ;
                 skos:prefLabel "Visible diffuse light"@en , "Fotografia a luce diffusa"@it .


###  https://w3id.org/crmrp#c_602dbf50
crmrp:c_602dbf50 rdf:type owl:NamedIndividual ,
                          skos:Concept ;
                 rdfs:label "Opus tessellatum"@en ;
                 skos:broader :c_b9a6a1c8 ;
                 skos:definition "Pavement made of small, regularly shaped, usually quadrangular, elements (generally 4 to 20 millimetres wide) placed side by side in rows. These elements, called tesserae, are obtained by cutting different materials such as stone (often marble or limestone), ceramic or glass."@en ;
                 skos:editorialNote "C. Fiori “Teoria e tecniche per la conservazione del mosaico”, Il Prato, Padova, 2002"@it ,
                                    "C. Giannini, “Dizionario del restauro - Tecniche diagnostica conservazione”, Nardini Editore, Firenze, 2010"@it ,
                                    "Getty Conservation Institute “Illustrated Glossary - Technician Training for the Maintenance of In Situ Mosaics”, Los Angeles, 2013"@en ;
                 skos:inScheme :Execution_Technique ;
                 skos:topConceptOf :Execution_Technique ;
                 skos:prefLabel "Opus tessellatum"@en , "Opus tessellatum"@it .


###  https://w3id.org/crmrp#c_607d4549
crmrp:c_607d4549 rdf:type owl:NamedIndividual ,
                          skos:Concept ;
                 rdfs:label "Removal"@en ;
                 skos:altLabel "Uncovering"@en ;
                 skos:definition "The removal of extraneous components from the artwork, such as plastering carried out during past restorations, repainting and/or layers of paintwork."@en ;
                 skos:editorialNote " A. Weyer et al., “EwaGlos - European Illustrated Glossary of conservation terms for wall paintings and architectural surfaces”, Michael Imhof Verlag, Petersberg, Germany"@en ,
                                    "Getty Conservation Institute “Illustrated Glossary - Definitions of terms used for the graphic documentation of in situ floor mosaics”, “Mosaics In Situ Project”, Los Angeles, 2003"@en ;
                 skos:inScheme :Intervention ;
                 skos:note "The preferred editorial note and the definition closest to the meaning is Getty Conservation Institute “Illustrated Glossary - Definitions of terms used for the graphic documentation of in situ floor mosaics”, “Mosaics In Situ Project”, Los Angeles, 2003"@en ;
                 skos:prefLabel "Removal"@en , "Rimozione"@it ;
                 skos:topConceptOf :Intervention .


###  https://w3id.org/crmrp#c_60903036
crmrp:c_60903036 rdf:type owl:NamedIndividual ,
                          skos:Concept ;
                 rdfs:label "Cretto"@en ;
                 skos:broader :c_8c762c3e ;
                 skos:definition "A term used to indicate a micro-fracture of the paint film that may result from phenomena of drying of the oily binder. In general, the crack is more pronounced in correspondence with dark dark and brown colours because earth colours are among the colours that absorb the most binder."@en ;
                 skos:editorialNote "C. Giannini, “Dizionario del restauro - Tecniche diagnostica conservazione”, Nardini Editore, Firenze, 2010"@it ;
                 skos:inScheme :Alteration ;
                 skos:topConceptOf :Alteration ;
                 skos:note "International references could not be found"@en ;
                 skos:prefLabel "Cretto"@en , "Cretto"@it .


###  https://w3id.org/crmrp#c_6108ee3a
crmrp:c_6108ee3a rdf:type owl:NamedIndividual ,
                          skos:Concept ;
                 rdfs:label "Surface profile measurement"@en ;
                 skos:broader :c_1fd6102e ;
                 skos:definition "To obtain this value, the profile is measured at a sufficient number of points to characterise the surface. It includes profilometry, rugosimetry and thicknessimetry."@en ;
                 skos:editorialNote "C. Giannini, “Dizionario del restauro - Tecniche diagnostica conservazione”, Nardini Editore, Firenze, 2010"@it ,
                                    "UNI EN 10049:2014 Misurazione della rugosità media Ra e del numero dei picchi RPc sui prodotti piani metallici"@it ,
                                    "UNI EN 14127:2011 Prove non distruttive - Misurazione dello spessore mediante ultrasuoni"@it ,
                                    "UNI EN ISO 18452:2016 Ceramiche fini (ceramiche avanzate, ceramiche tecniche avanzate) - Determinazione dello spessore di film ceramici con un profilometro a contatto"@it ;
                 skos:inScheme :Archeometric_and_Diagnostic_Analysis ;
                 skos:topConceptOf :Archeometric_and_Diagnostic_Analysis ;
                 skos:note "International references could not be found"@en ;
                 skos:prefLabel "Surface profile measurement"@en , "Misurazione profilo di superficie"@it .


###  https://w3id.org/crmrp#c_612bc334
crmrp:c_612bc334 rdf:type owl:NamedIndividual ,
                          skos:Concept ;
                 rdfs:label "Forma a tasselli"@en ;
                 skos:broader :c_17157ccd ;
                 skos:definition "Plaster form also known as the Good Form or Real Form because it is made up of many detachable elements, once made it allows numerous copies to be made and a long preservation period."@en ;
                 skos:editorialNote "C. Giannini, “Dizionario del restauro - Tecniche diagnostica conservazione”, Nardini Editore, Firenze, 2010"@it ;
                 skos:inScheme :Execution_Technique ;
                 skos:topConceptOf :Execution_Technique ;
                 skos:note "It was decided not to proceed with the English translation in order to avoid possible lexical errors and misunderstandings."@en ;
                 skos:prefLabel "Forma a tasselli"@en , "Forma a tasselli"@it .


###  https://w3id.org/crmrp#c_613f625a
crmrp:c_613f625a rdf:type owl:NamedIndividual ,
                          skos:Concept ;
                 rdfs:label "Structural monitoring"@en ;
                 skos:broader :c_1fd6102e ;
                 skos:definition "A structural monitoring system is a set of tools and procedures designed to monitor and assess the condition of a structure.It includes: endoscope, fissurimeter, pacometer"@en ;
                 skos:inScheme :Archeometric_and_Diagnostic_Analysis ;
                 skos:topConceptOf :Archeometric_and_Diagnostic_Analysis ;
                 skos:note "International references could not be found."@en ;
                 skos:prefLabel "Structural monitoring"@en , "Monitoraggio strutturale"@it .


###  https://w3id.org/crmrp#c_615accd9
crmrp:c_615accd9 rdf:type owl:NamedIndividual ,
                          skos:Concept ;
                 rdfs:label "Red chalk"@en ;
                 skos:broader :c_044b6056 ;
                 skos:definition "Drawing medium made from natural red clay containing iron ocher, ranging in color from reddish brown to blood red. It was used for wall paintings by ancient Egyptians and Romans; in the 16th century it was a popular drawing medium. Originally cut from deposits but later fabricated from the same material."@en ;
                 skos:editorialNote "Getty AAT http://vocab.getty.edu/page/aat/300080064"@en ;
                 skos:exactMatch <http://vocab.getty.edu/page/aat/300080064> ;
                 skos:inScheme :Execution_Technique ;
                 skos:topConceptOf :Execution_Technique ;
                 skos:prefLabel "Red chalk"@en , "Sanguigna"@it .


###  https://w3id.org/crmrp#c_61d92422
crmrp:c_61d92422 rdf:type owl:NamedIndividual ,
                          skos:Concept ;
                 rdfs:label "Humidity"@en ;
                 skos:definition "The amount of moisture present in the air or in a porous material (here referredto as moisture)."@en ;
                 skos:editorialNote "A. Weyer et al., “EwaGlos - European Illustrated Glossary of conservation terms for wall paintings and architectural surfaces”, Michael Imhof Verlag, Petersberg, Germany"@en ;
                 skos:inScheme :Alteration ;
                 skos:prefLabel "Humidity"@en , "Umidità"@it ;
                 skos:topConceptOf :Alteration .


###  https://w3id.org/crmrp#c_6278f32b
crmrp:c_6278f32b rdf:type owl:NamedIndividual ,
                          skos:Concept ;
                 rdfs:label "Radiography"@en ;
                 skos:broader :c_1fd6102e ;
                 skos:definition "The making of radiographs, images produced on photographic film by a radiation other than light, especially x-rays or gamma rays. Modern radiography systems are moving away from x-ray sensitive film to produce these images, with a digital plate replacing film."@en ;
                 skos:editorialNote "Getty AAT http://vocab.getty.edu/page/aat/300053450"@en ;
                 skos:exactMatch <http://vocab.getty.edu/page/aat/300053450> ;
                 skos:inScheme :Archeometric_and_Diagnostic_Analysis ;
                 skos:topConceptOf :Archeometric_and_Diagnostic_Analysis ;
                 skos:prefLabel "Radiography"@en , "Radiografia"@it .


###  https://w3id.org/crmrp#c_6407466f
crmrp:c_6407466f rdf:type owl:NamedIndividual ,
                          skos:Concept ;
                 rdfs:label "Metal"@en ;
                 skos:closeMatch <http://vocab.getty.edu/page/aat/300010900> ;
                 skos:definition "Any of a large group of substances that typically show a characteristic luster, are good conductors of electricity and heat, are opaque, can be fused, and are usually malleable or ductile."@en ;
                 skos:editorialNote "Getty AAT http://vocab.getty.edu/page/aat/300010900"@en ;
                 skos:inScheme :Material ;
                 skos:prefLabel "Metal"@en , "Metallo"@it ;
                 skos:topConceptOf :Material .


###  https://w3id.org/crmrp#c_6626f18c
crmrp:c_6626f18c rdf:type owl:NamedIndividual ,
                          skos:Concept ;
                 rdfs:label "Wall painting"@en ;
                 skos:editorialNote "A. Weyer et al., “EwaGlos - European Illustrated Glossary of conservation terms for wall paintings and architectural surfaces”, Michael Imhof Verlag, Petersberg, Germany"@en ;
                 skos:inScheme :Execution_Technique ;
                 skos:note "International references could not be found"@en ;
		 skos:prefLabel "Wall painting"@en , "Tecnica dipinto murale"@it ;
                 skos:topConceptOf :Execution_Technique .


###  https://w3id.org/crmrp#c_66314288
crmrp:c_66314288 rdf:type owl:NamedIndividual ,
                          skos:Concept ;
                 rdfs:label "Stampo a buona forma"@en ;
                 skos:broader :c_17157ccd ;
                 skos:definition "A mould that allows multiple copies to be made because it does not need to be broken or modified during demoulding"@en ;
                 skos:editorialNote "C. Giannini, “Dizionario del restauro - Tecniche diagnostica conservazione”, Nardini Editore, Firenze, 2010"@it ,
                                    "P. Clérin, “Manuale di scultura - Tecniche, materiali, realizzazioni”, Sovera editore, Roma, 1995"@it ;
                 skos:inScheme :Execution_Technique ;
                 skos:topConceptOf :Execution_Technique;
                 skos:note "It was decided not to proceed with the English translation in order to avoid possible lexical errors and misunderstandings."@en ;
                 skos:prefLabel "Stampo a buona forma"@en , "Stampo a buona forma"@it .


###  https://w3id.org/crmrp#c_6671d452
crmrp:c_6671d452 rdf:type owl:NamedIndividual ,
                          skos:Concept ;
                 rdfs:label "Silver"@en ;
                 skos:broader :c_6407466f ;
                 skos:definition "Pure metallic element having symbol Ag and atomic number 47; a malleable, ductile, white metal with characteristic sheen, considered a precious metal. Silver is widely distributed throughout the world, occurring rarely as metallic silver (in Peru, Norway) but more often as silver-gold alloys and silver ore. Today silver is obtained as a byproduct in the refinement of gold, lead, copper, or zinc ores. Silver was smelted from the ore galena as early as 3800 BCE. As a pure metal, silver is second to gold in malleability and ductility, can be polished to a highly reflective surface, and used -- typically in an alloy -- in jewelry, coinage, photography, mirrors, electrical contacts, and tableware."@en ;
                 skos:editorialNote "Getty AAT http://vocab.getty.edu/page/aat/300011029"@en ;
                 skos:exactMatch <http://vocab.getty.edu/page/aat/30001102> ;
                 skos:inScheme :Material ;
                 skos:topConceptOf :Material ;
                 skos:prefLabel "Silver"@en , "Argento"@it .


###  https://w3id.org/crmrp#c_6692ec2f
crmrp:c_6692ec2f rdf:type owl:NamedIndividual ,
                          skos:Concept ;
                 rdfs:label "Animal origin"@en ;
                 skos:definition "An animal artefact is an object made from materials derived from animals, such as bones, horns, ivory, leather, silk, wool, feathers or shells. Such artefacts may be tools, ornaments, garments or works of art, often with cultural, practical or symbolic meanings"@en ;
                 skos:inScheme :Material ;
                 skos:note "International references could not be found"@en ;
                 skos:prefLabel "Animal origin"@en , "Origine animale"@it ;
                 skos:topConceptOf :Material .


###  https://w3id.org/crmrp#c_66ff714b
crmrp:c_66ff714b rdf:type owl:NamedIndividual ,
                          skos:Concept ;
                 rdfs:label "Physical-mechanical testing"@en ;
                 skos:broader :c_abed88a5 ;
                 skos:defintion "Physical-mechanical tests are used to obtain information about the physical performance and mechanical behaviour of a component."@en ;
                 skos:editorialNote "S. Volpin e L. Appolonia “Le analisi di laboratorio applicate ai beni artistici policromi”, Il Prato, Padova, 1999"@it ;
                 skos:inScheme :Archeometric_and_Diagnostic_Analysis ;
                 skos:topConceptOf :Archeometric_and_Diagnostic_Analysis ;
                 skos:note "International references could not be found"@en ;
                 skos:prefLabel "Physical-mechanical testing"@en , "Test fisico-meccanico"@it .


###  https://w3id.org/crmrp#c_687df059
crmrp:c_687df059 rdf:type owl:NamedIndividual ,
                          skos:Concept ;
                 rdfs:label "Decorative apparatus of architecture"@en ;
                 skos:altLabel "Surface elements (architectural)"@en ;
                 skos:closeMatch <http://vocab.getty.edu/page/aat/300001987> ;
                 skos:definition "Architectural elements or components located on the surface"@en ;
                 skos:inScheme :Restoration_Object ;
		 skos:editorialNote "Getty AAT http://vocab.getty.edu/page/aat/300001987"@en ;
                 skos:prefLabel "Decorative apparatus of architecture"@en , "Apparato decorativo dell'architettura"@it ;
                 skos:topConceptOf :Restoration_Object .


###  https://w3id.org/crmrp#c_68cc67d0
crmrp:c_68cc67d0 rdf:type owl:NamedIndividual ,
                          skos:Concept ;
                 rdfs:label "Polarising optical microscope in reflected and transmitted light"@en ;
                 skos:broader :c_7ee727f3 ;
                 skos:definition "A polarising microscope, or transmitted-light polarising optical microscope, also known as a petrography microscope, is an optical microscope modified to use polarised light for sample observation."@en ;
                 skos:inScheme :Archeometric_and_Diagnostic_Analysis ;
                 skos:topConceptOf :Archeometric_and_Diagnostic_Analysis ;
		 skos:editorialNote "M.Ceroni, G.Elia, “Diagnostica per i beni culturali”, Alinea editrice, Firenze, 2008"@it ;
                 skos:prefLabel "Polarising optical microscope in reflected and transmitted light"@en , "Microscopio ottico polarizzatore in luce trasmessa e riflessa"@it .


###  https://w3id.org/crmrp#c_6920ec3f
crmrp:c_6920ec3f rdf:type owl:NamedIndividual ,
                          skos:Concept ;
                 rdfs:label "Tempera grassa"@en ;
                 skos:broader :c_77acfccf ;
                 skos:definition "Tempera grassa is produced by mixing egg yolk with linseed oil. Used extensively in the 15th century with the emergence of the first paintings on canvas following Flemish influence."@en ;
                 skos:editorialNote "C. Giannini, “Dizionario del restauro - Tecniche diagnostica conservazione”, Nardini Editore, Firenze, 2010"@it ;
                 skos:inScheme :Execution_Technique ;
                 skos:topConceptOf :Execution_Technique ;
                 skos:note "It was decided not to proceed with the English translation in order to avoid possible lexical errors and misunderstandings."@en ;
                 skos:prefLabel "Tempera grassa"@en , "Tempera grassa"@it .


###  https://w3id.org/crmrp#c_694546c0
crmrp:c_694546c0 rdf:type owl:NamedIndividual ,
                          skos:Concept ;
                 rdfs:label "Burins"@en ;
                 skos:broader :c_aee6a805 ;
                 skos:closeMatch <http://vocab.getty.edu/page/aat/300193147> ;
                 skos:definition "Tools used in printmaking for engraving metal plates or end-grain wood blocks, consisting of a small steel rod, of square or lozenge section, with a sharpened point, and having a half-round wood handle that fits in the palm of the hand. In the context of archaeology, a specialized flake or blade with a chisel edge; used to carve or engrave softer materials such as bone, wood, or antler. For various tools for chasing or engraving metal or wood, use gravers."@en ;
                 skos:editorialNote "Getty AAT http://vocab.getty.edu/page/aat/300193147"@en ;
                 skos:inScheme :Execution_Technique ;
                 skos:topConceptOf :Execution_Technique ;
                 skos:prefLabel "Burins"@en , "Bulino"@it .


###  https://w3id.org/crmrp#c_6a6dc187
crmrp:c_6a6dc187 rdf:type owl:NamedIndividual ,
                          skos:Concept ;
                 rdfs:label "Intarsia"@en ;
                 skos:broader :c_b9a6a1c8 ;
                 skos:definition "Type of sectional mosaic in which elements are cut with great precision and juxtaposed with each other so that the com almost invisible. The stones are chosen in so as to exploit the material's own colour material to achieve effects of chiaroscuro, shadows and shading."@en ;
                 skos:editorialNote "C. Fiori “Teoria e tecniche per la conservazione del mosaico”, Il Prato, Padova, 2002"@it ,
                                    "C. Giannini, “Dizionario del restauro - Tecniche diagnostica conservazione”, Nardini Editore, Firenze, 2010"@it ,
                                    "The Getty Conservation Institute, “The structural conservation of panel paintings”, Proceedings of a Symposium at the J. Paul Getty Museum, 24 - 28 April 1995"@en ;
                 skos:inScheme :Execution_Technique ;
                 skos:topConceptOf :Execution_Technique ;
                 skos:prefLabel "Intarsia"@en , "Commesso/Intarsio"@it .


###  https://w3id.org/crmrp#c_6aacbe2f
crmrp:c_6aacbe2f rdf:type owl:NamedIndividual ,
                          skos:Concept ;
                 rdfs:label "Exfoliation"@en ;
                 skos:altLabel "Delamination"@en ,
                               "Peeling"@en , "Delaminazione"@it ;
                 skos:definition "Separation into layers"@en ;
                 skos:editorialNote "A. Weyer et al., “EwaGlos - European Illustrated Glossary of conservation terms for wall paintings and architectural surfaces”, Michael Imhof Verlag, Petersberg, Germany"@en ,
                                    "Getty Conservation Institute “Illustrated Glossary - Definitions of terms used for the graphic documentation of in situ floor mosaics”, “Mosaics In Situ Project”, Los Angeles, 2003"@en ,
                                    "Uni Cen/Ts 17135:2021 - Conservation of cultural heritage. General terms and definitions"@en ,
                                    "Verg`es-Belmin et al., ICOMOS-ISCS: Illustrated glossary on stone deterioration patterns, vol. XV. Icomos International Council on Monuments and Sites, 2008"@en ;
                 skos:inScheme :Alteration ;
                 skos:prefLabel "Exfoliation"@en , "Esfoliazione"@it ;
                 skos:topConceptOf :Alteration .



###  https://w3id.org/crmrp#c_6d269f19
crmrp:c_6d269f19 rdf:type owl:NamedIndividual ,
                          skos:Concept ;
                 rdfs:label "Mecca gilding"@en ;
                 skos:broader :c_4d471b17 ;
                 skos:definition "Technique of applying paint known as mecha on tin or silver surfaces to achieve an optical effect similar to gilding"@en ;
                 skos:editorialNote "C. Giannini, “Dizionario del restauro - Tecniche diagnostica conservazione”, Nardini Editore, Firenze, 2010"@it ;
                 skos:inScheme :Execution_Technique ;
                 skos:topConceptOf :Execution_Technique ;
                 skos:note "International references could not be found"@en ;
                 skos:prefLabel "Mecca gilding"@en , "Meccatura"@it .


###  https://w3id.org/crmrp#c_6d7b8feb
crmrp:c_6d7b8feb rdf:type owl:NamedIndividual ,
                          skos:Concept ;
                 rdfs:label "Active xylophagous attack"@en ;
                 skos:broader :c_49988b8d ;
                 skos:definition "A xylophagus attack still in progress"@en ;
                 skos:inScheme :Alteration ;
                 skos:topConceptOf :Alteration ;
                 skos:note "International references could not be found"@en ;
                 skos:prefLabel "Active xylophagous attack"@en , "Attacco xilofago attivo"@it .


###  https://w3id.org/crmrp#c_6dba4fb3
crmrp:c_6dba4fb3 rdf:type owl:NamedIndividual ,
                          skos:Concept ;
                 rdfs:label "Loss"@en ;
                 skos:altLabel "Missing part"@en , "Mancanza"@it ;
                 skos:definition "Missing part of an object."@en ;
                 skos:editorialNote "Uni Cen/Ts 17135:2021 - Conservation of cultural heritage. General terms and definitions"@en ,
                                    "Verg`es-Belmin et al., ICOMOS-ISCS: Illustrated glossary on stone deterioration patterns, vol. XV. Icomos International Council on Monuments and Sites, 2008"@en ;
                 skos:inScheme :Alteration ;
                 skos:note "The preferred editorial note and the definition closest to the meaning is Uni Cen/Ts 17135:2021"@en ;
                 skos:prefLabel "Loss"@en , "Perdita"@it ;
                 skos:topConceptOf :Alteration .


###  https://w3id.org/crmrp#c_707c9e81
crmrp:c_707c9e81 rdf:type owl:NamedIndividual ,
                          skos:Concept ;
                 rdfs:label "Mould"@en ;
                 skos:broader :c_3ef20257 ;
                 skos:definition "Microscopic fungus which colonies, to the naked eye, look like a downy film or a network or star-like millimetric patches of filaments of diverse colours (white, grey, black)."@en ;
                 skos:editorialNote "Getty AAT http://vocab.getty.edu/page/aat/300378932"@en ,
                                    "Verg`es-Belmin et al., ICOMOS-ISCS: Illustrated glossary on stone deterioration patterns, vol. XV. Icomos International Council on Monuments and Sites, 2008"@en ;
                 skos:exactMatch <http://vocab.getty.edu/page/aat/300378932> ;
                 skos:inScheme :Alteration ;
                 skos:topConceptOf :Alteration;
                 skos:note "The preferred editorial note and the definition closest to the meaning is ICOMOS-ISCS: Illustrated glossary on stone deterioration patterns"@en ;
                 skos:prefLabel "Mould"@en , "Muffa"@it .


###  https://w3id.org/crmrp#c_717419a3
crmrp:c_717419a3 rdf:type owl:NamedIndividual ,
                          skos:Concept ;
                 rdfs:label "Plaster"@en ;
                 skos:broader :c_34d8fe56 ;
                 skos:definition "Protective and/or decorative coat which is applied to architectural surfaces. It is also used for moulding and casting decorative elements."@en ;
                 skos:editorialNote "A. Weyer et al., “EwaGlos - European Illustrated Glossary of conservation terms for wall paintings and architectural surfaces”, Michael Imhof Verlag, Petersberg, Germany"@en ;
                 skos:inScheme :Material ;
                 skos:topConceptOf :Material; 
                 skos:prefLabel "Plaster"@en , "Intonaco"@it .


###  https://w3id.org/crmrp#c_71e8a300
crmrp:c_71e8a300 rdf:type owl:NamedIndividual ,
                          skos:Concept ;
                 rdfs:label "Photogrammetric dataset"@en ;
                 skos:broader :c_773e0829 ;
                 skos:definition "Collection of all the photographs necessary to obtain a three-dimensional model"@en ;
                 skos:inScheme :Documentation ;
                 skos:topConceptOf :Documentation ; 
                 skos:note "International references could not be found"@en ;
                 skos:prefLabel "Photogrammetric dataset"@en , "Dataset fotogrammetrico"@it .


###  https://w3id.org/crmrp#c_73b09074
crmrp:c_73b09074 rdf:type owl:NamedIndividual ,
                          skos:Concept ;
                 rdfs:label "Stripe soiling"@en ;
                 skos:altLabel "Soiling"@en ;
                 skos:closeMatch <http://vocab.getty.edu/page/aat/300379469> ;
                 skos:definition "Deposit of a very thin layer of exogenous particles (eg. soot) giving a dirty appearance to the stone surface."@en ;
                 skos:editorialNote "Getty AAT http://vocab.getty.edu/page/aat/300379469"@en ,
                                    "Verg`es-Belmin et al., ICOMOS-ISCS: Illustrated glossary on stone deterioration patterns, vol. XV. Icomos International Council on Monuments and Sites, 2008"@en ;
                 skos:inScheme :Alteration ;
                 skos:note "The preferred editorial note and the definition closest to the meaning is ICOMOS-ISCS: Illustrated glossary on stone deterioration patterns"@en ;
                 skos:prefLabel "Stripe soiling"@en , "Colatura"@it ;
                 skos:topConceptOf :Alteration .


###  https://w3id.org/crmrp#c_7548d8b4
crmrp:c_7548d8b4 rdf:type owl:NamedIndividual ,
                          skos:Concept ;
                 rdfs:label "Synthetic polymer"@en ;
                 skos:altLabel "Polymers"@en ;
                 skos:closeMatch <http://vocab.getty.edu/page/aat/300218300> ;
                 skos:definition "High molecular weight compounds formed by the combination of one or more monomers, formed by the multiplication of molecules of the same species to produce a new compound with the same empirical formula but with higher molecular weight. Use copolymers for materials that combine molecules of differing chemical compounds."@en ;
                 skos:editorialNote "Getty AAT http://vocab.getty.edu/page/aat/300218300"@en ;
                 skos:inScheme :Material ;
                 skos:prefLabel "Synthetic polymer"@en , "Polimero sintetico"@it ;
                 skos:topConceptOf :Material .


###  https://w3id.org/crmrp#c_757ed6ec
crmrp:c_757ed6ec rdf:type owl:NamedIndividual ,
                          skos:Concept ;
                 rdfs:label "Water gilding"@en ;
                 skos:broader :c_8af455cd ;
                 skos:closeMatch <http://vocab.getty.edu/page/aat/300053795> ;
                 skos:definition "Technique of adhering precious-metal leaf to a gesso or bole ground that is moistened with water before each leaf is laid."@en ;
                 skos:editorialNote "Getty AAT http://vocab.getty.edu/page/aat/300053795"@en ;
                 skos:inScheme :Execution_Technique ;
                 skos:topConceptOf :Execution_Technique ;
                 skos:prefLabel "Water gilding"@en , "A guazzo"@it .


###  https://w3id.org/crmrp#c_75d8773c
crmrp:c_75d8773c rdf:type owl:NamedIndividual ,
                          skos:Concept ;
                 rdfs:label "Fusione a staffa"@en ;
                 skos:broader :c_0a9f4d42 ;
                 skos:definition "Stirrup casting allows for the re-use of dies: the model, which must necessarily be made of a consistent material, is inserted into a ‘stirrup’ composed of two coupling iron frames, into which refractory earth is pressed, obtaining the negative shape of the model to be reproduced, which is then removed and into the hollow that has been formed and through the previously prepared inlet channels, molten metal is thrown, which will fill all the empty spaces."@en ;
                 skos:editorialNote "A.Giuffredi “Formatura e fonderia”, Alinea editrice, Firenze, 2010"@it ,
                                    "C. Giannini, “Dizionario del restauro - Tecniche diagnostica conservazione”, Nardini Editore, Firenze, 2010"@it ;
                 skos:inScheme :Execution_Technique ;
                 skos:topConceptOf :Execution_Technique ;
                 skos:note "International references could not be found, but the preferred editorial note and the definition closest to the meaning is Formatura e fonderia"@en ;
                 skos:prefLabel "Fusione a staffa"@en , "Fusione a staffa"@it .


###  https://w3id.org/crmrp#c_7621b79d
crmrp:c_7621b79d rdf:type owl:NamedIndividual ,
                          skos:Concept ;
                 rdfs:label "Paintings"@en ;
                 skos:definition "Unique works in which images are formed primarily by the direct application of pigments suspended in oil, water, egg yolk, molten wax, or other liquid, arranged in masses of color, onto a generally two-dimensional surface."@en ;
                 skos:editorialNote "Getty AAT http://vocab.getty.edu/page/aat/300033618"@en ;
                 skos:exactMatch <http://vocab.getty.edu/page/aat/300033618> ;
                 skos:inScheme :Restoration_Object ;
                 skos:prefLabel "Painting"@en , "Dipinto"@it ;
                 skos:topConceptOf :Restoration_Object .


###  https://w3id.org/crmrp#c_767414bb
crmrp:c_767414bb rdf:type owl:NamedIndividual ,
                          skos:Concept ;
                 rdfs:label "Inactive xylophagous attack"@en ;
                 skos:broader :c_49988b8d ;
                 skos:definition "an inactive xylophagus attack."@en ;
                 skos:inScheme :Alteration ;
                 skos:topConceptOf :Alteration ;
                 skos:note "International references could not be found"@en ;
                 skos:prefLabel "Inactive xylophagous attack"@en , "Attacco xilofago inattivo"@it .


###  https://w3id.org/crmrp#c_773e0829
crmrp:c_773e0829 rdf:type owl:NamedIndividual ,
                          skos:Concept ;
                 rdfs:label "Photo documentation"@en ;
                 skos:altLabel "Photodocumentation"@en ;
                 skos:definition "The collection of all photographs concerning the work of art in question"@en ;
                 skos:inScheme :Documentation ;
                 skos:note "International references could not be found"@en ;
                 skos:prefLabel "Photo documentation"@en , "Documentazione fotografica"@it ;
                 skos:topConceptOf :Documentation .


###  https://w3id.org/crmrp#c_777a4068
crmrp:c_777a4068 rdf:type owl:NamedIndividual ,
                          skos:Concept ;
                 rdfs:label "Lacuna"@en ;
                 skos:altLabel "Lacunae"@en ;
                 skos:closeMatch <http://vocab.getty.edu/page/aat/300263354> ;
                 skos:definition "Loss with a form defined by its relation to the rest of the object."@en ;
                 skos:editorialNote "A. Weyer et al., “EwaGlos - European Illustrated Glossary of conservation terms for wall paintings and architectural surfaces”, Michael Imhof Verlag, Petersberg, Germany"@en ,
                                    "Getty AAT http://vocab.getty.edu/page/aat/300263354"@en ,
                                    "Uni Cen/Ts 17135:2021 - Conservation of cultural heritage. General terms and definitions"@en ,
                                    "Verg`es-Belmin et al., ICOMOS-ISCS: Illustrated glossary on stone deterioration patterns, vol. XV. Icomos International Council on Monuments and Sites, 2008"@en ;
                 skos:inScheme :Alteration ;
                 skos:note "The preferred editorial note and the definition closest to the meaning is Uni Cen/Ts 17135:2021"@en ;
                 skos:prefLabel "Lacuna"@en , "Lacuna"@it ;
                 skos:topConceptOf :Alteration .


###  https://w3id.org/crmrp#c_77acfccf
crmrp:c_77acfccf rdf:type owl:NamedIndividual ,
                          skos:Concept ;
                 rdfs:label "Tempera"@en ;
                 skos:broader :c_143349b9 , :c_051209b3 , :c_044b6056 ;
                 skos:definition "Paint formed of an emulsion of fatty and watery constituents. The standard emulsion is usually created with egg yolk and water, with variants of man-made emulsions created with whole egg, linseed oil, casein glue, gum, or wax."@en ;
                 skos:editorialNote "Getty AAT http://vocab.getty.edu/page/aat/300015062"@en ;
                 skos:exactMatch <http://vocab.getty.edu/page/aat/300015062> ;
                 skos:inScheme :Execution_Technique ;
                 skos:topConceptOf :Execution_Technique ;
                 skos:prefLabel "Tempera"@en , "Tempera"@it .


###  https://w3id.org/crmrp#c_789c3e32
crmrp:c_789c3e32 rdf:type owl:NamedIndividual ,
                          skos:Concept ;
                 rdfs:label "Spectroscopy"@en ;
                 skos:broader :c_abed88a5 ;
                 skos:closeMatch <http://vocab.getty.edu/page/aat/300179535> ;
                 skos:definition "Means of observing the way a substance transmits, emits, or responds to various wavelengths in the electromagnetic energy spectrum."@en ;
                 skos:editorialNote "Getty AAT http://vocab.getty.edu/page/aat/300179535"@en ;
                 skos:inScheme :Archeometric_and_Diagnostic_Analysis ;
                 skos:topConceptOf :Archeometric_and_Diagnostic_Analysis ;
                 skos:prefLabel "Spectroscopy"@en , "Spettroscopia"@it .


###  https://w3id.org/crmrp#c_78efb0c7
crmrp:c_78efb0c7 rdf:type owl:NamedIndividual ,
                          skos:Concept ;
                 rdfs:label "Fresco"@en ;
                 skos:broader :c_6626f18c ;
                 skos:definition "A wall painting technique in which pigments are mixed with clear water and applied to a fresh and still damp lime plaster (intonaco); pigments are fixed inside a thin layer of calcium carbonate formed on the plaster surface (carbonation)."@en ;
                 skos:editorialNote "A. Weyer et al., “EwaGlos - European Illustrated Glossary of conservation terms for wall paintings and architectural surfaces”, Michael Imhof Verlag, Petersberg, Germany"@en ,
                                    "Getty AAT http://vocab.getty.edu/page/aat/300177433"@en ;
                 skos:exactMatch <http://vocab.getty.edu/page/aat/300177433> ;
                 skos:inScheme :Execution_Technique ;
                 skos:topConceptOf :Execution_Technique ;
                 skos:note "The preferred editorial note and the definition closest to the meaning is EwaGlos - European Illustrated Glossary of conservation terms for wall paintings and architectural surfaces"@en ;
                 skos:prefLabel "Fresco"@en , "Affresco"@it .


###  https://w3id.org/crmrp#c_7988bd54
crmrp:c_7988bd54 rdf:type owl:NamedIndividual ,
                          skos:Concept ;
                 rdfs:label "Bioluminometric analysis"@en ;
                 skos:broader :c_1fd6102e ;
                 skos:definition " The bioluminometer measures the light generated, indicating the level of contamination of a surface."@en ;
                 skos:inScheme :Archeometric_and_Diagnostic_Analysis ;
                 skos:topConceptOf :Archeometric_and_Diagnostic_Analysis ;
                 skos:note "International references could not be found"@en ;
                 skos:prefLabel "Bioluminometric analysis"@en , "Analisi bioluminometrica"@it .


###  https://w3id.org/crmrp#c_7c664d13
crmrp:c_7c664d13 rdf:type owl:NamedIndividual ,
                          skos:Concept ;
                 rdfs:label "Computerised Axial Tomography (CAT)"@en ;
                 skos:broader :c_1fd6102e ;
                 skos:definition "Reconstruction of radiopacity differences in sections contiguous sections of a solid body, carried out using special radiographic equipment. The subject or sample to be investigated, immobile, is placed along its axis while the X source and the detector move radially in solidarity, detecting the radiopacity."@en ;
                 skos:editorialNote "C. Giannini, “Dizionario del restauro - Tecniche diagnostica conservazione”, Nardini Editore, Firenze, 2010"@it ,
                                    "M.Ceroni, G.Elia, “Diagnostica per i beni culturali”, Alinea editrice, Firenze, 2008"@it ;
                 skos:inScheme :Archeometric_and_Diagnostic_Analysis ;
                 skos:topConceptOf :Archeometric_and_Diagnostic_Analysis ;
                 skos:note "International references could not be found, but the preferred editorial note and the definition closest to the meaning is in Diagnostica per i beni culturali"@en ;
                 skos:prefLabel "Computerised Axial Tomography (CAT)"@en , "Tomografia assiale computerizzata (TAC)"@it .


###  https://w3id.org/crmrp#c_7cb6da0e
crmrp:c_7cb6da0e rdf:type owl:NamedIndividual ,
                          skos:Concept ;
                 rdfs:label "Graffiti"@en ;
                 skos:altLabel "Anthropically induced deterioration"@en ;
                 skos:definition "Human exèressions by engraving, scratching, addition of paint, link or other material applied to the surface of an object."@en ;
                 skos:editorialNote "A. Weyer et al., “EwaGlos - European Illustrated Glossary of conservation terms for wall paintings and architectural surfaces”, Michael Imhof Verlag, Petersberg, Germany"@en ,
                                    "Uni Cen/Ts 17135:2021 - Conservation of cultural heritage. General terms and definitions"@en ,
                                    "Verg`es-Belmin et al., ICOMOS-ISCS: Illustrated glossary on stone deterioration patterns, vol. XV. Icomos International Council on Monuments and Sites, 2008"@en ;
                 skos:inScheme :Alteration ;
                 skos:note "The preferred editorial note and the definition closest to the meaning is Uni Cen/Ts 17135:2021"@en ;
                 skos:prefLabel "Graffiti"@en , "Graffito"@it ;
                 skos:topConceptOf :Alteration .


###  https://w3id.org/crmrp#c_7d48691d
crmrp:c_7d48691d rdf:type owl:NamedIndividual ,
                          skos:Concept ;
                 rdfs:label "Opus sectile"@en ;
                 skos:broader :c_b9a6a1c8 ;
                 skos:definition "Pavement made of stone slabs, most commonly of different colored marble, cut in regular shapes and placed side by side to create a geometric pattern or figurative motif."@en ;
                 skos:editorialNote "C. Fiori “Teoria e tecniche per la conservazione del mosaico”, Il Prato, Padova, 2002"@it ,
                                    "C. Giannini, “Dizionario del restauro - Tecniche diagnostica conservazione”, Nardini Editore, Firenze, 2010"@it ,
                                    "Getty Conservation Institute “Illustrated Glossary - Technician Training for the Maintenance of In Situ Mosaics”, Los Angeles, 2013"@en ;
                 skos:inScheme :Execution_Technique ;
                 skos:topConceptOf :Execution_Technique ;
                 skos:prefLabel "Opus sectile"@en , "Opus sectile"@it .


###  https://w3id.org/crmrp#c_7db77b32
crmrp:c_7db77b32 rdf:type owl:NamedIndividual ,
                          skos:Concept ;
                 rdfs:label "Microphotography"@en ;
                 skos:broader :c_1fd6102e ;
                 skos:closeMatch <http://vocab.getty.edu/page/aat/300053550> ;
                 skos:definition "Techniques to photograph subjects that can be viewed only with the aid of a microscope or other magnifier"@en ;
                 skos:editorialNote "Getty AAT http://vocab.getty.edu/page/aat/300053550"@en ;
                 skos:inScheme :Archeometric_and_Diagnostic_Analysis ;
                 skos:topConceptOf :Archeometric_and_Diagnostic_Analysis ;
                 skos:prefLabel "Microphotography"@en , "Microfotografia"@it .


###  https://w3id.org/crmrp#c_7ee727f3
crmrp:c_7ee727f3 rdf:type owl:NamedIndividual ,
                          skos:Concept ;
                 rdfs:label "Microscopic analysis"@en ;
                 skos:broader :c_abed88a5 ;
                 skos:definition "Optical microscopy is an observation technique capable of producing images magnified images of objects or details of objects that are too small to be observed with the naked eye."@en ;
                 skos:editorialNote "M.Ceroni, G.Elia, “Diagnostica per i beni culturali”, Alinea editrice, Firenze, 2008"@it ;
                 skos:inScheme :Archeometric_and_Diagnostic_Analysis ;
                 skos:topConceptOf :Archeometric_and_Diagnostic_Analysis ;
                 skos:note "International references could not be found, but the preferred editorial note and the definition closest to the meaning is in Diagnostica per i beni culturali"@en ;
                 skos:prefLabel "Microscopic analysis"@en , "Microscopia"@it .


###  https://w3id.org/crmrp#c_7f750ff2
crmrp:c_7f750ff2 rdf:type owl:NamedIndividual ,
                          skos:Concept ;
                 rdfs:label "Infiltration"@en ;
                 skos:broader :c_61d92422 ;
                 skos:definition "The ingress of water through defects in a building."@en ;
                 skos:editorialNote "A. Weyer et al., “EwaGlos - European Illustrated Glossary of conservation terms for wall paintings and architectural surfaces”, Michael Imhof Verlag, Petersberg, Germany"@en ;
                 skos:inScheme :Alteration ;
                 skos:topConceptOf :Alteration ;
                 skos:prefLabel "Infiltration"@en , "Infiltrazione"@it .


###  https://w3id.org/crmrp#c_801d2563
crmrp:c_801d2563 rdf:type owl:NamedIndividual ,
                          skos:Concept ;
                 rdfs:label "Graphite pencils"@en ;
                 skos:broader :c_044b6056 ;
                 skos:definition "Pencils with a lead made of graphite."@en ;
                 skos:editorialNote "Getty AAT http://vocab.getty.edu/page/aat/300022443"@en ;
                 skos:exactMatch <http://vocab.getty.edu/page/aat/300022443> ;
                 skos:inScheme :Execution_Technique ;
                 skos:topConceptOf :Execution_Technique ;
                 skos:prefLabel "Graphite pencils"@en , "Grafite"@it .


###  https://w3id.org/crmrp#c_813d8e86
crmrp:c_813d8e86 rdf:type owl:NamedIndividual ,
                          skos:Concept ;
                 rdfs:label "Enamel paint"@en ;
                 skos:broader :c_143349b9 ;
                 skos:closeMatch <http://vocab.getty.edu/page/aat/300147678> ;
                 skos:definition "Paint made from oil, resin, varnish, or a combination of these, mixed with finely ground pigment; usually giving a glossy finish, but sometimes giving a semigloss or flat finish"@en ;
                 skos:editorialNote "Getty AAT http://vocab.getty.edu/page/aat/300147678"@en ;
  		 skos:prefLabel "Enamel paint"@en , "Smalto"@it ;
                 skos:topConceptOf :Execution_Technique;
                 skos:inScheme :Execution_Technique .


###  https://w3id.org/crmrp#c_830e6744
crmrp:c_830e6744 rdf:type owl:NamedIndividual ,
                          skos:Concept ;
                 rdfs:label "Cleaning"@en ;
                 skos:definition "Removal of unwanted material from an object"@en ;
                 skos:editorialNote "A. Weyer et al., “EwaGlos - European Illustrated Glossary of conservation terms for wall paintings and architectural surfaces”, Michael Imhof Verlag, Petersberg, Germany"@en ,
                                    "Getty AAT http://vocab.getty.edu/page/aat/300053027"@en ,
                                    "Getty Conservation Institute “Illustrated Glossary - Definitions of terms used for the graphic documentation of in situ floor mosaics”, “Mosaics In Situ Project”, Los Angeles, 2003"@en ,
                                    "Uni En 15898:2019 Conservazione del patrimonio culturale - Termini generali e definizioni"@it ;
                 skos:exactMatch <http://vocab.getty.edu/page/aat/300053027> ;
                 skos:inScheme :Intervention ;
                 skos:prefLabel "Cleaning"@en , "Pulitura"@it ;
                 skos:topConceptOf :Intervention .


###  https://w3id.org/crmrp#c_83de0482
crmrp:c_83de0482 rdf:type owl:NamedIndividual ,
                          skos:Concept ;
                 rdfs:label "Lime paint"@en ;
                 skos:broader :c_6626f18c ;
                 skos:definition "Mural painting technique used as an alternative and at the same time as ‘buon fresco'; pigments were diluted in milk of lime instead of water and spread even several times over a coat of lime, generally already carboborn and smoothed. This is an opaque paint recognisable by the body of the brushstroke."@en ;
                 skos:editorialNote "C. Giannini, “Dizionario del restauro - Tecniche diagnostica conservazione”, Nardini Editore, Firenze, 2010"@it ;
                 skos:inScheme :Execution_Technique ;
                 skos:topConceptOf :Execution_Technique ;
                 skos:note "International references could not be found"@en ;
                 skos:prefLabel "Lime paint"@en , "A calce"@it .


###  https://w3id.org/crmrp#c_847b008d
crmrp:c_847b008d rdf:type owl:NamedIndividual ,
                          skos:Concept ;
                 rdfs:label "Transfer"@en ;
                 skos:definition "Adhesion of a detached wall painting or mosaic or painting to a new support replacing the original."@en ;
                 skos:editorialNote "A. Weyer et al., “EwaGlos - European Illustrated Glossary of conservation terms for wall paintings and architectural surfaces”, Michael Imhof Verlag, Petersberg, Germany"@en ;
                 skos:inScheme :Intervention ;
                 skos:prefLabel "Transfer"@en , "Applicazione su nuovo supporto"@it ;
                 skos:topConceptOf :Intervention .


###  https://w3id.org/crmrp#c_8590c59f
crmrp:c_8590c59f rdf:type owl:NamedIndividual ,
                          skos:Concept ;
                 rdfs:label "Drying oil"@en ;
                 skos:broader :c_044b6056 ;
                 skos:definition "Vegetable oils which form a solid, elastic film after a period of exposure to the air."@en ;
                 skos:editorialNote "A. Weyer et al., “EwaGlos - European Illustrated Glossary of conservation terms for wall paintings and architectural surfaces”, Michael Imhof Verlag, Petersberg, Germany"@en ;
                 skos:inScheme :Execution_Technique ;
                 skos:topConceptOf :Execution_Technique ;
                 skos:prefLabel "Drying oil"@en , "Olio"@it .


###  https://w3id.org/crmrp#c_86abb308
crmrp:c_86abb308 rdf:type owl:NamedIndividual ,
                          skos:Concept ;
                 rdfs:label "Iron"@en ;
                 skos:broader :c_6407466f ;
                 skos:definition "Pure metallic element having symbol Fe and atomic number 26; metallic iron is silvery in color, lustrous, soft, ductile, malleable, and slightly magnetic; it rusts when exposed to moist air. It is rarely found as a native metal (telluric iron) except in meteorites (meteoric iron). Iron is most often found throughout the world as iron oxides (hematite, magnetite, limonite, and siderite) mixed with other ores."@en ;
                 skos:editorialNote "Getty AAT http://vocab.getty.edu/page/aat/300011002"@en ;
                 skos:exactMatch <http://vocab.getty.edu/page/aat/300011002> ;
                 skos:inScheme :Material ;
                 skos:topConceptOf :Material ;
                 skos:prefLabel "Iron"@en , "Ferro"@it .


###  https://w3id.org/crmrp#c_8a709acb
crmrp:c_8a709acb rdf:type owl:NamedIndividual ,
                          skos:Concept ;
                 rdfs:label "Enzyme-linked immunosorbent assay"@en ;
                 skos:broader :c_abed88a5 ;
                 skos:definition "Assay technique in which a monoclonal antibody is bound to an enzyme to detect and measure the presence of an antigen in a sample."@en ;
                 skos:editorialNote "Getty AAT http://vocab.getty.edu/page/aat/300380512"@en ;
                 skos:exactMatch <http://vocab.getty.edu/page/aat/300380512> ;
                 skos:inScheme :Archeometric_and_Diagnostic_Analysis ;
                 skos:topConceptOf :Archeometric_and_Diagnostic_Analysis ;
                 skos:prefLabel "Enzyme-linked immunosorbent assay"@en , "Saggio immunoenzimatico"@it .


###  https://w3id.org/crmrp#c_8af455cd
crmrp:c_8af455cd rdf:type owl:NamedIndividual ,
                          skos:Concept ;
                 rdfs:label "Gilding technique"@en ;
                 skos:broader :Execution_Technique ;
                 skos:closeMatch <http://vocab.getty.edu/page/aat/300053789> ;
                 skos:definition "Process involving the surface application of gold or another metal in the form of leaf, powder applied directly to the surface, powder mixed with a binder, electroplating, or other forms to approximate the effect of solid or inlaid metal."@en ;
                 skos:editorialNote "Getty AAT http://vocab.getty.edu/page/aat/300053789"@en ;
                 skos:inScheme :Execution_Technique ;
                 skos:prefLabel "Gilding technique"@en , "Tecnica di doratura"@it ;
                 skos:topConceptOf :Execution_Technique .


###  https://w3id.org/crmrp#c_8c553ab1
crmrp:c_8c553ab1 rdf:type owl:NamedIndividual ,
                          skos:Concept ;
                 rdfs:label "Dry-rot"@en ;
                 skos:broader :c_3ef20257 ;
                 skos:definition "Refers to a type of decomposition of timber by fungi."@en ;
                 skos:editorialNote "Getty AAT http://vocab.getty.edu/page/aat/300188725"@en ;
                 skos:exactMatch <http://vocab.getty.edu/page/aat/300188725> ;
                 skos:inScheme :Alteration ;
                 skos:topConceptOf :Alteration ;
                 skos:prefLabel "Dry-rot"@en , "Carie"@it .


###  https://w3id.org/crmrp#c_8c762c3e
crmrp:c_8c762c3e rdf:type owl:NamedIndividual ,
                          skos:Concept ;
                 rdfs:label "Crack"@en ;
                 skos:altLabel "Fracture"@en , "Fratturazione"@it ;
                 skos:definition "Separation of a solid material without breaking apart."@en ;
                 skos:editorialNote "A. Weyer et al., “EwaGlos - European Illustrated Glossary of conservation terms for wall paintings and architectural surfaces”, Michael Imhof Verlag, Petersberg, Germany"@en ,
                                    "Getty Conservation Institute “Illustrated Glossary - Definitions of terms used for the graphic documentation of in situ floor mosaics”, “Mosaics In Situ Project”, Los Angeles, 2003"@en ,
                                    "Uni Cen/Ts 17135:2021 - Conservation of cultural heritage. General terms and definitions"@en ,
                                    "Verg`es-Belmin et al., ICOMOS-ISCS: Illustrated glossary on stone deterioration patterns, vol. XV. Icomos International Council on Monuments and Sites, 2008"@en ;
                 skos:inScheme :Alteration ;
                 skos:note "The preferred editorial note and the definition closest to the meaning is Uni Cen/Ts 17135:2021"@en ;
                 skos:prefLabel "Crack"@en , "Fessurazione"@it ;
                 skos:topConceptOf :Alteration .


###  https://w3id.org/crmrp#c_8ce9910e
crmrp:c_8ce9910e rdf:type owl:NamedIndividual ,
                          skos:Concept ;
                 rdfs:label "Architecture"@en ;
                 skos:definition "Structures or parts of structures that are the result of conscious construction, are of practical use, are relatively stable and permanent, and are of a size and scale appropriate for--but not limited to--habitable buildings. Works of architecture are manifestations of the built environment that is typically classified as fine art, meaning it is generally considered to have aesthetic value, was designed by an architect (whether or not his or her name is known), and constructed with skilled labor."@en ;
                 skos:editorialNote "Getty AAT http://vocab.getty.edu/page/aat/300263552"@en ;
                 skos:exactMatch <http://vocab.getty.edu/page/aat/300263552> ;
                 skos:inScheme :Restoration_Object ;
                 skos:prefLabel "Architecture"@en , "Architettura"@it ;
                 skos:topConceptOf :Restoration_Object .


###  https://w3id.org/crmrp#c_8dcb0eb4
crmrp:c_8dcb0eb4 rdf:type owl:NamedIndividual ,
                          skos:Concept ;
                 rdfs:label "Print"@en ;
                 skos:definition "Pictorial works produced by transferring images by means of a matrix such as a plate, block, or screen, using any of various printing processes. When emphasizing the individual printed image, use impressions. Avoid the controversial expression original prints, except in reference to discussions of the expression's use. If prints are neither reproductive prints nor popular prints, use the simple term prints. With regard to photographs, prefer photographic prints; for types of reproductions of technical drawings and documents, see terms found under reprographic copies."@en ;
                 skos:exactMatch <http://vocab.getty.edu/page/aat/300041273> ;
                 skos:inScheme :Restoration_Object ;
                 skos:prefLabel "Prints"@en , "Stampa"@it ;
                 skos:editorialNote "Getty AAT http://vocab.getty.edu/page/aat/300041273"@en ;
                 skos:topConceptOf :Restoration_Object .


###  https://w3id.org/crmrp#c_8e940120
crmrp:c_8e940120 rdf:type owl:NamedIndividual ,
                          skos:Concept ;
                 rdfs:label "Mercury porosimetry"@en ;
                 skos:broader :c_abed88a5 ;
                 skos:definition "Porosimetry which uses mercury as the non-wetting liquid pressed into the pores of a material by the porosimeter."@en ;
                 skos:editorialNote "Getty AAT http://vocab.getty.edu/page/aat/300379676"@en ;
                 skos:exactMatch <http://vocab.getty.edu/page/aat/300379676> ;
                 skos:inScheme :Archeometric_and_Diagnostic_Analysis ;
                 skos:topConceptOf :Archeometric_and_Diagnostic_Analysis ;
                 skos:prefLabel "Mercury porosimetry"@en , "Porosimetria al mercurio"@it .


###  https://w3id.org/crmrp#c_8f129db5
crmrp:c_8f129db5 rdf:type owl:NamedIndividual ,
                          skos:Concept ;
                 rdfs:label "Sub-efflorescence"@en ;
                 skos:altLabel "Subflorescence"@en ;
                 skos:definition "Sub-efflorescence and crypto-efflorescence are visible when the surface falls apart or away"@en ;
                 skos:editorialNote "Uni Cen/Ts 17135:2021 - Conservation of cultural heritage. General terms and definitions"@en ,
                                    "Verg`es-Belmin et al., ICOMOS-ISCS: Illustrated glossary on stone deterioration patterns, vol. XV. Icomos International Council on Monuments and Sites, 2008"@en ;
                 skos:inScheme :Alteration ;
                 skos:note "The preferred editorial note and the definition closest to the meaning is Uni Cen/Ts 17135:2021"@en ;
                 skos:prefLabel "Sub-efflorescence"@en , "Subflorescenza"@it ;
                 skos:topConceptOf :Alteration .


###  https://w3id.org/crmrp#c_8fe789e5
crmrp:c_8fe789e5 rdf:type owl:NamedIndividual ,
                          skos:Concept ;
                 rdfs:label "Terracotta"@en ;
                 skos:broader :c_bd34e984 ;
                 skos:definition "A glazed or unglazed product made with clay and mixed with fillers (grog – calcinated clay, chamotte, brick dust or pot clay) and natural binders which are then baked at a high temperature (above 600 °C). Any kind of baked or semi-fired clay used to create utilitarian or decorative objects, or structural forms such as: floor tiles, roof tiles or decorative architectural elements"@en ;
                 skos:editorialNote "A. Weyer et al., “EwaGlos - European Illustrated Glossary of conservation terms for wall paintings and architectural surfaces”, Michael Imhof Verlag, Petersberg, Germany"@en ;
                 skos:inScheme :Material ;
                 skos:topConceptOf :Material ;
                 skos:prefLabel "Terracotta"@en , "Terracotta"@it .


###  https://w3id.org/crmrp#c_909e9d33
crmrp:c_909e9d33 rdf:type owl:NamedIndividual ,
                          skos:Concept ;
                 rdfs:label "Haze"@en ;
                 skos:broader :c_757ed6ec ;
                 skos:definition "Gold foil residues are removed with brushes or cotton to make the glaze opaque"@en ;
                 skos:editorialNote "G. Pignolo, “Effetti d’oro - Storia e tecnica della doratura nell’arte”, Editrice Compositori, Bologna, 2002"@it ;
                 skos:inScheme :Execution_Technique ;
                 skos:topConceptOf :Execution_Technique ;
                 skos:note "International references could not be found"@en ;
                 skos:prefLabel "Haze"@en , "Velatura"@it .


###  https://w3id.org/crmrp#c_90a8bb69
crmrp:c_90a8bb69 rdf:type owl:NamedIndividual ,
                          skos:Concept ;
                 rdfs:label "3D model"@en ;
                 skos:broader :c_f383c4d3 ;
                 skos:definition "A 3D model (or three-dimensional model) is a mathematical representation of a three-dimensional object."@en ;
                 skos:inScheme :Documentation ;
                 skos:topConceptOf :Documentation ;
                 skos:note "International references could not be found"@en ;
                 skos:prefLabel "3D model"@en , "Rilievo 3D"@it .


###  https://w3id.org/crmrp#c_931e5c94
crmrp:c_931e5c94 rdf:type owl:NamedIndividual ,
                          skos:Concept ;
                 rdfs:label "Monitoring"@en ;
                 skos:altLabel "Environmental control"@en ;
                 skos:broader :c_1fd6102e ;
                 skos:definition "Collection and evaluation of data on an object, a collection of objects or collection and/or their environment over time."@en ;
                 skos:editorialNote "A. Weyer et al., “EwaGlos - European Illustrated Glossary of conservation terms for wall paintings and architectural surfaces”, Michael Imhof Verlag, Petersberg, Germany"@en ,
                                    "Getty AAT http://vocab.getty.edu/page/aat/300229535"@en ,
                                    "UNI EN 15898:2019 Conservazione del patrimonio culturale - Termini generali e definizioni"@it ;
                 skos:inScheme :Archeometric_and_Diagnostic_Analysis ;
                 skos:topConceptOf :Archeometric_and_Diagnostic_Analysis ;
                 skos:note "The preferred editorial note and the definition closest to the meaning is UNI EN 15898:2019"@en ;
                 skos:prefLabel "Monitoring"@en , "Monitoraggio ambientale"@it .


###  https://w3id.org/crmrp#c_9393771d
crmrp:c_9393771d rdf:type owl:NamedIndividual ,
                          skos:Concept ;
                 rdfs:label "Opus figlinum"@en ;
                 skos:broader :c_b9a6a1c8 ;
                 skos:definition "Type of opus tessellatum pavement made of stone tesserae of different colors, all of the same size and rectangular shape. As with opus figlinum (page 14), the placement of the tesserae creates a visual impression of a basket weave pattern."@en ;
                 skos:editorialNote "Getty Conservation Institute “Illustrated Glossary - Technician Training for the Maintenance of In Situ Mosaics”, Los Angeles, 2013"@en ;
                 skos:inScheme :Execution_Technique ;
                 skos:topConceptOf :Execution_Technique ;
                 skos:prefLabel "Opus figlinum"@en , "Opus figlinum"@it .


###  https://w3id.org/crmrp#c_93c50ee0
crmrp:c_93c50ee0 rdf:type owl:NamedIndividual ,
                          skos:Concept ;
                 rdfs:label "Brass"@en ;
                 skos:broader :c_6407466f ;
                 skos:closeMatch <http://vocab.getty.edu/page/aat/300010946> ;
                 skos:definition "Alloy of copper and zinc, usually with copper as the major alloying element and zinc up to 40% by weight."@en ;
                 skos:editorialNote "Getty AAT http://vocab.getty.edu/page/aat/300010946"@en ;
                 skos:inScheme :Material ;
                 skos:topConceptOf :Material ;
                 skos:prefLabel "Brass"@en , "Ottone"@it .


###  https://w3id.org/crmrp#c_945b8f77
crmrp:c_945b8f77 rdf:type owl:NamedIndividual ,
                          skos:Concept ;
                 rdfs:label "Copper"@en ;
                 skos:broader :c_6407466f ;
                 skos:definition "Pure metallic element having the symbol Cu and atomic number 29; a reddish brown, ductile metal that is present in the earth's crust, occurring as a native metal and as ores of sulfide, sulfate and carbonate (azurite, malachite, etc.). It was the first metal used by humans, probably from about 8000 BCE, in the regions of Mesopotamia and India. By about 3800 BCE copper was made into bronze for weapons and knives. Today, copper is one of the most widely used metals because it has high electrical and thermal conductivity, can be easily fabricated, is ductile and polishes well. In moist air, copper forms a protective green film of basic carbonate. Metallic copper combines well with other metals to form alloys, most commonly brass and bronze. Copper and its alloys are used for wire, electrical devices, pipes, cooking vessels, ammunition, ornamental trim, roofing, grillwork, coins, musical instruments, jewelry, and sculptures."@en ;
                 skos:exactMatch <http://vocab.getty.edu/page/aat/300011020> ;
                 skos:inScheme :Material ;
                 skos:topConceptOf :Material ;
                 skos:prefLabel "Copper"@en , "Rame"@it ;
                 skos:source "Getty AAT http://vocab.getty.edu/page/aat/300011020"@en .


###  https://w3id.org/crmrp#c_94b88ed9
crmrp:c_94b88ed9 rdf:type owl:NamedIndividual ,
                          skos:Concept ;
                 rdfs:label "Ultraviolet reflectography"@en ;
                 skos:broader :c_1285fa71 ;
                 skos:definition "With UV reflectography, a work is illuminated with UV light and the resulting image is photographed with a camera using a UV lens filter. Since different materials will have different levels of opacity under UV than under visible or infrared light, this technique can provide clues to the material composition of pigments. Furthermore, it is a good choice for analysing roughness and surface details."@en ;
                 skos:inScheme :Archeometric_and_Diagnostic_Analysis ;
                 skos:topConceptOf :Archeometric_and_Diagnostic_Analysis ;
                 skos:note "International references could not be found"@en , "Riflettografia ultravioletta"@it ;
                 skos:prefLabel "Ultraviolet reflectography"@en , "Riflettografia ultravioletta"@it .


###  https://w3id.org/crmrp#c_96b092c5
crmrp:c_96b092c5 rdf:type owl:NamedIndividual ,
                          skos:Concept ;
                 rdfs:label "Manuscript"@en ;
                 skos:definition "Handwritten documents, particularly books and other documents created before the invention of the printing press. May also be used to distinguish certain documents from published or otherwise printed documents, as in the cases of typed personal letters or a typescript from which printed versions are made."@en ;
                 skos:editorialNote "Getty AAT http://vocab.getty.edu/page/aat/300028569"@en ;
                 skos:exactMatch <http://vocab.getty.edu/page/aat/300028569> ;
                 skos:inScheme :Restoration_Object ;
                 skos:prefLabel "Manuscript"@en , "Manoscritto"@it ;
                 skos:topConceptOf :Restoration_Object .


###  https://w3id.org/crmrp#c_977962bd
crmrp:c_977962bd rdf:type owl:NamedIndividual ,
                          skos:Concept ;
                 rdfs:label "Tin"@en ;
                 skos:broader :c_6407466f ;
                 skos:definition "Pure metallic element having symbol Sn and atomic number 50; a soft, pliable, silvery white metal. Use also for this metal as processed and formed, usually in combination with other substances, to make various objects and materials."@en ;
                 skos:editorialNote "Getty AAT http://vocab.getty.edu/page/aat/300133751"@en ;
                 skos:exactMatch <http://vocab.getty.edu/page/aat/300133751> ;
                 skos:inScheme :Material ;
                 skos:topConceptOf :Material ;
                 skos:prefLabel "Tin"@en , "Stagno"@it .


###  https://w3id.org/crmrp#c_98f7091c
crmrp:c_98f7091c rdf:type owl:NamedIndividual ,
                          skos:Concept ;
                 rdfs:label "High performance liquid chromatography (HPLC)"@en ;
                 skos:broader :c_2d5cde83 ;
                 skos:definition "Refers to an enhanced technique of liquid chromatography developed in the late 1960s in which stationary phase particles are smaller and packed more densely than in traditional liquid chromatography. The mobile phase solvent is then forced through the dense adsorbent by means of a pump. The technique was initially known as high pressure liquid chromatography (HPLC). The acronym remains but with a shift in emphasis to the high performance the method attains."@en ;
                 skos:editorialNote "Getty AAT http://vocab.getty.edu/page/aat/300379487"@en ;
                 skos:exactMatch <http://vocab.getty.edu/page/aat/300379487> ;
                 skos:inScheme :Archeometric_and_Diagnostic_Analysis ;
                 skos:topConceptOf :Archeometric_and_Diagnostic_Analysis ;
                 skos:prefLabel "High performance liquid chromatography (HPLC)"@en , "Cromatografia liquida ad alta pressione (HPLC)"@it .


###  https://w3id.org/crmrp#c_9d1ced39
crmrp:c_9d1ced39 rdf:type owl:NamedIndividual ,
                          skos:Concept ;
                 rdfs:label "Fusione a conchiglia"@en ;
                 skos:broader :c_0a9f4d42 ;
                 skos:definition "Clamshell casting is predominantly used in the mechanical engineering industry for the production of high-precision, high-volume parts. It involves making a demountable metal mould in which casting takes place. The casting does not adhere to the mould as it is kept cold."@en ;
                 skos:editorialNote "A.Giuffredi “Formatura e fonderia”, Alinea editrice, Firenze, 2010"@it ;
                 skos:inScheme :Execution_Technique ;
                 skos:topConceptOf :Execution_Technique ;
                 skos:note "International references could not be found"@en ;
                 skos:prefLabel "Fusione a conchiglia"@en , "Fusione a conchiglia"@it .


###  https://w3id.org/crmrp#c_9e69e4dd
crmrp:c_9e69e4dd rdf:type owl:NamedIndividual ,
                          skos:Concept ;
                 rdfs:label "Fusione dal vero"@en ;
                 skos:broader :c_0a9f4d42 ;
                 skos:definition "Small animals such as lizards, snakes, insects or plant elements can be faithfully reproduced by placing them in the refractory. During the baking of the moulds, the organic material burns away, leaving the void to be occupied by the metal."@en ;
                 skos:editorialNote "A.Giuffredi “Formatura e fonderia”, Alinea editrice, Firenze, 2010"@it ;
                 skos:inScheme :Execution_Technique ;
                 skos:topConceptOf :Execution_Technique ;
                 skos:note "International references could not be found"@en ;
                 skos:prefLabel "Fusione dal vero"@en , "Fusione dal vero"@it .


###  https://w3id.org/crmrp#c_9ff50f5a
crmrp:c_9ff50f5a rdf:type owl:NamedIndividual ,
                          skos:Concept ;
                 rdfs:label "Concretion"@en ;
                 skos:closeMatch <http://vocab.getty.edu/page/aat/300379825> ;
                 skos:definition "Hard adherent accumulation and coalescence of a deposit"@en ;
                 skos:editorialNote "Getty AAT http://vocab.getty.edu/page/aat/300379825"@en ,
                                    "Uni Cen/Ts 17135:2021 - Conservation of cultural heritage. General terms and definitions"@en ,
                                    "Verg`es-Belmin et al., ICOMOS-ISCS: Illustrated glossary on stone deterioration patterns, vol. XV. Icomos International Council on Monuments and Sites, 2008"@en ;
                 skos:inScheme :Alteration ;
                 skos:note "The preferred editorial note and the definition closest to the meaning is Uni Cen/Ts 17135:2021"@en ;
                 skos:prefLabel "Concretion"@en , "Concrezione"@it ;
                 skos:topConceptOf :Alteration .


###  https://w3id.org/crmrp#c_a08009f4
crmrp:c_a08009f4 rdf:type owl:NamedIndividual ,
                          skos:Concept ;
                 rdfs:label "Strappo"@en ;
                 skos:broader :c_4fe4d308 ;
                 skos:definition "The process by which a fresco is detached from a wall, used when the plaster on which it is painted has greatly deteriorated; the color layer is removed by a strong glue without removing excessive amounts of plaster."@en ;
                 skos:editorialNote "A. Weyer et al., “EwaGlos - European Illustrated Glossary of conservation terms for wall paintings and architectural surfaces”, Michael Imhof Verlag, Petersberg, Germany"@en ,
                                    "Getty AAT http://vocab.getty.edu/page/aat/300078735"@en ;
                 skos:exactMatch <http://vocab.getty.edu/page/aat/300078735> ;
                 skos:inScheme :Intervention ;
                 skos:topConceptOf :Intervention ;
                 skos:note "The preferred editorial note and the definition closest to the meaning is Getty AAT"@en ;
                 skos:prefLabel "Strappo"@en , "Strappo"@en .


###  https://w3id.org/crmrp#c_a3f0890c
crmrp:c_a3f0890c rdf:type owl:NamedIndividual ,
                          skos:Concept ;
                 rdfs:label "Gusset"@en ;
                 skos:broader :c_e8592f3b ;
                 skos:definition "Geometrically shaped block of stone, metal or wood that is inserted into a cavity of the same shape during maintenance or restoration work"@en ;
                 skos:editorialNote "C. Giannini, “Dizionario del restauro - Tecniche diagnostica conservazione”, Nardini Editore, Firenze, 2010"@it ;
                 skos:inScheme :Intervention ;
                 skos:topConceptOf :Intervention ;
                 skos:note "International references could not be found"@en ;
                 skos:prefLabel "Gusset"@en , "Tassello"@it .


###  https://w3id.org/crmrp#c_a5e9bb0b
crmrp:c_a5e9bb0b rdf:type owl:NamedIndividual ,
                          skos:Concept ;
                 rdfs:label "Pebble mosaic"@en ;
                 skos:broader :c_b9a6a1c8 ;
                 skos:definition "Mosaic pavement, generally bi-chrome, more rarely polychrome, made of natural pebbles of different sizes and placed on their edge, side by side, to create figures or geometric motifs."@en ;
                 skos:editorialNote "C. Fiori “Teoria e tecniche per la conservazione del mosaico”, Il Prato, Padova, 2002"@it ,
                                    "Getty Conservation Institute “Illustrated Glossary - Technician Training for the Maintenance of In Situ Mosaics”, Los Angeles, 2013"@en ;
                 skos:inScheme :Execution_Technique ;
                 skos:topConceptOf :Execution_Technique ;
                 skos:prefLabel "Pebble mosaic"@en , "Mosaico ciottoli"@it .


###  https://w3id.org/crmrp#c_a62f8c57
crmrp:c_a62f8c57 rdf:type owl:NamedIndividual ,
                          skos:Concept ;
                 rdfs:label "Structural consolidation"@en ;
                 skos:broader :c_b86776d0 ;
                 skos:definition "Consolidation intervention involving the innermost (structural) layers of the artwork."@en ;
                 skos:inScheme :Intervention ;
                 skos:topConceptOf :Intervention ;
                 skos:note "International references could not be found"@en ;
                 skos:prefLabel "Structural consolidation"@en , "Consolidamento strutturale"@it .


###  https://w3id.org/crmrp#c_a75330d3
crmrp:c_a75330d3 rdf:type owl:NamedIndividual ,
                          skos:Concept ;
                 rdfs:label "Tratteggio"@en ;
                 skos:broader :c_326da7e4 ;
                 skos:definition "Based on the conservation/restoration theory of Cesare Brandi, the shape and colour of a damaged area are reconstructed using short vertical lines."@en ;
                 skos:editorialNote "A. Weyer et al., “EwaGlos - European Illustrated Glossary of conservation terms for wall paintings and architectural surfaces”, Michael Imhof Verlag, Petersberg, Germany"@en ;
                 skos:inScheme :Intervention ;
                 skos:topConceptOf :Intervention ;
                 skos:prefLabel "Tratteggio"@en , "Tratteggio"@it .


###  https://w3id.org/crmrp#c_a8f1fa7e
crmrp:c_a8f1fa7e rdf:type owl:NamedIndividual ,
                          skos:Concept ;
                 rdfs:label "Gouache"@en ;
                 skos:broader :c_044b6056 ;
                 skos:closeMatch "Getty AAT http://vocab.getty.edu/page/aat/300404215"@en ;
                 skos:definition " A method of painting with matte, opaque watercolor paint. Gouache painting employs opaque layers of color rather than the transparent washes used in the aquarelle technique, due to the differing pigment densities of the media."@en ;
                 skos:editorialNote "Getty AAT http://vocab.getty.edu/page/aat/300404215"@en ;
                 skos:inScheme :Execution_Technique ;
                 skos:topConceptOf :Execution_Technique ;
                 skos:prefLabel "Gouache"@en , "Gouache"@it .


###  https://w3id.org/crmrp#c_a90ef012
crmrp:c_a90ef012 rdf:type owl:NamedIndividual ,
                          skos:Concept ;
                 rdfs:label "Shell gold"@en ;
                 skos:broader :c_8af455cd ;
                 skos:definition "Gold leaf ground into a powder and mixed with honey or other binder, used to produce powdered effects on leather bindings, to repair or restore gold tooling, and to gild manuscripts. Originally packaged in mussel shells, more recently it is sold in plastic containers shaped like mussel shells or in tablet or small block form."@en ;
                 skos:editorialNote "Getty AAT http://vocab.getty.edu/page/aat/300263579"@en ;
                 skos:exactMatch <http://vocab.getty.edu/page/aat/300263579> ;
                 skos:inScheme :Execution_Technique ;
                 skos:topConceptOf :Execution_Technique ;
                 skos:prefLabel "Shell gold"@en , "A conchiglia"@it .


###  https://w3id.org/crmrp#c_aa16888d
crmrp:c_aa16888d rdf:type owl:NamedIndividual ,
                          skos:Concept ;
                 rdfs:label "Tempera magra"@en ;
                 skos:broader :c_77acfccf ;
                 skos:definition "Lean tempera is made from egg white, vegetable glues or substances derived from casein, and was used for painting without preparation. It is very sensitive to the aqueous medium."@en ;
                 skos:editorialNote "C. Giannini, “Dizionario del restauro - Tecniche diagnostica conservazione”, Nardini Editore, Firenze, 2010"@it ;
                 skos:inScheme :Execution_Technique ;
                 skos:topConceptOf :Execution_Technique ;
                 skos:note "It was decided not to proceed with the English translation in order to avoid possible lexical errors and misunderstandings."@en ;
                 skos:prefLabel "Tempera magra"@en , "Tempera magra"@it .


###  https://w3id.org/crmrp#c_aa88700b
crmrp:c_aa88700b rdf:type owl:NamedIndividual ,
                          skos:Concept ;
                 rdfs:label "Warped"@en ;
                 skos:altLabel "Warping"@en ;
                 skos:broader :c_13f3ce9e ;
                 skos:closeMatch <http://vocab.getty.edu/page/aat/300155059> ;
                 skos:definition "Exhibiting irregular deformation in more than one plane."@en ;
                 skos:editorialNote "Getty AAT http://vocab.getty.edu/page/aat/300155059"@en ,
                                    "Uni Cen/Ts 17135:2021 - Conservation of cultural heritage. General terms and definitions"@en ;
                 skos:inScheme :Alteration ;
                 skos:topConceptOf :Alteration ;
                 skos:prefLabel "Warped"@en , "Svirgolatura"@it .


###  https://w3id.org/crmrp#c_ab5f4e0c
crmrp:c_ab5f4e0c rdf:type owl:NamedIndividual ,
                          skos:Concept ;
                 rdfs:label "Buffer solution"@en ;
                 skos:broader :c_5a83cd16 ;
                 skos:definition "Any substance capable in solution of neutralizing both acids and bases and thereby maintaining the original acidity or basicity of the solution."@en ;
                 skos:editorialNote "Getty AAT http://vocab.getty.edu/page/aat/300213366"@en ;
                 skos:exactMatch <http://vocab.getty.edu/page/aat/300213366> ;
                 skos:inScheme :Intervention ;
                 skos:topConceptOf :Intervention ;
                 skos:prefLabel "Buffer solution"@en , "Tampone"@it .


###  https://w3id.org/crmrp#c_abed88a5
crmrp:c_abed88a5 rdf:type owl:NamedIndividual ,
                          skos:Concept ;
                 rdfs:label "Microinvasive testing"@en ;
                 skos:definition "Testing techniques that penetrate or alter the sample at a microscopic level."@en ;
                 skos:editorialNote "Getty AAT http://vocab.getty.edu/page/aat/300448614"@en ;
                 skos:exactMatch <http://vocab.getty.edu/page/aat/300448614> ;
                 skos:inScheme :Archeometric_and_Diagnostic_Analysis ;
                 skos:topConceptOf :Archeometric_and_Diagnostic_Analysis ;
                 skos:prefLabel "Microinvasive testing"@en , "Indagine invasiva/microinvasiva"@it .


###  https://w3id.org/crmrp#c_ada0bb45
crmrp:c_ada0bb45 rdf:type owl:NamedIndividual ,
                          skos:Concept ;
                 rdfs:label "Twisted"@en ;
                 skos:broader :c_13f3ce9e ;
                 skos:definition "Exhibiting deformation around a single axis."@en ;
                 skos:editorialNote "Uni Cen/Ts 17135:2021 - Conservation of cultural heritage. General terms and definitions"@en ;
                 skos:inScheme :Alteration ;
                 skos:topConceptOf :Alteration ;
                 skos:prefLabel "Twisted"@en , "Ritorsione"@it .


###  https://w3id.org/crmrp#c_ae321441
crmrp:c_ae321441 rdf:type owl:NamedIndividual ,
                          skos:Concept ;
                 rdfs:label "Corroded"@en ;
                 skos:altLabel "Corrosion"@en ;
                 skos:definition "Exhibiting transformation by chemical reaction with the environment."@en ;
                 skos:editorialNote " A. Weyer et al., “EwaGlos - European Illustrated Glossary of conservation terms for wall paintings and architectural surfaces”, Michael Imhof Verlag, Petersberg, Germany"@en ,
                                    "Getty AAT http://vocab.getty.edu/page/aat/300054107"@en ,
                                    "Uni Cen/Ts 17135:2021 - Conservation of cultural heritage. General terms and definitions"@en ;
                 skos:exactMatch <http://vocab.getty.edu/page/aat/300054107> ;
                 skos:inScheme :Alteration ;
                 skos:note "The preferred editorial note and the definition closest to the meaning is Uni Cen/Ts 17135:2021"@en ;
                 skos:prefLabel "Corroded"@en , "Corrosione"@it ;
                 skos:topConceptOf :Alteration .


###  https://w3id.org/crmrp#c_ae6d1fdc
crmrp:c_ae6d1fdc rdf:type owl:NamedIndividual ,
                          skos:Concept ;
                 rdfs:label "Cold patinatura"@en ;
                 skos:broader :c_e5a56926 ;
                 skos:definition "Some varieties of enamels and inks need to be applied while the metal surface is hot."@en ;
                 skos:editorialNote "A.Giuffredi, “Formatura e fonderia”, Alinea editrice, Firenze"@it ;
                 skos:inScheme :Execution_Technique ;
                 skos:topConceptOf :Execution_Technique ;
                 skos:note "International references could not be found"@en ;
                 skos:prefLabel "Cold patinatura"@en , "Patinatura dipinta a freddo"@it .


###  https://w3id.org/crmrp#c_aea2f21f
crmrp:c_aea2f21f rdf:type owl:NamedIndividual ,
                          skos:Concept ;
                 rdfs:label "Ultrasound"@en ;
                 skos:broader :c_1fd6102e ;
                 skos:definition "Determining the propagation speed of ultrasonic pulses. In diagnostic applications in the field restoration and conservation, ultrasounds are used to identify discontinuities in materials by their propagation within them"@en ;
                 skos:editorialNote "C. Giannini, “Dizionario del restauro - Tecniche diagnostica conservazione”, Nardini Editore, Firenze, 2010"@it ,
                                    "M.Ceroni, G.Elia, “Diagnostica per i beni culturali”, Alinea editrice, Firenze, 2008"@it ;
                 skos:inScheme :Archeometric_and_Diagnostic_Analysis ;
                 skos:topConceptOf :Archeometric_and_Diagnostic_Analysis ;
                 skos:note "International references could not be found, but the preferred editorial note and the definition closest to the meaning is Dizionario del restauro - Tecniche diagnostica conservazione"@en ;
                 skos:prefLabel "Ultrasound"@en , "Ultrasuoni"@it .


###  https://w3id.org/crmrp#c_aee6a805
crmrp:c_aee6a805 rdf:type owl:NamedIndividual ,
                          skos:Concept ;
                 rdfs:label "Etching technique"@en ;
                 skos:closeMatch <http://vocab.getty.edu/page/aat/300053241> ;
                 skos:definition "Intaglio process in which the design is worked into an acid-resistant substance coating the metal printing plate; the plate is then exposed to acid, which etches the plate where the metal is exposed, to create lines and dark areas. For the single step of exposing the plate to acid, use biting."@en ;
                 skos:editorialNote "Getty AAT http://vocab.getty.edu/page/aat/300053241"@en ;
                 skos:inScheme :Execution_Technique ;
                 skos:prefLabel "Etching technique"@en , "Tecnica incisione"@it ;
                 skos:topConceptOf :Execution_Technique .


###  https://w3id.org/crmrp#c_af6b2d29
crmrp:c_af6b2d29 rdf:type owl:NamedIndividual ,
                          skos:Concept ;
                 rdfs:label "Superficial pre-consolidation"@en ;
                 skos:broader :c_e078e94e ;
                 skos:definition "Pre-consolidation intervention involving the surface layers (the substrate) of the artwork."@en ;
                 skos:inScheme :Intervention ;
                 skos:topConceptOf :Intervention ;
                 skos:note "International references could not be found"@en ;
                 skos:prefLabel "Superficial pre-consolidation"@en , "Pre-consolidamento superficiale"@it .


###  https://w3id.org/crmrp#c_af82711f
crmrp:c_af82711f rdf:type owl:NamedIndividual ,
                          skos:Concept ;
                 rdfs:label "Polymer paint"@en ;
                 skos:broader :c_051209b3 ;
                 skos:definition "Paint with a base that is polymer, which is compound formed by the combination of two or more molecules of the same substance to produce a new compound with the same empirical formula but with higher molecular weight. It is typically made from pigments in an acrylic resin or vinyl resin, which are polymers, or a combination of both resins. It is water based, spreads out in a layer, and forms a continuous, flexible, and waterproof film of plastic when the water evaporates."@en ;
                 skos:editorialNote "Getty AAT http://vocab.getty.edu/page/aat/300015055"@en ;
                 skos:exactMatch <http://vocab.getty.edu/page/aat/300015055> ;
                 skos:inScheme :Execution_Technique ;
                 skos:topConceptOf :Execution_Technique ;
                 skos:prefLabel "Polymer paint"@en , "Polimero sintetico"@it .



###  https://w3id.org/crmrp#c_b1c12a4d
crmrp:c_b1c12a4d rdf:type owl:NamedIndividual ,
                          skos:Concept ;
                 rdfs:label "Pastel"@en ;
                 skos:broader :c_044b6056 ;
                 skos:definition "General term for various combinations of ground, powdery pigment and aqueous binder that are used in drawing and dry painting, delivered via a crayon or stick. Pastel as a material is soft and blendable. For the crayons or sticks containing the pigment and binder, use pastels (crayons)."@en ;
                 skos:editorialNote "Getty AAT http://vocab.getty.edu/page/aat/300404632"@en ;
                 skos:exactMatch <http://vocab.getty.edu/page/aat/300404632> ;
                 skos:inScheme :Execution_Technique ;
                 skos:topConceptOf :Execution_Technique ;
                 skos:prefLabel "Pastel"@en , "Pastello"@it .


###  https://w3id.org/crmrp#c_b58f1659
crmrp:c_b58f1659 rdf:type owl:NamedIndividual ,
                          skos:Concept ;
                 rdfs:label "Audio documentation"@en ;
                 skos:definition "Any recording about an object or its manufacturer."@en ;
                 skos:inScheme :Documentation ;
                 skos:note "International references could not be found"@en ;
                 skos:prefLabel "Audio documentation"@en , "Documentazione audio"@it ;
                 skos:topConceptOf :Documentation .


###  https://w3id.org/crmrp#c_b7c4df2f
crmrp:c_b7c4df2f rdf:type owl:NamedIndividual ,
                          skos:Concept ;
                 rdfs:label "Grés"@en ;
                 skos:broader :c_bd34e984 ;
                 skos:closeMatch <http://vocab.getty.edu/page/aat/300010672> ;
                 skos:definition "A type of pottery midway between earthenware and porcelain being made of clay and a fusible stone. It is fired to a point where partial vitrification renders it impervious to liquids, but, unlike porcelain, it is very seldom more than faintly translucent. The vitrification makes it unnecessary to add a glaze, but for reasons of utility and appearance decorative glazes are sometimes used, such as salt glaze and lead glaze."@en ;
                 skos:editorialNote "Getty AAT http://vocab.getty.edu/page/aat/300010672"@en ;
                 skos:inScheme :Material ;
                 skos:topConceptOf :Material ;
                 skos:prefLabel "Grés"@en , "Grés"@it .


###  https://w3id.org/crmrp#c_b7ff54f8
crmrp:c_b7ff54f8 rdf:type owl:NamedIndividual ,
                          skos:Concept ;
                 rdfs:label "Solvent"@en ;
                 skos:broader :c_607d4549 ;
                 skos:definition "Any material, usually liquid, having the power of dissolving another material."@en ;
                 skos:editorialNote "Getty AAT http://vocab.getty.edu/page/aat/300015217"@en ;
                 skos:exactMatch <http://vocab.getty.edu/page/aat/300015217> ;
                 skos:inScheme :Intervention ;
                 skos:topConceptOf :Intervention ;
                 skos:prefLabel "Solvent"@en , "Solvent"@en .


###  https://w3id.org/crmrp#c_b8182893
crmrp:c_b8182893 rdf:type owl:NamedIndividual ,
                          skos:Concept ;
                 rdfs:label "Engraved matrix"@en ;
                 skos:altLabel "Matrices (copper molds)"@en ;
                 skos:closeMatch <http://vocab.getty.edu/page/aat/300266816> ;
                 skos:definition "Copper molds that have been struck with a punch and from which individual type letters are cast."@en ;
                 skos:editorialNote "Getty AAT http://vocab.getty.edu/page/aat/300266816"@en ;
                 skos:inScheme :Restoration_Object ;
                 skos:prefLabel "Engraved matrix"@en , "Matrice incisa"@it ;
                 skos:topConceptOf :Restoration_Object .


###  https://w3id.org/crmrp#c_b86776d0
crmrp:c_b86776d0 rdf:type owl:NamedIndividual ,
                          skos:Concept ;
                 rdfs:label "Consolidation"@en ;
                 skos:closeMatch <http://vocab.getty.edu/page/aat/300219960> ;
                 skos:definition "Improvement of internal cohesion or mechanical stability, usually by adding material"@en ;
                 skos:editorialNote "A. Weyer et al., “EwaGlos - European Illustrated Glossary of conservation terms for wall paintings and architectural surfaces”, Michael Imhof Verlag, Petersberg, Germany"@en ,
                                    "Getty AAT http://vocab.getty.edu/page/aat/300219960"@en ,
                                    "Getty Conservation Institute “Illustrated Glossary - Definitions of terms used for the graphic documentation of in situ floor mosaics”, “Mosaics In Situ Project”, Los Angeles, 2003"@en ,
                                    "Uni En 15898:2019 Conservazione del patrimonio culturale - Termini generali e definizioni"@it ;
                 skos:inScheme :Intervention ;
                 skos:note "The preferred editorial note and the definition closest to the meaning is Uni En 15898:2019"@en ;
                 skos:prefLabel "Consolidation"@en , "Consolidamento"@it ;
                 skos:topConceptOf :Intervention .


###  https://w3id.org/crmrp#c_b9a6a1c8
crmrp:c_b9a6a1c8 rdf:type owl:NamedIndividual ,
                          skos:Concept ;
                 rdfs:label "Mosaic technique"@en ;
                 skos:definition "The different techniques to produce a mosaic, which vary according to the shape and size of the tiles."@en ;
                 skos:inScheme :Execution_Technique ;
                 skos:note "International references could not be found"@en ;
                 skos:prefLabel "Mosaic technique"@en , "Opus musivo"@it ;
                 skos:topConceptOf :Execution_Technique .


###  https://w3id.org/crmrp#c_ba5a5776
crmrp:c_ba5a5776 rdf:type owl:NamedIndividual ,
                          skos:Concept ;
                 rdfs:label "Video documentation"@en ;
                 skos:definition "Any video of an object that testifies its history or the way it was made, especially interesting for contemporary art, where the artist is sometimes shown at work."@en ;
                 skos:inScheme :Documentation ;
                 skos:note "International references could not be found"@en ;
                 skos:prefLabel "Video documentation"@en , "Documentazione video-cinematografica"@it ;
                 skos:topConceptOf :Documentation .


###  https://w3id.org/crmrp#c_bbb3b219
crmrp:c_bbb3b219 rdf:type owl:NamedIndividual ,
                          skos:Concept ;
                 rdfs:label "Drying oil"@en ;
                 skos:broader :c_143349b9 ;
                 skos:definition "Vegetable oils which form a solid, elastic film after a period of exposure to the air."@en ;
                 skos:editorialNote "A. Weyer et al., “EwaGlos - European Illustrated Glossary of conservation terms for wall paintings and architectural surfaces”, Michael Imhof Verlag, Petersberg, Germany"@en ;
                 skos:inScheme :Execution_Technique ;
                 skos:topConceptOf :Execution_Technique ;
                 skos:prefLabel "Drying oil"@en , "Olio"@it .


###  https://w3id.org/crmrp#c_bc342552
crmrp:c_bc342552 rdf:type owl:NamedIndividual ,
                          skos:Concept ;
                 rdfs:label "Swelling"@en ;
                 skos:altLabel "Blistering"@en ,
                               "Bulge"@en ;
                 skos:broader :c_13f3ce9e ;
                 skos:closeMatch <http://vocab.getty.edu/page/aat/300228350> ;
                 skos:definition "Increase in dimensions."@en ;
                 skos:editorialNote "A. Weyer et al., “EwaGlos - European Illustrated Glossary of conservation terms for wall paintings and architectural surfaces”, Michael Imhof Verlag, Petersberg, Germany"@en ,
                                    "Getty AAT http://vocab.getty.edu/page/aat/300228350"@en ,
                                    "Getty Conservation Institute “Illustrated Glossary - Technician Training for the Maintenance of In Situ Mosaics”, Los Angeles, 2013"@en ,
                                    "Uni Cen/Ts 17135:2021 - Conservation of cultural heritage. General terms and definitions"@en ,
                                    "Verg`es-Belmin et al., ICOMOS-ISCS: Illustrated glossary on stone deterioration patterns, vol. XV. Icomos International Council on Monuments and Sites, 2008"@en ;
                 skos:inScheme :Alteration ;
                 skos:topConceptOf :Alteration ;
                 skos:note "The preferred editorial note and the definition closest to the meaning is Uni Cen/Ts 17135:2021"@en ;
                 skos:prefLabel "Swelling"@en , "Rigonfiamento"@it .


###  https://w3id.org/crmrp#c_bc53d2a2
crmrp:c_bc53d2a2 rdf:type owl:NamedIndividual ,
                          skos:Concept ;
                 rdfs:label "Buckled"@en ;
                 skos:altLabel "Buckling"@en ;
                 skos:broader :c_13f3ce9e ;
                 skos:closeMatch <http://vocab.getty.edu/page/aat/300072663> ;
                 skos:definition "Exhibiting wavelike deformation"@en ;
                 skos:editorialNote "Getty AAT http://vocab.getty.edu/page/aat/300072663"@en ,
                                    "Uni Cen/Ts 17135:2021 - Conservation of cultural heritage. General terms and definitions"@en ;
                 skos:inScheme :Alteration ;
                 skos:topConceptOf :Alteration ;
                 skos:note "The preferred editorial note and the definition closest to the meaning is Uni Cen/Ts 17135:2021"@en ;
                 skos:prefLabel "Buckled"@en , "Incurvatura"@it .


###  https://w3id.org/crmrp#c_bc7a9a95
crmrp:c_bc7a9a95 rdf:type owl:NamedIndividual ,
                          skos:Concept ;
                 rdfs:label "Darkened"@en ;
                 skos:broader :c_df05cb61 ;
skos:definition "Exhibiting reduced light reflectivity, hue and/or lightness"@en ;
                 skos:closeMatch <http://vocab.getty.edu/page/aat/300379491> ;
                 skos:editorialNote "A. Weyer et al., “EwaGlos - European Illustrated Glossary of conservation terms for wall paintings and architectural surfaces”, Michael Imhof Verlag, Petersberg, Germany"@en ,
                                    "Getty AAT http://vocab.getty.edu/page/aat/300379491"@en ,
                                    "Uni Cen/Ts 17135:2021 - Conservation of cultural heritage. General terms and definitions"@en ;
                 skos:inScheme :Alteration ;
                 skos:topConceptOf :Alteration ;
                 skos:note "The preferred editorial note and the definition closest to the meaning is Uni Cen/Ts 17135:2021"@en ;
                 skos:prefLabel "Darkened"@en , "Scurimento"@it .


###  https://w3id.org/crmrp#c_bcebc1fb
crmrp:c_bcebc1fb rdf:type owl:NamedIndividual ,
                          skos:Concept ;
                 rdfs:label "Encausto"@en ;
                 skos:altLabel "Encaustic painting"@en ;
                 skos:broader :c_6626f18c ;
                 skos:closeMatch <http://vocab.getty.edu/page/aat/300053353> ;
                 skos:definition "Painting technique using a heated mixture of pigments, molten wax and resin."@en ;
                 skos:editorialNote "A. Weyer et al., “EwaGlos - European Illustrated Glossary of conservation terms for wall paintings and architectural surfaces”, Michael Imhof Verlag, Petersberg, Germany"@en ,
                                    "AAT Getty http://vocab.getty.edu/page/aat/300053353"@en ;
                 skos:inScheme :Execution_Technique ;
                 skos:topConceptOf :Execution_Technique ;
                 skos:note "The preferred editorial note and the definition closest to the meaning is EwaGlos - European Illustrated Glossary of conservation terms for wall paintings and architectural surfaces"@en ;
                 skos:prefLabel "Encausto"@en , "Encausto"@it .


###  https://w3id.org/crmrp#c_bd34e984
crmrp:c_bd34e984 rdf:type owl:NamedIndividual ,
                          skos:Concept ;
                 rdfs:label "Ceramic"@en ;
                 skos:definition "A hard and brittle, heat- and corrosion-resistant material, made by shaping clay or similar earth materials and subsequently firing them at high temperatures."@en ;
                 skos:editorialNote "A. Weyer et al., “EwaGlos - European Illustrated Glossary of conservation terms for wall paintings and architectural surfaces”, Michael Imhof Verlag, Petersberg, Germany"@en ;
                 skos:inScheme :Material ;
                 skos:prefLabel "Ceramic"@en , "Ceramica"@it ;
                 skos:topConceptOf :Material .


###  https://w3id.org/crmrp#c_bd37c76d
crmrp:c_bd37c76d rdf:type owl:NamedIndividual ,
                          skos:Concept ;
                 rdfs:label "Graffito"@en ;
                 skos:broader :c_757ed6ec ;
                 skos:definition "The technique derives from the way gold leaf is treated in wall decoration. "@en ;
                 skos:editorialNote "G. Pignolo, “Effetti d’oro - Storia e tecnica della doratura nell’arte”, Editrice Compositori, Bologna, 2002"@it ;
                 skos:inScheme :Execution_Technique ;
                 skos:topConceptOf :Execution_Technique ;
                 skos:note "International references could not be found"@en ;
                 skos:prefLabel "Graffito"@en , "Graffito"@it .


###  https://w3id.org/crmrp#c_bfe86ad2
crmrp:c_bfe86ad2 rdf:type owl:NamedIndividual ,
                          skos:Concept ;
                 rdfs:label "Chemical patinatura"@en ;
                 skos:broader :c_f1c689bb ;
                 skos:definition "Chemical patinas always involve a chemical reaction between the metal and the reagent that will be used. Depending on the reagents and the exposure time, different results will occur."@en ;
                 skos:editorialNote "A.Giuffredi, “Formatura e fonderia”, Alinea editrice, Firenze, 2010"@it ;
                 skos:inScheme :Execution_Technique ;
                 skos:topConceptOf :Execution_Technique ;
                 skos:note "International references could not be found"@en ;
                 skos:prefLabel "Chemical patinatura"@en , "Patinatura chimica"@it .


###  https://w3id.org/crmrp#c_c006ffaa
crmrp:c_c006ffaa rdf:type owl:NamedIndividual ,
                          skos:Concept ;
                 rdfs:label "Photographic reproduction from archival sources"@en ;
                 skos:broader :c_773e0829 ;
                 skos:definition "Photographic document showing how the artwork looked in the past"@en ;
                 skos:inScheme :Documentation ;
                 skos:topConceptOf :Documentation ;
                 skos:note "International references could not be found"@en ;
                 skos:prefLabel "Photographic reproduction from archival sources"@en , "Riproduzione fotografica da fonte archivistica"@it .


###  https://w3id.org/crmrp#c_c10ff387
crmrp:c_c10ff387 rdf:type owl:NamedIndividual ,
                          skos:Concept ;
                 rdfs:label "Numismatics"@en ;
                 skos:closeMatch <http://vocab.getty.edu/page/aat/300054419> ;
                 skos:definition "Study of coins, tokens, medals, paper money, and objects closely resembling them in form or purpose."@en ;
                 skos:editorialNote "Getty AAT http://vocab.getty.edu/page/aat/300054419"@en ;
                 skos:inScheme :Restoration_Object ;
                 skos:prefLabel "Numismatica"@en , "Numismatico"@it ;
                 skos:topConceptOf :Restoration_Object .


###  https://w3id.org/crmrp#c_c202f020
crmrp:c_c202f020 rdf:type owl:NamedIndividual ,
                          skos:Concept ;
                 rdfs:label "Stratigraphic investigation"@en ;
                 skos:broader :c_abed88a5 ;
                 skos:definition "The stepwise removal of covering paint layers for analysis and determination of the chronological order of successive paint layers."@en ;
                 skos:editorialNote "A. Weyer et al., “EwaGlos - European Illustrated Glossary of conservation terms for wall paintings and architectural surfaces”, Michael Imhof Verlag, Petersberg, Germany"@en ;
                 skos:inScheme :Archeometric_and_Diagnostic_Analysis ;
                 skos:topConceptOf :Archeometric_and_Diagnostic_Analysis ;
                 skos:prefLabel "Stratigraphic investigation"@en , "Saggio stratigrafico"@it .


###  https://w3id.org/crmrp#c_c2349eb7
crmrp:c_c2349eb7 rdf:type owl:NamedIndividual ,
                          skos:Concept ;
                 rdfs:label "Emergency measure"@en ;
                 skos:altLabel "Securing"@en ;
                 skos:definition "Treatments that aim to temporarily halt active deterioration and preserve a part of or the entire artwork."@en ;
                 skos:editorialNote "A. Weyer et al., “EwaGlos - European Illustrated Glossary of conservation terms for wall paintings and architectural surfaces”, Michael Imhof Verlag, Petersberg, Germany"@en ;
                 skos:inScheme :Intervention ;
                 skos:prefLabel "Emergency measure"@en , "Messa in sicurezza"@it ;
                 skos:topConceptOf :Intervention .


###  https://w3id.org/crmrp#c_c246124b
crmrp:c_c246124b rdf:type owl:NamedIndividual ,
                          skos:Concept ;
                 rdfs:label "Project"@en ;
                 skos:broader :c_5b7fce15 ;
                 skos:definition "Conception, mostly accompanied by a study on the possibilities of implementation or execution."@en ;
                 skos:inScheme :Documentation ;
                 skos:topConceptOf :Documentation ;
                 skos:note "International references could not be found"@en ;
                 skos:prefLabel "Project"@en , "Progetto"@it .


###  https://w3id.org/crmrp#c_c41a962a
crmrp:c_c41a962a rdf:type owl:NamedIndividual ,
                          skos:Concept ;
                 rdfs:label "Hot-foil patinatura"@en ;
                 skos:broader :c_e5a56926 ;
                 skos:definition "Some varieties of enamels and inks need to be applied while the metal surface is hot."@en ;
                 skos:editorialNote "A.Giuffredi, “Formatura e fonderia”, Alinea editrice, Firenze"@it ;
                 skos:inScheme :Execution_Technique ;
                 skos:topConceptOf :Execution_Technique ;
                 skos:note "International references could not be found"@en ;
                 skos:prefLabel "Hot-foil patinatura"@en , "Patinatura dipinta a caldo"@it .


###  https://w3id.org/crmrp#c_c5481024
crmrp:c_c5481024 rdf:type owl:NamedIndividual ,
                          skos:Concept ;
                 rdfs:label "Ultraviolet-visible spectroscopy "@en ;
                 skos:broader :c_789c3e32 ;
                 skos:closeMatch <http://vocab.getty.edu/page/aat/300375717> ;
                 skos:definition "The study of emission and absorption spectra via absorption spectroscopy or reflectance spectroscopy over wavelengths in the ultraviolet and visible region of the electromagnetic spectrum"@en ;
                 skos:editorialNote "Getty AAT http://vocab.getty.edu/page/aat/300375717"@en ;
                 skos:inScheme :Archeometric_and_Diagnostic_Analysis ;
                 skos:topConceptOf :Archeometric_and_Diagnostic_Analysis ;
                 skos:prefLabel "Ultraviolet-visible spectroscopy"@en , "Spettrofotometria UV/Visibile"@it .


###  https://w3id.org/crmrp#c_c5825f0c
crmrp:c_c5825f0c rdf:type owl:NamedIndividual ,
                          skos:Concept ;
                 rdfs:label "Level of alkalinity/acidity"@en ;
                 skos:broader :c_1fd6102e ;
                 skos:definition "The pH value can be determined electrically, exploiting the potential created by the difference in hydrogen ion concentration on two sides of a glass membrane, using an electronic instrument known as a pH meter"@en ;
                 skos:inScheme :Archeometric_and_Diagnostic_Analysis ;
                 skos:topConceptOf :Archeometric_and_Diagnostic_Analysis ;
                 skos:note "International references could not be found"@en ;
                 skos:prefLabel "Level of alkalinity/acidity"@en , "Determinazione pH"@it .


###  https://w3id.org/crmrp#c_c7591bf7
crmrp:c_c7591bf7 rdf:type owl:NamedIndividual ,
                          skos:Concept ;
                 rdfs:label "Stacco"@en ;
                 skos:broader :c_4fe4d308 ;
                 skos:definition "The process of detaching a fresco painting from the wall by removing the pigment layer and a layer of intonaco. Cloth is glued to the painted surface and, when dry, the cloth, painting, and plaster are stripped from the wall."@en ;
                 skos:editorialNote "A. Weyer et al., “EwaGlos - European Illustrated Glossary of conservation terms for wall paintings and architectural surfaces”, Michael Imhof Verlag, Petersberg, Germany"@en ,
                                    "Getty AAT http://vocab.getty.edu/page/aat/300078739"@en ;
                 skos:exactMatch <http://vocab.getty.edu/page/aat/300078739> ;
                 skos:inScheme :Intervention ;
                 skos:topConceptOf :Intervention ;
                 skos:note "The preferred editorial note and the definition closest to the meaning is Getty AAT"@en ;
                 skos:prefLabel "Stacco"@en , "Stacco"@it .


###  https://w3id.org/crmrp#c_c7a69d6a
crmrp:c_c7a69d6a rdf:type owl:NamedIndividual ,
                          skos:Concept ;
                 rdfs:label "Ion-exchange chromatography (IC)"@en ;
                 skos:broader :c_2d5cde83 ;
                 skos:definition "Chromatography that depends on the reciprocal transfer of ions between a solution and a resin or other suitable solid."@en ;
                 skos:editorialNote "Getty AAT http://vocab.getty.edu/page/aat/300214723"@en ;
                 skos:exactMatch <http://vocab.getty.edu/page/aat/300214723> ;
                 skos:inScheme :Archeometric_and_Diagnostic_Analysis ;
                 skos:topConceptOf :Archeometric_and_Diagnostic_Analysis ;
                 skos:prefLabel "Ion-exchange chromatography (IC)"@en , "Cromatografia ionica (CI)"@it .


###  https://w3id.org/crmrp#c_c8704394
crmrp:c_c8704394 rdf:type owl:NamedIndividual ,
                          skos:Concept ;
                 rdfs:label "Astrazione cromatica"@en ;
                 skos:broader :c_326da7e4 ;
                 skos:definition "Using four pure colours on a light background applied with short hatched lines, an abstract structure is created. This structure merges optically with the contiguous original."@en ;
                 skos:editorialNote "A. Weyer et al., “EwaGlos - European Illustrated Glossary of conservation terms for wall paintings and architectural surfaces”, Michael Imhof Verlag, Petersberg, Germany"@en ;
                 skos:inScheme :Intervention ;
                 skos:topConceptOf :Intervention ;
                 skos:prefLabel "Astrazione cromatica"@en , "Astrazione cromatica"@it .


###  https://w3id.org/crmrp#c_cb6d58c9
crmrp:c_cb6d58c9 rdf:type owl:NamedIndividual ,
                          skos:Concept ;
                 rdfs:label "Wood"@en ;
                 skos:definition "The principal tissue of trees and other plants that provides both strength and a means of conducting nutrients. Wood is one of the most versatile materials known."@en ;
                 skos:editorialNote "Getty AAT http://vocab.getty.edu/page/aat/300014109"@en ;
                 skos:exactMatch <http://vocab.getty.edu/page/aat/300014109> ;
                 skos:inScheme :Material ;
                 skos:prefLabel "Wood"@en , "Legno"@it ;
                 skos:topConceptOf :Material .


###  https://w3id.org/crmrp#c_cbe3d99a
crmrp:c_cbe3d99a rdf:type owl:NamedIndividual ,
                          skos:Concept ;
                 rdfs:label "Splitting"@en ;
                 skos:broader :c_8c762c3e ;
                 skos:definition "Fracturing of a stone along planes of weakness such as microcracks or clay/silt layers, in case where the structural elements are orientated vertically. For instance, a column may split into several parts along bedding planes if the load above it is too high"@en ;
                 skos:editorialNote "Verg`es-Belmin et al., ICOMOS-ISCS: Illustrated glossary on stone deterioration patterns, vol. XV. Icomos International Council on Monuments and Sites, 2008"@en ;
                 skos:inScheme :Alteration ;
                 skos:topConceptOf :Alteration ;
                 skos:prefLabel "Splitting"@en , "Fenditura"@it .


###  https://w3id.org/crmrp#c_cc85125b
crmrp:c_cc85125b rdf:type owl:NamedIndividual ,
                          skos:Concept ;
                 rdfs:label "Screen printing"@en ;
                 skos:broader :c_aee6a805 ;
                 skos:closeMatch <http://vocab.getty.edu/page/aat/300053281> ;
                 skos:definition "Stencil technique of printing in which ink or dye is forced through a mesh, traditionally silk, on which a design has been formed by stopping out certain areas."@en ;
                 skos:editorialNote "Getty AAT http://vocab.getty.edu/page/aat/300053281"@en ;
                 skos:inScheme :Execution_Technique ;
                 skos:topConceptOf :Execution_Technique ;
                 skos:prefLabel "Screen printing"@en , "Serigrafia"@it .


###  https://w3id.org/crmrp#c_cf59824d
crmrp:c_cf59824d rdf:type owl:NamedIndividual ,
                          skos:Concept ;
                 rdfs:label "Clothing"@en ;
                 skos:closeMatch <http://vocab.getty.edu/page/aat/300266639> ;
                 skos:definition "Coverings for the torso, limbs, hands, feet, and head for warmth, fashion, or to cover nudity. It generally excludes other items of costume such as jewelry, crowns, and other accessories that are purely decorative or symbolic and have no practical function."@en ;
                 skos:editorialNote "Getty AAT http://vocab.getty.edu/page/aat/300266639"@en ;
                 skos:inScheme :Restoration_Object ;
                 skos:prefLabel "Clothing"@en , "Vestimento"@it ;
                 skos:topConceptOf :Restoration_Object .


###  https://w3id.org/crmrp#c_cf65605c
crmrp:c_cf65605c rdf:type owl:NamedIndividual ,
                          skos:Concept ;
                 rdfs:label "Glazed decoration"@en ;
                 skos:broader :c_bd34e984 ;
                 skos:closeMatch "Glazed decoration"@en ;
                 skos:definition "Façade and interior wall ornaments made with polychrome and glazed bricks or terracotta tiles."@en ;
                 skos:editorialNote "A. Weyer et al., “EwaGlos - European Illustrated Glossary of conservation terms for wall paintings and architectural surfaces”, Michael Imhof Verlag, Petersberg, Germany"@en ;
                 skos:inScheme :Material ;
                 skos:topConceptOf :Material ;
                 skos:prefLabel "Glazed decoration"@en , "Maiolica"@it .


###  https://w3id.org/crmrp#c_d02e5354
crmrp:c_d02e5354 rdf:type owl:NamedIndividual ,
                          skos:Concept ;
                 rdfs:label "Oxidation"@en ;
                 skos:broader :c_ae321441 ;
                 skos:definition "The process or result of combining with oxygen; sometimes contributing to the degradation of a surface, such as in corrosion."@en ;
                 skos:editorialNote "Getty AAT http://vocab.getty.edu/page/aat/300220235"@en ;
                 skos:exactMatch <http://vocab.getty.edu/page/aat/300220235> ;
                 skos:inScheme :Alteration ;
                 skos:topConceptOf :Alteration ;
                 skos:prefLabel "Oxidation"@en , "Ossidazione"@it .


###  https://w3id.org/crmrp#c_d057b901
crmrp:c_d057b901 rdf:type owl:NamedIndividual ,
                          skos:Concept ;
                 rdfs:label "Tear"@en ;
                 skos:altLabel "Tears"@en , "Strappo"@it ;
                 skos:closeMatch <http://vocab.getty.edu/page/aat/30025413> ;
                 skos:definition "Separation with irregular edges through the thickness of a visco-elastic material"@en ;
                 skos:editorialNote "Getty AAT http://vocab.getty.edu/page/aat/300254138"@en ,
                                    "Uni Cen/Ts 17135:2021 - Conservation of cultural heritage. General terms and definitions"@en ;
                 skos:inScheme :Alteration ;
                 skos:note "The preferred editorial note and the definition closest to the meaning is Uni Cen/Ts 17135:2021"@en ;
                 skos:prefLabel "Tear"@en , "Lacerazione"@it ;
                 skos:topConceptOf :Alteration .


###  https://w3id.org/crmrp#c_d342102c
crmrp:c_d342102c rdf:type owl:NamedIndividual ,
                          skos:Concept ;
                 rdfs:label "Protection"@en ;
                 skos:definition "Action involving the application of a film-forming substance applied in fluid form to the surface of an item; its task is to preserve the surface from contact with the environment."@en ;
                 skos:editorialNote "C. Giannini, “Dizionario del restauro - Tecniche diagnostica conservazione”, Nardini Editore, Firenze, 2010"@it ;
                 skos:inScheme :Intervention ;
                 skos:prefLabel "Protection"@en , "Protezione"@it ;
                 skos:topConceptOf :Intervention .


###  https://w3id.org/crmrp#c_d54b0be2
crmrp:c_d54b0be2 rdf:type owl:NamedIndividual ,
                          skos:Concept ;
                 rdfs:label "Detachment"@en ;
                 skos:definition "Break in continuity between layers of a plaster, both between them and in relation to the substrate, which generally preludes the fall of the layers themselves."@en ;
                 skos:editorialNote "Uni 11182:2006 - Materiali lapidei naturali ed artificiali. Descrizione della forma di alterazione - Termini e definizioni"@it ,
                                    "Verg`es-Belmin et al., ICOMOS-ISCS: Illustrated glossary on stone deterioration patterns, vol. XV. Icomos International Council on Monuments and Sites, 2008"@en ;
                 skos:inScheme :Alteration ;
                 skos:prefLabel "Detachment"@en , "Distacco"@it ;
                 skos:topConceptOf :Alteration .


###  https://w3id.org/crmrp#c_d5d25610
crmrp:c_d5d25610 rdf:type owl:NamedIndividual ,
                          skos:Concept ;
                 rdfs:label "Pastille gilding"@en ;
                 skos:broader :c_757ed6ec ;
                 skos:definition "A technique used by ancient decorators to reproduce friezes and high reliefs on different supports. The mixture consists of plaster, scagliola and starch glue."@en ;
                 skos:editorialNote "C. Giannini, “Dizionario del restauro - Tecniche diagnostica conservazione”, Nardini Editore, Firenze, 2010"@it ,
                                    "G. Pignolo, “Effetti d’oro - Storia e tecnica della doratura nell’arte”, Editrice Compositori, Bologna, 2002"@it ;
                 skos:inScheme :Execution_Technique ;
                 skos:topConceptOf :Execution_Technique ;
                 skos:note "International references could not be found, but the preferred editorial note and the definition closest to the meaning is Effetti d’oro - Storia e tecnica della doratura nell’arte"@en ;
                 skos:prefLabel "Pastille gilding"@en , "Pastiglia"@it .


###  https://w3id.org/crmrp#c_d68fd470
crmrp:c_d68fd470 rdf:type owl:NamedIndividual ,
                          skos:Concept ;
                 rdfs:label "Intarsia"@en ;
                 skos:broader :c_051209b3 ;
                 skos:closeMatch <http://vocab.getty.edu/page/aat/300053852> ;
                 skos:definition "Decorative wood process in which the design or pattern is made by assembling small pieces of veneer in various shapes. The term, which derives from 15th-century Italy, is commonly used to describe both marquetry, in which the entire surface is veneered, and wood inlay, in which the pattern pieces are laid into a solid ground. The term may also be used to refer to similar works of stone, glass, or another material. Distinguished from mosaics, as pieces in intarsia work are precision-cut to tightly fit together"@en ;
                 skos:editorialNote "Getty AAT http://vocab.getty.edu/page/aat/300053852"@en ,
                                    "The Getty Conservation Institute, “The structural conservation of panel paintings”, Proceedings of a Symposium at the J. Paul Getty Museum, 24 - 28 April 1995"@en ;
                 skos:inScheme :Execution_Technique ;
                 skos:topConceptOf :Execution_Technique ;
                 skos:note "The preferred editorial note and the definition closest to the meaning is Getty AAT"@en ;
                 skos:prefLabel "Intarsia"@en , "Intarsio"@it .


###  https://w3id.org/crmrp#c_d69776d7
crmrp:c_d69776d7 rdf:type owl:NamedIndividual ,
                          skos:Concept ;
                 rdfs:label "Treatment trials"@en ;
                 skos:broader :c_830e6744 ;
                 skos:definition "Small areas of the object on which cleaning, consolidation, or reintegration tests are carried out."@en ;
                 skos:editorialNote "A. Weyer et al., “EwaGlos - European Illustrated Glossary of conservation terms for wall paintings and architectural surfaces”, Michael Imhof Verlag, Petersberg, Germany"@en ;
                 skos:inScheme :Intervention ;
                 skos:topConceptOf :Intervention ;
                 skos:prefLabel "Treatment trials"@en , "Prova di pulitura"@it .


###  https://w3id.org/crmrp#c_d999bf3e
crmrp:c_d999bf3e rdf:type owl:NamedIndividual ,
                          skos:Concept ;
                 rdfs:label "Analytical techniques of Fourier transform infrared spectroscopy (FTIR)"@en ;
                 skos:broader :c_789c3e32 ;
                 skos:closeMatch <http://vocab.getty.edu/page/aat/300391288> ;
                 skos:definition "Fourier transform infrared spectroscopy adapted for selective analysis of components of heterogeneous samples on a micrometer scale."@en ;
                 skos:editorialNote "Getty AAT http://vocab.getty.edu/page/aat/300391288"@en ;
                 skos:inScheme :Archeometric_and_Diagnostic_Analysis ;
                 skos:topConceptOf :Archeometric_and_Diagnostic_Analysis ;
                 skos:prefLabel "Analytical techniques of Fourier transform infrared spectroscopy (FTIR)"@en , "Spettrofotometria infrarossa in trasformata di Fuorier (FTIR)"@it .


###  https://w3id.org/crmrp#c_d9bb34c7
crmrp:c_d9bb34c7 rdf:type owl:NamedIndividual ,
                          skos:Concept ;
                 rdfs:label "Bibliography"@en ;
                 skos:broader :c_5b7fce15 ;
                 skos:definition "List, note, or other recording of the bibliography for a work or other entity's documentation."@en ;
                 skos:editorialNote "Getty AAT http://vocab.getty.edu/page/aat/300435419"@en ;
                 skos:exactMatch <http://vocab.getty.edu/page/aat/300435419> ;
                 skos:inScheme :Documentation ;
                 skos:topConceptOf :Documentation ;
                 skos:prefLabel "Bibliography"@en , "Bibliografia"@it .


###  https://w3id.org/crmrp#c_db001ba3
crmrp:c_db001ba3 rdf:type owl:NamedIndividual ,
                          skos:Concept ;
                 rdfs:label "Determination of water content"@en ;
                 skos:broader :c_1fd6102e ;
                 skos:editorialNote "UNI 11085:2003 Beni culturali - Materiali lapidei naturali ed artificiali - Determinazione del contenuto d'acqua: Metodo ponderale"@it ;
                 skos:inScheme :Archeometric_and_Diagnostic_Analysis ;
                 skos:topConceptOf :Archeometric_and_Diagnostic_Analysis ;
                 skos:note "International references could not be found"@en ;
                 skos:prefLabel "Determination of water content"@en , "Determinazione del contenuto d'acqua"@it .


###  https://w3id.org/crmrp#c_dc1f704e
crmrp:c_dc1f704e rdf:type owl:NamedIndividual ,
                          skos:Concept ;
                 rdfs:label "Encausto"@en ;
                 skos:broader :c_051209b3 ;
                 skos:definition "Painting technique using wax as a binder wax as a binder, either hot or cold mixed with pigments and also with resins."@en ;
                 skos:editorialNote "A. Weyer et al., “EwaGlos - European Illustrated Glossary of conservation terms for wall paintings and architectural surfaces”, Michael Imhof Verlag, Petersberg, Germany"@en ;
                 skos:inScheme :Execution_Technique ;
                 skos:topConceptOf :Execution_Technique ;
                 skos:prefLabel "Encausto"@en , "Encausto"@it .


###  https://w3id.org/crmrp#c_dd7e90e1
crmrp:c_dd7e90e1 rdf:type owl:NamedIndividual ,
                          skos:Concept ;
                 rdfs:label "Haze"@en ;
                 skos:broader :c_4d471b17 ;
                 skos:definition "Gold foil residues are removed with brushes or cotton to make the glaze opaque"@en ;
                 skos:editorialNote "G. Pignolo, “Effetti d’oro - Storia e tecnica della doratura nell’arte”, Editrice Compositori, Bologna, 2002"@it ;
                 skos:inScheme :Execution_Technique ;
                 skos:topConceptOf :Execution_Technique ;
                 skos:note "International references could not be found"@en ;
                 skos:prefLabel "Haze"@en , "Velatura"@it .


###  https://w3id.org/crmrp#c_df05cb61
crmrp:c_df05cb61 rdf:type owl:NamedIndividual ,
                          skos:Concept ;
                 rdfs:label "Colour alteration"@en ;
                 skos:altLabel "Discolouration"@en ;
                 skos:definition "Change in at least one of the three colour parameters hue, lightness and chroma."@en ;
                 skos:editorialNote "Getty AAT http://vocab.getty.edu/page/aat/300053045"@en ,
                                    "Getty Conservation Institute “Illustrated Glossary - Definitions of terms used for the graphic documentation of in situ floor mosaics”, “Mosaics In Situ Project”, Los Angeles, 2003"@en ,
                                    "Uni Cen/Ts 17135:2021 - Conservation of cultural heritage. General terms and definitions"@en ,
                                    "Verg`es-Belmin et al., ICOMOS-ISCS: Illustrated glossary on stone deterioration patterns, vol. XV. Icomos International Council on Monuments and Sites, 2008"@en ;
                 skos:exactMatch <http://vocab.getty.edu/page/aat/300053045> ;
                 skos:inScheme :Alteration ;
                 skos:note "The preferred editorial note and the definition closest to the meaning is Uni Cen/Ts 17135:2021"@en ;
                 skos:prefLabel "Colour alteration"@en , "Alterazione cromatica"@it ;
                 skos:topConceptOf :Alteration .


###  https://w3id.org/crmrp#c_df7c7c9c
crmrp:c_df7c7c9c rdf:type owl:NamedIndividual ,
                          skos:Concept ;
                 rdfs:label "Collage"@en ;
                 skos:broader :c_143349b9, :c_051209b3;
                 skos:definition "Refers to the technique of making compositions in two dimensions or very low relief by gluing paper, fabrics, photographs, or other materials onto a flat surface."@en ;
                 skos:editorialNote "Getty AAT http://vocab.getty.edu/page/aat/300138699"@en ;
                 skos:exactMatch <http://vocab.getty.edu/page/aat/300138699> ;
                 skos:inScheme :Execution_Technique ;
                 skos:topConceptOf :Execution_Technique ;
                 skos:prefLabel "Collage"@en , "Collage"@it .




###  https://w3id.org/crmrp#c_e078e94e
crmrp:c_e078e94e rdf:type owl:NamedIndividual ,
                          skos:Concept ;
                 rdfs:label "Pre-consolidation"@en ;
                 skos:definition "Set of preventive treatments aimed at avoiding possible loss of material during subsequent restoration operations and/or preserving the artefact in its current state pending more specific targeted interventions in the immediate future."@en ;
                 skos:inScheme :Intervention ;
                 skos:note "International references could not be found"@en ;
                 skos:prefLabel "Pre-consolidation"@en , "Pre-consolidamento"@it ;
                 skos:topConceptOf :Intervention .


###  https://w3id.org/crmrp#c_e2f34e0a
crmrp:c_e2f34e0a rdf:type owl:NamedIndividual ,
                          skos:Concept ;
                 rdfs:label "Loss of gloss"@en ;
                 skos:broader :c_df05cb61 ;
                 skos:definition "Shift from a shiny toward a matt surface appearance"@en ;
                 skos:editorialNote "Uni Cen/Ts 17135:2021 - Conservation of cultural heritage. General terms and definitions"@en ;
                 skos:inScheme :Alteration ;
                 skos:topConceptOf :Alteration ;
                 skos:prefLabel "Loss of gloss"@en , "Opacizzazione"@it .


###  https://w3id.org/crmrp#c_e3781f70
crmrp:c_e3781f70 rdf:type owl:NamedIndividual ,
                          skos:Concept ;
                 rdfs:label "Infrared photography"@en ;
                 skos:broader :c_1fd6102e ;
                 skos:closeMatch <http://vocab.getty.edu/page/aat/300053463> ;
                 skos:definition " Technique using film sensitive to both some visible light waves and to wavelengths generated by the infrared segment of the electromagnetic spectum."@en ;
                 skos:editorialNote "Getty AAT http://vocab.getty.edu/page/aat/300053463"@en ;
                 skos:inScheme :Archeometric_and_Diagnostic_Analysis ;
                 skos:topConceptOf :Archeometric_and_Diagnostic_Analysis ;
                 skos:prefLabel "Infrared photography"@en , "Infrarosso fotografico"@it .


###  https://w3id.org/crmrp#c_e5a56926
crmrp:c_e5a56926 rdf:type owl:NamedIndividual ,
                          skos:Concept ;
                 rdfs:label "Painted patinatura"@en ;
                 skos:broader :c_f1c689bb ;
                 skos:definition "Painted patina involves the use of coloured waxes or enamels, which colour the surface of the metal. It is a type of non-chemical patina that therefore does not involve deterioration of the metal."@en ;
                 skos:editorialNote "A.Giuffredi, “Formatura e fonderia”, Alinea editrice, Firenze, 2010"@it ;
                 skos:inScheme :Execution_Technique ;
                 skos:topConceptOf :Execution_Technique ;
                 skos:note "International references could not be found"@en ;
                 skos:prefLabel "Painted patinatura"@en , "Patinatura dipinta"@it .


###  https://w3id.org/crmrp#c_e5ce4664
crmrp:c_e5ce4664 rdf:type owl:NamedIndividual ,
                          skos:Concept ;
                 rdfs:label "Determination of water vapour permeability (dp)"@en ;
                 skos:broader :c_1fd6102e ;
                 skos:definition "The test is a method for the determination of water vapour permeability under conditions of steady-state flow for low and high humidity conditions of a sample"@en ;
                 skos:editorialNote "UNI EN 15803:2010 Conservazione dei beni culturali - Metodi di prova - Determinazione della permeabilità al vapore d'acqua (dp)"@it ;
                 skos:inScheme :Archeometric_and_Diagnostic_Analysis ;
                 skos:topConceptOf :Archeometric_and_Diagnostic_Analysis ;
                 skos:prefLabel "Determination of water vapour permeability (dp)"@en , "Determinazione delle permeabilità al vapore d'acqua (dp)"@it .


###  https://w3id.org/crmrp#c_e5f8a87b
crmrp:c_e5f8a87b rdf:type owl:NamedIndividual ,
                          skos:Concept ;
                 rdfs:label "Thermogravimetry"@en ;
                 skos:broader :c_abed88a5 ;
                 skos:definition "A technique that chemically analyzes a substance by measuring changes in its weight due to increasing temperature. It can be used to study the stability of materials."@en ;
                 skos:editorialNote "Getty AAT http://vocab.getty.edu/page/aat/300393228"@en ;
                 skos:exactMatch <http://vocab.getty.edu/page/aat/300393228> ;
                 skos:inScheme :Archeometric_and_Diagnostic_Analysis;
                 skos:topConceptOf :Archeometric_and_Diagnostic_Analysis ;
                 skos:prefLabel "Thermogravimetry"@en , "Termogravimetria"@it .


###  https://w3id.org/crmrp#c_e763e25d
crmrp:c_e763e25d rdf:type owl:NamedIndividual ,
                          skos:Concept ;
                 rdfs:label "Efflorescence"@en ;
                 skos:definition "Accumulation of salt crystals on the surface of an object"@en ;
                 skos:editorialNote "A. Weyer et al., “EwaGlos - European Illustrated Glossary of conservation terms for wall paintings and architectural surfaces”, Michael Imhof Verlag, Petersberg, Germany"@en ,
                                    "Getty AAT http://vocab.getty.edu/page/aat/300214748"@en ,
                                    "Getty Conservation Institute “Illustrated Glossary - Definitions of terms used for the graphic documentation of in situ floor mosaics”, “Mosaics In Situ Project”, Los Angeles, 2003"@en ,
                                    "Uni Cen/Ts 17135:2021 - Conservation of cultural heritage. General terms and definitions"@en ,
                                    "Verg`es-Belmin et al., ICOMOS-ISCS: Illustrated glossary on stone deterioration patterns, vol. XV. Icomos International Council on Monuments and Sites, 2008"@en ;
                 skos:exactMatch <http://vocab.getty.edu/page/aat/300214748> ;
                 skos:inScheme :Alteration ;
                 skos:note "The preferred editorial note and the definition closest to the meaning is Uni Cen/Ts 17135:2021"@en ;
                 skos:prefLabel "Efflorescence"@en , "Efflorescenza"@it ;
                 skos:topConceptOf :Alteration .


###  https://w3id.org/crmrp#c_e7949d93
crmrp:c_e7949d93 rdf:type owl:NamedIndividual ,
                          skos:Concept ;
                 rdfs:label "Porcelain"@en ;
                 skos:broader :c_bd34e984 ;
                 skos:closeMatch <http://vocab.getty.edu/page/aat/300010662> ;
                 skos:definition "A material comprising white clay, or kaolin, and a feldspathic rock, that react when fired so the clay serves to hold the shape of the object and the rock fuses into a natural glass. In China, it includes any such ware that is highly fired enough to produce a ringing sound when struck. In Europe, it is limited to hard-fired ceramic that is translucent."@en ;
                 skos:editorialNote "Getty AAT http://vocab.getty.edu/page/aat/300010662"@en ;
                 skos:inScheme :Material ;
                 skos:topConceptOf :Material ;
                 skos:prefLabel "Porcelain"@en, "Porcellana"@it .


###  https://w3id.org/crmrp#c_e7a46f25
crmrp:c_e7a46f25 rdf:type owl:NamedIndividual ,
                          skos:Concept ;
                 rdfs:label "Radiocarbon dating"@en ;
                 skos:broader :c_abed88a5 ;
                 skos:definition "Method of dating, based on the known half-life of carbon-14, by measuring the amount of low-level radioactivity of carbon remaining in ancient and dead material of organic origin and thus determining when a plant or animal had died."@en ;
                 skos:editorialNote "Getty AAT http://vocab.getty.edu/page/aat/300054717"@en ;
                 skos:exactMatch <http://vocab.getty.edu/page/aat/300054717> ;
                 skos:inScheme :Archeometric_and_Diagnostic_Analysis ;
                 skos:topConceptOf :Archeometric_and_Diagnostic_Analysis ;
                 skos:prefLabel "Radiocarbon dating"@en , "Radiocarbonio"@it .


###  https://w3id.org/crmrp#c_e80de18f
crmrp:c_e80de18f rdf:type owl:NamedIndividual ,
                          skos:Concept ;
                 rdfs:label "Neutral reintegration"@en ;
                 skos:broader :c_326da7e4 ;
                 skos:definition "When a damaged area or lacuna cannot be reconstructed due to its size, lack of reliable sources, or the artistic importance of the work of art, its negative optical impact on the original can be reduced by toning down the damage or lacuna with a so-called “neutral” colour, thereby moving it into the background."@en ;
                 skos:editorialNote "A. Weyer et al., “EwaGlos - European Illustrated Glossary of conservation terms for wall paintings and architectural surfaces”, Michael Imhof Verlag, Petersberg, Germany"@en ;
                 skos:inScheme :Intervention ;
                 skos:topConceptOf :Intervention ;
                 skos:prefLabel "Neutral reintegration"@en , "Neutro"@it .


###  https://w3id.org/crmrp#c_e8592f3b
crmrp:c_e8592f3b rdf:type owl:NamedIndividual ,
                          skos:Concept ;
                 rdfs:label "Support restoration"@en ;
                 skos:definition "Restoration work on a wooden support involving the replacement of degraded parts with additions. The lemma is also used in a more general sense to indicate direct interventions on the artistic artefact aimed at eliminating phenomena of degradation that jeopardise its conservation (disinfestation, dehumidification, desalinisation)."@en ;
                 skos:editorialNote "C. Giannini, “Dizionario del restauro - Tecniche diagnostica conservazione”, Nardini Editore, Firenze, 2010"@it ;
                 skos:inScheme :Intervention ;
                 skos:note "International references could not be found"@en ;
                 skos:prefLabel "Support restoration"@en , "Risanamento del supporto"@it ;
                 skos:topConceptOf :Intervention .


###  https://w3id.org/crmrp#c_ea4e6f28
crmrp:c_ea4e6f28 rdf:type owl:NamedIndividual ,
                          skos:Concept ;
                 rdfs:label "Gypsum"@en ;
                 skos:broader :c_34d8fe56 ;
                 skos:definition "A soft mineral composed of calcium sulfate dihydrate."@en ;
                 skos:editorialNote "A. Weyer et al., “EwaGlos - European Illustrated Glossary of conservation terms for wall paintings and architectural surfaces”, Michael Imhof Verlag, Petersberg, Germany"@en ;
                 skos:exactMatch "Gypsum"@en ;
                 skos:inScheme :Material ;
                skos:topConceptOf :Material ;
                 skos:prefLabel "Gypsum"@en , "Gesso"@it .


###  https://w3id.org/crmrp#c_ea4ef6cd
crmrp:c_ea4ef6cd rdf:type owl:NamedIndividual ,
                          skos:Concept ;
                 rdfs:label "Sickle-shaped deformation"@en ;
                 skos:broader :c_13f3ce9e ;
                 skos:definition "A type of deformation of the wooden support of paintings that manifests itself in the sickle-like curvature of the boards."@en ;
                 skos:editorialNote "C. Giannini, “Dizionario del restauro - Tecniche diagnostica conservazione”, Nardini Editore, Firenze, 2010"@it ;
                 skos:inScheme :Alteration ;
                 skos:topConceptOf :Alteration ;
                 skos:note "International references could not be found"@en ;
                 skos:prefLabel "Sickle-shaped deformation"@en , "Falcatura"@it .


###  https://w3id.org/crmrp#c_eb357ebb
crmrp:c_eb357ebb rdf:type owl:NamedIndividual ,
                          skos:Concept ;
                 rdfs:label "Technique of contemporary arts"@en ;
                 skos:definition "Any execution technique of works created from the 1960s onwards, which does not correspond to traditional artistic techniques."@en ;
                 skos:inScheme :Execution_Technique ;
                 skos:note "International references could not be found"@en ;
                 skos:prefLabel "Technique of contemporary arts"@en , "Tecnica delle arti contemporanee"@it ;
                 skos:topConceptOf :Execution_Technique .


###  https://w3id.org/crmrp#c_ec7e0a6f
crmrp:c_ec7e0a6f rdf:type owl:NamedIndividual ,
                          skos:Concept ;
                 rdfs:label "Drying oil"@en ;
                 skos:broader :c_051209b3 ;
                 skos:definition "Vegetable oils which form a solid, elastic film after a period of exposure to the air."@en ;
                 skos:editorialNote "A. Weyer et al., “EwaGlos - European Illustrated Glossary of conservation terms for wall paintings and architectural surfaces”, Michael Imhof Verlag, Petersberg, Germany"@en ;
                 skos:inScheme :Execution_Technique ;
                 skos:topConceptOf :Execution_Technique ;
                 skos:prefLabel "Drying oil"@en , "Olio"@it .


###  https://w3id.org/crmrp#c_ef9ea44a
crmrp:c_ef9ea44a rdf:type owl:NamedIndividual ,
                          skos:Concept ;
                 rdfs:label "Curling"@en ;
                 skos:broader :c_13f3ce9e ;
                 skos:definition "The distortion of an object originally linear or planar so that it is curved or coiled in shape."@en ;
                 skos:editorialNote "Getty AAT http://vocab.getty.edu/page/aat/300053123"@en ;
                 skos:exactMatch <http://vocab.getty.edu/page/aat/300053123> ;
                 skos:inScheme :Alteration ;
                 skos:topConceptOf :Alteration ;
                 skos:prefLabel "Curling"@en , "Accartocciamento"@it .


###  https://w3id.org/crmrp#c_f1966944
crmrp:c_f1966944 rdf:type owl:NamedIndividual ,
                          skos:Concept ;
                 rdfs:label "Superficial consolidation"@en ;
                 skos:broader :c_b86776d0 ;
                 skos:definition "Consolidation intervention involving the surface layers (the substrate) of the artwork."@en ;
                 skos:inScheme :Intervention ;
                 skos:topConceptOf :Intervention ;
                 skos:note "International references could not be found"@en ;
                 skos:prefLabel "Superficial consolidation"@en , "Consolidamento superficiale"@it .


###  https://w3id.org/crmrp#c_f1c689bb
crmrp:c_f1c689bb rdf:type owl:NamedIndividual ,
                          skos:Concept ;
                 rdfs:label "Patinatura"@en ;
                 skos:definition "Any process by which an attempt is made to artificially impart a patina to objects, especially metal objects."@en ;
                 skos:editorialNote "A.Giuffredi “Formatura e fonderia”, Alinea editrice, Firenze, 2010"@it ,
                                    "C. Giannini, “Dizionario del restauro - Tecniche diagnostica conservazione”, Nardini Editore, Firenze, 2010"@it ;
                 skos:inScheme :Execution_Technique ;
                 skos:note "It was decided not to proceed with the English translation in order to avoid possible lexical errors and misunderstandings.The preferred editorial note and the definition closest to the meaning is Formatura e fonderia"@en ;
                 skos:prefLabel "Patinatura"@en , "Patinatura"@it ;
                 skos:topConceptOf :Execution_Technique .


###  https://w3id.org/crmrp#c_f1e8854b
crmrp:c_f1e8854b rdf:type owl:NamedIndividual ,
                          skos:Concept ;
                 rdfs:label "Lost wax process"@en ;
                 skos:broader :c_0a9f4d42 ;
                 skos:definition "A method of casting metal or glass in a mold, the cavity of which, or the positive of the form to be made, is formed with wax which is then melted or burned off, and displaced by molten metal or glass."@en ;
                 skos:editorialNote "Getty AAT http://vocab.getty.edu/page/aat/300053113"@en ;
                 skos:exactMatch <http://vocab.getty.edu/page/aat/300053113> ;
                 skos:inScheme :Execution_Technique ;
                 skos:topConceptOf :Execution_Technique ;
                 skos:prefLabel "Lost wax process"@en , "Fusione a cera persa"@it .


###  https://w3id.org/crmrp#c_f28c35d1
crmrp:c_f28c35d1 rdf:type owl:NamedIndividual ,
                          skos:Concept ;
                 rdfs:label "Sculpture in the round"@en ;
                 skos:broader :c_160c713a ;
                 skos:closeMatch <http://vocab.getty.edu/page/aat/300047264> ;
                 skos:definition "Sculpture in which forms are carved or modeled about their full circumference, as opposed to having forms projecting from or sunk into a continuous surface."@en ;
                 skos:editorialNote "Getty AAT http://vocab.getty.edu/page/aat/300047264"@en ;
                 skos:inScheme :Restoration_Object ;
                skos:topConceptOf :Restoration_Object ;
                 skos:prefLabel "Sculpture in the round"@en , "Tuttotondo"@it .


###  https://w3id.org/crmrp#c_f383c4d3
crmrp:c_f383c4d3 rdf:type owl:NamedIndividual ,
                          skos:Concept ;
                 rdfs:label "Graphic documentation"@en ;
                 skos:definition "Graphic documentation consists of the correlation of the representation of the artwork itself with that of the information, in the form of a collection of thematic mappings organised by type."@en ;
                 skos:inScheme :Documentation ;
                 skos:prefLabel "Graphic documentation"@en , "Documentazione grafica"@it ;
                 skos:topConceptOf :Documentation .


###  https://w3id.org/crmrp#c_f474cb91
crmrp:c_f474cb91 rdf:type owl:NamedIndividual ,
                          skos:Concept ;
                 rdfs:label "Lining"@en ;
                 skos:broader :c_e8592f3b ;
                 skos:closeMatch <http://vocab.getty.edu/page/aat/300162124> ;
                 skos:definition "The process of stregthening or stabilizing by use of an inner layer, usually using paper or fabric. In conservation and other contexts, the process of reinforcing a work by applying a paper or fabric lining with an adhesive, sewing, or another method; examples include lining applied to the support of a paper or canvas support of a work of art, or the lining applied to a garment as an inner layer of cloth."@en ;
                 skos:editorialNote "Getty AAT http://vocab.getty.edu/page/aat/300162124"@en ;
                 skos:inScheme :Intervention ;
                 skos:topConceptOf :Intervention ;
                 skos:prefLabel "Lining"@en , "Foderatura"@it .


###  https://w3id.org/crmrp#c_f4805ff2
crmrp:c_f4805ff2 rdf:type owl:NamedIndividual ,
                          skos:Concept ;
                 rdfs:label "Ink"@en ;
                 skos:broader :c_044b6056 ;
                 skos:closeMatch <http://vocab.getty.edu/page/aat/300015012> ;
                 skos:definition "A fluid medium used for drawings or tracings. An opaque, usually black, pigment is mixed with a vehicle such as water to produce a fluid which can be applied with a pen or brush. Through the end of the 19th century, ink was supplied dried in stick or block form which was ground and mixed with water as needed. At the beginning of this century prepared ink became popular."@en ;
                 skos:editorialNote "Getty AAT http://vocab.getty.edu/page/aat/300015012"@en ;
                 skos:inScheme :Execution_Technique ;
                 skos:topConceptOf :Execution_Technique ;
                 skos:prefLabel "Ink"@en , "Inchiostro"@it .


###  https://w3id.org/crmrp#c_f50f0996
crmrp:c_f50f0996 rdf:type owl:NamedIndividual ,
                          skos:Concept ;
                 rdfs:label "Biocleaning"@en ;
                 skos:altLabel "Treatment of microbiological organisms"@en ;
                 skos:closeMatch <http://vocab.getty.edu/page/aat/300438543> ;
                 skos:definition "Removing dirt, surface coatings, accretions, discolorations, or other undesired matter from a substrate using biological agents e.g. bacteria, enzymes, plant-based surfactants."@en ;
                 skos:editorialNote "A. Weyer et al., “EwaGlos - European Illustrated Glossary of conservation terms for wall paintings and architectural surfaces”, Michael Imhof Verlag, Petersberg, Germany"@en ,
                                    "Getty AAT http://vocab.getty.edu/page/aat/300438543"@en ,
                                    "Getty Conservation Institute “Illustrated Glossary - Definitions of terms used for the graphic documentation of in situ floor mosaics”, “Mosaics In Situ Project”, Los Angeles, 2003"@en ;
                 skos:inScheme :Intervention ;
                 skos:note "The preferred editorial note and the definition closest to the meaning is Getty AAT"@en ;
                 skos:prefLabel "Biocleaning"@en , "Bonifica"@it ;
                 skos:topConceptOf :Intervention .


###  https://w3id.org/crmrp#c_f6d57140
crmrp:c_f6d57140 rdf:type owl:NamedIndividual ,
                          skos:Concept ;
                 rdfs:label "Musical instruments"@en ;
                 skos:definition "Sound-producing apparatuses whose primary function is to play music."@en ;
                 skos:editorialNote "Getty AAT http://vocab.getty.edu/page/aat/300041620"@en ;
                 skos:exactMatch <http://vocab.getty.edu/page/aat/300041620> ;
                 skos:inScheme :Restoration_Object ;
                 skos:prefLabel "Musical instruments"@en , "Strumento musicale"@it ;
                 skos:topConceptOf :Restoration_Object .


###  https://w3id.org/crmrp#c_f80c2aa3
crmrp:c_f80c2aa3 rdf:type owl:NamedIndividual ,
                          skos:Concept ;
                 rdfs:label "Plant"@en ;
                 skos:altLabel "Plant intrusion"@en ;
                 skos:broader :c_3ef20257 ;
                 skos:definition "Vegetal living being, having, when complete, root, stem, and leaves, though consisting sometimes only of a single leafy expansion (e.g. Tree, fern, herb)."@en ;
                 skos:editorialNote "Getty Conservation Institute “Illustrated Glossary - Definitions of terms used for the graphic documentation of in situ floor mosaics”, “Mosaics In Situ Project”, Los Angeles, 2003"@en ,
                                    "Verg`es-Belmin et al., ICOMOS-ISCS: Illustrated glossary on stone deterioration patterns, vol. XV. Icomos International Council on Monuments and Sites, 2008"@en ;
                 skos:inScheme :Alteration ;
                 skos:topConceptOf :Alteration ;
                 skos:note "The preferred editorial note and the definition closest to the meaning is ICOMOS-ISCS: Illustrated glossary on stone deterioration patterns"@en ;
                 skos:prefLabel "Plant"@en , "Presenza di vegetazione"@it .


###  https://w3id.org/crmrp#c_f8c1b2e8
crmrp:c_f8c1b2e8 rdf:type owl:NamedIndividual ,
                          skos:Concept ;
                 rdfs:label "Depression"@en ;
                 skos:altLabel "Dent"@en, "Ammaccatura"@it ;
                 skos:broader :c_13f3ce9e ;
                 skos:closeMatch <http://vocab.getty.edu/page/aat/300400799> ;
                 skos:definition "Local hollow. A depression can occur with or without a loss of material"@en ;
                 skos:editorialNote "Getty AAT http://vocab.getty.edu/page/aat/300400799"@en ,
                                    "Getty Conservation Institute “Illustrated Glossary - Definitions of terms used for the graphic documentation of in situ floor mosaics”, “Mosaics In Situ Project”, Los Angeles, 2003"@en ,
                                    "Uni Cen/Ts 17135:2021 - Conservation of cultural heritage. General terms and definitions"@en ;
                 skos:inScheme :Alteration ;
                 skos:topConceptOf :Alteration ;
                 skos:prefLabel "Depression"@en , "Avvallamento"@it .


###  https://w3id.org/crmrp#c_f8deca36
crmrp:c_f8deca36 rdf:type owl:NamedIndividual ,
                          skos:Concept ;
                 rdfs:label "Flake"@en ;
                 skos:altLabel "Flaking"@en , "Sfaldamento"@it ;
                 skos:broader :c_d54b0be2 ;
                 skos:definition "Thin piece completely detached from the surface of an object."@en ;
                 skos:editorialNote "A. Weyer et al., “EwaGlos - European Illustrated Glossary of conservation terms for wall paintings and architectural surfaces”, Michael Imhof Verlag, Petersberg, Germany"@en ,
                                    "Uni Cen/Ts 17135:2021 - Conservation of cultural heritage. General terms and definitions"@en ,
                                    "Verg`es-Belmin et al., ICOMOS-ISCS: Illustrated glossary on stone deterioration patterns, vol. XV. Icomos International Council on Monuments and Sites, 2008"@en ;
                 skos:inScheme :Alteration ;
                 skos:topConceptOf :Alteration ;
                 skos:note "The preferred editorial note and the definition closest to the meaning is Uni Cen/Ts 17135:2021"@en ;
                 skos:prefLabel "Flake"@en , "Scagliatura"@it .


###  https://w3id.org/crmrp#c_f8f782c5
crmrp:c_f8f782c5 rdf:type owl:NamedIndividual ,
                          skos:Concept ;
                 rdfs:label "Foxing"@en ;
                 skos:broader :c_df05cb61 ;
                 skos:closeMatch <http://vocab.getty.edu/page/aat/300078853> ;
                 skos:definition "Multiple spots on paper or textile"@en ;
                 skos:editorialNote "Getty AAT http://vocab.getty.edu/page/aat/300078853"@en ,
                                    "Uni Cen/Ts 17135:2021 - Conservation of cultural heritage. General terms and definitions"@en ;
                 skos:inScheme :Alteration ;
                 skos:topConceptOf :Alteration ;
                 skos:note "The preferred editorial note and the definition closest to the meaning is Uni Cen/Ts 17135:2021"@en ;
                 skos:prefLabel "Foxing"@en , "Foxing"@it .


###  https://w3id.org/crmrp#c_fa940954
crmrp:c_fa940954 rdf:type owl:NamedIndividual ,
                          skos:Concept ;
                 rdfs:label "Consumption"@en ;
                 skos:definition "Form of degradation by rubbing to which floors with mosaic, stone, ceramic etc. decorations are subjected due to continuous trampling; it can lead to the total loss of the coating. The term is also used in relation to the state of conservation of paintings or to indicate the alteration of a work, linked to a particular religious cult, subjected to the touch or continuous rubbing of the faithful on one or more points of the surface. It may refer more generally to the wear and tear of objects of artistic value as a consequence of the use that was originally made of them."@en ;
                 skos:editorialNote "C. Giannini, “Dizionario del restauro - Tecniche diagnostica conservazione”, Nardini Editore, Firenze, 2010"@it ;
                 skos:inScheme :Alteration ;
                 skos:note "International references could not be found"@en ;
                 skos:prefLabel "Consumption"@en , "Consunzione"@it ;
                 skos:topConceptOf :Alteration .


###  https://w3id.org/crmrp#c_fc8da886
crmrp:c_fc8da886 rdf:type owl:NamedIndividual ,
                          skos:Concept ;
                 rdfs:label "Rigatino"@en ;
                 skos:broader :c_326da7e4 ;
                 skos:definition "Type of pictorial integration that allows the gap to be identified. It is called also called ‘righettino’ and is carried out by means of vertical hatching in harmony with local chromatic values; at a distance, the intervention is imperceptible, while it is visible at close range, in accordance with the principle of recognisability."@en ;
                 skos:editorialNote "C. Giannini, “Dizionario del restauro - Tecniche diagnostica conservazione”, Nardini Editore, Firenze, 2010"@it ;
                 skos:inScheme :Intervention ;
                 skos:topConceptOf :Intervention ;
                 skos:note "It was decided not to proceed with the English translation in order to avoid possible lexical errors and misunderstandings."@en ;
                 skos:prefLabel "Rigatino"@en , "Rigatino"@it .


###  https://w3id.org/crmrp#c_fca0ce9d
crmrp:c_fca0ce9d rdf:type owl:NamedIndividual ,
                          skos:Concept ;
                 rdfs:label "Structural pre-consolidation"@en ;
                 skos:broader :c_e078e94e ;
                 skos:definition "Pre-consolidation intervention involving the innermost (structural) layers of the artwork."@en ;
                 skos:inScheme :Intervention ;
                 skos:note "International references could not be found"@en ;
                 skos:prefLabel "Structural pre-consolidation"@en , "Pre-consolidamento strutturale"@it .


###  https://w3id.org/crmrp#c_fd0e78d4
crmrp:c_fd0e78d4 rdf:type owl:NamedIndividual ,
                          skos:Concept ;
                 rdfs:label "Rock"@en ;
                 skos:broader :c_34d8fe56 ;
                 skos:closeMatch <http://vocab.getty.edu/page/aat/300011176> ;
                 skos:definition "Naturally formed aggregate of one or more minerals. For processed or dressed rock use stone."@en ;
                 skos:editorialNote "Getty AAT http://vocab.getty.edu/page/aat/300011176"@en ;
                 skos:inScheme :Material ;
                 skos:topConceptOf :Material ;
                 skos:prefLabel "Rock"@en , "Pietra"@it .


###  https://w3id.org/crmrp#c_fd858a66
crmrp:c_fd858a66 rdf:type owl:NamedIndividual ,
                          skos:Concept ;
                 rdfs:label "Opus signinum"@en ;
                 skos:broader :c_b9a6a1c8 ;
                 skos:definition "Pavement usually made of same-sized rectangular ceramic fragments, inserted on their smaller side and assembled together in groups of a few elements. The orientation of adjacent groups is alternated so that their juxtaposition creates the visual impression of a basket weave pattern."@en ;
                 skos:editorialNote "C. Fiori “Teoria e tecniche per la conservazione del mosaico”, Il Prato, Padova, 2002"@it ,
                                    "Getty Conservation Institute “Illustrated Glossary - Technician Training for the Maintenance of In Situ Mosaics”, Los Angeles, 2013"@en ;
                 skos:inScheme :Execution_Technique ;
                 skos:topConceptOf :Execution_Technique ;
                 skos:prefLabel "Opus signinum"@en , "Opus signinum"@it .


###  https://w3id.org/crmrp#c_fdaf0926
crmrp:c_fdaf0926 rdf:type owl:NamedIndividual ,
                          skos:Concept ;
                 rdfs:label "Stacco a massello"@en ;
                 skos:broader :c_4fe4d308 ;
                 skos:definition "Method for the removal of wall paintings involving the removal of the arriccio together with the wall support."@en ;
                 skos:editorialNote "Getty AAT http://vocab.getty.edu/page/aat/300266091"@en ;
                 skos:exactMatch <http://vocab.getty.edu/page/aat/300266091> ;
                 skos:inScheme :Intervention ;
                 skos:topConceptOf :Intervention ;
                 skos:prefLabel "Stacco a massello"@en , "Stacco a massello"@it .


###  https://w3id.org/crmrp#c_fec56823
crmrp:c_fec56823 rdf:type owl:NamedIndividual ,
                          skos:Concept ;
                 rdfs:label "Xylography"@en ;
                 skos:broader :c_aee6a805 ;
                 skos:closeMatch <http://vocab.getty.edu/page/aat/300312031> ;
                 skos:definition "Process of using woodblocks, as distinct from type, in printing texts or images."@en ;
                 skos:editorialNote "Getty AAT http://vocab.getty.edu/page/aat/300312031"@en ;
                 skos:inScheme :Execution_Technique ;
                 skos:topConceptOf :Execution_Technique ;
                 skos:prefLabel "Xylography"@en , "Xilografia"@it .


###  https://w3id.org/crmrp#c_ff5d2cf3
crmrp:c_ff5d2cf3 rdf:type owl:NamedIndividual ,
                          skos:Concept ;
                 rdfs:label "Polymer paint"@en ;
                 skos:broader :c_044b6056 ;
                 skos:definition "Paint with a base that is polymer, which is compound formed by the combination of two or more molecules of the same substance to produce a new compound with the same empirical formula but with higher molecular weight. It is typically made from pigments in an acrylic resin or vinyl resin, which are polymers, or a combination of both resins. It is water based, spreads out in a layer, and forms a continuous, flexible, and waterproof film of plastic when the water evaporates."@en ;
                 skos:editorialNote "Getty AAT http://vocab.getty.edu/page/aat/300015055"@en ;
                 skos:exactMatch <http://vocab.getty.edu/page/aat/300015055> ;
                 skos:inScheme :Execution_Technique ;
                 skos:topConceptOf :Execution_Technique ;
                 skos:prefLabel "Polymer paint"@en , "Polimero sintetico"@it .


###  https://w3id.org/crmrp#c_ffb2bf28
crmrp:c_ffb2bf28 rdf:type owl:NamedIndividual ,
                          skos:Concept ;
                 rdfs:label "Particle size analysis"@en ;
                 skos:broader :c_abed88a5 ;
                 skos:definition "Refers to procedures and techniques which determine range of sizes or mean or average size of particles in a granular or powder sample."@en ;
                 skos:editorialNote "Getty AAT http://vocab.getty.edu/page/aat/300379895"@en ;
                 skos:exactMatch <http://vocab.getty.edu/page/aat/30037989> ;
                 skos:inScheme :Archeometric_and_Diagnostic_Analysis ;
                 skos:topConceptOf :Archeometric_and_Diagnostic_Analysis ;
                 skos:prefLabel "Particle size analysis"@en , "Analisi granulometrica"@it .
