<rdf:RDF
    xmlns:dct="http://purl.org/dc/terms/"
    xmlns:rdf="http://www.w3.org/1999/02/22-rdf-syntax-ns#"
    xmlns:dc="http://purl.org/dc/elements/1.1/"
    xmlns:crmrp="https://w3id.org/crmrp#"
    xmlns:owl="http://www.w3.org/2002/07/owl#"
    xmlns:skos="http://www.w3.org/2004/02/skos/core#"
    xmlns:rdfs="http://www.w3.org/2000/01/rdf-schema#"
    xmlns:grddl="http://www.w3.org/2003/g/data-view#"
    xmlns:xsd="http://www.w3.org/2001/XMLSchema#" > 
  <rdf:Description rdf:about="https://w3id.org/crmrp#c_6108ee3a">
    <skos:editorialNote xml:lang="it">UNI EN 14127:2011 Prove non distruttive - Misurazione dello spessore mediante ultrasuoni</skos:editorialNote>
    <skos:inScheme rdf:resource="https://w3id.org/crmrp#Archeometric_and_Diagnostic_Analysis"/>
    <skos:editorialNote xml:lang="it">UNI EN 10049:2014 Misurazione della rugosità media Ra e del numero dei picchi RPc sui prodotti piani metallici</skos:editorialNote>
    <skos:definition xml:lang="en">To obtain this value, the profile is measured at a sufficient number of points to characterise the surface. It includes profilometry, rugosimetry and thicknessimetry.</skos:definition>
    <rdf:type rdf:resource="http://www.w3.org/2004/02/skos/core#Concept"/>
    <skos:broader rdf:resource="https://w3id.org/crmrp#c_1fd6102e"/>
    <rdfs:label xml:lang="en">Surface profile measurement</rdfs:label>
    <skos:prefLabel xml:lang="it">Misurazione profilo di superficie</skos:prefLabel>
    <skos:prefLabel xml:lang="en">Surface profile measurement</skos:prefLabel>
    <skos:editorialNote xml:lang="it">UNI EN ISO 18452:2016 Ceramiche fini (ceramiche avanzate, ceramiche tecniche avanzate) - Determinazione dello spessore di film ceramici con un profilometro a contatto</skos:editorialNote>
    <skos:topConceptOf rdf:resource="https://w3id.org/crmrp#Archeometric_and_Diagnostic_Analysis"/>
    <rdf:type rdf:resource="http://www.w3.org/2002/07/owl#NamedIndividual"/>
    <skos:note xml:lang="en">International references could not be found</skos:note>
    <skos:editorialNote xml:lang="it">C. Giannini, “Dizionario del restauro - Tecniche diagnostica conservazione”, Nardini Editore, Firenze, 2010</skos:editorialNote>
  </rdf:Description>
  <rdf:Description rdf:about="https://w3id.org/crmrp#c_3b8e5779">
    <rdf:type rdf:resource="http://www.w3.org/2002/07/owl#NamedIndividual"/>
    <skos:prefLabel xml:lang="it">Scagliola</skos:prefLabel>
    <skos:exactMatch rdf:resource="http://vocab.getty.edu/page/aat/300014963"/>
    <skos:topConceptOf rdf:resource="https://w3id.org/crmrp#Execution_Technique"/>
    <skos:prefLabel xml:lang="en">Scagliola</skos:prefLabel>
    <rdfs:label xml:lang="en">Scagliola</rdfs:label>
    <skos:broader rdf:resource="https://w3id.org/crmrp#c_17157ccd"/>
    <skos:editorialNote xml:lang="en">Getty AAT http://vocab.getty.edu/page/aat/300014963</skos:editorialNote>
    <skos:editorialNote xml:lang="en">A. Weyer et al., “EwaGlos - European Illustrated Glossary of conservation terms for wall paintings and architectural surfaces”, Michael Imhof Verlag, Petersberg, Germany</skos:editorialNote>
    <skos:inScheme rdf:resource="https://w3id.org/crmrp#Execution_Technique"/>
    <rdf:type rdf:resource="http://www.w3.org/2004/02/skos/core#Concept"/>
  </rdf:Description>
  <rdf:Description rdf:about="https://w3id.org/crmrp#c_6dba4fb3">
    <skos:definition xml:lang="en">Missing part of an object.</skos:definition>
    <skos:altLabel xml:lang="en">Missing part</skos:altLabel>
    <skos:topConceptOf rdf:resource="https://w3id.org/crmrp#Alteration"/>
    <skos:note xml:lang="en">The preferred editorial note and the definition closest to the meaning is Uni Cen/Ts 17135:2021</skos:note>
    <rdf:type rdf:resource="http://www.w3.org/2004/02/skos/core#Concept"/>
    <skos:editorialNote xml:lang="en">Uni Cen/Ts 17135:2021 - Conservation of cultural heritage. General terms and definitions</skos:editorialNote>
    <rdfs:label xml:lang="en">Loss</rdfs:label>
    <skos:inScheme rdf:resource="https://w3id.org/crmrp#Alteration"/>
    <rdf:type rdf:resource="http://www.w3.org/2002/07/owl#NamedIndividual"/>
    <skos:prefLabel xml:lang="en">Loss</skos:prefLabel>
    <skos:editorialNote xml:lang="en">Verg`es-Belmin et al., ICOMOS-ISCS: Illustrated glossary on stone deterioration patterns, vol. XV. Icomos International Council on Monuments and Sites, 2008</skos:editorialNote>
    <skos:altLabel xml:lang="it">Mancanza</skos:altLabel>
    <skos:prefLabel xml:lang="it">Perdita</skos:prefLabel>
  </rdf:Description>
  <rdf:Description rdf:about="https://w3id.org/crmrp#c_f6d57140">
    <skos:definition xml:lang="en">Sound-producing apparatuses whose primary function is to play music.</skos:definition>
    <rdfs:label xml:lang="en">Musical instruments</rdfs:label>
    <rdf:type rdf:resource="http://www.w3.org/2004/02/skos/core#Concept"/>
    <skos:prefLabel xml:lang="it">Strumento musicale</skos:prefLabel>
    <skos:editorialNote xml:lang="en">Getty AAT http://vocab.getty.edu/page/aat/300041620</skos:editorialNote>
    <skos:topConceptOf rdf:resource="https://w3id.org/crmrp#Restoration_Object"/>
    <skos:exactMatch rdf:resource="http://vocab.getty.edu/page/aat/300041620"/>
    <skos:prefLabel xml:lang="en">Musical instruments</skos:prefLabel>
    <skos:inScheme rdf:resource="https://w3id.org/crmrp#Restoration_Object"/>
    <rdf:type rdf:resource="http://www.w3.org/2002/07/owl#NamedIndividual"/>
  </rdf:Description>
  <rdf:Description rdf:about="https://w3id.org/crmrp#c_2ce35f2b">
    <skos:topConceptOf rdf:resource="https://w3id.org/crmrp#Archeometric_and_Diagnostic_Analysis"/>
    <skos:broader rdf:resource="https://w3id.org/crmrp#c_1fd6102e"/>
    <skos:definition xml:lang="en">The contact angle, θ (theta), is a quantitative measure of the wettability of a solid by a liquid</skos:definition>
    <skos:editorialNote xml:lang="it">UNI EN 15802:2010 Conservazione dei beni culturali - Metodi di prova - Determinazione dell'angolo di contatto statico</skos:editorialNote>
    <skos:inScheme rdf:resource="https://w3id.org/crmrp#Archeometric_and_Diagnostic_Analysis"/>
    <rdf:type rdf:resource="http://www.w3.org/2004/02/skos/core#Concept"/>
    <skos:prefLabel xml:lang="it">Determinazione dell'angolo di contatto</skos:prefLabel>
    <skos:prefLabel xml:lang="en">Determination of the static contact angle</skos:prefLabel>
    <rdfs:label xml:lang="en">Determination of the static contact angle</rdfs:label>
    <rdf:type rdf:resource="http://www.w3.org/2002/07/owl#NamedIndividual"/>
    <skos:note xml:lang="en">International references could not be found</skos:note>
  </rdf:Description>
  <rdf:Description rdf:about="https://w3id.org/crmrp#c_05e03365">
    <skos:note xml:lang="en">International references could not be found</skos:note>
    <skos:prefLabel xml:lang="it">Ortofoto</skos:prefLabel>
    <rdfs:label xml:lang="en">Orthophoto</rdfs:label>
    <skos:broader rdf:resource="https://w3id.org/crmrp#c_773e0829"/>
    <skos:topConceptOf rdf:resource="https://w3id.org/crmrp#Documentation"/>
    <skos:definition xml:lang="en">Orthophoto is an image obtained after photo-rectification (also known as photogrammetric straightening). It is an image that has undergone treatment, scaled and geometrically, in order to become an orthogonal projection and thus be measurable.</skos:definition>
    <skos:prefLabel xml:lang="en">Orthophoto</skos:prefLabel>
    <rdf:type rdf:resource="http://www.w3.org/2002/07/owl#NamedIndividual"/>
    <rdf:type rdf:resource="http://www.w3.org/2004/02/skos/core#Concept"/>
    <skos:inScheme rdf:resource="https://w3id.org/crmrp#Documentation"/>
  </rdf:Description>
  <rdf:Description rdf:about="https://w3id.org/crmrp#R11_Non-invasive_archaeometric_and_diagnostic_analysis">
    <rdfs:label xml:lang="en">Non-invasive archaeometric and diagnostic analysis</rdfs:label>
    <rdfs:comment xml:lang="en">This class describe the non-invasive archaeometric and diagnostic analysis.
Non-invasive investigations are those that do not require a sample to be taken from the artwork.</rdfs:comment>
    <rdfs:subClassOf rdf:resource="http://www.cidoc-crm.org/extensions/crmsci/S21_Measurement"/>
    <rdf:type rdf:resource="http://www.w3.org/2002/07/owl#Class"/>
  </rdf:Description>
  <rdf:Description rdf:about="https://w3id.org/crmrp#c_2471b55e">
    <skos:prefLabel xml:lang="en">Thermoluminescence</skos:prefLabel>
    <skos:editorialNote xml:lang="en">Getty ATT http://vocab.getty.edu/page/aat/300056215</skos:editorialNote>
    <skos:inScheme rdf:resource="https://w3id.org/crmrp#Archeometric_and_Diagnostic_Analysis"/>
    <skos:topConceptOf rdf:resource="https://w3id.org/crmrp#Archeometric_and_Diagnostic_Analysis"/>
    <rdfs:label xml:lang="en">Thermoluminescence</rdfs:label>
    <rdf:type rdf:resource="http://www.w3.org/2002/07/owl#NamedIndividual"/>
    <skos:prefLabel xml:lang="it">Termoluminescenza</skos:prefLabel>
    <skos:closeMatch rdf:resource="http://vocab.getty.edu/page/aat/300056215"/>
    <skos:definition xml:lang="en">The glow or emission of light produced by the application of heat.</skos:definition>
    <rdf:type rdf:resource="http://www.w3.org/2004/02/skos/core#Concept"/>
    <skos:broader rdf:resource="https://w3id.org/crmrp#c_abed88a5"/>
  </rdf:Description>
  <rdf:Description rdf:about="https://w3id.org/crmrp#c_560a9552">
    <skos:editorialNote xml:lang="it">G. Pignolo, “Effetti d’oro - Storia e tecnica della doratura nell’arte”, Editrice Compositori, Bologna, 2002</skos:editorialNote>
    <skos:inScheme rdf:resource="https://w3id.org/crmrp#Execution_Technique"/>
    <skos:note xml:lang="en">International references could not be found</skos:note>
    <rdf:type rdf:resource="http://www.w3.org/2002/07/owl#NamedIndividual"/>
    <rdf:type rdf:resource="http://www.w3.org/2004/02/skos/core#Concept"/>
    <skos:broader rdf:resource="https://w3id.org/crmrp#c_4d471b17"/>
    <skos:definition xml:lang="en">The final appearance is half-veined and can be achieved by passing the agate stone over the bolus before the leaf is applied.</skos:definition>
    <skos:prefLabel xml:lang="en">Satin finishing</skos:prefLabel>
    <skos:prefLabel xml:lang="it">Satinatura</skos:prefLabel>
    <rdfs:label xml:lang="en">Satin finishing</rdfs:label>
    <skos:topConceptOf rdf:resource="https://w3id.org/crmrp#Execution_Technique"/>
  </rdf:Description>
  <rdf:Description rdf:about="https://w3id.org/crmrp#c_1f7aff6a">
    <skos:prefLabel xml:lang="it">Fluorescenza ai raggi X (XRF)</skos:prefLabel>
    <skos:editorialNote xml:lang="it">M.Ceroni, G.Elia, “Diagnostica per i beni culturali”, Alinea editrice, Firenze, 2008</skos:editorialNote>
    <skos:note xml:lang="en">International references could not be found</skos:note>
    <skos:editorialNote xml:lang="it">C. Giannini, “Dizionario del restauro - Tecniche diagnostica conservazione”, Nardini Editore, Firenze, 2010</skos:editorialNote>
    <skos:definition xml:lang="en">XRF is an X-ray emission spectroscopy technique that allows the identification of chemical elements that are present in, or make up, the sample</skos:definition>
    <skos:inScheme rdf:resource="https://w3id.org/crmrp#Archeometric_and_Diagnostic_Analysis"/>
    <skos:broader rdf:resource="https://w3id.org/crmrp#c_1fd6102e"/>
    <skos:topConceptOf rdf:resource="https://w3id.org/crmrp#Archeometric_and_Diagnostic_Analysis"/>
    <skos:prefLabel xml:lang="en">X-ray fluorescence (XRF)</skos:prefLabel>
    <rdf:type rdf:resource="http://www.w3.org/2002/07/owl#NamedIndividual"/>
    <rdfs:label xml:lang="en">X-ray fluorescence (XRF)</rdfs:label>
    <skos:editorialNote xml:lang="it">S. Volpin e L. Appolonia “Le analisi di laboratorio applicate ai beni artistici policromi”, Il Prato, Padova, 1999</skos:editorialNote>
    <rdf:type rdf:resource="http://www.w3.org/2004/02/skos/core#Concept"/>
  </rdf:Description>
  <rdf:Description rdf:about="https://w3id.org/crmrp#c_4fe4d308">
    <skos:definition xml:lang="en">Removal of a wall painting by separating the paint layer, with or without intonaco, arriccio and part of the wall support. It is done when there are problems in the supporting structure, or when the painting needs to be moved. This operation is usually carried out on murals but can also be developed in artworks with different media</skos:definition>
    <skos:altLabel xml:lang="en">Detaching</skos:altLabel>
    <skos:editorialNote xml:lang="en">Getty AAT http://vocab.getty.edu/page/aat/300264843</skos:editorialNote>
    <rdf:type rdf:resource="http://www.w3.org/2002/07/owl#NamedIndividual"/>
    <rdfs:label xml:lang="en">Detachment</rdfs:label>
    <skos:topConceptOf rdf:resource="https://w3id.org/crmrp#Intervention"/>
    <skos:prefLabel xml:lang="en">Detachment</skos:prefLabel>
    <skos:prefLabel xml:lang="it">Trasporto</skos:prefLabel>
    <skos:inScheme rdf:resource="https://w3id.org/crmrp#Intervention"/>
    <skos:editorialNote xml:lang="en">A. Weyer et al., “EwaGlos - European Illustrated Glossary of conservation terms for wall paintings and architectural surfaces”, Michael Imhof Verlag, Petersberg, Germany</skos:editorialNote>
    <skos:note xml:lang="en">The preferred editorial note and the definition closest to the meaning is EwaGlos - European Illustrated Glossary of conservation terms for wall paintings and architectural surfaces</skos:note>
    <rdf:type rdf:resource="http://www.w3.org/2004/02/skos/core#Concept"/>
  </rdf:Description>
  <rdf:Description rdf:about="https://w3id.org/crmrp#c_1e25ce8c">
    <rdf:type rdf:resource="http://www.w3.org/2004/02/skos/core#Concept"/>
    <skos:editorialNote xml:lang="it">Uni En 15898:2019 Conservazione del patrimonio culturale - Termini generali e definizioni</skos:editorialNote>
    <skos:inScheme rdf:resource="https://w3id.org/crmrp#Intervention"/>
    <skos:prefLabel xml:lang="it">Ricostruzione</skos:prefLabel>
    <skos:topConceptOf rdf:resource="https://w3id.org/crmrp#Intervention"/>
    <skos:prefLabel xml:lang="en">Reconstruction</skos:prefLabel>
    <skos:definition xml:lang="en">Restoration of an object to an inferred previous form using existing and/or replacement material</skos:definition>
    <rdf:type rdf:resource="http://www.w3.org/2002/07/owl#NamedIndividual"/>
    <rdfs:label xml:lang="en">Reconstruction</rdfs:label>
    <skos:broader rdf:resource="https://w3id.org/crmrp#c_24cc76d5"/>
  </rdf:Description>
  <rdf:Description rdf:about="https://w3id.org/crmrp#c_5d7824f1">
    <skos:prefLabel xml:lang="en">Installations</skos:prefLabel>
    <skos:definition xml:lang="en">Works dating from the 1960s or later that use their exhibition space as part of their design. Demanding a viewer's active engagement, installations are often created by artists in direct opposition to the notion of permanent artwork, or art as a commodity.</skos:definition>
    <skos:editorialNote xml:lang="en">Getty AAT http://vocab.getty.edu/page/aat/300047896</skos:editorialNote>
    <skos:exactMatch rdf:resource="http://vocab.getty.edu/page/aat/300047896"/>
    <skos:topConceptOf rdf:resource="https://w3id.org/crmrp#Restoration_Object"/>
    <skos:prefLabel xml:lang="it">Installazione</skos:prefLabel>
    <rdf:type rdf:resource="http://www.w3.org/2002/07/owl#NamedIndividual"/>
    <rdfs:label xml:lang="en">Installations</rdfs:label>
    <rdf:type rdf:resource="http://www.w3.org/2004/02/skos/core#Concept"/>
    <skos:inScheme rdf:resource="https://w3id.org/crmrp#Restoration_Object"/>
  </rdf:Description>
  <rdf:Description rdf:about="https://w3id.org/crmrp#c_24cc76d5">
    <skos:broader rdf:resource="https://w3id.org/crmrp#c_0f7eacd7"/>
    <skos:prefLabel xml:lang="en">Materic Integration</skos:prefLabel>
    <skos:editorialNote xml:lang="it">C. Giannini, “Dizionario del restauro - Tecniche diagnostica  conservazione”, Nardini Editore, Firenze, 2010</skos:editorialNote>
    <skos:topConceptOf rdf:resource="https://w3id.org/crmrp#Intervention"/>
    <rdf:type rdf:resource="http://www.w3.org/2004/02/skos/core#Concept"/>
    <skos:definition xml:lang="en">integrative intervention often indispensable to restore legibility to heavily degraded artefacts.</skos:definition>
    <skos:inScheme rdf:resource="https://w3id.org/crmrp#Intervention"/>
    <skos:prefLabel xml:lang="it">Reintegrazione materica</skos:prefLabel>
    <rdf:type rdf:resource="http://www.w3.org/2002/07/owl#NamedIndividual"/>
    <rdfs:label xml:lang="en">Materic Integration</rdfs:label>
  </rdf:Description>
  <rdf:Description rdf:about="https://w3id.org/crmrp#c_390901fa">
    <rdf:type rdf:resource="http://www.w3.org/2002/07/owl#NamedIndividual"/>
    <rdfs:label xml:lang="en">X-ray diffraction (XRD)</rdfs:label>
    <skos:editorialNote xml:lang="en">Getty AAT http://vocab.getty.edu/page/aat/300233218</skos:editorialNote>
    <skos:exactMatch rdf:resource="http://vocab.getty.edu/page/aat/300233218"/>
    <skos:inScheme rdf:resource="https://w3id.org/crmrp#Archeometric_and_Diagnostic_Analysis"/>
    <skos:definition xml:lang="en">Diffraction of x-rays by the regularly spaced atoms of a substance, useful for determining the arrangement of atoms and thereby the nature or composition of a substance</skos:definition>
    <skos:topConceptOf rdf:resource="https://w3id.org/crmrp#Archeometric_and_Diagnostic_Analysis"/>
    <skos:prefLabel xml:lang="it">Diffrazione ai raggi X (XRD)</skos:prefLabel>
    <skos:broader rdf:resource="https://w3id.org/crmrp#c_789c3e32"/>
    <skos:prefLabel xml:lang="en">X-ray diffraction (XRD)</skos:prefLabel>
    <rdf:type rdf:resource="http://www.w3.org/2004/02/skos/core#Concept"/>
  </rdf:Description>
  <rdf:Description rdf:about="https://w3id.org/crmrp#c_272b9517">
    <rdf:type rdf:resource="http://www.w3.org/2002/07/owl#NamedIndividual"/>
    <rdf:type rdf:resource="http://www.w3.org/2004/02/skos/core#Concept"/>
    <skos:definition xml:lang="en">Moulding technique implemented during the 19th century that allows hollow models to be obtained by pouring liquid plaster into the mould in several pours</skos:definition>
    <rdfs:label xml:lang="en">Sciacquo</rdfs:label>
    <skos:editorialNote xml:lang="it">A.Giuffredi, “Formatura e fonderia”, Alinea editrice, Firenze, 2010</skos:editorialNote>
    <skos:prefLabel xml:lang="it">Sciacquo</skos:prefLabel>
    <skos:inScheme rdf:resource="https://w3id.org/crmrp#Execution_Technique"/>
    <skos:prefLabel xml:lang="en">Sciacquo</skos:prefLabel>
    <skos:broader rdf:resource="https://w3id.org/crmrp#c_17157ccd"/>
    <skos:topConceptOf rdf:resource="https://w3id.org/crmrp#Execution_Technique"/>
    <skos:note xml:lang="en">It was decided not to proceed with the English translation in order to avoid possible lexical errors and misunderstandings.</skos:note>
  </rdf:Description>
  <rdf:Description rdf:about="https://w3id.org/crmrp#c_42f16f05">
    <skos:broader rdf:resource="https://w3id.org/crmrp#c_1fd6102e"/>
    <rdf:type rdf:resource="http://www.w3.org/2002/07/owl#NamedIndividual"/>
    <skos:note xml:lang="en">International references could not be found.</skos:note>
    <skos:inScheme rdf:resource="https://w3id.org/crmrp#Archeometric_and_Diagnostic_Analysis"/>
    <rdf:type rdf:resource="http://www.w3.org/2004/02/skos/core#Concept"/>
    <skos:prefLabel xml:lang="en">RTI (Reflectance Transformation Imaging)</skos:prefLabel>
    <skos:prefLabel xml:lang="it">RTI (Reflectance Transformation Imaging)</skos:prefLabel>
    <skos:topConceptOf rdf:resource="https://w3id.org/crmrp#Archeometric_and_Diagnostic_Analysis"/>
    <rdfs:label xml:lang="en">RTI (Reflectance Transformation Imaging)</rdfs:label>
    <skos:definition xml:lang="en">Reflectance Transformation Imaging (RTI) is a new imaging technique that creates hyper-realistic digital surrogates that are interactively controlled by the viewer. This new method is based upon the synthesis of multiple digital images of a subject in a fixed position collected from a fixed camera position.</skos:definition>
  </rdf:Description>
  <rdf:Description rdf:about="https://w3id.org/crmrp#c_e078e94e">
    <skos:topConceptOf rdf:resource="https://w3id.org/crmrp#Intervention"/>
    <skos:prefLabel xml:lang="it">Pre-consolidamento</skos:prefLabel>
    <skos:prefLabel xml:lang="en">Pre-consolidation</skos:prefLabel>
    <skos:note xml:lang="en">International references could not be found</skos:note>
    <skos:inScheme rdf:resource="https://w3id.org/crmrp#Intervention"/>
    <skos:definition xml:lang="en">Set of preventive treatments aimed at avoiding possible loss of material during subsequent restoration operations and/or preserving the artefact in its current state pending more specific targeted interventions in the immediate future.</skos:definition>
    <rdfs:label xml:lang="en">Pre-consolidation</rdfs:label>
    <rdf:type rdf:resource="http://www.w3.org/2004/02/skos/core#Concept"/>
    <rdf:type rdf:resource="http://www.w3.org/2002/07/owl#NamedIndividual"/>
  </rdf:Description>
  <rdf:Description rdf:about="https://w3id.org/crmrp#c_af6b2d29">
    <skos:topConceptOf rdf:resource="https://w3id.org/crmrp#Intervention"/>
    <skos:broader rdf:resource="https://w3id.org/crmrp#c_e078e94e"/>
    <rdfs:label xml:lang="en">Superficial pre-consolidation</rdfs:label>
    <skos:inScheme rdf:resource="https://w3id.org/crmrp#Intervention"/>
    <skos:definition xml:lang="en">Pre-consolidation intervention involving the surface layers (the substrate) of the artwork.</skos:definition>
    <rdf:type rdf:resource="http://www.w3.org/2004/02/skos/core#Concept"/>
    <skos:prefLabel xml:lang="en">Superficial pre-consolidation</skos:prefLabel>
    <skos:prefLabel xml:lang="it">Pre-consolidamento superficiale</skos:prefLabel>
    <rdf:type rdf:resource="http://www.w3.org/2002/07/owl#NamedIndividual"/>
    <skos:note xml:lang="en">International references could not be found</skos:note>
  </rdf:Description>
  <rdf:Description rdf:about="https://w3id.org/crmrp#c_e80de18f">
    <skos:editorialNote xml:lang="en">A. Weyer et al., “EwaGlos - European Illustrated Glossary of conservation terms for wall paintings and architectural surfaces”, Michael Imhof Verlag, Petersberg, Germany</skos:editorialNote>
    <rdf:type rdf:resource="http://www.w3.org/2004/02/skos/core#Concept"/>
    <rdf:type rdf:resource="http://www.w3.org/2002/07/owl#NamedIndividual"/>
    <skos:definition xml:lang="en">When a damaged area or lacuna cannot be reconstructed due to its size, lack of reliable sources, or the artistic importance of the work of art, its negative optical impact on the original can be reduced by toning down the damage or lacuna with a so-called “neutral” colour, thereby moving it into the background.</skos:definition>
    <skos:broader rdf:resource="https://w3id.org/crmrp#c_326da7e4"/>
    <skos:prefLabel xml:lang="it">Neutro</skos:prefLabel>
    <skos:inScheme rdf:resource="https://w3id.org/crmrp#Intervention"/>
    <skos:prefLabel xml:lang="en">Neutral reintegration</skos:prefLabel>
    <rdfs:label xml:lang="en">Neutral reintegration</rdfs:label>
    <skos:topConceptOf rdf:resource="https://w3id.org/crmrp#Intervention"/>
  </rdf:Description>
  <rdf:Description rdf:about="https://w3id.org/crmrp#c_d69776d7">
    <rdf:type rdf:resource="http://www.w3.org/2004/02/skos/core#Concept"/>
    <skos:inScheme rdf:resource="https://w3id.org/crmrp#Intervention"/>
    <skos:editorialNote xml:lang="en">A. Weyer et al., “EwaGlos - European Illustrated Glossary of conservation terms for wall paintings and architectural surfaces”, Michael Imhof Verlag, Petersberg, Germany</skos:editorialNote>
    <skos:topConceptOf rdf:resource="https://w3id.org/crmrp#Intervention"/>
    <skos:definition xml:lang="en">Small areas of the object on which cleaning, consolidation, or reintegration tests are carried out.</skos:definition>
    <skos:broader rdf:resource="https://w3id.org/crmrp#c_830e6744"/>
    <skos:prefLabel xml:lang="it">Prova di pulitura</skos:prefLabel>
    <rdf:type rdf:resource="http://www.w3.org/2002/07/owl#NamedIndividual"/>
    <skos:prefLabel xml:lang="en">Treatment trials</skos:prefLabel>
    <rdfs:label xml:lang="en">Treatment trials</rdfs:label>
  </rdf:Description>
  <rdf:Description rdf:about="https://w3id.org/crmrp#c_1e84806e">
    <rdf:type rdf:resource="http://www.w3.org/2004/02/skos/core#Concept"/>
    <skos:topConceptOf rdf:resource="https://w3id.org/crmrp#Execution_Technique"/>
    <rdfs:label xml:lang="en">Woodworking</rdfs:label>
    <skos:prefLabel xml:lang="it">Tecnica di lavorazione del legno</skos:prefLabel>
    <skos:prefLabel xml:lang="en">Woodworking</skos:prefLabel>
    <skos:inScheme rdf:resource="https://w3id.org/crmrp#Execution_Technique"/>
    <rdf:type rdf:resource="http://www.w3.org/2002/07/owl#NamedIndividual"/>
    <skos:definition xml:lang="en">Refers broadly to the activity of fashioning in wood. For the art of making fine furniture and intricate woodwork, see cabinetmaking. See the narrower carpentry for constructing buildings and other structures with wood, including the installation of floors, windows, and other trim work.</skos:definition>
    <skos:closeMatch rdf:resource="http://vocab.getty.edu/page/aat/300054083"/>
    <skos:editorialNote xml:lang="en">Getty AAT http://vocab.getty.edu/page/aat/300054083</skos:editorialNote>
  </rdf:Description>
  <rdf:Description rdf:about="https://w3id.org/crmrp#c_2d586e2e">
    <rdfs:label xml:lang="en">Contact sponge</rdfs:label>
    <skos:prefLabel xml:lang="en">Contact sponge</skos:prefLabel>
    <skos:prefLabel xml:lang="it">Misura della capacità di assorbimento di acqua mediante spugna di contatto</skos:prefLabel>
    <skos:topConceptOf rdf:resource="https://w3id.org/crmrp#Archeometric_and_Diagnostic_Analysis"/>
    <skos:definition xml:lang="en">The contact sponge method is a test of water absorption by the material under test, which can also be carried out in situ. A sponge of a predetermined type and size is loaded with a quantity of water such that, when kept in contact with constant pressure and for a short time, it does not drip. A circular plastic plate is used to facilitate and maintain adhesion of the sponge to the surface. The amount of water absorbed by the surface is calculated by difference, weighing the sponge before and after application using an analytical balance.</skos:definition>
    <skos:broader rdf:resource="https://w3id.org/crmrp#c_1fd6102e"/>
    <rdf:type rdf:resource="http://www.w3.org/2002/07/owl#NamedIndividual"/>
    <rdf:type rdf:resource="http://www.w3.org/2004/02/skos/core#Concept"/>
    <skos:note xml:lang="en">International references could not be found</skos:note>
    <skos:editorialNote xml:lang="it">UNI 11432:2011 Beni culturali - Materiali lapidei naturali ed artificiali - Misura della capacità di assorbimento di acqua mediante spugna di contatto</skos:editorialNote>
    <skos:inScheme rdf:resource="https://w3id.org/crmrp#Archeometric_and_Diagnostic_Analysis"/>
  </rdf:Description>
  <rdf:Description rdf:about="https://w3id.org/crmrp#c_150915f4">
    <skos:definition xml:lang="en">Enzymes make it possible to remove the protein films that often form on the surface of works of art. There are essentially two enzymes used in restoration: proteases and lipases. The former are capable of breaking down protein molecules. Lipases are capable of dissolving fats (or lipids), catalysing the hydrolysis of triglycerides, the basic components of oils (e.g. linseed oil)</skos:definition>
    <skos:prefLabel xml:lang="en">Enzymes</skos:prefLabel>
    <rdfs:label xml:lang="en">Enzymes</rdfs:label>
    <rdf:type rdf:resource="http://www.w3.org/2004/02/skos/core#Concept"/>
    <skos:editorialNote xml:lang="it">P.Cremonesi, E. Signorini, “Un approccio alla pulitura dei dipinti mobili”, Il Prato, Padova, 2016</skos:editorialNote>
    <skos:inScheme rdf:resource="https://w3id.org/crmrp#Intervention"/>
    <skos:broader rdf:resource="https://w3id.org/crmrp#c_5a83cd16"/>
    <skos:note xml:lang="en">International references could not be found</skos:note>
    <rdf:type rdf:resource="http://www.w3.org/2002/07/owl#NamedIndividual"/>
    <skos:prefLabel xml:lang="it">Enzimi</skos:prefLabel>
    <skos:TopConceptOf rdf:resource="https://w3id.org/crmrp#Intervention"/>
  </rdf:Description>
  <rdf:Description rdf:about="https://w3id.org/crmrp#RP1i_needed_intervention">
    <rdfs:label xml:lang="en">needed intervention</rdfs:label>
    <rdfs:comment>This property links R1 Restoration Object and R7 Restoration Project
This property RP1 intervents on (needed intervention) allows you to indicate which artwork the restoration project refers to.</rdfs:comment>
    <rdfs:range rdf:resource="https://w3id.org/crmrp#R8_Intervention"/>
    <rdfs:range rdf:resource="https://w3id.org/crmrp#R7_Restoration_Project"/>
    <rdfs:domain rdf:resource="https://w3id.org/crmrp#R1_Restoration_Object"/>
    <rdfs:domain rdf:resource="http://www.cidoc-crm.org/extensions/crmsci/S18_Alteration"/>
    <rdf:type rdf:resource="http://www.w3.org/2002/07/owl#ObjectProperty"/>
  </rdf:Description>
  <rdf:Description rdf:about="https://w3id.org/crmrp#c_8f129db5">
    <skos:topConceptOf rdf:resource="https://w3id.org/crmrp#Alteration"/>
    <rdfs:label xml:lang="en">Sub-efflorescence</rdfs:label>
    <rdf:type rdf:resource="http://www.w3.org/2004/02/skos/core#Concept"/>
    <rdf:type rdf:resource="http://www.w3.org/2002/07/owl#NamedIndividual"/>
    <skos:inScheme rdf:resource="https://w3id.org/crmrp#Alteration"/>
    <skos:altLabel xml:lang="en">Subflorescence</skos:altLabel>
    <skos:editorialNote xml:lang="en">Uni Cen/Ts 17135:2021 - Conservation of cultural heritage. General terms and definitions</skos:editorialNote>
    <skos:prefLabel xml:lang="it">Subflorescenza</skos:prefLabel>
    <skos:definition xml:lang="en">Sub-efflorescence and crypto-efflorescence are visible when the surface falls apart or away</skos:definition>
    <skos:note xml:lang="en">The preferred editorial note and the definition closest to the meaning is Uni Cen/Ts 17135:2021</skos:note>
    <skos:editorialNote xml:lang="en">Verg`es-Belmin et al., ICOMOS-ISCS: Illustrated glossary on stone deterioration patterns, vol. XV. Icomos International Council on Monuments and Sites, 2008</skos:editorialNote>
    <skos:prefLabel xml:lang="en">Sub-efflorescence</skos:prefLabel>
  </rdf:Description>
  <rdf:Description rdf:about="http://www.cidoc-crm.org/cidoc-crm/P56_bears_feature">
    <rdfs:range rdf:resource="https://w3id.org/crmrp#R10_Sign_of_Workmanship"/>
    <rdfs:domain rdf:resource="https://w3id.org/crmrp#R1_Restoration_Object"/>
  </rdf:Description>
  <rdf:Description rdf:about="https://w3id.org/crmrp#c_f474cb91">
    <skos:inScheme rdf:resource="https://w3id.org/crmrp#Intervention"/>
    <skos:prefLabel xml:lang="it">Foderatura</skos:prefLabel>
    <skos:topConceptOf rdf:resource="https://w3id.org/crmrp#Intervention"/>
    <skos:broader rdf:resource="https://w3id.org/crmrp#c_e8592f3b"/>
    <skos:prefLabel xml:lang="en">Lining</skos:prefLabel>
    <rdf:type rdf:resource="http://www.w3.org/2002/07/owl#NamedIndividual"/>
    <skos:definition xml:lang="en">The process of stregthening or stabilizing by use of an inner layer, usually using paper or fabric. In conservation and other contexts, the process of reinforcing a work by applying a paper or fabric lining with an adhesive, sewing, or another method; examples include lining applied to the support of a paper or canvas support of a work of art, or the lining applied to a garment as an inner layer of cloth.</skos:definition>
    <skos:editorialNote xml:lang="en">Getty AAT http://vocab.getty.edu/page/aat/300162124</skos:editorialNote>
    <skos:closeMatch rdf:resource="http://vocab.getty.edu/page/aat/300162124"/>
    <rdfs:label xml:lang="en">Lining</rdfs:label>
    <rdf:type rdf:resource="http://www.w3.org/2004/02/skos/core#Concept"/>
  </rdf:Description>
  <rdf:Description rdf:about="https://w3id.org/crmrp#c_b8182893">
    <skos:definition xml:lang="en">Copper molds that have been struck with a punch and from which individual type letters are cast.</skos:definition>
    <skos:topConceptOf rdf:resource="https://w3id.org/crmrp#Restoration_Object"/>
    <rdfs:label xml:lang="en">Engraved matrix</rdfs:label>
    <rdf:type rdf:resource="http://www.w3.org/2002/07/owl#NamedIndividual"/>
    <skos:altLabel xml:lang="en">Matrices (copper molds)</skos:altLabel>
    <skos:inScheme rdf:resource="https://w3id.org/crmrp#Restoration_Object"/>
    <skos:prefLabel xml:lang="en">Engraved matrix</skos:prefLabel>
    <skos:prefLabel xml:lang="it">Matrice incisa</skos:prefLabel>
    <skos:editorialNote xml:lang="en">Getty AAT http://vocab.getty.edu/page/aat/300266816</skos:editorialNote>
    <skos:closeMatch rdf:resource="http://vocab.getty.edu/page/aat/300266816"/>
    <rdf:type rdf:resource="http://www.w3.org/2004/02/skos/core#Concept"/>
  </rdf:Description>
  <rdf:Description rdf:about="https://w3id.org/crmrp#c_bc53d2a2">
    <rdf:type rdf:resource="http://www.w3.org/2002/07/owl#NamedIndividual"/>
    <skos:prefLabel xml:lang="en">Buckled</skos:prefLabel>
    <skos:altLabel xml:lang="en">Buckling</skos:altLabel>
    <skos:definition xml:lang="en">Exhibiting wavelike deformation</skos:definition>
    <skos:note xml:lang="en">The preferred editorial note and the definition closest to the meaning is Uni Cen/Ts 17135:2021</skos:note>
    <skos:topConceptOf rdf:resource="https://w3id.org/crmrp#Alteration"/>
    <skos:broader rdf:resource="https://w3id.org/crmrp#c_13f3ce9e"/>
    <skos:editorialNote xml:lang="en">Getty AAT http://vocab.getty.edu/page/aat/300072663</skos:editorialNote>
    <skos:inScheme rdf:resource="https://w3id.org/crmrp#Alteration"/>
    <skos:prefLabel xml:lang="it">Incurvatura</skos:prefLabel>
    <rdf:type rdf:resource="http://www.w3.org/2004/02/skos/core#Concept"/>
    <skos:editorialNote xml:lang="en">Uni Cen/Ts 17135:2021 - Conservation of cultural heritage. General terms and definitions</skos:editorialNote>
    <skos:closeMatch rdf:resource="http://vocab.getty.edu/page/aat/300072663"/>
    <rdfs:label xml:lang="en">Buckled</rdfs:label>
  </rdf:Description>
  <rdf:Description rdf:about="https://w3id.org/crmrp#c_143349b9">
    <skos:editorialNote xml:lang="en">Getty AAT http://vocab.getty.edu/page/aat/300410350</skos:editorialNote>
    <skos:prefLabel xml:lang="en">Canvas painting technique</skos:prefLabel>
    <rdf:type rdf:resource="http://www.w3.org/2002/07/owl#NamedIndividual"/>
    <skos:inScheme rdf:resource="https://w3id.org/crmrp#Execution_Technique"/>
    <rdf:type rdf:resource="http://www.w3.org/2004/02/skos/core#Concept"/>
    <rdfs:label xml:lang="en">Canvas painting technique</rdfs:label>
    <skos:prefLabel xml:lang="it">Tecnica dipinto su tela</skos:prefLabel>
    <skos:definition xml:lang="en">Painting for which canvas is the support, typically using canvas stretched over stretcher bars or another secondary support.</skos:definition>
    <skos:topConceptOf rdf:resource="https://w3id.org/crmrp#Execution_Technique"/>
    <skos:exactMatch rdf:resource="http://vocab.getty.edu/page/aat/300410350"/>
  </rdf:Description>
  <rdf:Description rdf:about="https://w3id.org/crmrp#c_909e9d33">
    <rdf:type rdf:resource="http://www.w3.org/2002/07/owl#NamedIndividual"/>
    <rdf:type rdf:resource="http://www.w3.org/2004/02/skos/core#Concept"/>
    <skos:editorialNote xml:lang="it">G. Pignolo, “Effetti d’oro - Storia e tecnica della doratura nell’arte”, Editrice Compositori, Bologna, 2002</skos:editorialNote>
    <skos:prefLabel xml:lang="en">Haze</skos:prefLabel>
    <skos:inScheme rdf:resource="https://w3id.org/crmrp#Execution_Technique"/>
    <skos:topConceptOf rdf:resource="https://w3id.org/crmrp#Execution_Technique"/>
    <skos:note xml:lang="en">International references could not be found</skos:note>
    <skos:broader rdf:resource="https://w3id.org/crmrp#c_757ed6ec"/>
    <skos:definition xml:lang="en">Gold foil residues are removed with brushes or cotton to make the glaze opaque</skos:definition>
    <rdfs:label xml:lang="en">Haze</rdfs:label>
    <skos:prefLabel xml:lang="it">Velatura</skos:prefLabel>
  </rdf:Description>
  <rdf:Description rdf:about="https://w3id.org/crmrp#c_e5a56926">
    <skos:definition xml:lang="en">Painted patina involves the use of coloured waxes or enamels, which colour the surface of the metal. It is a type of non-chemical patina that therefore does not involve deterioration of the metal.</skos:definition>
    <skos:prefLabel xml:lang="it">Patinatura dipinta</skos:prefLabel>
    <skos:editorialNote xml:lang="it">A.Giuffredi, “Formatura e fonderia”, Alinea editrice, Firenze, 2010</skos:editorialNote>
    <rdfs:label xml:lang="en">Painted patinatura</rdfs:label>
    <rdf:type rdf:resource="http://www.w3.org/2004/02/skos/core#Concept"/>
    <skos:prefLabel xml:lang="en">Painted patinatura</skos:prefLabel>
    <rdf:type rdf:resource="http://www.w3.org/2002/07/owl#NamedIndividual"/>
    <skos:inScheme rdf:resource="https://w3id.org/crmrp#Execution_Technique"/>
    <skos:broader rdf:resource="https://w3id.org/crmrp#c_f1c689bb"/>
    <skos:topConceptOf rdf:resource="https://w3id.org/crmrp#Execution_Technique"/>
    <skos:note xml:lang="en">International references could not be found</skos:note>
  </rdf:Description>
  <rdf:Description rdf:about="https://w3id.org/crmrp#c_dc1f704e">
    <skos:editorialNote xml:lang="en">A. Weyer et al., “EwaGlos - European Illustrated Glossary of conservation terms for wall paintings and architectural surfaces”, Michael Imhof Verlag, Petersberg, Germany</skos:editorialNote>
    <skos:broader rdf:resource="https://w3id.org/crmrp#c_051209b3"/>
    <skos:definition xml:lang="en">Painting technique using wax as a binder wax as a binder, either hot or cold mixed with pigments and also with resins.</skos:definition>
    <skos:prefLabel xml:lang="it">Encausto</skos:prefLabel>
    <skos:prefLabel xml:lang="en">Encausto</skos:prefLabel>
    <skos:inScheme rdf:resource="https://w3id.org/crmrp#Execution_Technique"/>
    <skos:topConceptOf rdf:resource="https://w3id.org/crmrp#Execution_Technique"/>
    <rdf:type rdf:resource="http://www.w3.org/2002/07/owl#NamedIndividual"/>
    <rdf:type rdf:resource="http://www.w3.org/2004/02/skos/core#Concept"/>
    <rdfs:label xml:lang="en">Encausto</rdfs:label>
  </rdf:Description>
  <rdf:Description rdf:about="https://w3id.org/crmrp#c_5f3ffc3c">
    <skos:topConceptOf rdf:resource="https://w3id.org/crmrp#Alteration"/>
    <skos:prefLabel xml:lang="it">Pitting</skos:prefLabel>
    <skos:prefLabel xml:lang="en">Pitting</skos:prefLabel>
    <skos:editorialNote xml:lang="en">Getty Conservation Institute “Illustrated Glossary - Definitions of terms used for the graphic documentation of in situ floor mosaics”, “Mosaics In Situ Project”, Los Angeles, 2003</skos:editorialNote>
    <rdfs:label xml:lang="en">Pitting</rdfs:label>
    <skos:editorialNote xml:lang="en">Uni Cen/Ts 17135:2021 - Conservation of cultural heritage. General terms and definitions</skos:editorialNote>
    <skos:note xml:lang="en">The preferred editorial note and the definition closest to the meaning is Uni Cen/Ts 17135:2021</skos:note>
    <skos:editorialNote xml:lang="en">Getty AAT http://vocab.getty.edu/page/aat/300054130</skos:editorialNote>
    <skos:editorialNote xml:lang="en">Verg`es-Belmin et al., ICOMOS-ISCS: Illustrated glossary on stone deterioration patterns, vol. XV. Icomos International Council on Monuments and Sites, 2008</skos:editorialNote>
    <skos:closeMatc rdf:resource="http://vocab.getty.edu/page/aat/300054130"/>
    <skos:definition xml:lang="en">Numerous, densely packed shallow cavities on a surface.</skos:definition>
    <skos:inScheme rdf:resource="https://w3id.org/crmrp#Alteration"/>
    <rdf:type rdf:resource="http://www.w3.org/2004/02/skos/core#Concept"/>
    <rdf:type rdf:resource="http://www.w3.org/2002/07/owl#NamedIndividual"/>
  </rdf:Description>
  <rdf:Description rdf:about="https://w3id.org/crmrp#c_e2f34e0a">
    <rdf:type rdf:resource="http://www.w3.org/2004/02/skos/core#Concept"/>
    <skos:editorialNote xml:lang="en">Uni Cen/Ts 17135:2021 - Conservation of cultural heritage. General terms and definitions</skos:editorialNote>
    <skos:topConceptOf rdf:resource="https://w3id.org/crmrp#Alteration"/>
    <skos:prefLabel xml:lang="it">Opacizzazione</skos:prefLabel>
    <skos:definition xml:lang="en">Shift from a shiny toward a matt surface appearance</skos:definition>
    <skos:inScheme rdf:resource="https://w3id.org/crmrp#Alteration"/>
    <rdf:type rdf:resource="http://www.w3.org/2002/07/owl#NamedIndividual"/>
    <skos:prefLabel xml:lang="en">Loss of gloss</skos:prefLabel>
    <rdfs:label xml:lang="en">Loss of gloss</rdfs:label>
    <skos:broader rdf:resource="https://w3id.org/crmrp#c_df05cb61"/>
  </rdf:Description>
  <rdf:Description rdf:about="http://www.cidoc-crm.org/cidoc-crm/P45_consists_of">
    <rdfs:range rdf:resource="http://www.cidoc-crm.org/cidoc-crm/E57_Material"/>
    <rdfs:domain rdf:resource="https://w3id.org/crmrp#R1_Restoration_Object"/>
  </rdf:Description>
  <rdf:Description rdf:about="https://w3id.org/crmrp#c_db001ba3">
    <skos:note xml:lang="en">International references could not be found</skos:note>
    <rdf:type rdf:resource="http://www.w3.org/2002/07/owl#NamedIndividual"/>
    <skos:inScheme rdf:resource="https://w3id.org/crmrp#Archeometric_and_Diagnostic_Analysis"/>
    <skos:editorialNote xml:lang="it">UNI 11085:2003 Beni culturali - Materiali lapidei naturali ed artificiali - Determinazione del contenuto d'acqua: Metodo ponderale</skos:editorialNote>
    <skos:topConceptOf rdf:resource="https://w3id.org/crmrp#Archeometric_and_Diagnostic_Analysis"/>
    <skos:broader rdf:resource="https://w3id.org/crmrp#c_1fd6102e"/>
    <rdf:type rdf:resource="http://www.w3.org/2004/02/skos/core#Concept"/>
    <skos:prefLabel xml:lang="en">Determination of water content</skos:prefLabel>
    <rdfs:label xml:lang="en">Determination of water content</rdfs:label>
    <skos:prefLabel xml:lang="it">Determinazione del contenuto d'acqua</skos:prefLabel>
  </rdf:Description>
  <rdf:Description rdf:about="https://w3id.org/crmrp#R13_Execution_Technique">
    <rdfs:label>Execution Technique</rdfs:label>
    <rdfs:comment xml:lang="en">The purpose of this class is to indicate the execution techniques used in the creation of a work of art.</rdfs:comment>
    <rdfs:subClassOf rdf:resource="http://www.cidoc-crm.org/cidoc-crm/E12_Production"/>
    <rdf:type rdf:resource="http://www.w3.org/2002/07/owl#Class"/>
  </rdf:Description>
  <rdf:Description rdf:about="https://w3id.org/crmrp#c_d057b901">
    <skos:editorialNote xml:lang="en">Getty AAT http://vocab.getty.edu/page/aat/300254138</skos:editorialNote>
    <skos:definition xml:lang="en">Separation with irregular edges through the thickness of a visco-elastic material</skos:definition>
    <skos:note xml:lang="en">The preferred editorial note and the definition closest to the meaning is Uni Cen/Ts 17135:2021</skos:note>
    <skos:editorialNote xml:lang="en">Uni Cen/Ts 17135:2021 - Conservation of cultural heritage. General terms and definitions</skos:editorialNote>
    <skos:topConceptOf rdf:resource="https://w3id.org/crmrp#Alteration"/>
    <skos:prefLabel xml:lang="en">Tear</skos:prefLabel>
    <rdf:type rdf:resource="http://www.w3.org/2004/02/skos/core#Concept"/>
    <skos:altLabel xml:lang="it">Strappo</skos:altLabel>
    <rdf:type rdf:resource="http://www.w3.org/2002/07/owl#NamedIndividual"/>
    <skos:closeMatch rdf:resource="http://vocab.getty.edu/page/aat/30025413"/>
    <rdfs:label xml:lang="en">Tear</rdfs:label>
    <skos:prefLabel xml:lang="it">Lacerazione</skos:prefLabel>
    <skos:altLabel xml:lang="en">Tears</skos:altLabel>
    <skos:inScheme rdf:resource="https://w3id.org/crmrp#Alteration"/>
  </rdf:Description>
  <rdf:Description rdf:about="https://w3id.org/crmrp#c_fec56823">
    <skos:prefLabel xml:lang="it">Xilografia</skos:prefLabel>
    <rdf:type rdf:resource="http://www.w3.org/2002/07/owl#NamedIndividual"/>
    <rdf:type rdf:resource="http://www.w3.org/2004/02/skos/core#Concept"/>
    <skos:topConceptOf rdf:resource="https://w3id.org/crmrp#Execution_Technique"/>
    <rdfs:label xml:lang="en">Xylography</rdfs:label>
    <skos:prefLabel xml:lang="en">Xylography</skos:prefLabel>
    <skos:definition xml:lang="en">Process of using woodblocks, as distinct from type, in printing texts or images.</skos:definition>
    <skos:closeMatch rdf:resource="http://vocab.getty.edu/page/aat/300312031"/>
    <skos:inScheme rdf:resource="https://w3id.org/crmrp#Execution_Technique"/>
    <skos:broader rdf:resource="https://w3id.org/crmrp#c_aee6a805"/>
    <skos:editorialNote xml:lang="en">Getty AAT http://vocab.getty.edu/page/aat/300312031</skos:editorialNote>
  </rdf:Description>
  <rdf:Description rdf:about="https://w3id.org/crmrp#c_61d92422">
    <skos:topConceptOf rdf:resource="https://w3id.org/crmrp#Alteration"/>
    <skos:prefLabel xml:lang="it">Umidità</skos:prefLabel>
    <skos:prefLabel xml:lang="en">Humidity</skos:prefLabel>
    <skos:inScheme rdf:resource="https://w3id.org/crmrp#Alteration"/>
    <skos:editorialNote xml:lang="en">A. Weyer et al., “EwaGlos - European Illustrated Glossary of conservation terms for wall paintings and architectural surfaces”, Michael Imhof Verlag, Petersberg, Germany</skos:editorialNote>
    <skos:definition xml:lang="en">The amount of moisture present in the air or in a porous material (here referredto as moisture).</skos:definition>
    <rdfs:label xml:lang="en">Humidity</rdfs:label>
    <rdf:type rdf:resource="http://www.w3.org/2004/02/skos/core#Concept"/>
    <rdf:type rdf:resource="http://www.w3.org/2002/07/owl#NamedIndividual"/>
  </rdf:Description>
  <rdf:Description rdf:about="https://w3id.org/crmrp#c_bc7a9a95">
    <rdf:type rdf:resource="http://www.w3.org/2004/02/skos/core#Concept"/>
    <skos:inScheme rdf:resource="https://w3id.org/crmrp#Alteration"/>
    <rdfs:label xml:lang="en">Darkened</rdfs:label>
    <skos:prefLabel xml:lang="it">Scurimento</skos:prefLabel>
    <rdf:type rdf:resource="http://www.w3.org/2002/07/owl#NamedIndividual"/>
    <skos:prefLabel xml:lang="en">Darkened</skos:prefLabel>
    <skos:editorialNote xml:lang="en">A. Weyer et al., “EwaGlos - European Illustrated Glossary of conservation terms for wall paintings and architectural surfaces”, Michael Imhof Verlag, Petersberg, Germany</skos:editorialNote>
    <skos:note xml:lang="en">The preferred editorial note and the definition closest to the meaning is Uni Cen/Ts 17135:2021</skos:note>
    <skos:definition xml:lang="en">Exhibiting reduced light reflectivity, hue and/or lightness</skos:definition>
    <skos:closeMatch rdf:resource="http://vocab.getty.edu/page/aat/300379491"/>
    <skos:editorialNote xml:lang="en">Uni Cen/Ts 17135:2021 - Conservation of cultural heritage. General terms and definitions</skos:editorialNote>
    <skos:topConceptOf rdf:resource="https://w3id.org/crmrp#Alteration"/>
    <skos:editorialNote xml:lang="en">Getty AAT http://vocab.getty.edu/page/aat/300379491</skos:editorialNote>
    <skos:broader rdf:resource="https://w3id.org/crmrp#c_df05cb61"/>
  </rdf:Description>
  <rdf:Description rdf:about="https://w3id.org/crmrp#c_4823a051">
    <rdf:type rdf:resource="http://www.w3.org/2004/02/skos/core#Concept"/>
    <skos:note xml:lang="en">International references could not be found</skos:note>
    <skos:topConceptOf rdf:resource="https://w3id.org/crmrp#Intervention"/>
    <skos:definition xml:lang="en">integrative restoration of the gaps in the tapestries that can be combined with the principle of abstraction or colour selection.</skos:definition>
    <skos:broader rdf:resource="https://w3id.org/crmrp#c_24cc76d5"/>
    <skos:inScheme rdf:resource="https://w3id.org/crmrp#Intervention"/>
    <rdf:type rdf:resource="http://www.w3.org/2002/07/owl#NamedIndividual"/>
    <skos:editorialNote xml:lang="it">C. Giannini, “Dizionario del restauro - Tecniche diagnostica  conservazione”, Nardini Editore, Firenze, 2010</skos:editorialNote>
    <skos:prefLabel xml:lang="it">Ritessitura</skos:prefLabel>
    <rdfs:label xml:lang="en">Revowen</rdfs:label>
    <skos:prefLabel xml:lang="en">Revowen</skos:prefLabel>
  </rdf:Description>
  <rdf:Description rdf:about="https://w3id.org/crmrp#c_37bf4517">
    <skos:editorialNote xml:lang="it">A.Giuffredi “Formatura e fonderia”, Alinea editrice, Firenze, 2010</skos:editorialNote>
    <skos:topConceptOf rdf:resource="https://w3id.org/crmrp#Execution_Technique"/>
    <skos:definition xml:lang="en">This type of technique is used for the production of mechanical parts, especially in the weapons industry. The advantages of ceramic casting are precision and fidelity in the reproduction of the smallest details. The limitations are mainly the small dimensions that can be achieved.</skos:definition>
    <skos:note xml:lang="en">International references could not be found</skos:note>
    <skos:prefLabel xml:lang="en">Fusion with ceramic coating</skos:prefLabel>
    <rdfs:label xml:lang="en">Fusion with ceramic coating</rdfs:label>
    <rdf:type rdf:resource="http://www.w3.org/2002/07/owl#NamedIndividual"/>
    <rdf:type rdf:resource="http://www.w3.org/2004/02/skos/core#Concept"/>
    <skos:prefLabel xml:lang="it">Fusione a rivestimento ceramico</skos:prefLabel>
    <skos:inScheme rdf:resource="https://w3id.org/crmrp#Execution_Technique"/>
    <skos:broader rdf:resource="https://w3id.org/crmrp#c_0a9f4d42"/>
  </rdf:Description>
  <rdf:Description rdf:about="https://w3id.org/crmrp#c_9393771d">
    <skos:definition xml:lang="en">Type of opus tessellatum pavement made of stone tesserae of different colors, all of the same size and rectangular shape. As with opus figlinum (page 14), the placement of the tesserae creates a visual impression of a basket weave pattern.</skos:definition>
    <skos:inScheme rdf:resource="https://w3id.org/crmrp#Execution_Technique"/>
    <rdf:type rdf:resource="http://www.w3.org/2002/07/owl#NamedIndividual"/>
    <skos:topConceptOf rdf:resource="https://w3id.org/crmrp#Execution_Technique"/>
    <rdf:type rdf:resource="http://www.w3.org/2004/02/skos/core#Concept"/>
    <skos:broader rdf:resource="https://w3id.org/crmrp#c_b9a6a1c8"/>
    <skos:prefLabel xml:lang="it">Opus figlinum</skos:prefLabel>
    <skos:prefLabel xml:lang="en">Opus figlinum</skos:prefLabel>
    <rdfs:label xml:lang="en">Opus figlinum</rdfs:label>
    <skos:editorialNote xml:lang="en">Getty Conservation Institute “Illustrated Glossary - Technician Training for the Maintenance of In Situ Mosaics”, Los Angeles, 2013</skos:editorialNote>
  </rdf:Description>
  <rdf:Description rdf:about="https://w3id.org/crmrp#c_75d8773c">
    <rdf:type rdf:resource="http://www.w3.org/2002/07/owl#NamedIndividual"/>
    <skos:broader rdf:resource="https://w3id.org/crmrp#c_0a9f4d42"/>
    <skos:definition xml:lang="en">Stirrup casting allows for the re-use of dies: the model, which must necessarily be made of a consistent material, is inserted into a ‘stirrup’ composed of two coupling iron frames, into which refractory earth is pressed, obtaining the negative shape of the model to be reproduced, which is then removed and into the hollow that has been formed and through the previously prepared inlet channels, molten metal is thrown, which will fill all the empty spaces.</skos:definition>
    <skos:prefLabel xml:lang="it">Fusione a staffa</skos:prefLabel>
    <skos:prefLabel xml:lang="en">Fusione a staffa</skos:prefLabel>
    <skos:editorialNote xml:lang="it">A.Giuffredi “Formatura e fonderia”, Alinea editrice, Firenze, 2010</skos:editorialNote>
    <skos:editorialNote xml:lang="it">C. Giannini, “Dizionario del restauro - Tecniche diagnostica conservazione”, Nardini Editore, Firenze, 2010</skos:editorialNote>
    <skos:note xml:lang="en">International references could not be found, but the preferred editorial note and the definition closest to the meaning is Formatura e fonderia</skos:note>
    <rdfs:label xml:lang="en">Fusione a staffa</rdfs:label>
    <rdf:type rdf:resource="http://www.w3.org/2004/02/skos/core#Concept"/>
    <skos:topConceptOf rdf:resource="https://w3id.org/crmrp#Execution_Technique"/>
    <skos:inScheme rdf:resource="https://w3id.org/crmrp#Execution_Technique"/>
  </rdf:Description>
  <rdf:Description rdf:about="https://w3id.org/crmrp#c_547cec21">
    <rdf:type rdf:resource="http://www.w3.org/2004/02/skos/core#Concept"/>
    <rdfs:label xml:lang="en">Disgregation</rdfs:label>
    <skos:altLabel xml:lang="en">Chalking</skos:altLabel>
    <skos:editorialNote xml:lang="en">Getty Conservation Institute “Illustrated Glossary - Definitions of terms used for the graphic documentation of in situ floor mosaics”, “Mosaics In Situ Project”, Los Angeles, 2003</skos:editorialNote>
    <skos:altLabel xml:lang="it">Polverizzazione</skos:altLabel>
    <skos:editorialNote xml:lang="en">A. Weyer et al., “EwaGlos - European Illustrated Glossary of conservation terms for wall paintings and architectural surfaces”, Michael Imhof Verlag, Petersberg, Germany</skos:editorialNote>
    <skos:inScheme rdf:resource="https://w3id.org/crmrp#Alteration"/>
    <skos:topConceptOf rdf:resource="https://w3id.org/crmrp#Alteration"/>
    <skos:prefLabel xml:lang="en">Disgregation</skos:prefLabel>
    <skos:altLabel xml:lang="en">Powdering</skos:altLabel>
    <skos:prefLabel xml:lang="it">Disgregazione</skos:prefLabel>
    <skos:closeMatch rdf:resource="http://vocab.getty.edu/page/aat/300379824"/>
    <rdf:type rdf:resource="http://www.w3.org/2002/07/owl#NamedIndividual"/>
    <skos:note xml:lang="en">The preferred editorial note and the definition closest to the meaning is ICOMOS-ISCS: Illustrated glossary on stone deterioration patterns</skos:note>
    <skos:editorialNote xml:lang="en">Verg`es-Belmin et al., ICOMOS-ISCS: Illustrated glossary on stone deterioration patterns, vol. XV. Icomos International Council on Monuments and Sites, 2008</skos:editorialNote>
    <skos:editorialNote xml:lang="en">Getty AAT http://vocab.getty.edu/page/aat/300379824</skos:editorialNote>
    <skos:definition xml:lang="en">Detachment of single grains or aggregates of grains.</skos:definition>
  </rdf:Description>
  <rdf:Description rdf:about="http://www.cidoc-crm.org/extensions/crmsci/O24_measured">
    <rdfs:range rdf:resource="http://www.cidoc-crm.org/extensions/crmsci/S18_Alteration"/>
    <rdfs:domain rdf:resource="https://w3id.org/crmrp#R12_Invasive_archaeometric_and_diagnostic_analysis"/>
    <rdfs:domain rdf:resource="https://w3id.org/crmrp#R11_Non-invasive_archaeometric_and_diagnostic_analysis"/>
  </rdf:Description>
  <rdf:Description rdf:about="https://w3id.org/crmrp#c_0143a1d7">
    <rdf:type rdf:resource="http://www.w3.org/2004/02/skos/core#Concept"/>
    <skos:topConceptOf rdf:resource="https://w3id.org/crmrp#Alteration"/>
    <rdf:type rdf:resource="http://www.w3.org/2002/07/owl#NamedIndividual"/>
    <rdfs:label xml:lang="en">Hairline crack</rdfs:label>
    <skos:editorialNote xml:lang="en">Uni Cen/Ts 17135:2021 - Conservation of cultural heritage. General terms and definitions</skos:editorialNote>
    <skos:definition xml:lang="en">Depending on the shape, size and number of cracks a specific term as hairline crack</skos:definition>
    <skos:inScheme rdf:resource="https://w3id.org/crmrp#Alteration"/>
    <skos:prefLabel xml:lang="en">Hairline crack</skos:prefLabel>
    <skos:broader rdf:resource="https://w3id.org/crmrp#c_8c762c3e"/>
    <skos:prefLabel xml:lang="it">Cavillatura</skos:prefLabel>
  </rdf:Description>
  <rdf:Description rdf:about="https://w3id.org/crmrp#c_c7a69d6a">
    <skos:prefLabel xml:lang="it">Cromatografia ionica (CI)</skos:prefLabel>
    <skos:editorialNote xml:lang="en">Getty AAT http://vocab.getty.edu/page/aat/300214723</skos:editorialNote>
    <skos:broader rdf:resource="https://w3id.org/crmrp#c_2d5cde83"/>
    <skos:exactMatch rdf:resource="http://vocab.getty.edu/page/aat/300214723"/>
    <rdf:type rdf:resource="http://www.w3.org/2002/07/owl#NamedIndividual"/>
    <skos:topConceptOf rdf:resource="https://w3id.org/crmrp#Archeometric_and_Diagnostic_Analysis"/>
    <skos:definition xml:lang="en">Chromatography that depends on the reciprocal transfer of ions between a solution and a resin or other suitable solid.</skos:definition>
    <skos:prefLabel xml:lang="en">Ion-exchange chromatography (IC)</skos:prefLabel>
    <rdf:type rdf:resource="http://www.w3.org/2004/02/skos/core#Concept"/>
    <rdfs:label xml:lang="en">Ion-exchange chromatography (IC)</rdfs:label>
    <skos:inScheme rdf:resource="https://w3id.org/crmrp#Archeometric_and_Diagnostic_Analysis"/>
  </rdf:Description>
  <rdf:Description rdf:about="https://w3id.org/crmrp#c_4f621a84">
    <skos:inScheme rdf:resource="https://w3id.org/crmrp#Alteration"/>
    <skos:editorialNote xml:lang="it">C. Giannini, “Dizionario del restauro - Tecniche diagnostica conservazione”, Nardini Editore, Firenze, 2010</skos:editorialNote>
    <rdf:type rdf:resource="http://www.w3.org/2004/02/skos/core#Concept"/>
    <skos:topConceptOf rdf:resource="https://w3id.org/crmrp#Alteration"/>
    <skos:prefLabel xml:lang="it">Fungo</skos:prefLabel>
    <rdfs:label xml:lang="en">Fungus</rdfs:label>
    <rdf:type rdf:resource="http://www.w3.org/2002/07/owl#NamedIndividual"/>
    <skos:prefLabel xml:lang="en">Fungus</skos:prefLabel>
    <skos:broader rdf:resource="https://w3id.org/crmrp#c_3ef20257"/>
    <skos:definition xml:lang="en">A micro-organism that usually develops as a result of moisture and attacks mainly canvas, paper, natural and artificial stone surfaces; it forms black, greenish or yellow colonies preferably in the presence of glues and on painted parts that are then altered. Mycological studies have demonstrated the great ability of fungal species to adapt to different microclimates, confirming their harmfulness to various types of artistic artefacts.</skos:definition>
    <skos:note xml:lang="en">International references could not be found</skos:note>
  </rdf:Description>
  <rdf:Description rdf:about="https://w3id.org/crmrp#c_613f625a">
    <rdf:type rdf:resource="http://www.w3.org/2004/02/skos/core#Concept"/>
    <skos:broader rdf:resource="https://w3id.org/crmrp#c_1fd6102e"/>
    <skos:prefLabel xml:lang="it">Monitoraggio strutturale</skos:prefLabel>
    <skos:prefLabel xml:lang="en">Structural monitoring</skos:prefLabel>
    <skos:definition xml:lang="en">A structural monitoring system is a set of tools and procedures designed to monitor and assess the condition of a structure.It includes: endoscope, fissurimeter, pacometer</skos:definition>
    <rdf:type rdf:resource="http://www.w3.org/2002/07/owl#NamedIndividual"/>
    <rdfs:label xml:lang="en">Structural monitoring</rdfs:label>
    <skos:topConceptOf rdf:resource="https://w3id.org/crmrp#Archeometric_and_Diagnostic_Analysis"/>
    <skos:note xml:lang="en">International references could not be found.</skos:note>
    <skos:inScheme rdf:resource="https://w3id.org/crmrp#Archeometric_and_Diagnostic_Analysis"/>
  </rdf:Description>
  <rdf:Description rdf:about="https://w3id.org/crmrp#c_3cbfcf7b">
    <skos:editorialNote xml:lang="en">Getty AAT http://vocab.getty.edu/page/aat/300266192</skos:editorialNote>
    <skos:broader rdf:resource="https://w3id.org/crmrp#c_789c3e32"/>
    <skos:prefLabel xml:lang="en">Raman spectroscopy</skos:prefLabel>
    <rdf:type rdf:resource="http://www.w3.org/2004/02/skos/core#Concept"/>
    <skos:definition xml:lang="en">Technique of scattering a monochromatic light, such as a laser, changing the vibrational, rotational, or electronic energy of a sample, the results of which help determine its molecular structure. Discovered by Indian physicist Sir Chandrasekhara Venkata Raman (1888-1970).</skos:definition>
    <rdf:type rdf:resource="http://www.w3.org/2002/07/owl#NamedIndividual"/>
    <rdfs:label xml:lang="en">Raman spectroscopy</rdfs:label>
    <skos:exactMatch rdf:resource="http://vocab.getty.edu/page/aat/300266192"/>
    <skos:topConceptOf rdf:resource="https://w3id.org/crmrp#Archeometric_and_Diagnostic_Analysis"/>
    <skos:prefLabel xml:lang="it">Spettrofotometria Raman</skos:prefLabel>
    <skos:inScheme rdf:resource="https://w3id.org/crmrp#Archeometric_and_Diagnostic_Analysis"/>
  </rdf:Description>
  <rdf:Description rdf:about="https://w3id.org/crmrp#c_19d7c1db">
    <skos:broader rdf:resource="https://w3id.org/crmrp#c_6626f18c"/>
    <skos:inScheme rdf:resource="https://w3id.org/crmrp#Execution_Technique"/>
    <rdfs:label xml:lang="en">Sgraffito (graffito)</rdfs:label>
    <skos:note xml:lang="en">The preferred editorial note and the definition closest to the meaning is EwaGlos - European Illustrated Glossary of conservation terms for wall paintings and architectural surfaces</skos:note>
    <skos:exactMatch rdf:resource="http://vocab.getty.edu/page/aat/300266416"/>
    <skos:editorialNote xml:lang="en">Getty AAT http://vocab.getty.edu/page/aat/300266416</skos:editorialNote>
    <rdf:type rdf:resource="http://www.w3.org/2004/02/skos/core#Concept"/>
    <skos:topConceptOf rdf:resource="https://w3id.org/crmrp#Execution_Technique"/>
    <skos:prefLabel xml:lang="it">Sgraffito (graffito)</skos:prefLabel>
    <skos:prefLabel xml:lang="en">Sgraffito (graffito)</skos:prefLabel>
    <rdf:type rdf:resource="http://www.w3.org/2002/07/owl#NamedIndividual"/>
    <skos:definition xml:lang="en">Multi-layer decoration technique executed by scratching the upper plaster layer to reveal parts of the underlying (e.g. dark plaster) layer.</skos:definition>
    <skos:editorialNote xml:lang="en">A. Weyer et al., “EwaGlos - European Illustrated Glossary of conservation terms for wall paintings and architectural surfaces”, Michael Imhof Verlag, Petersberg, Germany</skos:editorialNote>
  </rdf:Description>
  <rdf:Description rdf:about="https://w3id.org/crmrp#c_c5825f0c">
    <skos:prefLabel xml:lang="en">Level of alkalinity/acidity</skos:prefLabel>
    <skos:definition xml:lang="en">The pH value can be determined electrically, exploiting the potential created by the difference in hydrogen ion concentration on two sides of a glass membrane, using an electronic instrument known as a pH meter</skos:definition>
    <skos:note xml:lang="en">International references could not be found</skos:note>
    <skos:prefLabel xml:lang="it">Determinazione pH</skos:prefLabel>
    <rdf:type rdf:resource="http://www.w3.org/2002/07/owl#NamedIndividual"/>
    <skos:topConceptOf rdf:resource="https://w3id.org/crmrp#Archeometric_and_Diagnostic_Analysis"/>
    <rdf:type rdf:resource="http://www.w3.org/2004/02/skos/core#Concept"/>
    <skos:broader rdf:resource="https://w3id.org/crmrp#c_1fd6102e"/>
    <skos:inScheme rdf:resource="https://w3id.org/crmrp#Archeometric_and_Diagnostic_Analysis"/>
    <rdfs:label xml:lang="en">Level of alkalinity/acidity</rdfs:label>
  </rdf:Description>
  <rdf:Description rdf:about="https://w3id.org/crmrp#c_66ff714b">
    <rdf:type rdf:resource="http://www.w3.org/2004/02/skos/core#Concept"/>
    <skos:editorialNote xml:lang="it">S. Volpin e L. Appolonia “Le analisi di laboratorio applicate ai beni artistici policromi”, Il Prato, Padova, 1999</skos:editorialNote>
    <skos:broader rdf:resource="https://w3id.org/crmrp#c_abed88a5"/>
    <skos:prefLabel xml:lang="it">Test fisico-meccanico</skos:prefLabel>
    <skos:note xml:lang="en">International references could not be found</skos:note>
    <rdf:type rdf:resource="http://www.w3.org/2002/07/owl#NamedIndividual"/>
    <skos:prefLabel xml:lang="en">Physical-mechanical testing</skos:prefLabel>
    <skos:defintion xml:lang="en">Physical-mechanical tests are used to obtain information about the physical performance and mechanical behaviour of a component.</skos:defintion>
    <rdfs:label xml:lang="en">Physical-mechanical testing</rdfs:label>
    <skos:inScheme rdf:resource="https://w3id.org/crmrp#Archeometric_and_Diagnostic_Analysis"/>
    <skos:topConceptOf rdf:resource="https://w3id.org/crmrp#Archeometric_and_Diagnostic_Analysis"/>
  </rdf:Description>
  <rdf:Description rdf:about="https://w3id.org/crmrp#c_1283fc77">
    <skos:prefLabel xml:lang="en">Sculpture technique</skos:prefLabel>
    <skos:closeMatch rdf:resource="http://vocab.getty.edu/page/aat/300053618"/>
    <skos:prefLabel xml:lang="it">Tecnica del marmo e delle pietre dure</skos:prefLabel>
    <rdf:type rdf:resource="http://www.w3.org/2002/07/owl#NamedIndividual"/>
    <skos:editorialNote xml:lang="en">Getty AAt http://vocab.getty.edu/page/aat/300053618</skos:editorialNote>
    <skos:topConceptOf rdf:resource="https://w3id.org/crmrp#Execution_Technique"/>
    <rdf:type rdf:resource="http://www.w3.org/2004/02/skos/core#Concept"/>
    <skos:inScheme rdf:resource="https://w3id.org/crmrp#Execution_Technique"/>
    <skos:definition xml:lang="en">Describes techniques for creating three-dimensional objects with malleable or hard materials, such as clay, wood, stone, bronze, ivory, and found objects.</skos:definition>
    <rdfs:label xml:lang="en">Sculpture technique</rdfs:label>
  </rdf:Description>
  <rdf:Description rdf:about="https://w3id.org/crmrp#c_c7591bf7">
    <rdf:type rdf:resource="http://www.w3.org/2002/07/owl#NamedIndividual"/>
    <skos:editorialNote xml:lang="en">A. Weyer et al., “EwaGlos - European Illustrated Glossary of conservation terms for wall paintings and architectural surfaces”, Michael Imhof Verlag, Petersberg, Germany</skos:editorialNote>
    <skos:topConceptOf rdf:resource="https://w3id.org/crmrp#Intervention"/>
    <skos:prefLabel xml:lang="it">Stacco</skos:prefLabel>
    <skos:prefLabel xml:lang="en">Stacco</skos:prefLabel>
    <rdf:type rdf:resource="http://www.w3.org/2004/02/skos/core#Concept"/>
    <skos:inScheme rdf:resource="https://w3id.org/crmrp#Intervention"/>
    <skos:definition xml:lang="en">The process of detaching a fresco painting from the wall by removing the pigment layer and a layer of intonaco. Cloth is glued to the painted surface and, when dry, the cloth, painting, and plaster are stripped from the wall.</skos:definition>
    <skos:note xml:lang="en">The preferred editorial note and the definition closest to the meaning is Getty AAT</skos:note>
    <skos:editorialNote xml:lang="en">Getty AAT http://vocab.getty.edu/page/aat/300078739</skos:editorialNote>
    <skos:exactMatch rdf:resource="http://vocab.getty.edu/page/aat/300078739"/>
    <skos:broader rdf:resource="https://w3id.org/crmrp#c_4fe4d308"/>
    <rdfs:label xml:lang="en">Stacco</rdfs:label>
  </rdf:Description>
  <rdf:Description rdf:about="https://w3id.org/crmrp#c_0e594482">
    <skos:prefLabel xml:lang="it">Analisi elettrochimica</skos:prefLabel>
    <skos:prefLabel xml:lang="en">Electrochemical analysis</skos:prefLabel>
    <skos:topConceptOf rdf:resource="https://w3id.org/crmrp#Archeometric_and_Diagnostic_Analysis"/>
    <skos:inScheme rdf:resource="https://w3id.org/crmrp#Archeometric_and_Diagnostic_Analysis"/>
    <skos:definition xml:lang="en">Electrochemical analysis is based on the use of conductive probes or electrodes connected to electronic devices capable of measuring the electrical parameters generated by the oxidation-reduction reaction of species in solution.</skos:definition>
    <skos:broader rdf:resource="https://w3id.org/crmrp#c_abed88a5"/>
    <rdfs:label xml:lang="en">Electrochemical analysis</rdfs:label>
    <rdf:type rdf:resource="http://www.w3.org/2004/02/skos/core#Concept"/>
    <rdf:type rdf:resource="http://www.w3.org/2002/07/owl#NamedIndividual"/>
  </rdf:Description>
  <rdf:Description rdf:about="https://w3id.org/crmrp#c_25d4058b">
    <skos:inScheme rdf:resource="https://w3id.org/crmrp#Archeometric_and_Diagnostic_Analysis"/>
    <rdf:type rdf:resource="http://www.w3.org/2004/02/skos/core#Concept"/>
    <skos:prefLabel xml:lang="en">Weighting method humidity measurement</skos:prefLabel>
    <skos:prefLabel xml:lang="it">Misura ponderale umidità nelle murature</skos:prefLabel>
    <skos:definition xml:lang="en">The weighing method involves taking dust samples from bricks or mortar by drilling, in order to calculate the weight humidity in the wall</skos:definition>
    <skos:editorialNote xml:lang="it">UNI 11085:2003 Beni culturali - Materiali lapidei naturali ed artificiali - Determinazione del contenuto d'acqua: Metodo ponderale</skos:editorialNote>
    <skos:note xml:lang="en">International references could not be found</skos:note>
    <skos:topConceptOf rdf:resource="https://w3id.org/crmrp#Archeometric_and_Diagnostic_Analysis"/>
    <skos:broader rdf:resource="https://w3id.org/crmrp#c_abed88a5"/>
    <rdfs:label xml:lang="en">Weighting method humidity measurement</rdfs:label>
    <rdf:type rdf:resource="http://www.w3.org/2002/07/owl#NamedIndividual"/>
  </rdf:Description>
  <rdf:Description rdf:about="https://w3id.org/crmrp#Archeometric_and_Diagnostic_Analysis">
    <skos:prefLabel xml:lang="it">Indagine archeometrica e diagnostica</skos:prefLabel>
    <skos:prefLabel xml:lang="en">Archaeometric and diagnostic analysis</skos:prefLabel>
    <skos:note xml:lang="en">International references could not be found</skos:note>
    <rdf:type rdf:resource="http://www.w3.org/2004/02/skos/core#ConceptScheme"/>
    <rdf:type rdf:resource="http://www.w3.org/2002/07/owl#NamedIndividual"/>
  </rdf:Description>
  <rdf:Description rdf:about="https://w3id.org/crmrp#c_5b84d202">
    <skos:broader rdf:resource="https://w3id.org/crmrp#c_1fd6102e"/>
    <skos:editorialNote xml:lang="it">C. Giannini, “Dizionario del restauro - Tecniche diagnostica conservazione”, Nardini Editore, Firenze, 2010</skos:editorialNote>
    <rdf:type rdf:resource="http://www.w3.org/2002/07/owl#NamedIndividual"/>
    <skos:topConceptOf rdf:resource="https://w3id.org/crmrp#Archeometric_and_Diagnostic_Analysis"/>
    <skos:editorialNote xml:lang="it">A. Aldrovandi, M. Picollo “Metodi di documentazione indagini non invasive sui dipinti”, Il Prato, Padova</skos:editorialNote>
    <rdfs:label xml:lang="en">Transillumination</rdfs:label>
    <skos:prefLabel xml:lang="it">Transilluminazione</skos:prefLabel>
    <skos:prefLabel xml:lang="en">Transillumination</skos:prefLabel>
    <skos:definition xml:lang="en">Technique of observation in the visible where the is placed between the illumination source and the observer. Transillumination can only be used only on materials that are partially or fully transparent to visible radiation</skos:definition>
    <skos:editorialNote xml:lang="it">M.Ceroni, G.Elia, “Diagnostica per i beni culturali”, Alinea editrice, Firenze, 2008</skos:editorialNote>
    <skos:inScheme rdf:resource="https://w3id.org/crmrp#Archeometric_and_Diagnostic_Analysis"/>
    <skos:note xml:lang="en">International references could not be found, but the preferred editorial note and the definition closest to the meaning is Dizionario del restauro - Tecniche diagnostica conservazione</skos:note>
    <skos:editorialNote xml:lang="it">P.Cremonesi, E. Signorini, “Un approccio alla pulitura dei dipinti mobili”, Il Prato, Padova, 2016</skos:editorialNote>
    <rdf:type rdf:resource="http://www.w3.org/2004/02/skos/core#Concept"/>
  </rdf:Description>
  <rdf:Description rdf:about="https://w3id.org/crmrp#c_7f750ff2">
    <rdf:type rdf:resource="http://www.w3.org/2004/02/skos/core#Concept"/>
    <skos:prefLabel xml:lang="en">Infiltration</skos:prefLabel>
    <skos:editorialNote xml:lang="en">A. Weyer et al., “EwaGlos - European Illustrated Glossary of conservation terms for wall paintings and architectural surfaces”, Michael Imhof Verlag, Petersberg, Germany</skos:editorialNote>
    <skos:topConceptOf rdf:resource="https://w3id.org/crmrp#Alteration"/>
    <rdf:type rdf:resource="http://www.w3.org/2002/07/owl#NamedIndividual"/>
    <skos:definition xml:lang="en">The ingress of water through defects in a building.</skos:definition>
    <skos:prefLabel xml:lang="it">Infiltrazione</skos:prefLabel>
    <rdfs:label xml:lang="en">Infiltration</rdfs:label>
    <skos:inScheme rdf:resource="https://w3id.org/crmrp#Alteration"/>
    <skos:broader rdf:resource="https://w3id.org/crmrp#c_61d92422"/>
  </rdf:Description>
  <rdf:Description rdf:about="https://w3id.org/crmrp#c_830e6744">
    <skos:prefLabel xml:lang="en">Cleaning</skos:prefLabel>
    <skos:inScheme rdf:resource="https://w3id.org/crmrp#Intervention"/>
    <skos:editorialNote xml:lang="en">Getty AAT http://vocab.getty.edu/page/aat/300053027</skos:editorialNote>
    <skos:topConceptOf rdf:resource="https://w3id.org/crmrp#Intervention"/>
    <skos:editorialNote xml:lang="en">Getty Conservation Institute “Illustrated Glossary - Definitions of terms used for the graphic documentation of in situ floor mosaics”, “Mosaics In Situ Project”, Los Angeles, 2003</skos:editorialNote>
    <skos:prefLabel xml:lang="it">Pulitura</skos:prefLabel>
    <skos:editorialNote xml:lang="it">Uni En 15898:2019 Conservazione del patrimonio culturale - Termini generali e definizioni</skos:editorialNote>
    <rdf:type rdf:resource="http://www.w3.org/2002/07/owl#NamedIndividual"/>
    <skos:editorialNote xml:lang="en">A. Weyer et al., “EwaGlos - European Illustrated Glossary of conservation terms for wall paintings and architectural surfaces”, Michael Imhof Verlag, Petersberg, Germany</skos:editorialNote>
    <rdf:type rdf:resource="http://www.w3.org/2004/02/skos/core#Concept"/>
    <skos:definition xml:lang="en">Removal of unwanted material from an object</skos:definition>
    <skos:exactMatch rdf:resource="http://vocab.getty.edu/page/aat/300053027"/>
    <rdfs:label xml:lang="en">Cleaning</rdfs:label>
  </rdf:Description>
  <rdf:Description rdf:about="https://w3id.org/crmrp#c_3b191842">
    <skos:note xml:lang="en">The preferred editorial note and the definition closest to the meaning is Uni Cen/Ts 17135:2021</skos:note>
    <skos:altLabel xml:lang="en">Bulge</skos:altLabel>
    <skos:topConceptOf rdf:resource="https://w3id.org/crmrp#Alteration"/>
    <skos:editorialNote xml:lang="en"> A. Weyer et al., “EwaGlos - European Illustrated Glossary of conservation terms for wall paintings and architectural surfaces”, Michael Imhof Verlag, Petersberg, Germany</skos:editorialNote>
    <skos:inScheme rdf:resource="https://w3id.org/crmrp#Alteration"/>
    <skos:prefLabel xml:lang="it">Sbollatura</skos:prefLabel>
    <skos:prefLabel xml:lang="en">Blister</skos:prefLabel>
    <rdf:type rdf:resource="http://www.w3.org/2004/02/skos/core#Concept"/>
    <rdf:type rdf:resource="http://www.w3.org/2002/07/owl#NamedIndividual"/>
    <rdfs:label xml:lang="en">Blister</rdfs:label>
    <skos:broader rdf:resource="https://w3id.org/crmrp#c_13f3ce9e"/>
    <skos:definition xml:lang="en">Domed surface with a cavity beneath.</skos:definition>
    <skos:editorialNote xml:lang="en">Uni Cen/Ts 17135:2021 - Conservation of cultural heritage. General terms and definitions</skos:editorialNote>
  </rdf:Description>
  <rdf:Description rdf:about="https://w3id.org/crmrp#c_287887a9">
    <skos:inScheme rdf:resource="https://w3id.org/crmrp#Documentation"/>
    <skos:definition xml:lang="en">Graphical representation of a single or several patterns on an object.</skos:definition>
    <skos:topConceptOf rdf:resource="https://w3id.org/crmrp#Documentation"/>
    <skos:prefLabel xml:lang="en">Mapping</skos:prefLabel>
    <rdf:type rdf:resource="http://www.w3.org/2004/02/skos/core#Concept"/>
    <skos:prefLabel xml:lang="it">CAD 2D</skos:prefLabel>
    <rdfs:label xml:lang="en">Mapping</rdfs:label>
    <skos:editorialNote xml:lang="en">A. Weyer et al., “EwaGlos - European Illustrated Glossary of conservation terms for wall paintings and architectural surfaces”, Michael Imhof Verlag, Petersberg, Germany</skos:editorialNote>
    <rdf:type rdf:resource="http://www.w3.org/2002/07/owl#NamedIndividual"/>
    <skos:broader rdf:resource="https://w3id.org/crmrp#c_f383c4d3"/>
  </rdf:Description>
  <rdf:Description rdf:about="https://w3id.org/crmrp#c_df7c7c9c">
    <skos:topConceptOf rdf:resource="https://w3id.org/crmrp#Execution_Technique"/>
    <skos:definition xml:lang="en">Refers to the technique of making compositions in two dimensions or very low relief by gluing paper, fabrics, photographs, or other materials onto a flat surface.</skos:definition>
    <rdfs:label xml:lang="en">Collage</rdfs:label>
    <rdf:type rdf:resource="http://www.w3.org/2002/07/owl#NamedIndividual"/>
    <rdf:type rdf:resource="http://www.w3.org/2004/02/skos/core#Concept"/>
    <skos:inScheme rdf:resource="https://w3id.org/crmrp#Execution_Technique"/>
    <skos:prefLabel xml:lang="it">Collage</skos:prefLabel>
    <skos:prefLabel xml:lang="en">Collage</skos:prefLabel>
    <skos:broader rdf:resource="https://w3id.org/crmrp#c_143349b9"/>
    <skos:editorialNote xml:lang="en">Getty AAT http://vocab.getty.edu/page/aat/300138699</skos:editorialNote>
    <skos:broader rdf:resource="https://w3id.org/crmrp#c_051209b3"/>
    <skos:exactMatch rdf:resource="http://vocab.getty.edu/page/aat/300138699"/>
  </rdf:Description>
  <rdf:Description rdf:about="https://w3id.org/crmrp#c_c10ff387">
    <skos:topConceptOf rdf:resource="https://w3id.org/crmrp#Restoration_Object"/>
    <rdf:type rdf:resource="http://www.w3.org/2002/07/owl#NamedIndividual"/>
    <skos:definition xml:lang="en">Study of coins, tokens, medals, paper money, and objects closely resembling them in form or purpose.</skos:definition>
    <rdfs:label xml:lang="en">Numismatics</rdfs:label>
    <skos:prefLabel xml:lang="en">Numismatica</skos:prefLabel>
    <skos:prefLabel xml:lang="it">Numismatico</skos:prefLabel>
    <skos:closeMatch rdf:resource="http://vocab.getty.edu/page/aat/300054419"/>
    <rdf:type rdf:resource="http://www.w3.org/2004/02/skos/core#Concept"/>
    <skos:inScheme rdf:resource="https://w3id.org/crmrp#Restoration_Object"/>
    <skos:editorialNote xml:lang="en">Getty AAT http://vocab.getty.edu/page/aat/300054419</skos:editorialNote>
  </rdf:Description>
  <rdf:Description rdf:about="https://w3id.org/crmrp#R6_Video_Documentation">
    <rdfs:label xml:lang="en">Video Documentation</rdfs:label>
    <rdfs:comment xml:lang="en">This class represents the video documentation of an object.
In particular, in the case of contemporary art, it is possible to find a few recorded interviews of the artist and to understand the execution techniques or the artist's idea about the restoration of their works.</rdfs:comment>
    <rdfs:subClassOf rdf:resource="http://www.cidoc-crm.org/cidoc-crm/E31_Document"/>
    <rdf:type rdf:resource="http://www.w3.org/2002/07/owl#Class"/>
  </rdf:Description>
  <rdf:Description rdf:about="https://w3id.org/crmrp#c_46b47593">
    <skos:prefLabel xml:lang="en">Dendrochronology</skos:prefLabel>
    <rdfs:label xml:lang="en">Dendrochronology</rdfs:label>
    <skos:inScheme rdf:resource="https://w3id.org/crmrp#Archeometric_and_Diagnostic_Analysis"/>
    <skos:broader rdf:resource="https://w3id.org/crmrp#c_abed88a5"/>
    <rdf:type rdf:resource="http://www.w3.org/2004/02/skos/core#Concept"/>
    <rdf:type rdf:resource="http://www.w3.org/2002/07/owl#NamedIndividual"/>
    <skos:definition xml:lang="en"> The technique of dating events, intervals of time, and variations in environment understood by studying the sequence of and differences between rings of growth in trees and aged wood.</skos:definition>
    <skos:exactMatch rdf:resource="http://vocab.getty.edu/page/aat/300054715"/>
    <skos:topConceptOf rdf:resource="https://w3id.org/crmrp#Archeometric_and_Diagnostic_Analysis"/>
    <skos:prefLabel xml:lang="it">Dendrocronologia</skos:prefLabel>
    <skos:editorialNote xml:lang="en">Getty AAT http://vocab.getty.edu/page/aat/300054715</skos:editorialNote>
  </rdf:Description>
  <rdf:Description rdf:about="https://w3id.org/crmrp#R2_Audio_Documentation">
    <rdfs:label xml:lang="en">Audio Documentation</rdfs:label>
    <rdfs:comment xml:lang="en">This class represents the audio documentation of an object.
In the case of contemporary art, it is possible to find a few recorded interviews of the artist and to understand the execution techniques or the artist's idea about the restoration of their works.
Furthermore, it might be possible to rediscover the sound of an ancient instrument that is currently too fragile to be played.</rdfs:comment>
    <rdfs:subClassOf rdf:resource="http://www.cidoc-crm.org/cidoc-crm/E31_Document"/>
    <rdf:type rdf:resource="http://www.w3.org/2002/07/owl#Class"/>
  </rdf:Description>
  <rdf:Description rdf:about="https://w3id.org/crmrp#c_4ed58c32">
    <skos:inScheme rdf:resource="https://w3id.org/crmrp#Execution_Technique"/>
    <skos:definition xml:lang="en">Prints made from an etched printing plate, which is a metal plate on which a design is made by coating the plate with an acid-resistant substance, creating a design in the coating, and then exposing the plate to acid, which etches the plate where the metal is exposed. For designs incised directly into a copper plate using a burin or graver, use engravings (prints).</skos:definition>
    <skos:closeMatch rdf:resource="http://vocab.getty.edu/page/aat/300041365"/>
    <skos:prefLabel xml:lang="it">Acquaforte</skos:prefLabel>
    <skos:prefLabel xml:lang="en">Etchings</skos:prefLabel>
    <rdf:type rdf:resource="http://www.w3.org/2004/02/skos/core#Concept"/>
    <skos:broader rdf:resource="https://w3id.org/crmrp#c_aee6a805"/>
    <rdfs:label xml:lang="en">Etchings</rdfs:label>
    <rdf:type rdf:resource="http://www.w3.org/2002/07/owl#NamedIndividual"/>
    <skos:topConceptOf rdf:resource="https://w3id.org/crmrp#Execution_Technique"/>
    <skos:editorialNote xml:lang="en">Getty AAT http://vocab.getty.edu/page/aat/300041365</skos:editorialNote>
  </rdf:Description>
  <rdf:Description rdf:about="https://w3id.org/crmrp#c_ab5f4e0c">
    <skos:exactMatch rdf:resource="http://vocab.getty.edu/page/aat/300213366"/>
    <rdf:type rdf:resource="http://www.w3.org/2002/07/owl#NamedIndividual"/>
    <rdfs:label xml:lang="en">Buffer solution</rdfs:label>
    <skos:prefLabel xml:lang="en">Buffer solution</skos:prefLabel>
    <skos:topConceptOf rdf:resource="https://w3id.org/crmrp#Intervention"/>
    <rdf:type rdf:resource="http://www.w3.org/2004/02/skos/core#Concept"/>
    <skos:prefLabel xml:lang="it">Tampone</skos:prefLabel>
    <skos:editorialNote xml:lang="en">Getty AAT http://vocab.getty.edu/page/aat/300213366</skos:editorialNote>
    <skos:inScheme rdf:resource="https://w3id.org/crmrp#Intervention"/>
    <skos:definition xml:lang="en">Any substance capable in solution of neutralizing both acids and bases and thereby maintaining the original acidity or basicity of the solution.</skos:definition>
    <skos:broader rdf:resource="https://w3id.org/crmrp#c_5a83cd16"/>
  </rdf:Description>
  <rdf:Description rdf:about="https://w3id.org/crmrp#R1_Restoration_Object">
    <rdfs:label xml:lang="en">Restoration Object</rdfs:label>
    <rdfs:comment xml:lang="en">This class is the core concept of the schema and denotes the artefact to be (or that has been) restored. 
As C. Brandi states in Theory of Restoration: "restoration constitutes the methodological moment of recognition of an artwork". This implies that an artefact must first be recognised as an object of cultural interest to be passed on to the future in order to be considered restorable. Hence, a "Restoration object" is a "Cultural Object", and as such, it has been catalogued, and its catalogue sheet provides all the principal historical and artistic information. This is also the case for composite artworks and for their individual components, such as a painted panel of a polyptych, or a painting that is part of a cycle.</rdfs:comment>
    <rdfs:subClassOf rdf:resource="http://www.cidoc-crm.org/cidoc-crm/E22_Human-Made_Object"/>
    <rdf:type rdf:resource="http://www.w3.org/2002/07/owl#Class"/>
  </rdf:Description>
  <rdf:Description rdf:about="https://w3id.org/crmrp#c_0f7eacd7">
    <rdf:type rdf:resource="http://www.w3.org/2002/07/owl#NamedIndividual"/>
    <skos:prefLabel xml:lang="en">Reintegration</skos:prefLabel>
    <skos:definition xml:lang="en">Restoration action consisting in the addition of material for the reconstruction of appearance (e.g. pictorial retouching, insertion, repainting, filling, etc.)</skos:definition>
    <skos:inScheme rdf:resource="https://w3id.org/crmrp#Intervention"/>
    <skos:editorialNote xml:lang="en">A. Weyer et al., “EwaGlos - European Illustrated Glossary of conservation terms for wall paintings and architectural surfaces”, Michael Imhof Verlag, Petersberg, Germany</skos:editorialNote>
    <rdf:type rdf:resource="http://www.w3.org/2004/02/skos/core#Concept"/>
    <skos:editorialNote xml:lang="it">Uni En 15898:2019 Conservazione del patrimonio culturale - Termini generali e definizioni</skos:editorialNote>
    <rdfs:label xml:lang="en">Reintegration</rdfs:label>
    <skos:topConceptOf rdf:resource="https://w3id.org/crmrp#Intervention"/>
    <skos:prefLabel xml:lang="it">Reintegrazione</skos:prefLabel>
    <skos:note xml:lang="en">The preferred editorial note and the definition closest to the meaning is Uni En 15898:2019</skos:note>
  </rdf:Description>
  <rdf:Description rdf:about="https://w3id.org/crmrp#c_96b092c5">
    <skos:topConceptOf rdf:resource="https://w3id.org/crmrp#Restoration_Object"/>
    <skos:editorialNote xml:lang="en">Getty AAT http://vocab.getty.edu/page/aat/300028569</skos:editorialNote>
    <skos:exactMatch rdf:resource="http://vocab.getty.edu/page/aat/300028569"/>
    <skos:prefLabel xml:lang="it">Manoscritto</skos:prefLabel>
    <skos:definition xml:lang="en">Handwritten documents, particularly books and other documents created before the invention of the printing press. May also be used to distinguish certain documents from published or otherwise printed documents, as in the cases of typed personal letters or a typescript from which printed versions are made.</skos:definition>
    <rdfs:label xml:lang="en">Manuscript</rdfs:label>
    <rdf:type rdf:resource="http://www.w3.org/2004/02/skos/core#Concept"/>
    <skos:inScheme rdf:resource="https://w3id.org/crmrp#Restoration_Object"/>
    <skos:prefLabel xml:lang="en">Manuscript</skos:prefLabel>
    <rdf:type rdf:resource="http://www.w3.org/2002/07/owl#NamedIndividual"/>
  </rdf:Description>
  <rdf:Description rdf:about="https://w3id.org/crmrp#c_612bc334">
    <rdf:type rdf:resource="http://www.w3.org/2002/07/owl#NamedIndividual"/>
    <skos:editorialNote xml:lang="it">C. Giannini, “Dizionario del restauro - Tecniche diagnostica conservazione”, Nardini Editore, Firenze, 2010</skos:editorialNote>
    <skos:note xml:lang="en">It was decided not to proceed with the English translation in order to avoid possible lexical errors and misunderstandings.</skos:note>
    <skos:topConceptOf rdf:resource="https://w3id.org/crmrp#Execution_Technique"/>
    <skos:broader rdf:resource="https://w3id.org/crmrp#c_17157ccd"/>
    <rdf:type rdf:resource="http://www.w3.org/2004/02/skos/core#Concept"/>
    <rdfs:label xml:lang="en">Forma a tasselli</rdfs:label>
    <skos:definition xml:lang="en">Plaster form also known as the Good Form or Real Form because it is made up of many detachable elements, once made it allows numerous copies to be made and a long preservation period.</skos:definition>
    <skos:inScheme rdf:resource="https://w3id.org/crmrp#Execution_Technique"/>
    <skos:prefLabel xml:lang="it">Forma a tasselli</skos:prefLabel>
    <skos:prefLabel xml:lang="en">Forma a tasselli</skos:prefLabel>
  </rdf:Description>
  <rdf:Description rdf:about="https://w3id.org/crmrp#R10_Sign_of_Workmanship">
    <rdfs:label xml:lang="en">Sign of Workmanship</rdfs:label>
    <rdfs:comment xml:lang="en">This class describe the signs of workmanship visible on an artwork.
These may be grooves left on the surface by tools or marks indicative of the execution technique used by the artist.</rdfs:comment>
    <rdfs:subClassOf rdf:resource="http://www.cidoc-crm.org/cidoc-crm/E25_Human-Made_Feature"/>
    <rdf:type rdf:resource="http://www.w3.org/2002/07/owl#Class"/>
  </rdf:Description>
  <rdf:Description rdf:about="https://w3id.org/crmrp#c_07895c25">
    <rdfs:label xml:lang="en">Engraving</rdfs:label>
    <skos:topConceptOf rdf:resource="https://w3id.org/crmrp#Execution_Technique"/>
    <rdf:type rdf:resource="http://www.w3.org/2002/07/owl#NamedIndividual"/>
    <skos:editorialNote xml:lang="en">Getty AAT http://vocab.getty.edu/page/aat/300053829</skos:editorialNote>
    <skos:broader rdf:resource="https://w3id.org/crmrp#c_757ed6ec"/>
    <skos:prefLabel xml:lang="it">Bulinatura</skos:prefLabel>
    <skos:closeMatch rdf:resource="http://vocab.getty.edu/page/aat/300053829"/>
    <skos:inScheme rdf:resource="https://w3id.org/crmrp#Execution_Technique"/>
    <skos:prefLabel xml:lang="en">Engraving</skos:prefLabel>
    <rdf:type rdf:resource="http://www.w3.org/2004/02/skos/core#Concept"/>
    <skos:definition xml:lang="en">Creating marks on the surface of a hard material, such as metal or glass, by incising with a sharp tool, when the designs or images created are for their own sake and not to be printed from.</skos:definition>
  </rdf:Description>
  <rdf:Description rdf:about="https://w3id.org/crmrp#c_01bba8b4">
    <rdfs:label xml:lang="en">Opus vermiculatum</rdfs:label>
    <skos:editorialNote xml:lang="en">C. Fiori “Teoria e tecniche per la conservazione del mosaico”, Il Prato, Padova, 2002</skos:editorialNote>
    <rdf:type rdf:resource="http://www.w3.org/2002/07/owl#NamedIndividual"/>
    <skos:inScheme rdf:resource="https://w3id.org/crmrp#Execution_Technique"/>
    <skos:prefLabel xml:lang="it">Opus vermiculatum</skos:prefLabel>
    <skos:prefLabel xml:lang="en">Opus vermiculatum</skos:prefLabel>
    <skos:broader rdf:resource="https://w3id.org/crmrp#c_b9a6a1c8"/>
    <skos:topConceptOf rdf:resource="https://w3id.org/crmrp#Execution_Technique"/>
    <skos:editorialNote xml:lang="en">Getty Conservation Institute “Illustrated Glossary - Technician Training for the Maintenance of In Situ Mosaics”, Los Angeles, 2013</skos:editorialNote>
    <rdf:type rdf:resource="http://www.w3.org/2004/02/skos/core#Concept"/>
    <skos:definition xml:lang="en">Type of opus tessellatum made of tesserae of very small dimensions (generally less than 4 mm wide). A small mosaic panel (usually less than a square meter) made in opus vermiculatum and inserted in a mosaic pavement (or sometimes on a vertical surface) is called an emblema. It is generally made separately on a stone slab or large ceramic tile in a workshop prior to the making of the mosaic into which it is inserted. This type of mosaic was also made as a portable work of art, independent from any building.</skos:definition>
  </rdf:Description>
  <rdf:Description rdf:about="http://www.w3.org/2004/02/skos/core#editorialNote">
    <rdfs:subPropertyOf rdf:resource="http://www.w3.org/2000/01/rdf-schema#label"/>
    <rdf:type rdf:resource="http://www.w3.org/2002/07/owl#AnnotationProperty"/>
  </rdf:Description>
  <rdf:Description rdf:about="http://www.cidoc-crm.org/cidoc-crm/P39i_was_measured_by">
    <rdfs:range rdf:resource="https://w3id.org/crmrp#R12_Invasive_archaeometric_and_diagnostic_analysis"/>
    <rdfs:range rdf:resource="https://w3id.org/crmrp#R11_Non-invasive_archaeometric_and_diagnostic_analysis"/>
    <rdfs:domain rdf:resource="https://w3id.org/crmrp#R1_Restoration_Object"/>
    <rdfs:domain rdf:resource="http://www.cidoc-crm.org/extensions/crmsci/S18_Alteration"/>
  </rdf:Description>
  <rdf:Description rdf:about="https://w3id.org/crmrp#c_c5481024">
    <skos:prefLabel xml:lang="en">Ultraviolet-visible spectroscopy</skos:prefLabel>
    <skos:definition xml:lang="en">The study of emission and absorption spectra via absorption spectroscopy or reflectance spectroscopy over wavelengths in the ultraviolet and visible region of the electromagnetic spectrum</skos:definition>
    <skos:prefLabel xml:lang="it">Spettrofotometria UV/Visibile</skos:prefLabel>
    <skos:closeMatch rdf:resource="http://vocab.getty.edu/page/aat/300375717"/>
    <skos:inScheme rdf:resource="https://w3id.org/crmrp#Archeometric_and_Diagnostic_Analysis"/>
    <skos:editorialNote xml:lang="en">Getty AAT http://vocab.getty.edu/page/aat/300375717</skos:editorialNote>
    <skos:broader rdf:resource="https://w3id.org/crmrp#c_789c3e32"/>
    <skos:topConceptOf rdf:resource="https://w3id.org/crmrp#Archeometric_and_Diagnostic_Analysis"/>
    <rdf:type rdf:resource="http://www.w3.org/2004/02/skos/core#Concept"/>
    <rdfs:label xml:lang="en">Ultraviolet-visible spectroscopy </rdfs:label>
    <rdf:type rdf:resource="http://www.w3.org/2002/07/owl#NamedIndividual"/>
  </rdf:Description>
  <rdf:Description rdf:about="http://www.w3.org/2004/02/skos/core#ConceptScheme">
    <rdf:type rdf:resource="http://www.w3.org/2002/07/owl#Class"/>
  </rdf:Description>
  <rdf:Description rdf:about="https://w3id.org/crmrp#c_93c50ee0">
    <skos:definition xml:lang="en">Alloy of copper and zinc, usually with copper as the major alloying element and zinc up to 40% by weight.</skos:definition>
    <skos:editorialNote xml:lang="en">Getty AAT http://vocab.getty.edu/page/aat/300010946</skos:editorialNote>
    <rdfs:label xml:lang="en">Brass</rdfs:label>
    <skos:closeMatch rdf:resource="http://vocab.getty.edu/page/aat/300010946"/>
    <skos:prefLabel xml:lang="en">Brass</skos:prefLabel>
    <skos:inScheme rdf:resource="https://w3id.org/crmrp#Material"/>
    <rdf:type rdf:resource="http://www.w3.org/2004/02/skos/core#Concept"/>
    <skos:broader rdf:resource="https://w3id.org/crmrp#c_6407466f"/>
    <skos:topConceptOf rdf:resource="https://w3id.org/crmrp#Material"/>
    <skos:prefLabel xml:lang="it">Ottone</skos:prefLabel>
    <rdf:type rdf:resource="http://www.w3.org/2002/07/owl#NamedIndividual"/>
  </rdf:Description>
  <rdf:Description rdf:about="https://w3id.org/crmrp#c_3edabaad">
    <skos:topConceptOf rdf:resource="https://w3id.org/crmrp#Execution_Technique"/>
    <rdf:type rdf:resource="http://www.w3.org/2004/02/skos/core#Concept"/>
    <skos:broader rdf:resource="https://w3id.org/crmrp#c_757ed6ec"/>
    <skos:prefLabel xml:lang="en">Polishing</skos:prefLabel>
    <skos:definition xml:lang="en">Process of rubbing a surface to make it smooth or shiny.</skos:definition>
    <skos:prefLabel xml:lang="it">Brunitura</skos:prefLabel>
    <skos:editorialNote xml:lang="en">Getty AAT http://vocab.getty.edu/page/aat/300053867</skos:editorialNote>
    <skos:exactMatch rdf:resource="http://vocab.getty.edu/page/aat/300053867"/>
    <skos:inScheme rdf:resource="https://w3id.org/crmrp#Execution_Technique"/>
    <rdf:type rdf:resource="http://www.w3.org/2002/07/owl#NamedIndividual"/>
    <rdfs:label xml:lang="en">Polishing</rdfs:label>
  </rdf:Description>
  <rdf:Description rdf:about="https://w3id.org/crmrp#c_18db1b80">
    <rdf:type rdf:resource="http://www.w3.org/2004/02/skos/core#Concept"/>
    <skos:definition xml:lang="en">The lacuna is reintegrated with short parallel lines in pure colours on a light background, which follow the shapes and contours of the original alongside them.</skos:definition>
    <skos:editorialNote xml:lang="en">A. Weyer et al., “EwaGlos - European Illustrated Glossary of conservation terms for wall paintings and architectural surfaces”, Michael Imhof Verlag, Petersberg, Germany</skos:editorialNote>
    <skos:broader rdf:resource="https://w3id.org/crmrp#c_326da7e4"/>
    <skos:inScheme rdf:resource="https://w3id.org/crmrp#Intervention"/>
    <rdf:type rdf:resource="http://www.w3.org/2002/07/owl#NamedIndividual"/>
    <rdfs:label xml:lang="en">Selezione cromatica</rdfs:label>
    <skos:topConceptOf rdf:resource="https://w3id.org/crmrp#Intervention"/>
    <skos:prefLabel xml:lang="en">Selezione cromatica</skos:prefLabel>
    <skos:prefLabel xml:lang="it">Selezione cromatica</skos:prefLabel>
  </rdf:Description>
  <rdf:Description rdf:about="https://w3id.org/crmrp#c_f8c1b2e8">
    <rdf:type rdf:resource="http://www.w3.org/2002/07/owl#NamedIndividual"/>
    <skos:closeMatch rdf:resource="http://vocab.getty.edu/page/aat/300400799"/>
    <skos:editorialNote xml:lang="en">Getty Conservation Institute “Illustrated Glossary - Definitions of terms used for the graphic documentation of in situ floor mosaics”, “Mosaics In Situ Project”, Los Angeles, 2003</skos:editorialNote>
    <skos:inScheme rdf:resource="https://w3id.org/crmrp#Alteration"/>
    <skos:altLabel xml:lang="it">Ammaccatura</skos:altLabel>
    <skos:broader rdf:resource="https://w3id.org/crmrp#c_13f3ce9e"/>
    <rdf:type rdf:resource="http://www.w3.org/2004/02/skos/core#Concept"/>
    <skos:altLabel xml:lang="en">Dent</skos:altLabel>
    <skos:topConceptOf rdf:resource="https://w3id.org/crmrp#Alteration"/>
    <skos:editorialNote xml:lang="en">Getty AAT http://vocab.getty.edu/page/aat/300400799</skos:editorialNote>
    <skos:definition xml:lang="en">Local hollow. A depression can occur with or without a loss of material</skos:definition>
    <skos:prefLabel xml:lang="it">Avvallamento</skos:prefLabel>
    <skos:editorialNote xml:lang="en">Uni Cen/Ts 17135:2021 - Conservation of cultural heritage. General terms and definitions</skos:editorialNote>
    <skos:prefLabel xml:lang="en">Depression</skos:prefLabel>
    <rdfs:label xml:lang="en">Depression</rdfs:label>
  </rdf:Description>
  <rdf:Description rdf:about="https://w3id.org/crmrp#c_931e5c94">
    <skos:editorialNote xml:lang="en">Getty AAT http://vocab.getty.edu/page/aat/300229535</skos:editorialNote>
    <skos:editorialNote xml:lang="it">UNI EN 15898:2019 Conservazione del patrimonio culturale - Termini generali e definizioni</skos:editorialNote>
    <skos:definition xml:lang="en">Collection and evaluation of data on an object, a collection of objects or collection and/or their environment over time.</skos:definition>
    <rdfs:label xml:lang="en">Monitoring</rdfs:label>
    <skos:editorialNote xml:lang="en">A. Weyer et al., “EwaGlos - European Illustrated Glossary of conservation terms for wall paintings and architectural surfaces”, Michael Imhof Verlag, Petersberg, Germany</skos:editorialNote>
    <skos:prefLabel xml:lang="it">Monitoraggio ambientale</skos:prefLabel>
    <rdf:type rdf:resource="http://www.w3.org/2002/07/owl#NamedIndividual"/>
    <skos:topConceptOf rdf:resource="https://w3id.org/crmrp#Archeometric_and_Diagnostic_Analysis"/>
    <skos:prefLabel xml:lang="en">Monitoring</skos:prefLabel>
    <skos:note xml:lang="en">The preferred editorial note and the definition closest to the meaning is UNI EN 15898:2019</skos:note>
    <skos:altLabel xml:lang="en">Environmental control</skos:altLabel>
    <skos:inScheme rdf:resource="https://w3id.org/crmrp#Archeometric_and_Diagnostic_Analysis"/>
    <rdf:type rdf:resource="http://www.w3.org/2004/02/skos/core#Concept"/>
    <skos:broader rdf:resource="https://w3id.org/crmrp#c_1fd6102e"/>
  </rdf:Description>
  <rdf:Description rdf:about="https://w3id.org/crmrp#c_f28c35d1">
    <skos:prefLabel xml:lang="en">Sculpture in the round</skos:prefLabel>
    <skos:editorialNote xml:lang="en">Getty AAT http://vocab.getty.edu/page/aat/300047264</skos:editorialNote>
    <skos:inScheme rdf:resource="https://w3id.org/crmrp#Restoration_Object"/>
    <skos:closeMatch rdf:resource="http://vocab.getty.edu/page/aat/300047264"/>
    <rdf:type rdf:resource="http://www.w3.org/2004/02/skos/core#Concept"/>
    <skos:topConceptOf rdf:resource="https://w3id.org/crmrp#Restoration_Object"/>
    <skos:prefLabel xml:lang="it">Tuttotondo</skos:prefLabel>
    <rdf:type rdf:resource="http://www.w3.org/2002/07/owl#NamedIndividual"/>
    <skos:definition xml:lang="en">Sculpture in which forms are carved or modeled about their full circumference, as opposed to having forms projecting from or sunk into a continuous surface.</skos:definition>
    <skos:broader rdf:resource="https://w3id.org/crmrp#c_160c713a"/>
    <rdfs:label xml:lang="en">Sculpture in the round</rdfs:label>
  </rdf:Description>
  <rdf:Description rdf:about="https://w3id.org/crmrp#c_380df6b8">
    <skos:broader rdf:resource="https://w3id.org/crmrp#c_5b7fce15"/>
    <skos:inScheme rdf:resource="https://w3id.org/crmrp#Documentation"/>
    <skos:prefLabel xml:lang="it">Relazione tecnico-scientifica</skos:prefLabel>
    <skos:topConceptOf rdf:resource="https://w3id.org/crmrp#Documentation"/>
    <rdf:type rdf:resource="http://www.w3.org/2002/07/owl#NamedIndividual"/>
    <rdf:type rdf:resource="http://www.w3.org/2004/02/skos/core#Concept"/>
    <skos:definition xml:lang="en">A document which gives brief information concerning the history of the building, the wall painting, conservation and past restoration campaigns and results arising from tests and scientific studies, as well as environmental aspects, mapping, building and site surveys etc.</skos:definition>
    <skos:editorialNote xml:lang="en">A. Weyer et al., “EwaGlos - European Illustrated Glossary of conservation terms for wall paintings and architectural surfaces”, Michael Imhof Verlag, Petersberg, Germany</skos:editorialNote>
    <skos:prefLabel xml:lang="en">Conservation report</skos:prefLabel>
    <rdfs:label xml:lang="en">Conservation report</rdfs:label>
  </rdf:Description>
  <rdf:Description rdf:about="https://w3id.org/crmrp#c_5885a25d">
    <skos:topConceptOf rdf:resource="https://w3id.org/crmrp#Alteration"/>
    <rdfs:label xml:lang="en">Deposit</rdfs:label>
    <skos:editorialNote xml:lang="en">Verg`es-Belmin et al., ICOMOS-ISCS: Illustrated glossary on stone deterioration patterns, vol. XV. Icomos International Council on Monuments and Sites, 2008</skos:editorialNote>
    <skos:editorialNote xml:lang="en">Getty Conservation Institute “Illustrated Glossary - Definitions of terms used for the graphic documentation of in situ floor mosaics”, “Mosaics In Situ Project”, Los Angeles, 2003</skos:editorialNote>
    <skos:editorialNote xml:lang="en">Getty AAT http://vocab.getty.edu/page/aat/300264846</skos:editorialNote>
    <skos:definition xml:lang="en">Exogenic substance on the surface of an object.</skos:definition>
    <rdf:type rdf:resource="http://www.w3.org/2002/07/owl#NamedIndividual"/>
    <skos:editorialNote xml:lang="en">Uni Cen/Ts 17135:2021 - Conservation of cultural heritage. General terms and definitions</skos:editorialNote>
    <skos:note xml:lang="en">The preferred editorial note and the definition closest to the meaning is Uni Cen/Ts 17135:2021</skos:note>
    <skos:prefLabel xml:lang="en">Deposit</skos:prefLabel>
    <skos:closeMatch rdf:resource="http://vocab.getty.edu/page/aat/300264846"/>
    <skos:inScheme rdf:resource="https://w3id.org/crmrp#Alteration"/>
    <rdf:type rdf:resource="http://www.w3.org/2004/02/skos/core#Concept"/>
    <skos:prefLabel xml:lang="it">Deposito superficiale</skos:prefLabel>
  </rdf:Description>
  <rdf:Description rdf:about="https://w3id.org/crmrp#R9_Altered_Area">
    <rdfs:label xml:lang="en">Altered Area</rdfs:label>
    <rdfs:comment xml:lang="en">This class indicates the area altered by an alteration event or an intervention.
It is useful to know where an alteration form is found on an artwork because this fact can help restorers to understand the cause of the alteration or the way to resolve it and, moreover, to prevent it in the future.</rdfs:comment>
    <rdfs:subClassOf rdf:resource="http://www.cidoc-crm.org/extensions/crmdig/D35_Area"/>
    <rdf:type rdf:resource="http://www.w3.org/2002/07/owl#Class"/>
  </rdf:Description>
  <rdf:Description rdf:about="https://w3id.org/crmrp#c_2ff31b40">
    <skos:editorialNote xml:lang="en">Getty Conservation Institute “Illustrated Glossary - Technician Training for the Maintenance of In Situ Mosaics”, Los Angeles, 2013</skos:editorialNote>
    <skos:editorialNote xml:lang="it">C. Fiori “Teoria e tecniche per la conservazione del mosaico”, Il Prato, Padova, 2002</skos:editorialNote>
    <skos:prefLabel xml:lang="it">Opus segmentatum</skos:prefLabel>
    <skos:prefLabel xml:lang="en">Opus segmentatum</skos:prefLabel>
    <skos:inScheme rdf:resource="https://w3id.org/crmrp#Execution_Technique"/>
    <rdf:type rdf:resource="http://www.w3.org/2004/02/skos/core#Concept"/>
    <skos:broader rdf:resource="https://w3id.org/crmrp#c_b9a6a1c8"/>
    <rdfs:label xml:lang="en">Opus segmentatum</rdfs:label>
    <rdf:type rdf:resource="http://www.w3.org/2002/07/owl#NamedIndividual"/>
    <skos:topConceptOf rdf:resource="https://w3id.org/crmrp#Execution_Technique"/>
    <skos:definition xml:lang="en">Pavement made of stone slab fragments, most commonly marble, of different colors, cut in irregular shapes and placed side by side without creating any geometric or figurative motif.</skos:definition>
  </rdf:Description>
  <rdf:Description rdf:about="http://www.w3.org/2004/02/skos/core#note">
    <rdf:type rdf:resource="http://www.w3.org/2002/07/owl#AnnotationProperty"/>
  </rdf:Description>
  <rdf:Description rdf:about="https://w3id.org/crmrp#c_ffb2bf28">
    <skos:definition xml:lang="en">Refers to procedures and techniques which determine range of sizes or mean or average size of particles in a granular or powder sample.</skos:definition>
    <skos:editorialNote xml:lang="en">Getty AAT http://vocab.getty.edu/page/aat/300379895</skos:editorialNote>
    <skos:inScheme rdf:resource="https://w3id.org/crmrp#Archeometric_and_Diagnostic_Analysis"/>
    <skos:exactMatch rdf:resource="http://vocab.getty.edu/page/aat/30037989"/>
    <skos:prefLabel xml:lang="en">Particle size analysis</skos:prefLabel>
    <rdf:type rdf:resource="http://www.w3.org/2002/07/owl#NamedIndividual"/>
    <skos:prefLabel xml:lang="it">Analisi granulometrica</skos:prefLabel>
    <skos:broader rdf:resource="https://w3id.org/crmrp#c_abed88a5"/>
    <skos:topConceptOf rdf:resource="https://w3id.org/crmrp#Archeometric_and_Diagnostic_Analysis"/>
    <rdfs:label xml:lang="en">Particle size analysis</rdfs:label>
    <rdf:type rdf:resource="http://www.w3.org/2004/02/skos/core#Concept"/>
  </rdf:Description>
  <rdf:Description rdf:about="https://w3id.org/crmrp#c_249b3e7c">
    <skos:editorialNote xml:lang="en">Getty AAT http://vocab.getty.edu/page/aat/300037680</skos:editorialNote>
    <skos:prefLabel xml:lang="it">Arredo</skos:prefLabel>
    <skos:broader rdf:resource="https://w3id.org/crmrp#Restoration_Object"/>
    <rdfs:label xml:lang="en">Furniture</rdfs:label>
    <skos:definition xml:lang="en">Movable or fixed objects or equipment, which may be either functional or ornamental, particularly objects for sitting, reclining, or storage, such as chairs, beds, tables, cabinets, etc., in a dwelling, business, or public space.</skos:definition>
    <skos:exactMatch rdf:resource="http://vocab.getty.edu/page/aat/300037680"/>
    <skos:inScheme rdf:resource="https://w3id.org/crmrp#Restoration_Object"/>
    <skos:topConceptOf rdf:resource="https://w3id.org/crmrp#Restoration_Object"/>
    <skos:prefLabel xml:lang="en">Furniture</skos:prefLabel>
    <rdf:type rdf:resource="http://www.w3.org/2004/02/skos/core#Concept"/>
    <rdf:type rdf:resource="http://www.w3.org/2002/07/owl#NamedIndividual"/>
  </rdf:Description>
  <rdf:Description rdf:about="https://w3id.org/crmrp#c_33b4c491">
    <rdf:type rdf:resource="http://www.w3.org/2002/07/owl#NamedIndividual"/>
    <skos:editorialNote xml:lang="en">Uni Cen/Ts 17135:2021 - Conservation of cultural heritage. General terms and definitions</skos:editorialNote>
    <skos:topConceptOf rdf:resource="https://w3id.org/crmrp#Alteration"/>
    <skos:note xml:lang="en">The preferred editorial note and the definition closest to the meaning is Uni Cen/Ts 17135:2021</skos:note>
    <skos:inScheme rdf:resource="https://w3id.org/crmrp#Alteration"/>
    <skos:prefLabel xml:lang="it">Ristringimento</skos:prefLabel>
    <skos:prefLabel xml:lang="en">Shrinkage</skos:prefLabel>
    <skos:broader rdf:resource="https://w3id.org/crmrp#c_13f3ce9e"/>
    <rdfs:label xml:lang="en">Shrinkage</rdfs:label>
    <rdf:type rdf:resource="http://www.w3.org/2004/02/skos/core#Concept"/>
    <skos:editorialNote xml:lang="en">Getty AAT http://vocab.getty.edu/page/aat/300054120</skos:editorialNote>
    <skos:exactMatch rdf:resource="http://vocab.getty.edu/page/aat/300054120"/>
    <skos:definition xml:lang="en">Decrease in dimensions.</skos:definition>
  </rdf:Description>
  <rdf:Description rdf:about="https://w3id.org/crmrp#c_602dbf50">
    <skos:definition xml:lang="en">Pavement made of small, regularly shaped, usually quadrangular, elements (generally 4 to 20 millimetres wide) placed side by side in rows. These elements, called tesserae, are obtained by cutting different materials such as stone (often marble or limestone), ceramic or glass.</skos:definition>
    <rdf:type rdf:resource="http://www.w3.org/2002/07/owl#NamedIndividual"/>
    <skos:broader rdf:resource="https://w3id.org/crmrp#c_b9a6a1c8"/>
    <rdf:type rdf:resource="http://www.w3.org/2004/02/skos/core#Concept"/>
    <skos:editorialNote xml:lang="en">Getty Conservation Institute “Illustrated Glossary - Technician Training for the Maintenance of In Situ Mosaics”, Los Angeles, 2013</skos:editorialNote>
    <rdfs:label xml:lang="en">Opus tessellatum</rdfs:label>
    <skos:editorialNote xml:lang="it">C. Giannini, “Dizionario del restauro - Tecniche diagnostica conservazione”, Nardini Editore, Firenze, 2010</skos:editorialNote>
    <skos:editorialNote xml:lang="it">C. Fiori “Teoria e tecniche per la conservazione del mosaico”, Il Prato, Padova, 2002</skos:editorialNote>
    <skos:inScheme rdf:resource="https://w3id.org/crmrp#Execution_Technique"/>
    <skos:topConceptOf rdf:resource="https://w3id.org/crmrp#Execution_Technique"/>
    <skos:prefLabel xml:lang="it">Opus tessellatum</skos:prefLabel>
    <skos:prefLabel xml:lang="en">Opus tessellatum</skos:prefLabel>
  </rdf:Description>
  <rdf:Description rdf:about="https://w3id.org/crmrp#c_6d7b8feb">
    <skos:broader rdf:resource="https://w3id.org/crmrp#c_49988b8d"/>
    <skos:prefLabel xml:lang="en">Active xylophagous attack</skos:prefLabel>
    <skos:topConceptOf rdf:resource="https://w3id.org/crmrp#Alteration"/>
    <skos:definition xml:lang="en">A xylophagus attack still in progress</skos:definition>
    <rdf:type rdf:resource="http://www.w3.org/2002/07/owl#NamedIndividual"/>
    <rdfs:label xml:lang="en">Active xylophagous attack</rdfs:label>
    <skos:inScheme rdf:resource="https://w3id.org/crmrp#Alteration"/>
    <skos:prefLabel xml:lang="it">Attacco xilofago attivo</skos:prefLabel>
    <rdf:type rdf:resource="http://www.w3.org/2004/02/skos/core#Concept"/>
    <skos:note xml:lang="en">International references could not be found</skos:note>
  </rdf:Description>
  <rdf:Description rdf:about="https://w3id.org/crmrp#RP2_targets">
    <rdfs:label xml:lang="en">targets</rdfs:label>
    <rdfs:range rdf:resource="https://w3id.org/crmrp#R9_Altered_Area"/>
    <rdfs:domain rdf:resource="https://w3id.org/crmrp#R8_Intervention"/>
    <rdfs:domain rdf:resource="http://www.cidoc-crm.org/extensions/crmsci/S18_Alteration"/>
    <rdf:type rdf:resource="http://www.w3.org/2002/07/owl#ObjectProperty"/>
  </rdf:Description>
  <rdf:Description rdf:about="https://w3id.org/crmrp#RP6_is_pre-intervention">
    <rdfs:label xml:lang="en">is pre-intervention</rdfs:label>
    <rdfs:comment xml:lang="en">This property links Invasive archaeometric and diagnostic analysis and Non-invasive achaeometric and diagnostic analysis to Intervention.
Indeed, some archaeometric and diagnostic analyses are sometimes repeated before and after specific interventions.</rdfs:comment>
    <rdfs:range rdf:resource="https://w3id.org/crmrp#R8_Intervention"/>
    <rdfs:domain rdf:resource="https://w3id.org/crmrp#R12_Invasive_archaeometric_and_diagnostic_analysis"/>
    <rdfs:domain rdf:resource="https://w3id.org/crmrp#R11_Non-invasive_archaeometric_and_diagnostic_analysis"/>
    <rdf:type rdf:resource="http://www.w3.org/2002/07/owl#ObjectProperty"/>
  </rdf:Description>
  <rdf:Description rdf:about="https://w3id.org/crmrp#c_ea4ef6cd">
    <skos:topConceptOf rdf:resource="https://w3id.org/crmrp#Alteration"/>
    <skos:broader rdf:resource="https://w3id.org/crmrp#c_13f3ce9e"/>
    <skos:definition xml:lang="en">A type of deformation of the wooden support of paintings that manifests itself in the sickle-like curvature of the boards.</skos:definition>
    <skos:prefLabel xml:lang="it">Falcatura</skos:prefLabel>
    <rdf:type rdf:resource="http://www.w3.org/2002/07/owl#NamedIndividual"/>
    <rdfs:label xml:lang="en">Sickle-shaped deformation</rdfs:label>
    <skos:prefLabel xml:lang="en">Sickle-shaped deformation</skos:prefLabel>
    <skos:inScheme rdf:resource="https://w3id.org/crmrp#Alteration"/>
    <skos:note xml:lang="en">International references could not be found</skos:note>
    <rdf:type rdf:resource="http://www.w3.org/2004/02/skos/core#Concept"/>
    <skos:editorialNote xml:lang="it">C. Giannini, “Dizionario del restauro - Tecniche diagnostica conservazione”, Nardini Editore, Firenze, 2010</skos:editorialNote>
  </rdf:Description>
  <rdf:Description rdf:about="https://w3id.org/crmrp#c_e5f8a87b">
    <skos:editorialNote xml:lang="en">Getty AAT http://vocab.getty.edu/page/aat/300393228</skos:editorialNote>
    <skos:inScheme rdf:resource="https://w3id.org/crmrp#Archeometric_and_Diagnostic_Analysis"/>
    <skos:broader rdf:resource="https://w3id.org/crmrp#c_abed88a5"/>
    <rdfs:label xml:lang="en">Thermogravimetry</rdfs:label>
    <skos:exactMatch rdf:resource="http://vocab.getty.edu/page/aat/300393228"/>
    <rdf:type rdf:resource="http://www.w3.org/2004/02/skos/core#Concept"/>
    <rdf:type rdf:resource="http://www.w3.org/2002/07/owl#NamedIndividual"/>
    <skos:definition xml:lang="en">A technique that chemically analyzes a substance by measuring changes in its weight due to increasing temperature. It can be used to study the stability of materials.</skos:definition>
    <skos:prefLabel xml:lang="it">Termogravimetria</skos:prefLabel>
    <skos:prefLabel xml:lang="en">Thermogravimetry</skos:prefLabel>
    <skos:topConceptOf rdf:resource="https://w3id.org/crmrp#Archeometric_and_Diagnostic_Analysis"/>
  </rdf:Description>
  <rdf:Description rdf:about="https://w3id.org/crmrp#c_c246124b">
    <skos:prefLabel xml:lang="it">Progetto</skos:prefLabel>
    <skos:prefLabel xml:lang="en">Project</skos:prefLabel>
    <skos:definition xml:lang="en">Conception, mostly accompanied by a study on the possibilities of implementation or execution.</skos:definition>
    <rdfs:label xml:lang="en">Project</rdfs:label>
    <skos:topConceptOf rdf:resource="https://w3id.org/crmrp#Documentation"/>
    <skos:inScheme rdf:resource="https://w3id.org/crmrp#Documentation"/>
    <rdf:type rdf:resource="http://www.w3.org/2002/07/owl#NamedIndividual"/>
    <rdf:type rdf:resource="http://www.w3.org/2004/02/skos/core#Concept"/>
    <skos:note xml:lang="en">International references could not be found</skos:note>
    <skos:broader rdf:resource="https://w3id.org/crmrp#c_5b7fce15"/>
  </rdf:Description>
  <rdf:Description rdf:about="https://w3id.org/crmrp#c_90a8bb69">
    <rdf:type rdf:resource="http://www.w3.org/2004/02/skos/core#Concept"/>
    <rdfs:label xml:lang="en">3D model</rdfs:label>
    <skos:definition xml:lang="en">A 3D model (or three-dimensional model) is a mathematical representation of a three-dimensional object.</skos:definition>
    <skos:broader rdf:resource="https://w3id.org/crmrp#c_f383c4d3"/>
    <skos:inScheme rdf:resource="https://w3id.org/crmrp#Documentation"/>
    <skos:prefLabel xml:lang="en">3D model</skos:prefLabel>
    <skos:note xml:lang="en">International references could not be found</skos:note>
    <rdf:type rdf:resource="http://www.w3.org/2002/07/owl#NamedIndividual"/>
    <skos:prefLabel xml:lang="it">Rilievo 3D</skos:prefLabel>
    <skos:topConceptOf rdf:resource="https://w3id.org/crmrp#Documentation"/>
  </rdf:Description>
  <rdf:Description rdf:about="http://www.w3.org/2004/02/skos/core#Concept">
    <rdf:type rdf:resource="http://www.w3.org/2002/07/owl#Class"/>
  </rdf:Description>
  <rdf:Description rdf:about="https://w3id.org/crmrp#c_5f7995a8">
    <skos:topConceptOf rdf:resource="https://w3id.org/crmrp#Intervention"/>
    <rdf:type rdf:resource="http://www.w3.org/2004/02/skos/core#Concept"/>
    <skos:editorialNote xml:lang="it">C. Giannini, “Dizionario del restauro - Tecniche diagnostica conservazione”, Nardini Editore, Firenze, 2010</skos:editorialNote>
    <skos:prefLabel xml:lang="en">Wedge</skos:prefLabel>
    <skos:definition xml:lang="en">A wooden element used in the restoration of painted or sculpted boards to restore cracks or splits in the support, or to give renewed stability and flatness to bent boards.</skos:definition>
    <skos:note xml:lang="en">International references could not be found</skos:note>
    <skos:prefLabel xml:lang="it">Cuneo</skos:prefLabel>
    <skos:inScheme rdf:resource="https://w3id.org/crmrp#Intervention"/>
    <skos:broader rdf:resource="https://w3id.org/crmrp#c_e8592f3b"/>
    <rdf:type rdf:resource="http://www.w3.org/2002/07/owl#NamedIndividual"/>
    <rdfs:label xml:lang="en">Wedge</rdfs:label>
  </rdf:Description>
  <rdf:Description rdf:about="https://w3id.org/crmrp#c_757ed6ec">
    <rdf:type rdf:resource="http://www.w3.org/2002/07/owl#NamedIndividual"/>
    <skos:prefLabel xml:lang="en">Water gilding</skos:prefLabel>
    <skos:prefLabel xml:lang="it">A guazzo</skos:prefLabel>
    <skos:inScheme rdf:resource="https://w3id.org/crmrp#Execution_Technique"/>
    <skos:definition xml:lang="en">Technique of adhering precious-metal leaf to a gesso or bole ground that is moistened with water before each leaf is laid.</skos:definition>
    <rdf:type rdf:resource="http://www.w3.org/2004/02/skos/core#Concept"/>
    <skos:topConceptOf rdf:resource="https://w3id.org/crmrp#Execution_Technique"/>
    <skos:editorialNote xml:lang="en">Getty AAT http://vocab.getty.edu/page/aat/300053795</skos:editorialNote>
    <rdfs:label xml:lang="en">Water gilding</rdfs:label>
    <skos:closeMatch rdf:resource="http://vocab.getty.edu/page/aat/300053795"/>
    <skos:broader rdf:resource="https://w3id.org/crmrp#c_8af455cd"/>
  </rdf:Description>
  <rdf:Description rdf:about="https://w3id.org/crmrp#c_0a209790">
    <rdf:type rdf:resource="http://www.w3.org/2002/07/owl#NamedIndividual"/>
    <skos:prefLabel xml:lang="it">Vetro</skos:prefLabel>
    <skos:topConceptOf rdf:resource="https://w3id.org/crmrp#Material"/>
    <skos:editorialNote xml:lang="en">Getty AAT http://vocab.getty.edu/page/aat/300010797</skos:editorialNote>
    <rdfs:label xml:lang="en">Glass</rdfs:label>
    <skos:inScheme rdf:resource="https://w3id.org/crmrp#Material"/>
    <skos:definition xml:lang="en">An amorphous, inorganic substance made by fusing silica (silicon dioxide) with a basic oxide; generally transparent but often translucent or opaque. Its characteristic properties are its hardness and rigidity at ordinary temperatures, its capacity for plastic working at elevated temperatures, and its resistance to weathering and to most chemicals except hydrofluoric acid. Used for both utilitarian and decorative purposes, it can be formed into various shapes, colored or decorated. Glass originated as a glaze in Mesopotamia in about 3500 BCE and the first objects made wholly of glass date to about 2500 BCE.</skos:definition>
    <rdf:type rdf:resource="http://www.w3.org/2004/02/skos/core#Concept"/>
    <skos:prefLabel xml:lang="en">Glass</skos:prefLabel>
    <skos:exactMatch rdf:resource="http://vocab.getty.edu/page/aat/300010797"/>
  </rdf:Description>
  <rdf:Description rdf:about="https://w3id.org/crmrp#c_2d5cde83">
    <skos:prefLabel xml:lang="en">Chromatography</skos:prefLabel>
    <skos:broader rdf:resource="https://w3id.org/crmrp#c_abed88a5"/>
    <skos:definition xml:lang="en">The separation of chemical substances by making use of differences in the rates at which the substances travel through or along a stationary medium.</skos:definition>
    <skos:prefLabel xml:lang="it">Cromatografia</skos:prefLabel>
    <skos:topConceptOf rdf:resource="https://w3id.org/crmrp#Archeometric_and_Diagnostic_Analysis"/>
    <skos:closeMatch rdf:resource="http://vocab.getty.edu/page/aat/300214721"/>
    <rdf:type rdf:resource="http://www.w3.org/2002/07/owl#NamedIndividual"/>
    <rdfs:label xml:lang="en">Chromatography</rdfs:label>
    <skos:editorialNote xml:lang="en">Getty AAT http://vocab.getty.edu/page/aat/300214721</skos:editorialNote>
    <rdf:type rdf:resource="http://www.w3.org/2004/02/skos/core#Concept"/>
    <skos:inScheme rdf:resource="https://w3id.org/crmrp#Archeometric_and_Diagnostic_Analysis"/>
  </rdf:Description>
  <rdf:Description rdf:about="http://www.w3.org/2004/02/skos/core#topConceptOf">
    <rdf:type rdf:resource="http://www.w3.org/2002/07/owl#AnnotationProperty"/>
  </rdf:Description>
  <rdf:Description rdf:about="https://w3id.org/crmrp#c_404ba9c8">
    <skos:editorialNote xml:lang="en">Getty AAT http://vocab.getty.edu/page/aat/300191590</skos:editorialNote>
    <skos:broader rdf:resource="https://w3id.org/crmrp#c_3ef20257"/>
    <skos:prefLabel xml:lang="en">Excrement</skos:prefLabel>
    <skos:closeMatch rdf:resource="http://vocab.getty.edu/page/aat/300191590"/>
    <skos:definition xml:lang="en">Waste matter discharged from the body.</skos:definition>
    <skos:prefLabel xml:lang="it">Guano</skos:prefLabel>
    <skos:inScheme rdf:resource="https://w3id.org/crmrp#Alteration"/>
    <skos:topConceptOf rdf:resource="https://w3id.org/crmrp#Alteration"/>
    <rdf:type rdf:resource="http://www.w3.org/2004/02/skos/core#Concept"/>
    <rdfs:label xml:lang="en">Excrement</rdfs:label>
    <rdf:type rdf:resource="http://www.w3.org/2002/07/owl#NamedIndividual"/>
  </rdf:Description>
  <rdf:Description rdf:about="http://www.cidoc-crm.org/cidoc-crm/P2_has_type">
    <rdfs:range rdf:resource="http://www.cidoc-crm.org/cidoc-crm/E55_Type"/>
    <rdfs:domain rdf:resource="https://w3id.org/crmrp#R8_Intervention"/>
    <rdfs:domain rdf:resource="https://w3id.org/crmrp#R5_Source_and_Document"/>
    <rdfs:domain rdf:resource="https://w3id.org/crmrp#R1_Restoration_Object"/>
    <rdfs:domain rdf:resource="https://w3id.org/crmrp#R12_Invasive_archaeometric_and_diagnostic_analysis"/>
    <rdfs:domain rdf:resource="https://w3id.org/crmrp#R11_Non-invasive_archaeometric_and_diagnostic_analysis"/>
    <rdfs:domain rdf:resource="https://w3id.org/crmrp#R10_Sign_of_Workmanship"/>
    <rdfs:domain rdf:resource="http://www.cidoc-crm.org/extensions/crmsci/S18_Alteration"/>
    <rdfs:domain rdf:resource="http://www.cidoc-crm.org/cidoc-crm/R13_Execution_Technique"/>
  </rdf:Description>
  <rdf:Description rdf:about="https://w3id.org/crmrp#c_d5d25610">
    <skos:editorialNote xml:lang="it">C. Giannini, “Dizionario del restauro - Tecniche diagnostica conservazione”, Nardini Editore, Firenze, 2010</skos:editorialNote>
    <skos:note xml:lang="en">International references could not be found, but the preferred editorial note and the definition closest to the meaning is Effetti d’oro - Storia e tecnica della doratura nell’arte</skos:note>
    <skos:prefLabel xml:lang="it">Pastiglia</skos:prefLabel>
    <rdf:type rdf:resource="http://www.w3.org/2004/02/skos/core#Concept"/>
    <rdf:type rdf:resource="http://www.w3.org/2002/07/owl#NamedIndividual"/>
    <skos:editorialNote xml:lang="it">G. Pignolo, “Effetti d’oro - Storia e tecnica della doratura nell’arte”, Editrice Compositori, Bologna, 2002</skos:editorialNote>
    <rdfs:label xml:lang="en">Pastille gilding</rdfs:label>
    <skos:inScheme rdf:resource="https://w3id.org/crmrp#Execution_Technique"/>
    <skos:definition xml:lang="en">A technique used by ancient decorators to reproduce friezes and high reliefs on different supports. The mixture consists of plaster, scagliola and starch glue.</skos:definition>
    <skos:prefLabel xml:lang="en">Pastille gilding</skos:prefLabel>
    <skos:topConceptOf rdf:resource="https://w3id.org/crmrp#Execution_Technique"/>
    <skos:broader rdf:resource="https://w3id.org/crmrp#c_757ed6ec"/>
  </rdf:Description>
  <rdf:Description rdf:about="https://w3id.org/crmrp#c_1b678edf">
    <skos:prefLabel xml:lang="it">Erosione</skos:prefLabel>
    <skos:exactMatch rdf:resource="http://vocab.getty.edu/page/aat/300054116"/>
    <skos:altLabel xml:lang="en">Eroded</skos:altLabel>
    <skos:inScheme rdf:resource="https://w3id.org/crmrp#Alteration"/>
    <skos:editorialNote xml:lang="en">Getty AAT http://vocab.getty.edu/page/aat/300054116</skos:editorialNote>
    <rdfs:label xml:lang="en">Erosion</rdfs:label>
    <skos:editorialNote xml:lang="en">Uni Cen/Ts 17135:2021 - Conservation of cultural heritage. General terms and definitions</skos:editorialNote>
    <rdf:type rdf:resource="http://www.w3.org/2002/07/owl#NamedIndividual"/>
    <skos:editorialNote xml:lang="en">Getty Conservation Institute “Illustrated Glossary - Definitions of terms used for the graphic documentation of in situ floor mosaics”, “Mosaics In Situ Project”, Los Angeles, 2003</skos:editorialNote>
    <rdf:type rdf:resource="http://www.w3.org/2004/02/skos/core#Concept"/>
    <skos:note xml:lang="en">The preferred editorial note and the closest definition to the meaning is Uni Cen/Ts 17135:2021</skos:note>
    <skos:definition xml:lang="en">Gradual loss of surface material due to external factors.</skos:definition>
    <skos:prefLabel xml:lang="en">Erosion</skos:prefLabel>
    <skos:editorialNote xml:lang="en">Verg`es-Belmin et al., ICOMOS-ISCS: Illustrated glossary on stone deterioration patterns, vol. XV. Icomos International Council on Monuments and Sites, 2008</skos:editorialNote>
    <skos:topConceptOf rdf:resource="https://w3id.org/crmrp#Alteration"/>
  </rdf:Description>
  <rdf:Description rdf:about="https://w3id.org/crmrp#c_f4805ff2">
    <skos:inScheme rdf:resource="https://w3id.org/crmrp#Execution_Technique"/>
    <skos:broader rdf:resource="https://w3id.org/crmrp#c_044b6056"/>
    <rdf:type rdf:resource="http://www.w3.org/2004/02/skos/core#Concept"/>
    <skos:prefLabel xml:lang="en">Ink</skos:prefLabel>
    <skos:editorialNote xml:lang="en">Getty AAT http://vocab.getty.edu/page/aat/300015012</skos:editorialNote>
    <skos:prefLabel xml:lang="it">Inchiostro</skos:prefLabel>
    <rdf:type rdf:resource="http://www.w3.org/2002/07/owl#NamedIndividual"/>
    <skos:topConceptOf rdf:resource="https://w3id.org/crmrp#Execution_Technique"/>
    <rdfs:label xml:lang="en">Ink</rdfs:label>
    <skos:definition xml:lang="en">A fluid medium used for drawings or tracings. An opaque, usually black, pigment is mixed with a vehicle such as water to produce a fluid which can be applied with a pen or brush. Through the end of the 19th century, ink was supplied dried in stick or block form which was ground and mixed with water as needed. At the beginning of this century prepared ink became popular.</skos:definition>
    <skos:closeMatch rdf:resource="http://vocab.getty.edu/page/aat/300015012"/>
  </rdf:Description>
  <rdf:Description rdf:about="https://w3id.org/crmrp#c_b7ff54f8">
    <skos:definition xml:lang="en">Any material, usually liquid, having the power of dissolving another material.</skos:definition>
    <rdfs:label xml:lang="en">Solvent</rdfs:label>
    <skos:topConceptOf rdf:resource="https://w3id.org/crmrp#Intervention"/>
    <rdf:type rdf:resource="http://www.w3.org/2004/02/skos/core#Concept"/>
    <skos:broader rdf:resource="https://w3id.org/crmrp#c_607d4549"/>
    <skos:prefLabel xml:lang="en">Solvent</skos:prefLabel>
    <rdf:type rdf:resource="http://www.w3.org/2002/07/owl#NamedIndividual"/>
    <skos:exactMatch rdf:resource="http://vocab.getty.edu/page/aat/300015217"/>
    <skos:editorialNote xml:lang="en">Getty AAT http://vocab.getty.edu/page/aat/300015217</skos:editorialNote>
    <skos:inScheme rdf:resource="https://w3id.org/crmrp#Intervention"/>
  </rdf:Description>
  <rdf:Description rdf:about="https://w3id.org/crmrp#c_73b09074">
    <rdfs:label xml:lang="en">Stripe soiling</rdfs:label>
    <rdf:type rdf:resource="http://www.w3.org/2004/02/skos/core#Concept"/>
    <skos:note xml:lang="en">The preferred editorial note and the definition closest to the meaning is ICOMOS-ISCS: Illustrated glossary on stone deterioration patterns</skos:note>
    <skos:definition xml:lang="en">Deposit of a very thin layer of exogenous particles (eg. soot) giving a dirty appearance to the stone surface.</skos:definition>
    <skos:prefLabel xml:lang="it">Colatura</skos:prefLabel>
    <skos:editorialNote xml:lang="en">Getty AAT http://vocab.getty.edu/page/aat/300379469</skos:editorialNote>
    <skos:editorialNote xml:lang="en">Verg`es-Belmin et al., ICOMOS-ISCS: Illustrated glossary on stone deterioration patterns, vol. XV. Icomos International Council on Monuments and Sites, 2008</skos:editorialNote>
    <rdf:type rdf:resource="http://www.w3.org/2002/07/owl#NamedIndividual"/>
    <skos:prefLabel xml:lang="en">Stripe soiling</skos:prefLabel>
    <skos:topConceptOf rdf:resource="https://w3id.org/crmrp#Alteration"/>
    <skos:altLabel xml:lang="en">Soiling</skos:altLabel>
    <skos:closeMatch rdf:resource="http://vocab.getty.edu/page/aat/300379469"/>
    <skos:inScheme rdf:resource="https://w3id.org/crmrp#Alteration"/>
  </rdf:Description>
  <rdf:Description rdf:about="https://w3id.org/crmrp#c_326da7e4">
    <skos:prefLabel xml:lang="it">Reintegrazione pittorica</skos:prefLabel>
    <rdfs:label xml:lang="en">Inpainting</rdfs:label>
    <rdf:type rdf:resource="http://www.w3.org/2002/07/owl#NamedIndividual"/>
    <skos:editorialNote xml:lang="en">Getty AAT http://vocab.getty.edu/page/aat/300053723</skos:editorialNote>
    <skos:definition xml:lang="en"> In the conservation of paintings, the introduction of new paint into and limited to areas of loss in the original paint layer in order to restore design continuity.</skos:definition>
    <skos:broader rdf:resource="https://w3id.org/crmrp#c_0f7eacd7"/>
    <skos:topConceptOf rdf:resource="https://w3id.org/crmrp#Intervention"/>
    <skos:closeMatch rdf:resource="http://vocab.getty.edu/page/aat/300053723"/>
    <rdf:type rdf:resource="http://www.w3.org/2004/02/skos/core#Concept"/>
    <skos:altLabel xml:lang="en">Retouching</skos:altLabel>
    <skos:prefLabel xml:lang="en">Inpainting</skos:prefLabel>
    <skos:inScheme rdf:resource="https://w3id.org/crmrp#Intervention"/>
    <skos:altLabel xml:lang="en">Pictorial retouching</skos:altLabel>
  </rdf:Description>
  <rdf:Description rdf:about="https://w3id.org/crmrp#c_58e9ad7f">
    <skos:exactMatch rdf:resource="http://vocab.getty.edu/page/aat/30026484"/>
    <skos:prefLabel xml:lang="en">Infill</skos:prefLabel>
    <rdf:type rdf:resource="http://www.w3.org/2002/07/owl#NamedIndividual"/>
    <skos:editorialNote xml:lang="en">Getty Conservation Institute “Illustrated Glossary - Definitions of terms used for the graphic documentation of in situ floor mosaics”, “Mosaics In Situ Project”, Los Angeles, 2003</skos:editorialNote>
    <skos:editorialNote xml:lang="en">A. Weyer et al., “EwaGlos - European Illustrated Glossary of conservation terms for wall paintings and architectural surfaces”, Michael Imhof Verlag, Petersberg, Germany</skos:editorialNote>
    <skos:prefLabel xml:lang="it">Stuccatura</skos:prefLabel>
    <skos:editorialNote xml:lang="en">Getty AAT http://vocab.getty.edu/page/aat/300264840</skos:editorialNote>
    <rdf:type rdf:resource="http://www.w3.org/2004/02/skos/core#Concept"/>
    <skos:topConceptOf rdf:resource="https://w3id.org/crmrp#Intervention"/>
    <skos:note xml:lang="en">The preferred editorial note and the definition closest to the meaning is EwaGlos - European Illustrated Glossary of conservation terms for wall paintings and architectural surfaces</skos:note>
    <skos:altLabel xml:lang="en">Filling</skos:altLabel>
    <skos:broader rdf:resource="https://w3id.org/crmrp#c_24cc76d5"/>
    <skos:inScheme rdf:resource="https://w3id.org/crmrp#Intervention"/>
    <skos:definition xml:lang="en">Definition: To re-establish continuity between layers reinstating their structural and aesthetic properties.</skos:definition>
    <rdfs:label xml:lang="en">Infill</rdfs:label>
  </rdf:Description>
  <rdf:Description rdf:about="https://w3id.org/crmrp#c_60903036">
    <skos:prefLabel xml:lang="it">Cretto</skos:prefLabel>
    <skos:prefLabel xml:lang="en">Cretto</skos:prefLabel>
    <skos:broader rdf:resource="https://w3id.org/crmrp#c_8c762c3e"/>
    <skos:topConceptOf rdf:resource="https://w3id.org/crmrp#Alteration"/>
    <rdf:type rdf:resource="http://www.w3.org/2002/07/owl#NamedIndividual"/>
    <rdfs:label xml:lang="en">Cretto</rdfs:label>
    <rdf:type rdf:resource="http://www.w3.org/2004/02/skos/core#Concept"/>
    <skos:inScheme rdf:resource="https://w3id.org/crmrp#Alteration"/>
    <skos:definition xml:lang="en">A term used to indicate a micro-fracture of the paint film that may result from phenomena of drying of the oily binder. In general, the crack is more pronounced in correspondence with dark dark and brown colours because earth colours are among the colours that absorb the most binder.</skos:definition>
    <skos:note xml:lang="en">International references could not be found</skos:note>
    <skos:editorialNote xml:lang="it">C. Giannini, “Dizionario del restauro - Tecniche diagnostica conservazione”, Nardini Editore, Firenze, 2010</skos:editorialNote>
  </rdf:Description>
  <rdf:Description rdf:about="http://www.w3.org/2004/02/skos/core#source">
    <rdf:type rdf:resource="http://www.w3.org/2002/07/owl#AnnotationProperty"/>
  </rdf:Description>
  <rdf:Description rdf:about="https://w3id.org/crmrp#c_0ca4ad6d">
    <rdf:type rdf:resource="http://www.w3.org/2004/02/skos/core#Concept"/>
    <skos:topConceptOf rdf:resource="https://w3id.org/crmrp#Material"/>
    <skos:inScheme rdf:resource="https://w3id.org/crmrp#Material"/>
    <skos:prefLabel xml:lang="it">Carta</skos:prefLabel>
    <rdf:type rdf:resource="http://www.w3.org/2002/07/owl#NamedIndividual"/>
    <skos:prefLabel xml:lang="en">Paper</skos:prefLabel>
    <skos:exactMatch rdf:resource="http://vocab.getty.edu/page/aat/300014109"/>
    <skos:definition xml:lang="en">Refers generally to all types of thin matted or felted sheets or webs of fiber formed and dried on a fine screen from a pulpy water suspension. The fibers may be animal, such as hair, silk or wool, or mineral, such as asbestos, or synthetic. However most paper is made from cellulosic plant fiber, such as from wood pulp, grass, cotton, linen, and straw.</skos:definition>
    <skos:editorialNote xml:lang="en">Getty AAT http://vocab.getty.edu/page/aat/300014109</skos:editorialNote>
    <rdfs:label xml:lang="en">Paper</rdfs:label>
  </rdf:Description>
  <rdf:Description rdf:about="https://w3id.org/crmrp#c_564ad901">
    <skos:inScheme rdf:resource="https://w3id.org/crmrp#Archeometric_and_Diagnostic_Analysis"/>
    <skos:editorialNote xml:lang="en">Getty AAT http://vocab.getty.edu/page/aat/300379552</skos:editorialNote>
    <skos:prefLabel xml:lang="it">Fluorescenza ultravioletta</skos:prefLabel>
    <skos:definition xml:lang="en">Visible fluorescence emitted by materials in paintings and other objects exposed to ultraviolet radiation</skos:definition>
    <skos:topConceptOf rdf:resource="https://w3id.org/crmrp#Archeometric_and_Diagnostic_Analysis"/>
    <skos:broader rdf:resource="https://w3id.org/crmrp#c_1fd6102e"/>
    <rdf:type rdf:resource="http://www.w3.org/2002/07/owl#NamedIndividual"/>
    <rdf:type rdf:resource="http://www.w3.org/2004/02/skos/core#Concept"/>
    <skos:closeMatch rdf:resource="http://vocab.getty.edu/page/aat/300379552"/>
    <rdfs:label xml:lang="en">Ultraviolet fluorescence</rdfs:label>
    <skos:prefLabel xml:lang="en">Ultraviolet fluorescence</skos:prefLabel>
  </rdf:Description>
  <rdf:Description rdf:about="https://w3id.org/crmrp#c_27b869ee">
    <rdf:type rdf:resource="http://www.w3.org/2004/02/skos/core#Concept"/>
    <skos:prefLabel xml:lang="en">Gold</skos:prefLabel>
    <rdf:type rdf:resource="http://www.w3.org/2002/07/owl#NamedIndividual"/>
    <skos:editorialNote xml:lang="en">Getty AAT http://vocab.getty.edu/page/aat/300011021</skos:editorialNote>
    <skos:prefLabel xml:lang="it">Oro</skos:prefLabel>
    <skos:inScheme rdf:resource="https://w3id.org/crmrp#Material"/>
    <rdfs:label xml:lang="en">Gold</rdfs:label>
    <skos:topConceptOf rdf:resource="https://w3id.org/crmrp#Material"/>
    <skos:broader rdf:resource="https://w3id.org/crmrp#c_6407466f"/>
    <skos:definition xml:lang="en">Pure metallic element having symbol Au and atomic number 79; a soft, inert, shiny reddish yellow metal that is very malleable and ductile. Gold has been highly valued and found in artifacts dating to before 5000 BCE. Native gold, found in quartz veins (vein gold) and alluvial deposits (placer gold), generally contains some silver and copper. Gold is purified by dissolution in mercury or cyanide solutions, by melting, or by electrodeposition. The purity of commercial gold is expressed in karats which is the number of parts of gold in 24 parts of the alloy. Today gold is primarily used for monetary systems and for jewelry.</skos:definition>
    <skos:exactMatch rdf:resource="http://vocab.getty.edu/page/aat/300011021"/>
  </rdf:Description>
  <rdf:Description rdf:about="https://w3id.org/crmrp#c_ea4e6f28">
    <skos:definition xml:lang="en">A soft mineral composed of calcium sulfate dihydrate.</skos:definition>
    <skos:exactMatch xml:lang="en">Gypsum</skos:exactMatch>
    <skos:prefLabel xml:lang="en">Gypsum</skos:prefLabel>
    <skos:broader rdf:resource="https://w3id.org/crmrp#c_34d8fe56"/>
    <rdfs:label xml:lang="en">Gypsum</rdfs:label>
    <skos:editorialNote xml:lang="en">A. Weyer et al., “EwaGlos - European Illustrated Glossary of conservation terms for wall paintings and architectural surfaces”, Michael Imhof Verlag, Petersberg, Germany</skos:editorialNote>
    <skos:topConceptOf rdf:resource="https://w3id.org/crmrp#Material"/>
    <rdf:type rdf:resource="http://www.w3.org/2004/02/skos/core#Concept"/>
    <rdf:type rdf:resource="http://www.w3.org/2002/07/owl#NamedIndividual"/>
    <skos:prefLabel xml:lang="it">Gesso</skos:prefLabel>
    <skos:inScheme rdf:resource="https://w3id.org/crmrp#Material"/>
  </rdf:Description>
  <rdf:Description rdf:about="https://w3id.org/crmrp#c_51f2e48a">
    <skos:inScheme rdf:resource="https://w3id.org/crmrp#Restoration_Object"/>
    <skos:exactMatch rdf:resource="http://vocab.getty.edu/page/aat/300046300"/>
    <rdf:type rdf:resource="http://www.w3.org/2002/07/owl#NamedIndividual"/>
    <skos:topConceptOf rdf:resource="https://w3id.org/crmrp#Restoration_Object"/>
    <skos:prefLabel xml:lang="it">Fotografia</skos:prefLabel>
    <skos:editorialNote xml:lang="en">Getty AAT http://vocab.getty.edu/page/aat/300046300</skos:editorialNote>
    <rdf:type rdf:resource="http://www.w3.org/2004/02/skos/core#Concept"/>
    <rdfs:label xml:lang="en">Photographs</rdfs:label>
    <skos:definition xml:lang="en">Refers to still images produced from radiation-sensitive materials (sensitive to light, electron beams, or nuclear radiation), generally by means of the chemical action of light on a sensitive film, paper, glass, or metal. Photographs may be positive or negative, opaque or transparent. The concept does not include reproductive prints of documents and technical drawings. The concept may include photographs made by digital means.</skos:definition>
    <skos:prefLabel xml:lang="en">Photographs</skos:prefLabel>
  </rdf:Description>
  <rdf:Description rdf:about="https://w3id.org/crmrp#c_cb6d58c9">
    <skos:definition xml:lang="en">The principal tissue of trees and other plants that provides both strength and a means of conducting nutrients. Wood is one of the most versatile materials known.</skos:definition>
    <skos:topConceptOf rdf:resource="https://w3id.org/crmrp#Material"/>
    <skos:editorialNote xml:lang="en">Getty AAT http://vocab.getty.edu/page/aat/300014109</skos:editorialNote>
    <rdfs:label xml:lang="en">Wood</rdfs:label>
    <skos:inScheme rdf:resource="https://w3id.org/crmrp#Material"/>
    <rdf:type rdf:resource="http://www.w3.org/2004/02/skos/core#Concept"/>
    <rdf:type rdf:resource="http://www.w3.org/2002/07/owl#NamedIndividual"/>
    <skos:prefLabel xml:lang="en">Wood</skos:prefLabel>
    <skos:exactMatch rdf:resource="http://vocab.getty.edu/page/aat/300014109"/>
    <skos:prefLabel xml:lang="it">Legno</skos:prefLabel>
  </rdf:Description>
  <rdf:Description rdf:about="https://w3id.org/crmrp#c_bc342552">
    <skos:editorialNote xml:lang="en">Verg`es-Belmin et al., ICOMOS-ISCS: Illustrated glossary on stone deterioration patterns, vol. XV. Icomos International Council on Monuments and Sites, 2008</skos:editorialNote>
    <skos:inScheme rdf:resource="https://w3id.org/crmrp#Alteration"/>
    <skos:broader rdf:resource="https://w3id.org/crmrp#c_13f3ce9e"/>
    <rdf:type rdf:resource="http://www.w3.org/2002/07/owl#NamedIndividual"/>
    <skos:editorialNote xml:lang="en">Getty Conservation Institute “Illustrated Glossary - Technician Training for the Maintenance of In Situ Mosaics”, Los Angeles, 2013</skos:editorialNote>
    <skos:altLabel xml:lang="en">Bulge</skos:altLabel>
    <skos:altLabel xml:lang="en">Blistering</skos:altLabel>
    <skos:closeMatch rdf:resource="http://vocab.getty.edu/page/aat/300228350"/>
    <rdfs:label xml:lang="en">Swelling</rdfs:label>
    <skos:editorialNote xml:lang="en">Getty AAT http://vocab.getty.edu/page/aat/300228350</skos:editorialNote>
    <skos:prefLabel xml:lang="en">Swelling</skos:prefLabel>
    <skos:note xml:lang="en">The preferred editorial note and the definition closest to the meaning is Uni Cen/Ts 17135:2021</skos:note>
    <skos:editorialNote xml:lang="en">Uni Cen/Ts 17135:2021 - Conservation of cultural heritage. General terms and definitions</skos:editorialNote>
    <skos:definition xml:lang="en">Increase in dimensions.</skos:definition>
    <skos:prefLabel xml:lang="it">Rigonfiamento</skos:prefLabel>
    <skos:editorialNote xml:lang="en">A. Weyer et al., “EwaGlos - European Illustrated Glossary of conservation terms for wall paintings and architectural surfaces”, Michael Imhof Verlag, Petersberg, Germany</skos:editorialNote>
    <rdf:type rdf:resource="http://www.w3.org/2004/02/skos/core#Concept"/>
    <skos:topConceptOf rdf:resource="https://w3id.org/crmrp#Alteration"/>
  </rdf:Description>
  <rdf:Description rdf:about="https://w3id.org/crmrp#c_cf59824d">
    <skos:prefLabel xml:lang="en">Clothing</skos:prefLabel>
    <skos:prefLabel xml:lang="it">Vestimento</skos:prefLabel>
    <skos:definition xml:lang="en">Coverings for the torso, limbs, hands, feet, and head for warmth, fashion, or to cover nudity. It generally excludes other items of costume such as jewelry, crowns, and other accessories that are purely decorative or symbolic and have no practical function.</skos:definition>
    <rdf:type rdf:resource="http://www.w3.org/2002/07/owl#NamedIndividual"/>
    <skos:editorialNote xml:lang="en">Getty AAT http://vocab.getty.edu/page/aat/300266639</skos:editorialNote>
    <skos:inScheme rdf:resource="https://w3id.org/crmrp#Restoration_Object"/>
    <rdf:type rdf:resource="http://www.w3.org/2004/02/skos/core#Concept"/>
    <rdfs:label xml:lang="en">Clothing</rdfs:label>
    <skos:topConceptOf rdf:resource="https://w3id.org/crmrp#Restoration_Object"/>
    <skos:closeMatch rdf:resource="http://vocab.getty.edu/page/aat/300266639"/>
  </rdf:Description>
  <rdf:Description rdf:about="https://w3id.org/crmrp#c_07e518a1">
    <rdf:type rdf:resource="http://www.w3.org/2004/02/skos/core#Concept"/>
    <skos:inScheme rdf:resource="https://w3id.org/crmrp#Material"/>
    <skos:prefLabel xml:lang="it">Tessile</skos:prefLabel>
    <skos:prefLabel xml:lang="en">Textile materials</skos:prefLabel>
    <skos:exactMatch rdf:resource="http://vocab.getty.edu/page/aat/300231565"/>
    <rdfs:label xml:lang="en">Textile materials</rdfs:label>
    <rdf:type rdf:resource="http://www.w3.org/2002/07/owl#NamedIndividual"/>
    <skos:topConceptOf rdf:resource="https://w3id.org/crmrp#Material"/>
    <skos:editorialNote xml:lang="en">Getty AAT http://vocab.getty.edu/page/aat/300231565</skos:editorialNote>
    <skos:definition xml:lang="en">Materials produced by weaving, felting, knotting, twining, or otherwise processing natural or synthetic fibers so that they cohere into a form or unit; traditionally excludes fiberboard, paper, papier-mâché, and papyrus, which, though also fiber products, are considered as separate types of material.</skos:definition>
  </rdf:Description>
  <rdf:Description rdf:about="http://www.cidoc-crm.org/cidoc-crm/P4_has_time-span">
    <rdfs:range rdf:resource="http://www.cidoc-crm.org/cidoc-crm/E52_Time-Span"/>
    <rdfs:domain rdf:resource="https://w3id.org/crmrp#R8_Intervention"/>
    <rdfs:domain rdf:resource="https://w3id.org/crmrp#R7_Restoration_Project"/>
  </rdf:Description>
  <rdf:Description rdf:about="https://w3id.org/crmrp#c_a5e9bb0b">
    <skos:editorialNote xml:lang="en">Getty Conservation Institute “Illustrated Glossary - Technician Training for the Maintenance of In Situ Mosaics”, Los Angeles, 2013</skos:editorialNote>
    <rdfs:label xml:lang="en">Pebble mosaic</rdfs:label>
    <skos:definition xml:lang="en">Mosaic pavement, generally bi-chrome, more rarely polychrome, made of natural pebbles of different sizes and placed on their edge, side by side, to create figures or geometric motifs.</skos:definition>
    <rdf:type rdf:resource="http://www.w3.org/2002/07/owl#NamedIndividual"/>
    <rdf:type rdf:resource="http://www.w3.org/2004/02/skos/core#Concept"/>
    <skos:editorialNote xml:lang="it">C. Fiori “Teoria e tecniche per la conservazione del mosaico”, Il Prato, Padova, 2002</skos:editorialNote>
    <skos:prefLabel xml:lang="en">Pebble mosaic</skos:prefLabel>
    <skos:inScheme rdf:resource="https://w3id.org/crmrp#Execution_Technique"/>
    <skos:topConceptOf rdf:resource="https://w3id.org/crmrp#Execution_Technique"/>
    <skos:prefLabel xml:lang="it">Mosaico ciottoli</skos:prefLabel>
    <skos:broader rdf:resource="https://w3id.org/crmrp#c_b9a6a1c8"/>
  </rdf:Description>
  <rdf:Description rdf:about="https://w3id.org/crmrp#c_b58f1659">
    <skos:topConceptOf rdf:resource="https://w3id.org/crmrp#Documentation"/>
    <skos:prefLabel xml:lang="it">Documentazione audio</skos:prefLabel>
    <skos:prefLabel xml:lang="en">Audio documentation</skos:prefLabel>
    <skos:note xml:lang="en">International references could not be found</skos:note>
    <skos:inScheme rdf:resource="https://w3id.org/crmrp#Documentation"/>
    <skos:definition xml:lang="en">Any recording about an object or its manufacturer.</skos:definition>
    <rdfs:label xml:lang="en">Audio documentation</rdfs:label>
    <rdf:type rdf:resource="http://www.w3.org/2004/02/skos/core#Concept"/>
    <rdf:type rdf:resource="http://www.w3.org/2002/07/owl#NamedIndividual"/>
  </rdf:Description>
  <rdf:Description rdf:about="https://w3id.org/crmrp#c_9d1ced39">
    <skos:broader rdf:resource="https://w3id.org/crmrp#c_0a9f4d42"/>
    <skos:definition xml:lang="en">Clamshell casting is predominantly used in the mechanical engineering industry for the production of high-precision, high-volume parts. It involves making a demountable metal mould in which casting takes place. The casting does not adhere to the mould as it is kept cold.</skos:definition>
    <skos:inScheme rdf:resource="https://w3id.org/crmrp#Execution_Technique"/>
    <skos:editorialNote xml:lang="it">A.Giuffredi “Formatura e fonderia”, Alinea editrice, Firenze, 2010</skos:editorialNote>
    <rdf:type rdf:resource="http://www.w3.org/2002/07/owl#NamedIndividual"/>
    <rdf:type rdf:resource="http://www.w3.org/2004/02/skos/core#Concept"/>
    <skos:note xml:lang="en">International references could not be found</skos:note>
    <rdfs:label xml:lang="en">Fusione a conchiglia</rdfs:label>
    <skos:topConceptOf rdf:resource="https://w3id.org/crmrp#Execution_Technique"/>
    <skos:prefLabel xml:lang="it">Fusione a conchiglia</skos:prefLabel>
    <skos:prefLabel xml:lang="en">Fusione a conchiglia</skos:prefLabel>
  </rdf:Description>
  <rdf:Description rdf:about="https://w3id.org/crmrp#c_051209b3">
    <skos:closeMatch rdf:resource="http://vocab.getty.edu/page/aat/300033656"/>
    <rdfs:label xml:lang="en">Panel painting technique</rdfs:label>
    <skos:inScheme rdf:resource="https://w3id.org/crmrp#Execution_Technique"/>
    <skos:definition xml:lang="en">Refers to paintings on wooden supports, including smaller portable paintings and medium-sized paintings, such as altarpieces, for which several planks of wood were joined to form a larger panel. The term is typically used to refer to paintings on a wooden support in Western art, generally dating from ancient Greece and Rome through the Renaissance, after which time canvas became the standard support for paintings in this size range. Panel paintings are still common today in Greek and Russian Orthodox icons.</skos:definition>
    <skos:prefLabel xml:lang="it">Tecnica su tavola</skos:prefLabel>
    <skos:prefLabel xml:lang="en">Panel painting technique</skos:prefLabel>
    <rdf:type rdf:resource="http://www.w3.org/2002/07/owl#NamedIndividual"/>
    <skos:topConceptOf rdf:resource="https://w3id.org/crmrp#Execution_Technique"/>
    <rdf:type rdf:resource="http://www.w3.org/2004/02/skos/core#Concept"/>
    <skos:editorialNote xml:lang="en">Getty AAT http://vocab.getty.edu/page/aat/300033656</skos:editorialNote>
  </rdf:Description>
  <rdf:Description rdf:about="https://w3id.org/crmrp#c_6692ec2f">
    <skos:topConceptOf rdf:resource="https://w3id.org/crmrp#Material"/>
    <skos:prefLabel xml:lang="it">Origine animale</skos:prefLabel>
    <skos:prefLabel xml:lang="en">Animal origin</skos:prefLabel>
    <skos:note xml:lang="en">International references could not be found</skos:note>
    <skos:inScheme rdf:resource="https://w3id.org/crmrp#Material"/>
    <skos:definition xml:lang="en">An animal artefact is an object made from materials derived from animals, such as bones, horns, ivory, leather, silk, wool, feathers or shells. Such artefacts may be tools, ornaments, garments or works of art, often with cultural, practical or symbolic meanings</skos:definition>
    <rdfs:label xml:lang="en">Animal origin</rdfs:label>
    <rdf:type rdf:resource="http://www.w3.org/2004/02/skos/core#Concept"/>
    <rdf:type rdf:resource="http://www.w3.org/2002/07/owl#NamedIndividual"/>
  </rdf:Description>
  <rdf:Description rdf:about="https://w3id.org/crmrp#c_570dee40">
    <skos:topConceptOf rdf:resource="https://w3id.org/crmrp#Archeometric_and_Diagnostic_Analysis"/>
    <skos:broader rdf:resource="https://w3id.org/crmrp#c_1fd6102e"/>
    <skos:editorialNote xml:lang="en">A. Weyer et al., “EwaGlos - European Illustrated Glossary of conservation terms for wall paintings and architectural surfaces”, Michael Imhof Verlag, Petersberg, Germany</skos:editorialNote>
    <rdf:type rdf:resource="http://www.w3.org/2002/07/owl#NamedIndividual"/>
    <skos:definition xml:lang="en">The surface is lit, preferably using daylight-spots at a specific angle, in order to show the relief through shadow effects.</skos:definition>
    <skos:prefLabel xml:lang="it">Fotografia a luce radente</skos:prefLabel>
    <skos:inScheme rdf:resource="https://w3id.org/crmrp#Archeometric_and_Diagnostic_Analysis"/>
    <skos:prefLabel xml:lang="en">Raking light</skos:prefLabel>
    <rdf:type rdf:resource="http://www.w3.org/2004/02/skos/core#Concept"/>
    <rdfs:label xml:lang="en">Raking light</rdfs:label>
  </rdf:Description>
  <rdf:Description rdf:about="https://w3id.org/crmrp#Alteration">
    <skos:altLabel xml:lang="it">Stato di conservazione</skos:altLabel>
    <skos:altLabel xml:lang="en">Conservation state</skos:altLabel>
    <skos:prefLabel xml:lang="it">Alterazione</skos:prefLabel>
    <skos:prefLabel xml:lang="en">Alteration</skos:prefLabel>
    <skos:note xml:lang="en">Uni Cen/Ts 17135:2021 - Conservation of cultural heritage. General terms and definitions</skos:note>
    <skos:definition xml:lang="en">Change in condition, beneficial or not, intentional or not.</skos:definition>
    <rdf:type rdf:resource="http://www.w3.org/2004/02/skos/core#ConceptScheme"/>
    <rdf:type rdf:resource="http://www.w3.org/2002/07/owl#NamedIndividual"/>
  </rdf:Description>
  <rdf:Description rdf:about="https://w3id.org/crmrp#c_7d48691d">
    <skos:editorialNote xml:lang="it">C. Giannini, “Dizionario del restauro - Tecniche diagnostica conservazione”, Nardini Editore, Firenze, 2010</skos:editorialNote>
    <skos:editorialNote xml:lang="en">Getty Conservation Institute “Illustrated Glossary - Technician Training for the Maintenance of In Situ Mosaics”, Los Angeles, 2013</skos:editorialNote>
    <skos:editorialNote xml:lang="it">C. Fiori “Teoria e tecniche per la conservazione del mosaico”, Il Prato, Padova, 2002</skos:editorialNote>
    <skos:topConceptOf rdf:resource="https://w3id.org/crmrp#Execution_Technique"/>
    <skos:definition xml:lang="en">Pavement made of stone slabs, most commonly of different colored marble, cut in regular shapes and placed side by side to create a geometric pattern or figurative motif.</skos:definition>
    <rdfs:label xml:lang="en">Opus sectile</rdfs:label>
    <skos:prefLabel xml:lang="it">Opus sectile</skos:prefLabel>
    <skos:prefLabel xml:lang="en">Opus sectile</skos:prefLabel>
    <skos:broader rdf:resource="https://w3id.org/crmrp#c_b9a6a1c8"/>
    <skos:inScheme rdf:resource="https://w3id.org/crmrp#Execution_Technique"/>
    <rdf:type rdf:resource="http://www.w3.org/2002/07/owl#NamedIndividual"/>
    <rdf:type rdf:resource="http://www.w3.org/2004/02/skos/core#Concept"/>
  </rdf:Description>
  <rdf:Description rdf:about="https://w3id.org/crmrp#c_d02e5354">
    <skos:editorialNote xml:lang="en">Getty AAT http://vocab.getty.edu/page/aat/300220235</skos:editorialNote>
    <skos:prefLabel xml:lang="it">Ossidazione</skos:prefLabel>
    <rdf:type rdf:resource="http://www.w3.org/2002/07/owl#NamedIndividual"/>
    <skos:exactMatch rdf:resource="http://vocab.getty.edu/page/aat/300220235"/>
    <skos:inScheme rdf:resource="https://w3id.org/crmrp#Alteration"/>
    <rdf:type rdf:resource="http://www.w3.org/2004/02/skos/core#Concept"/>
    <skos:definition xml:lang="en">The process or result of combining with oxygen; sometimes contributing to the degradation of a surface, such as in corrosion.</skos:definition>
    <skos:broader rdf:resource="https://w3id.org/crmrp#c_ae321441"/>
    <skos:prefLabel xml:lang="en">Oxidation</skos:prefLabel>
    <skos:topConceptOf rdf:resource="https://w3id.org/crmrp#Alteration"/>
    <rdfs:label xml:lang="en">Oxidation</rdfs:label>
  </rdf:Description>
  <rdf:Description rdf:about="https://w3id.org/crmrp#c_1440c4b3">
    <skos:editorialNote xml:lang="en">A. Weyer et al., “EwaGlos - European Illustrated Glossary of conservation terms for wall paintings and architectural surfaces”, Michael Imhof Verlag, Petersberg, Germany</skos:editorialNote>
    <skos:closeMatch rdf:resource="http://vocab.getty.edu/page/aat/300053097"/>
    <skos:definition xml:lang="en">Application of an adhesive product able to join together layers of plaster, renders or painting layers and fill voids or gaps in between.</skos:definition>
    <rdfs:label xml:lang="en">Fixing</rdfs:label>
    <skos:inScheme rdf:resource="https://w3id.org/crmrp#Intervention"/>
    <skos:prefLabel xml:lang="it">Riadesione</skos:prefLabel>
    <skos:prefLabel xml:lang="en">Fixing</skos:prefLabel>
    <skos:topConceptOf rdf:resource="https://w3id.org/crmrp#Intervention"/>
    <skos:note xml:lang="en">The preferred editorial note and the definition closest to the meaning is A. Weyer et al., “EwaGlos - European Illustrated Glossary of conservation terms for wall paintings and architectural surfaces”, Michael Imhof Verlag, Petersberg, Germany</skos:note>
    <rdf:type rdf:resource="http://www.w3.org/2004/02/skos/core#Concept"/>
    <skos:editorialNote xml:lang="en">Getty AAT http://vocab.getty.edu/page/aat/300053097</skos:editorialNote>
    <skos:editorialNote xml:lang="en">etty Conservation Institute “Illustrated Glossary - Definitions of terms used for the graphic documentation of in situ floor mosaics”, “Mosaics In Situ Project”, Los Angeles, 2003</skos:editorialNote>
    <rdf:type rdf:resource="http://www.w3.org/2002/07/owl#NamedIndividual"/>
  </rdf:Description>
  <rdf:Description rdf:about="https://w3id.org/crmrp#c_6d269f19">
    <skos:note xml:lang="en">International references could not be found</skos:note>
    <rdf:type rdf:resource="http://www.w3.org/2002/07/owl#NamedIndividual"/>
    <skos:editorialNote xml:lang="it">C. Giannini, “Dizionario del restauro - Tecniche diagnostica conservazione”, Nardini Editore, Firenze, 2010</skos:editorialNote>
    <skos:broader rdf:resource="https://w3id.org/crmrp#c_4d471b17"/>
    <skos:prefLabel xml:lang="it">Meccatura</skos:prefLabel>
    <skos:inScheme rdf:resource="https://w3id.org/crmrp#Execution_Technique"/>
    <rdf:type rdf:resource="http://www.w3.org/2004/02/skos/core#Concept"/>
    <skos:prefLabel xml:lang="en">Mecca gilding</skos:prefLabel>
    <rdfs:label xml:lang="en">Mecca gilding</rdfs:label>
    <skos:topConceptOf rdf:resource="https://w3id.org/crmrp#Execution_Technique"/>
    <skos:definition xml:lang="en">Technique of applying paint known as mecha on tin or silver surfaces to achieve an optical effect similar to gilding</skos:definition>
  </rdf:Description>
  <rdf:Description rdf:about="https://w3id.org/crmrp#c_f8deca36">
    <skos:definition xml:lang="en">Thin piece completely detached from the surface of an object.</skos:definition>
    <skos:editorialNote xml:lang="en">A. Weyer et al., “EwaGlos - European Illustrated Glossary of conservation terms for wall paintings and architectural surfaces”, Michael Imhof Verlag, Petersberg, Germany</skos:editorialNote>
    <skos:note xml:lang="en">The preferred editorial note and the definition closest to the meaning is Uni Cen/Ts 17135:2021</skos:note>
    <skos:inScheme rdf:resource="https://w3id.org/crmrp#Alteration"/>
    <rdfs:label xml:lang="en">Flake</rdfs:label>
    <rdf:type rdf:resource="http://www.w3.org/2004/02/skos/core#Concept"/>
    <skos:broader rdf:resource="https://w3id.org/crmrp#c_d54b0be2"/>
    <skos:editorialNote xml:lang="en">Verg`es-Belmin et al., ICOMOS-ISCS: Illustrated glossary on stone deterioration patterns, vol. XV. Icomos International Council on Monuments and Sites, 2008</skos:editorialNote>
    <skos:topConceptOf rdf:resource="https://w3id.org/crmrp#Alteration"/>
    <skos:prefLabel xml:lang="en">Flake</skos:prefLabel>
    <skos:altLabel xml:lang="en">Flaking</skos:altLabel>
    <skos:prefLabel xml:lang="it">Scagliatura</skos:prefLabel>
    <skos:editorialNote xml:lang="en">Uni Cen/Ts 17135:2021 - Conservation of cultural heritage. General terms and definitions</skos:editorialNote>
    <rdf:type rdf:resource="http://www.w3.org/2002/07/owl#NamedIndividual"/>
    <skos:altLabel xml:lang="it">Sfaldamento</skos:altLabel>
  </rdf:Description>
  <rdf:Description rdf:about="https://w3id.org/crmrp#R4_Photographic_Documentation">
    <rdfs:label xml:lang="en">Photographic Documentation</rdfs:label>
    <rdfs:comment xml:lang="en">This class represents the photographic documentation of an object.
Before and during restoration work, it is necessary to know more about the history of artefacts, so sometimes a few photos from the past can help restorers better understand the artworks and how they looked in the past.</rdfs:comment>
    <rdfs:subClassOf rdf:resource="http://www.cidoc-crm.org/cidoc-crm/E31_Document"/>
    <rdf:type rdf:resource="http://www.w3.org/2002/07/owl#Class"/>
  </rdf:Description>
  <rdf:Description rdf:about="https://w3id.org/crmrp#c_a8f1fa7e">
    <skos:prefLabel xml:lang="it">Gouache</skos:prefLabel>
    <skos:prefLabel xml:lang="en">Gouache</skos:prefLabel>
    <skos:inScheme rdf:resource="https://w3id.org/crmrp#Execution_Technique"/>
    <skos:definition xml:lang="en"> A method of painting with matte, opaque watercolor paint. Gouache painting employs opaque layers of color rather than the transparent washes used in the aquarelle technique, due to the differing pigment densities of the media.</skos:definition>
    <rdf:type rdf:resource="http://www.w3.org/2004/02/skos/core#Concept"/>
    <skos:broader rdf:resource="https://w3id.org/crmrp#c_044b6056"/>
    <rdf:type rdf:resource="http://www.w3.org/2002/07/owl#NamedIndividual"/>
    <skos:closeMatch xml:lang="en">Getty AAT http://vocab.getty.edu/page/aat/300404215</skos:closeMatch>
    <rdfs:label xml:lang="en">Gouache</rdfs:label>
    <skos:editorialNote xml:lang="en">Getty AAT http://vocab.getty.edu/page/aat/300404215</skos:editorialNote>
    <skos:topConceptOf rdf:resource="https://w3id.org/crmrp#Execution_Technique"/>
  </rdf:Description>
  <rdf:Description rdf:about="https://w3id.org/crmrp#c_687df059">
    <skos:editorialNote xml:lang="en">Getty AAT http://vocab.getty.edu/page/aat/300001987</skos:editorialNote>
    <skos:closeMatch rdf:resource="http://vocab.getty.edu/page/aat/300001987"/>
    <skos:topConceptOf rdf:resource="https://w3id.org/crmrp#Restoration_Object"/>
    <rdfs:label xml:lang="en">Decorative apparatus of architecture</rdfs:label>
    <skos:altLabel xml:lang="en">Surface elements (architectural)</skos:altLabel>
    <rdf:type rdf:resource="http://www.w3.org/2004/02/skos/core#Concept"/>
    <skos:prefLabel xml:lang="it">Apparato decorativo dell'architettura</skos:prefLabel>
    <rdf:type rdf:resource="http://www.w3.org/2002/07/owl#NamedIndividual"/>
    <skos:prefLabel xml:lang="en">Decorative apparatus of architecture</skos:prefLabel>
    <skos:inScheme rdf:resource="https://w3id.org/crmrp#Restoration_Object"/>
    <skos:definition xml:lang="en">Architectural elements or components located on the surface</skos:definition>
  </rdf:Description>
  <rdf:Description rdf:about="https://w3id.org/crmrp#c_33e199bc">
    <rdf:type rdf:resource="http://www.w3.org/2002/07/owl#NamedIndividual"/>
    <skos:prefLabel xml:lang="it">Cromatografia su strato sottile (TLC)</skos:prefLabel>
    <skos:definition xml:lang="en">Chromatography in which glass plates coated with thin layers of alumina, silica gel, or cellulose are used as an adsorbent.</skos:definition>
    <skos:editorialNote xml:lang="en">Getty AAT http://vocab.getty.edu/page/aat/300214726</skos:editorialNote>
    <skos:topConceptOf rdf:resource="https://w3id.org/crmrp#Archeometric_and_Diagnostic_Analysis"/>
    <skos:broader rdf:resource="https://w3id.org/crmrp#c_2d5cde83"/>
    <skos:prefLabel xml:lang="en">Thin layer chromatography (TLC)</skos:prefLabel>
    <skos:closeMatch rdf:resource="http://vocab.getty.edu/page/aat/300214726"/>
    <rdf:type rdf:resource="http://www.w3.org/2004/02/skos/core#Concept"/>
    <skos:inScheme rdf:resource="https://w3id.org/crmrp#Archeometric_and_Diagnostic_Analysis"/>
    <rdfs:label xml:lang="en">Thin layer chromatography (TLC)</rdfs:label>
  </rdf:Description>
  <rdf:Description rdf:about="https://w3id.org/crmrp#c_e5ce4664">
    <rdf:type rdf:resource="http://www.w3.org/2002/07/owl#NamedIndividual"/>
    <rdfs:label xml:lang="en">Determination of water vapour permeability (dp)</rdfs:label>
    <skos:topConceptOf rdf:resource="https://w3id.org/crmrp#Archeometric_and_Diagnostic_Analysis"/>
    <skos:prefLabel xml:lang="en">Determination of water vapour permeability (dp)</skos:prefLabel>
    <skos:broader rdf:resource="https://w3id.org/crmrp#c_1fd6102e"/>
    <skos:definition xml:lang="en">The test is a method for the determination of water vapour permeability under conditions of steady-state flow for low and high humidity conditions of a sample</skos:definition>
    <rdf:type rdf:resource="http://www.w3.org/2004/02/skos/core#Concept"/>
    <skos:prefLabel xml:lang="it">Determinazione delle permeabilità al vapore d'acqua (dp)</skos:prefLabel>
    <skos:inScheme rdf:resource="https://w3id.org/crmrp#Archeometric_and_Diagnostic_Analysis"/>
    <skos:editorialNote xml:lang="it">UNI EN 15803:2010 Conservazione dei beni culturali - Metodi di prova - Determinazione della permeabilità al vapore d'acqua (dp)</skos:editorialNote>
  </rdf:Description>
  <rdf:Description rdf:about="https://w3id.org/crmrp#c_0f7fe37e">
    <skos:editorialNote xml:lang="en">Getty AAT http://vocab.getty.edu/page/aat/300390518</skos:editorialNote>
    <skos:prefLabel xml:lang="en">Mass Spectrometry Matrix-Assisted Laser Desorption/Ionization (MALDI-MS)</skos:prefLabel>
    <skos:exactMatch rdf:resource="http://vocab.getty.edu/page/aat/300390518"/>
    <skos:prefLabel xml:lang="it">Spettrometria di massa  Matrix-Assisted Laser Desorption/Ionization (MALDI-MS)</skos:prefLabel>
    <rdfs:label xml:lang="en">Mass Spectrometry Matrix-Assisted Laser Desorption/Ionization (MALDI-MS)</rdfs:label>
    <skos:topConceptOf rdf:resource="https://w3id.org/crmrp#Archeometric_and_Diagnostic_Analysis"/>
    <skos:inScheme rdf:resource="https://w3id.org/crmrp#Archeometric_and_Diagnostic_Analysis"/>
    <skos:broader rdf:resource="https://w3id.org/crmrp#c_789c3e32"/>
    <rdf:type rdf:resource="http://www.w3.org/2002/07/owl#NamedIndividual"/>
    <skos:definition xml:lang="en">Method of ionizing samples for use in mass spectrometry allowing the analysis of fragile biomolecules and organic molecules which fragment when ionized by other methods. The analyte is prepared in or on an organic matrix that is coated on a surface which is then irradiated by laser photons, removing the analyte from the surface and ionizing it for analysis.</skos:definition>
    <rdf:type rdf:resource="http://www.w3.org/2004/02/skos/core#Concept"/>
  </rdf:Description>
  <rdf:Description rdf:about="https://w3id.org/crmrp#c_502e151f">
    <rdf:type rdf:resource="http://www.w3.org/2004/02/skos/core#Concept"/>
    <rdfs:label xml:lang="en">Fusione all'osso di seppia</rdfs:label>
    <rdf:type rdf:resource="http://www.w3.org/2002/07/owl#NamedIndividual"/>
    <skos:topConceptOf rdf:resource="https://w3id.org/crmrp#Execution_Technique"/>
    <skos:prefLabel xml:lang="it">Fusione all'osso di seppia</skos:prefLabel>
    <skos:prefLabel xml:lang="en">Fusione all'osso di seppia</skos:prefLabel>
    <skos:inScheme rdf:resource="https://w3id.org/crmrp#Execution_Technique"/>
    <skos:definition xml:lang="en">Cuttlebone casting exploits the special characteristics of these types of bones: workability and resistance to molten metal. Two cuttlefish bones are taken and flattened on the softer side, thus creating two matching surfaces on which the negative can be cast.</skos:definition>
    <skos:editorialNote xml:lang="it">A.Giuffredi “Formatura e fonderia”, Alinea editrice, Firenze, 2010</skos:editorialNote>
    <skos:note xml:lang="en">International references could not be found</skos:note>
    <skos:broader rdf:resource="https://w3id.org/crmrp#c_0a9f4d42"/>
  </rdf:Description>
  <rdf:Description rdf:about="https://w3id.org/crmrp#c_615accd9">
    <rdfs:label xml:lang="en">Red chalk</rdfs:label>
    <skos:definition xml:lang="en">Drawing medium made from natural red clay containing iron ocher, ranging in color from reddish brown to blood red. It was used for wall paintings by ancient Egyptians and Romans; in the 16th century it was a popular drawing medium. Originally cut from deposits but later fabricated from the same material.</skos:definition>
    <skos:topConceptOf rdf:resource="https://w3id.org/crmrp#Execution_Technique"/>
    <skos:prefLabel xml:lang="it">Sanguigna</skos:prefLabel>
    <rdf:type rdf:resource="http://www.w3.org/2004/02/skos/core#Concept"/>
    <rdf:type rdf:resource="http://www.w3.org/2002/07/owl#NamedIndividual"/>
    <skos:exactMatch rdf:resource="http://vocab.getty.edu/page/aat/300080064"/>
    <skos:prefLabel xml:lang="en">Red chalk</skos:prefLabel>
    <skos:broader rdf:resource="https://w3id.org/crmrp#c_044b6056"/>
    <skos:inScheme rdf:resource="https://w3id.org/crmrp#Execution_Technique"/>
    <skos:editorialNote xml:lang="en">Getty AAT http://vocab.getty.edu/page/aat/300080064</skos:editorialNote>
  </rdf:Description>
  <rdf:Description rdf:about="https://w3id.org/crmrp#c_4d9c61a1">
    <skos:prefLabel xml:lang="it">Chelante</skos:prefLabel>
    <rdf:type rdf:resource="http://www.w3.org/2004/02/skos/core#Concept"/>
    <skos:prefLabel xml:lang="en">Chelator</skos:prefLabel>
    <skos:definition xml:lang="en">Chelants are substances that can be used to remove metal ions. From an application point of view, this can result in different operations, depending on the type of work being worked on.</skos:definition>
    <skos:note xml:lang="en">International references could not be found</skos:note>
    <rdfs:label xml:lang="en">Chelator</rdfs:label>
    <rdf:type rdf:resource="http://www.w3.org/2002/07/owl#NamedIndividual"/>
    <skos:inScheme rdf:resource="https://w3id.org/crmrp#Intervention"/>
    <skos:editorialNote xml:lang="en">P.Cremonesi, E. Signorini, “Un approccio alla pulitura dei dipinti mobili”, Il Prato, Padova, 2016</skos:editorialNote>
    <skos:topConceptOf rdf:resource="https://w3id.org/crmrp#Intervention"/>
    <skos:broader rdf:resource="https://w3id.org/crmrp#c_5a83cd16"/>
  </rdf:Description>
  <rdf:Description rdf:about="https://w3id.org/crmrp#R3_Graphic_Documentation">
    <rdfs:label xml:lang="en">Graphic Documentation</rdfs:label>
    <rdfs:comment xml:lang="en">This class represents the graphic or cartographic documentation of an object.
Before and during restoration work, it is necessary to produce graphical representations of the conservation state of the artifact before the restoration, showing all alterations and their extent, as well as illustrating the interventions carried out and their area. This can help clients to understand the restoration and restorers to calculate the value of their work.</rdfs:comment>
    <rdfs:subClassOf rdf:resource="http://www.cidoc-crm.org/cidoc-crm/E31_Document"/>
    <rdf:type rdf:resource="http://www.w3.org/2002/07/owl#Class"/>
  </rdf:Description>
  <rdf:Description rdf:about="https://w3id.org/crmrp#RP7_is_post-intervention">
    <rdfs:label xml:lang="en">is post-intervention</rdfs:label>
    <rdfs:comment xml:lang="en">This property links Invasive archaeometric and diagnostic analysis and Non-invasive achaeometric and diagnostic analysis to Intervention.
Indeed, some archaeometric and diagnostic analyses are sometimes repeated before and after specific interventions.</rdfs:comment>
    <rdfs:range rdf:resource="https://w3id.org/crmrp#R8_Intervention"/>
    <rdfs:domain rdf:resource="https://w3id.org/crmrp#R12_Invasive_archaeometric_and_diagnostic_analysis"/>
    <rdfs:domain rdf:resource="https://w3id.org/crmrp#R11_Non-invasive_archaeometric_and_diagnostic_analysis"/>
    <rdf:type rdf:resource="http://www.w3.org/2002/07/owl#ObjectProperty"/>
  </rdf:Description>
  <rdf:Description rdf:about="https://w3id.org/crmrp#c_42b93bd2">
    <skos:inScheme rdf:resource="https://w3id.org/crmrp#Archeometric_and_Diagnostic_Analysis"/>
    <skos:prefLabel xml:lang="it">Riflettografia infrarossa</skos:prefLabel>
    <skos:definition xml:lang="en">Infrared reflectography is a digital imaging technique that allows study of layers beneath the surface of a painting by capturing absorption/emission characteristics of reflected infrared radiation. A complementary technique to x-radiography, IRR uncovers somewhat different information.The longer wavelengths of infrared radiation penetrate most surface pigments and reveal charcoal or graphite underdrawings, the underlying initial stages of a composition</skos:definition>
    <skos:broader rdf:resource="https://w3id.org/crmrp#c_1285fa71"/>
    <skos:editorialNote xml:lang="en">Getty AAT http://vocab.getty.edu/page/aat/300379538</skos:editorialNote>
    <skos:exactMatch rdf:resource="http://vocab.getty.edu/page/aat/300379538"/>
    <skos:prefLabel xml:lang="en">Infra-red reflectography</skos:prefLabel>
    <rdfs:label xml:lang="en">Infra-red reflectography</rdfs:label>
    <rdf:type rdf:resource="http://www.w3.org/2002/07/owl#NamedIndividual"/>
    <rdf:type rdf:resource="http://www.w3.org/2004/02/skos/core#Concept"/>
    <skos:topConceptOf rdf:resource="https://w3id.org/crmrp#Archeometric_and_Diagnostic_Analysis"/>
  </rdf:Description>
  <rdf:Description rdf:about="https://w3id.org/crmrp#c_25bbe064">
    <skos:prefLabel xml:lang="en">Determination of water absorption by capillarity</skos:prefLabel>
    <skos:definition xml:lang="en">Capillary water absorption is the determination of the amount of water absorbed per unit area, as a function of time, at ambient pressure and temperature, by a sample having its base surface in contact with deionised water.</skos:definition>
    <skos:prefLabel xml:lang="it">Determinazione dell'assorbimento d'acqua per capillarità</skos:prefLabel>
    <skos:note xml:lang="en">International references could not be found</skos:note>
    <skos:topConceptOf rdf:resource="https://w3id.org/crmrp#Archeometric_and_Diagnostic_Analysis"/>
    <rdfs:label xml:lang="en">Determination of water absorption by capillarity</rdfs:label>
    <rdf:type rdf:resource="http://www.w3.org/2002/07/owl#NamedIndividual"/>
    <rdf:type rdf:resource="http://www.w3.org/2004/02/skos/core#Concept"/>
    <skos:broader rdf:resource="https://w3id.org/crmrp#c_1fd6102e"/>
    <skos:inScheme rdf:resource="https://w3id.org/crmrp#Archeometric_and_Diagnostic_Analysis"/>
    <skos:editorialNote xml:lang="it">UNI EN 15801:2010 Conservazione dei beni culturali - Metodi di prova - Determinazione dell'assorbimento dell'acqua per capillarità</skos:editorialNote>
  </rdf:Description>
  <rdf:Description rdf:about="https://w3id.org/crmrp#c_607d4549">
    <rdf:type rdf:resource="http://www.w3.org/2002/07/owl#NamedIndividual"/>
    <rdfs:label xml:lang="en">Removal</rdfs:label>
    <skos:altLabel xml:lang="en">Uncovering</skos:altLabel>
    <rdf:type rdf:resource="http://www.w3.org/2004/02/skos/core#Concept"/>
    <skos:topConceptOf rdf:resource="https://w3id.org/crmrp#Intervention"/>
    <skos:note xml:lang="en">The preferred editorial note and the definition closest to the meaning is Getty Conservation Institute “Illustrated Glossary - Definitions of terms used for the graphic documentation of in situ floor mosaics”, “Mosaics In Situ Project”, Los Angeles, 2003</skos:note>
    <skos:inScheme rdf:resource="https://w3id.org/crmrp#Intervention"/>
    <skos:prefLabel xml:lang="it">Rimozione</skos:prefLabel>
    <skos:definition xml:lang="en">The removal of extraneous components from the artwork, such as plastering carried out during past restorations, repainting and/or layers of paintwork.</skos:definition>
    <skos:editorialNote xml:lang="en">Getty Conservation Institute “Illustrated Glossary - Definitions of terms used for the graphic documentation of in situ floor mosaics”, “Mosaics In Situ Project”, Los Angeles, 2003</skos:editorialNote>
    <skos:prefLabel xml:lang="en">Removal</skos:prefLabel>
    <skos:editorialNote xml:lang="en"> A. Weyer et al., “EwaGlos - European Illustrated Glossary of conservation terms for wall paintings and architectural surfaces”, Michael Imhof Verlag, Petersberg, Germany</skos:editorialNote>
  </rdf:Description>
  <rdf:Description rdf:about="https://w3id.org/crmrp#c_f50f0996">
    <skos:editorialNote xml:lang="en">Getty AAT http://vocab.getty.edu/page/aat/300438543</skos:editorialNote>
    <skos:note xml:lang="en">The preferred editorial note and the definition closest to the meaning is Getty AAT</skos:note>
    <skos:topConceptOf rdf:resource="https://w3id.org/crmrp#Intervention"/>
    <skos:editorialNote xml:lang="en">Getty Conservation Institute “Illustrated Glossary - Definitions of terms used for the graphic documentation of in situ floor mosaics”, “Mosaics In Situ Project”, Los Angeles, 2003</skos:editorialNote>
    <rdf:type rdf:resource="http://www.w3.org/2002/07/owl#NamedIndividual"/>
    <skos:closeMatch rdf:resource="http://vocab.getty.edu/page/aat/300438543"/>
    <rdfs:label xml:lang="en">Biocleaning</rdfs:label>
    <skos:prefLabel xml:lang="it">Bonifica</skos:prefLabel>
    <skos:prefLabel xml:lang="en">Biocleaning</skos:prefLabel>
    <rdf:type rdf:resource="http://www.w3.org/2004/02/skos/core#Concept"/>
    <skos:altLabel xml:lang="en">Treatment of microbiological organisms</skos:altLabel>
    <skos:inScheme rdf:resource="https://w3id.org/crmrp#Intervention"/>
    <skos:editorialNote xml:lang="en">A. Weyer et al., “EwaGlos - European Illustrated Glossary of conservation terms for wall paintings and architectural surfaces”, Michael Imhof Verlag, Petersberg, Germany</skos:editorialNote>
    <skos:definition xml:lang="en">Removing dirt, surface coatings, accretions, discolorations, or other undesired matter from a substrate using biological agents e.g. bacteria, enzymes, plant-based surfactants.</skos:definition>
  </rdf:Description>
  <rdf:Description rdf:about="https://w3id.org/crmrp#c_8af455cd">
    <skos:topConceptOf rdf:resource="https://w3id.org/crmrp#Execution_Technique"/>
    <rdf:type rdf:resource="http://www.w3.org/2002/07/owl#NamedIndividual"/>
    <rdf:type rdf:resource="http://www.w3.org/2004/02/skos/core#Concept"/>
    <skos:prefLabel xml:lang="it">Tecnica di doratura</skos:prefLabel>
    <skos:prefLabel xml:lang="en">Gilding technique</skos:prefLabel>
    <rdfs:label xml:lang="en">Gilding technique</rdfs:label>
    <skos:closeMatch rdf:resource="http://vocab.getty.edu/page/aat/300053789"/>
    <skos:definition xml:lang="en">Process involving the surface application of gold or another metal in the form of leaf, powder applied directly to the surface, powder mixed with a binder, electroplating, or other forms to approximate the effect of solid or inlaid metal.</skos:definition>
    <skos:broader rdf:resource="https://w3id.org/crmrp#Execution_Technique"/>
    <skos:inScheme rdf:resource="https://w3id.org/crmrp#Execution_Technique"/>
    <skos:editorialNote xml:lang="en">Getty AAT http://vocab.getty.edu/page/aat/300053789</skos:editorialNote>
  </rdf:Description>
  <rdf:Description rdf:about="https://w3id.org/crmrp#c_7c664d13">
    <skos:prefLabel xml:lang="it">Tomografia assiale computerizzata (TAC)</skos:prefLabel>
    <skos:prefLabel xml:lang="en">Computerised Axial Tomography (CAT)</skos:prefLabel>
    <skos:inScheme rdf:resource="https://w3id.org/crmrp#Archeometric_and_Diagnostic_Analysis"/>
    <skos:editorialNote xml:lang="it">C. Giannini, “Dizionario del restauro - Tecniche diagnostica conservazione”, Nardini Editore, Firenze, 2010</skos:editorialNote>
    <rdfs:label xml:lang="en">Computerised Axial Tomography (CAT)</rdfs:label>
    <skos:broader rdf:resource="https://w3id.org/crmrp#c_1fd6102e"/>
    <skos:note xml:lang="en">International references could not be found, but the preferred editorial note and the definition closest to the meaning is in Diagnostica per i beni culturali</skos:note>
    <skos:editorialNote xml:lang="it">M.Ceroni, G.Elia, “Diagnostica per i beni culturali”, Alinea editrice, Firenze, 2008</skos:editorialNote>
    <rdf:type rdf:resource="http://www.w3.org/2004/02/skos/core#Concept"/>
    <skos:topConceptOf rdf:resource="https://w3id.org/crmrp#Archeometric_and_Diagnostic_Analysis"/>
    <rdf:type rdf:resource="http://www.w3.org/2002/07/owl#NamedIndividual"/>
    <skos:definition xml:lang="en">Reconstruction of radiopacity differences in sections contiguous sections of a solid body, carried out using special radiographic equipment. The subject or sample to be investigated, immobile, is placed along its axis while the X source and the detector move radially in solidarity, detecting the radiopacity.</skos:definition>
  </rdf:Description>
  <rdf:Description rdf:about="https://w3id.org/crmrp#c_71e8a300">
    <rdf:type rdf:resource="http://www.w3.org/2002/07/owl#NamedIndividual"/>
    <skos:topConceptOf rdf:resource="https://w3id.org/crmrp#Documentation"/>
    <rdf:type rdf:resource="http://www.w3.org/2004/02/skos/core#Concept"/>
    <skos:inScheme rdf:resource="https://w3id.org/crmrp#Documentation"/>
    <skos:prefLabel xml:lang="it">Dataset fotogrammetrico</skos:prefLabel>
    <rdfs:label xml:lang="en">Photogrammetric dataset</rdfs:label>
    <skos:note xml:lang="en">International references could not be found</skos:note>
    <skos:broader rdf:resource="https://w3id.org/crmrp#c_773e0829"/>
    <skos:prefLabel xml:lang="en">Photogrammetric dataset</skos:prefLabel>
    <skos:definition xml:lang="en">Collection of all the photographs necessary to obtain a three-dimensional model</skos:definition>
  </rdf:Description>
  <rdf:Description rdf:about="https://w3id.org/crmrp#c_8a709acb">
    <skos:inScheme rdf:resource="https://w3id.org/crmrp#Archeometric_and_Diagnostic_Analysis"/>
    <skos:prefLabel xml:lang="en">Enzyme-linked immunosorbent assay</skos:prefLabel>
    <skos:exactMatch rdf:resource="http://vocab.getty.edu/page/aat/300380512"/>
    <rdf:type rdf:resource="http://www.w3.org/2004/02/skos/core#Concept"/>
    <skos:prefLabel xml:lang="it">Saggio immunoenzimatico</skos:prefLabel>
    <rdf:type rdf:resource="http://www.w3.org/2002/07/owl#NamedIndividual"/>
    <skos:editorialNote xml:lang="en">Getty AAT http://vocab.getty.edu/page/aat/300380512</skos:editorialNote>
    <skos:definition xml:lang="en">Assay technique in which a monoclonal antibody is bound to an enzyme to detect and measure the presence of an antigen in a sample.</skos:definition>
    <skos:broader rdf:resource="https://w3id.org/crmrp#c_abed88a5"/>
    <rdfs:label xml:lang="en">Enzyme-linked immunosorbent assay</rdfs:label>
    <skos:topConceptOf rdf:resource="https://w3id.org/crmrp#Archeometric_and_Diagnostic_Analysis"/>
  </rdf:Description>
  <rdf:Description rdf:about="https://w3id.org/crmrp#c_5cbafe21">
    <skos:prefLabel xml:lang="it">Sbiancamento</skos:prefLabel>
    <skos:note xml:lang="en">The preferred editorial note and the definition closest to the meaning is Uni Cen/Ts 17135:2021</skos:note>
    <rdf:type rdf:resource="http://www.w3.org/2002/07/owl#NamedIndividual"/>
    <skos:editorialNote xml:lang="en">Getty AAT http://vocab.getty.edu/page/aat/300186215</skos:editorialNote>
    <skos:definition xml:lang="en">Haze on a surface</skos:definition>
    <skos:inScheme rdf:resource="https://w3id.org/crmrp#Alteration"/>
    <rdf:type rdf:resource="http://www.w3.org/2004/02/skos/core#Concept"/>
    <skos:prefLabel xml:lang="en">Bloom</skos:prefLabel>
    <skos:topConceptOf rdf:resource="https://w3id.org/crmrp#Alteration"/>
    <skos:exactMatch rdf:resource="http://vocab.getty.edu/page/aat/300186215"/>
    <rdfs:label xml:lang="en">Bloom</rdfs:label>
    <skos:broader rdf:resource="https://w3id.org/crmrp#c_df05cb61"/>
    <skos:editorialNote xml:lang="en">Uni Cen/Ts 17135:2021 - Conservation of cultural heritage. General terms and definitions</skos:editorialNote>
  </rdf:Description>
  <rdf:Description rdf:about="https://w3id.org/crmrp#c_11b3f32e">
    <skos:prefLabel xml:lang="it">Imbarcamento</skos:prefLabel>
    <skos:definition xml:lang="en">A type of warping usually associated with wood when one face of a length of lumber shrinks more than the other, resulting in a bowed curvature. Less commonly this process may occur in stone such as marble, due to residual stresses, anisotropic thermal expansion of calcitic grains, variation of fluid contents, and dissolution processes.</skos:definition>
    <skos:closeMatch rdf:resource="http://vocab.getty.edu/page/aat/300389996"/>
    <rdf:type rdf:resource="http://www.w3.org/2004/02/skos/core#Concept"/>
    <skos:inScheme rdf:resource="https://w3id.org/crmrp#Alteration"/>
    <skos:editorialNote xml:lang="en">Getty AAT http://vocab.getty.edu/page/aat/300389996</skos:editorialNote>
    <skos:prefLabel xml:lang="en">Bowing</skos:prefLabel>
    <rdf:type rdf:resource="http://www.w3.org/2002/07/owl#NamedIndividual"/>
    <skos:topConceptOf rdf:resource="https://w3id.org/crmrp#Alteration"/>
    <rdfs:label xml:lang="en">Bowing</rdfs:label>
    <skos:broader rdf:resource="https://w3id.org/crmrp#c_13f3ce9e"/>
  </rdf:Description>
  <rdf:Description rdf:about="https://w3id.org/crmrp#c_4d471b17">
    <skos:editorialNote xml:lang="it">C. Giannini, “Dizionario del restauro - Tecniche diagnostica conservazione”, Nardini Editore, Firenze, 2010</skos:editorialNote>
    <skos:editorialNote xml:lang="it">G. Pignolo, “Effetti d’oro - Storia e tecnica della doratura nell’arte”, Editrice Compositori, Bologna, 2002</skos:editorialNote>
    <rdf:type rdf:resource="http://www.w3.org/2002/07/owl#NamedIndividual"/>
    <skos:note xml:lang="en">International references could not be found, but the preferred editorial note and the definition closest to the meaning is Effetti d’oro - Storia e tecnica della doratura nell’arte</skos:note>
    <rdf:type rdf:resource="http://www.w3.org/2004/02/skos/core#Concept"/>
    <skos:definition xml:lang="en">Mission gilding is a definitive gilding because an irreversible adhesive is used as a leaf adhesive. The preparation of the object is the same as for gouache gilding, right down to the bolus preparation. Oil mission is more resistant than water mission and is used for objects placed outdoors.</skos:definition>
    <skos:topConceptOf rdf:resource="https://w3id.org/crmrp#Execution_Technique"/>
    <skos:broader rdf:resource="https://w3id.org/crmrp#c_8af455cd"/>
    <rdfs:label xml:lang="en">Size gilding</rdfs:label>
    <skos:prefLabel xml:lang="en">Size gilding</skos:prefLabel>
    <skos:prefLabel xml:lang="it">A missione</skos:prefLabel>
    <skos:inScheme rdf:resource="https://w3id.org/crmrp#Execution_Technique"/>
  </rdf:Description>
  <rdf:Description rdf:about="https://w3id.org/crmrp#c_bfe86ad2">
    <skos:definition xml:lang="en">Chemical patinas always involve a chemical reaction between the metal and the reagent that will be used. Depending on the reagents and the exposure time, different results will occur.</skos:definition>
    <skos:inScheme rdf:resource="https://w3id.org/crmrp#Execution_Technique"/>
    <skos:note xml:lang="en">International references could not be found</skos:note>
    <skos:prefLabel xml:lang="en">Chemical patinatura</skos:prefLabel>
    <rdfs:label xml:lang="en">Chemical patinatura</rdfs:label>
    <rdf:type rdf:resource="http://www.w3.org/2004/02/skos/core#Concept"/>
    <skos:editorialNote xml:lang="it">A.Giuffredi, “Formatura e fonderia”, Alinea editrice, Firenze, 2010</skos:editorialNote>
    <skos:broader rdf:resource="https://w3id.org/crmrp#c_f1c689bb"/>
    <skos:prefLabel xml:lang="it">Patinatura chimica</skos:prefLabel>
    <rdf:type rdf:resource="http://www.w3.org/2002/07/owl#NamedIndividual"/>
    <skos:topConceptOf rdf:resource="https://w3id.org/crmrp#Execution_Technique"/>
  </rdf:Description>
  <rdf:Description rdf:about="https://w3id.org/crmrp#c_0146af00">
    <rdfs:label xml:lang="en">Tempera</rdfs:label>
    <skos:exactMatch rdf:resource="http://vocab.getty.edu/page/aat/300015062"/>
    <skos:definition xml:lang="en">Paint formed of an emulsion of fatty and watery constituents. The standard emulsion is usually created with egg yolk and water, with variants of man-made emulsions created with whole egg, linseed oil, casein glue, gum, or wax.</skos:definition>
    <rdf:type rdf:resource="http://www.w3.org/2002/07/owl#NamedIndividual"/>
    <rdf:type rdf:resource="http://www.w3.org/2004/02/skos/core#Concept"/>
    <skos:topConceptOf rdf:resource="https://w3id.org/crmrp#Execution_Technique"/>
    <skos:broader rdf:resource="https://w3id.org/crmrp#c_051209b3"/>
    <skos:prefLabel xml:lang="it">Tempera</skos:prefLabel>
    <skos:prefLabel xml:lang="en">Tempera</skos:prefLabel>
    <skos:inScheme rdf:resource="https://w3id.org/crmrp#Execution_Technique"/>
    <skos:editorialNote xml:lang="en">Getty AAT http://vocab.getty.edu/page/aat/300015062</skos:editorialNote>
  </rdf:Description>
  <rdf:Description rdf:about="https://w3id.org/crmrp#c_7ee727f3">
    <rdfs:label xml:lang="en">Microscopic analysis</rdfs:label>
    <skos:topConceptOf rdf:resource="https://w3id.org/crmrp#Archeometric_and_Diagnostic_Analysis"/>
    <rdf:type rdf:resource="http://www.w3.org/2004/02/skos/core#Concept"/>
    <skos:editorialNote xml:lang="it">M.Ceroni, G.Elia, “Diagnostica per i beni culturali”, Alinea editrice, Firenze, 2008</skos:editorialNote>
    <skos:prefLabel xml:lang="en">Microscopic analysis</skos:prefLabel>
    <skos:prefLabel xml:lang="it">Microscopia</skos:prefLabel>
    <skos:note xml:lang="en">International references could not be found, but the preferred editorial note and the definition closest to the meaning is in Diagnostica per i beni culturali</skos:note>
    <skos:broader rdf:resource="https://w3id.org/crmrp#c_abed88a5"/>
    <skos:definition xml:lang="en">Optical microscopy is an observation technique capable of producing images magnified images of objects or details of objects that are too small to be observed with the naked eye.</skos:definition>
    <rdf:type rdf:resource="http://www.w3.org/2002/07/owl#NamedIndividual"/>
    <skos:inScheme rdf:resource="https://w3id.org/crmrp#Archeometric_and_Diagnostic_Analysis"/>
  </rdf:Description>
  <rdf:Description rdf:about="https://w3id.org/crmrp#c_a62f8c57">
    <skos:prefLabel xml:lang="it">Consolidamento strutturale</skos:prefLabel>
    <skos:topConceptOf rdf:resource="https://w3id.org/crmrp#Intervention"/>
    <rdf:type rdf:resource="http://www.w3.org/2004/02/skos/core#Concept"/>
    <skos:definition xml:lang="en">Consolidation intervention involving the innermost (structural) layers of the artwork.</skos:definition>
    <skos:broader rdf:resource="https://w3id.org/crmrp#c_b86776d0"/>
    <skos:inScheme rdf:resource="https://w3id.org/crmrp#Intervention"/>
    <rdf:type rdf:resource="http://www.w3.org/2002/07/owl#NamedIndividual"/>
    <skos:note xml:lang="en">International references could not be found</skos:note>
    <rdfs:label xml:lang="en">Structural consolidation</rdfs:label>
    <skos:prefLabel xml:lang="en">Structural consolidation</skos:prefLabel>
  </rdf:Description>
  <rdf:Description rdf:about="https://w3id.org/crmrp#c_07ae8f41">
    <rdf:type rdf:resource="http://www.w3.org/2002/07/owl#NamedIndividual"/>
    <skos:prefLabel xml:lang="en">Mosaics</skos:prefLabel>
    <rdfs:label xml:lang="en">Mosaics</rdfs:label>
    <skos:prefLabel xml:lang="it">Mosaico</skos:prefLabel>
    <rdf:type rdf:resource="http://www.w3.org/2004/02/skos/core#Concept"/>
    <skos:exactMatch rdf:resource="http://vocab.getty.edu/page/aat/300015342"/>
    <skos:editorialNote xml:lang="en">Getty AAT http://vocab.getty.edu/page/aat/300015342</skos:editorialNote>
    <skos:inScheme rdf:resource="https://w3id.org/crmrp#Restoration_Object"/>
    <skos:definition xml:lang="en">Images or patterns composed of small, regularly shaped pieces of durable material, usually stone or colored glass.</skos:definition>
    <skos:topConceptOf rdf:resource="https://w3id.org/crmrp#Restoration_Object"/>
  </rdf:Description>
  <rdf:Description rdf:about="http://www.cidoc-crm.org/extensions/crmsci/O18i_was_altered_by">
    <rdfs:range rdf:resource="http://www.cidoc-crm.org/extensions/crmsci/S18_Alteration"/>
    <rdfs:domain rdf:resource="https://w3id.org/crmrp#R1_Restoration_Object"/>
  </rdf:Description>
  <rdf:Description rdf:about="https://w3id.org/crmrp#c_aa88700b">
    <skos:altLabel xml:lang="en">Warping</skos:altLabel>
    <skos:editorialNote xml:lang="en">Getty AAT http://vocab.getty.edu/page/aat/300155059</skos:editorialNote>
    <rdf:type rdf:resource="http://www.w3.org/2004/02/skos/core#Concept"/>
    <skos:editorialNote xml:lang="en">Uni Cen/Ts 17135:2021 - Conservation of cultural heritage. General terms and definitions</skos:editorialNote>
    <skos:closeMatch rdf:resource="http://vocab.getty.edu/page/aat/300155059"/>
    <skos:prefLabel xml:lang="it">Svirgolatura</skos:prefLabel>
    <skos:broader rdf:resource="https://w3id.org/crmrp#c_13f3ce9e"/>
    <skos:prefLabel xml:lang="en">Warped</skos:prefLabel>
    <rdf:type rdf:resource="http://www.w3.org/2002/07/owl#NamedIndividual"/>
    <skos:inScheme rdf:resource="https://w3id.org/crmrp#Alteration"/>
    <skos:definition xml:lang="en">Exhibiting irregular deformation in more than one plane.</skos:definition>
    <rdfs:label xml:lang="en">Warped</rdfs:label>
    <skos:topConceptOf rdf:resource="https://w3id.org/crmrp#Alteration"/>
  </rdf:Description>
  <rdf:Description rdf:about="https://w3id.org/crmrp#c_3ba05aa7">
    <rdf:type rdf:resource="http://www.w3.org/2004/02/skos/core#Concept"/>
    <skos:prefLabel xml:lang="it">Resistografia</skos:prefLabel>
    <skos:broader rdf:resource="https://w3id.org/crmrp#c_abed88a5"/>
    <rdf:type rdf:resource="http://www.w3.org/2002/07/owl#NamedIndividual"/>
    <skos:topConceptOf rdf:resource="https://w3id.org/crmrp#Archeometric_and_Diagnostic_Analysis"/>
    <skos:editorialNote xml:lang="it">M.Ceroni, G.Elia, “Diagnostica per i beni culturali”, Alinea editrice, Firenze, 2008</skos:editorialNote>
    <skos:note xml:lang="en">International references could not be found</skos:note>
    <rdfs:label xml:lang="en">Resistography</rdfs:label>
    <skos:prefLabel xml:lang="en">Resistography</skos:prefLabel>
    <skos:inScheme rdf:resource="https://w3id.org/crmrp#Archeometric_and_Diagnostic_Analysis"/>
    <skos:definition xml:lang="en">Resistographic analysis allows field diagnosis and visualisation of density variations in timber structures</skos:definition>
  </rdf:Description>
  <rdf:Description rdf:about="https://w3id.org/crmrp#c_044b6056">
    <skos:topConceptOf rdf:resource="https://w3id.org/crmrp#Execution_Technique"/>
    <skos:inScheme rdf:resource="https://w3id.org/crmrp#Execution_Technique"/>
    <skos:prefLabel xml:lang="it">Tecnica su carta</skos:prefLabel>
    <skos:prefLabel xml:lang="en">Paper technique</skos:prefLabel>
    <skos:note xml:lang="en">International references could not be found</skos:note>
    <skos:definition xml:lang="en">Indicates the differences in types of paper art techniques</skos:definition>
    <rdfs:label xml:lang="en">Paper technique</rdfs:label>
    <rdf:type rdf:resource="http://www.w3.org/2004/02/skos/core#Concept"/>
    <rdf:type rdf:resource="http://www.w3.org/2002/07/owl#NamedIndividual"/>
  </rdf:Description>
  <rdf:Description rdf:about="https://w3id.org/crmrp#c_9e69e4dd">
    <skos:definition xml:lang="en">Small animals such as lizards, snakes, insects or plant elements can be faithfully reproduced by placing them in the refractory. During the baking of the moulds, the organic material burns away, leaving the void to be occupied by the metal.</skos:definition>
    <skos:inScheme rdf:resource="https://w3id.org/crmrp#Execution_Technique"/>
    <skos:note xml:lang="en">International references could not be found</skos:note>
    <skos:topConceptOf rdf:resource="https://w3id.org/crmrp#Execution_Technique"/>
    <rdf:type rdf:resource="http://www.w3.org/2004/02/skos/core#Concept"/>
    <rdfs:label xml:lang="en">Fusione dal vero</rdfs:label>
    <rdf:type rdf:resource="http://www.w3.org/2002/07/owl#NamedIndividual"/>
    <skos:broader rdf:resource="https://w3id.org/crmrp#c_0a9f4d42"/>
    <skos:prefLabel xml:lang="it">Fusione dal vero</skos:prefLabel>
    <skos:prefLabel xml:lang="en">Fusione dal vero</skos:prefLabel>
    <skos:editorialNote xml:lang="it">A.Giuffredi “Formatura e fonderia”, Alinea editrice, Firenze, 2010</skos:editorialNote>
  </rdf:Description>
  <rdf:Description rdf:about="https://w3id.org/crmrp#c_1d7e9880">
    <rdf:type rdf:resource="http://www.w3.org/2004/02/skos/core#Concept"/>
    <skos:prefLabel xml:lang="en">Alveolisation</skos:prefLabel>
    <skos:definition xml:lang="en">The formation of numerous cavities of various shapes and sizes on stone.</skos:definition>
    <rdf:type rdf:resource="http://www.w3.org/2002/07/owl#NamedIndividual"/>
    <skos:topConceptOf rdf:resource="https://w3id.org/crmrp#Alteration"/>
    <skos:inScheme rdf:resource="https://w3id.org/crmrp#Alteration"/>
    <skos:editorialNote xml:lang="en">Uni Cen/Ts 17135:2021 - Conservation of cultural heritage. General terms and definitions</skos:editorialNote>
    <skos:editorialNote xml:lang="en">Verg`es-Belmin et al., ICOMOS-ISCS: Illustrated glossary on stone deterioration patterns, vol. XV. Icomos International Council on Monuments and Sites, 2008</skos:editorialNote>
    <rdfs:label xml:lang="en">Alveolisation</rdfs:label>
    <skos:prefLabel xml:lang="it">Alveolizzazione</skos:prefLabel>
    <skos:altLabel xml:lang="en">Alveolization</skos:altLabel>
    <skos:note xml:lang="en">The preferred editorial note and the closest definition to the meaning is Uni Cen/Ts 17135:2021</skos:note>
  </rdf:Description>
  <rdf:Description rdf:about="https://w3id.org/crmrp#c_8ce9910e">
    <rdfs:label xml:lang="en">Architecture</rdfs:label>
    <skos:prefLabel xml:lang="en">Architecture</skos:prefLabel>
    <skos:definition xml:lang="en">Structures or parts of structures that are the result of conscious construction, are of practical use, are relatively stable and permanent, and are of a size and scale appropriate for--but not limited to--habitable buildings. Works of architecture are manifestations of the built environment that is typically classified as fine art, meaning it is generally considered to have aesthetic value, was designed by an architect (whether or not his or her name is known), and constructed with skilled labor.</skos:definition>
    <skos:prefLabel xml:lang="it">Architettura</skos:prefLabel>
    <rdf:type rdf:resource="http://www.w3.org/2004/02/skos/core#Concept"/>
    <skos:exactMatch rdf:resource="http://vocab.getty.edu/page/aat/300263552"/>
    <skos:topConceptOf rdf:resource="https://w3id.org/crmrp#Restoration_Object"/>
    <rdf:type rdf:resource="http://www.w3.org/2002/07/owl#NamedIndividual"/>
    <skos:editorialNote xml:lang="en">Getty AAT http://vocab.getty.edu/page/aat/300263552</skos:editorialNote>
    <skos:inScheme rdf:resource="https://w3id.org/crmrp#Restoration_Object"/>
  </rdf:Description>
  <rdf:Description rdf:about="https://w3id.org/crmrp#c_fca0ce9d">
    <skos:prefLabel xml:lang="it">Pre-consolidamento strutturale</skos:prefLabel>
    <skos:prefLabel xml:lang="en">Structural pre-consolidation</skos:prefLabel>
    <skos:note xml:lang="en">International references could not be found</skos:note>
    <skos:inScheme rdf:resource="https://w3id.org/crmrp#Intervention"/>
    <skos:definition xml:lang="en">Pre-consolidation intervention involving the innermost (structural) layers of the artwork.</skos:definition>
    <skos:broader rdf:resource="https://w3id.org/crmrp#c_e078e94e"/>
    <rdfs:label xml:lang="en">Structural pre-consolidation</rdfs:label>
    <rdf:type rdf:resource="http://www.w3.org/2004/02/skos/core#Concept"/>
    <rdf:type rdf:resource="http://www.w3.org/2002/07/owl#NamedIndividual"/>
  </rdf:Description>
  <rdf:Description rdf:about="https://w3id.org/crmrp#c_f383c4d3">
    <skos:topConceptOf rdf:resource="https://w3id.org/crmrp#Documentation"/>
    <skos:prefLabel xml:lang="it">Documentazione grafica</skos:prefLabel>
    <skos:prefLabel xml:lang="en">Graphic documentation</skos:prefLabel>
    <skos:inScheme rdf:resource="https://w3id.org/crmrp#Documentation"/>
    <skos:definition xml:lang="en">Graphic documentation consists of the correlation of the representation of the artwork itself with that of the information, in the form of a collection of thematic mappings organised by type.</skos:definition>
    <rdfs:label xml:lang="en">Graphic documentation</rdfs:label>
    <rdf:type rdf:resource="http://www.w3.org/2004/02/skos/core#Concept"/>
    <rdf:type rdf:resource="http://www.w3.org/2002/07/owl#NamedIndividual"/>
  </rdf:Description>
  <rdf:Description rdf:about="https://w3id.org/crmrp#c_5422ce57">
    <skos:editorialNote xml:lang="en">Getty AAT http://vocab.getty.edu/page/aat/300011022</skos:editorialNote>
    <skos:exactMatch rdf:resource="http://vocab.getty.edu/page/aat/300011022"/>
    <skos:definition xml:lang="en">Pure metallic element having symbol Pb and atomic number 82; soft, dense ductile metal of a dull gray color, shiny when freshly cut, occuring naturally most often as a sulfide in the mineral galena. Other lead minerals include anglesite (lead sulfate) and cerussite (lead carbonate). Native metallic lead was found and used from about 3600-2600 BCE when the technique for obtaining lead from roasting the sulfide ore (galena) was discovered. Lead was used to make small cast items such as coins and statuettes, plumbing pipes, spires, statues, cisterns, gargoyles, pigments (lead white, litharge, orange mineral, etc.), as a component in pottery glazes, for roofing, flashing, stained glass windows, as a soft solder, and as radiation shielding.</skos:definition>
    <skos:prefLabel xml:lang="en">Lead</skos:prefLabel>
    <skos:topConceptOf rdf:resource="https://w3id.org/crmrp#Material"/>
    <rdf:type rdf:resource="http://www.w3.org/2004/02/skos/core#Concept"/>
    <skos:inScheme rdf:resource="https://w3id.org/crmrp#Material"/>
    <rdfs:label xml:lang="en">Lead</rdfs:label>
    <rdf:type rdf:resource="http://www.w3.org/2002/07/owl#NamedIndividual"/>
    <skos:prefLabel xml:lang="it">Piombo</skos:prefLabel>
    <skos:broader rdf:resource="https://w3id.org/crmrp#c_6407466f"/>
  </rdf:Description>
  <rdf:Description rdf:about="https://w3id.org/crmrp#c_a3f0890c">
    <skos:prefLabel xml:lang="en">Gusset</skos:prefLabel>
    <skos:definition xml:lang="en">Geometrically shaped block of stone, metal or wood that is inserted into a cavity of the same shape during maintenance or restoration work</skos:definition>
    <skos:broader rdf:resource="https://w3id.org/crmrp#c_e8592f3b"/>
    <skos:prefLabel xml:lang="it">Tassello</skos:prefLabel>
    <skos:note xml:lang="en">International references could not be found</skos:note>
    <skos:inScheme rdf:resource="https://w3id.org/crmrp#Intervention"/>
    <rdfs:label xml:lang="en">Gusset</rdfs:label>
    <skos:topConceptOf rdf:resource="https://w3id.org/crmrp#Intervention"/>
    <rdf:type rdf:resource="http://www.w3.org/2002/07/owl#NamedIndividual"/>
    <skos:editorialNote xml:lang="it">C. Giannini, “Dizionario del restauro - Tecniche diagnostica conservazione”, Nardini Editore, Firenze, 2010</skos:editorialNote>
    <rdf:type rdf:resource="http://www.w3.org/2004/02/skos/core#Concept"/>
  </rdf:Description>
  <rdf:Description rdf:about="https://w3id.org/crmrp#c_56afc892">
    <skos:inScheme rdf:resource="https://w3id.org/crmrp#Material"/>
    <rdf:type rdf:resource="http://www.w3.org/2004/02/skos/core#Concept"/>
    <skos:closeMatch xml:lang="en">Stucco</skos:closeMatch>
    <skos:topConceptOf rdf:resource="https://w3id.org/crmrp#Material"/>
    <skos:definition xml:lang="en">The plastic moulding of all kinds of mortars on architectural surfaces for decorative purposes.</skos:definition>
    <rdfs:label xml:lang="en">Stucco</rdfs:label>
    <rdf:type rdf:resource="http://www.w3.org/2002/07/owl#NamedIndividual"/>
    <skos:broader rdf:resource="https://w3id.org/crmrp#c_34d8fe56"/>
    <skos:prefLabel xml:lang="it">Stucco</skos:prefLabel>
    <skos:prefLabel xml:lang="en">Stucco</skos:prefLabel>
    <skos:editorialNote xml:lang="en">A. Weyer et al., “EwaGlos - European Illustrated Glossary of conservation terms for wall paintings and architectural surfaces”, Michael Imhof Verlag, Petersberg, Germany</skos:editorialNote>
  </rdf:Description>
  <rdf:Description rdf:about="https://w3id.org/crmrp#c_24a7d5f2">
    <skos:definition xml:lang="en">Chromatography of volatile substances existing in or converted to a vapor state.</skos:definition>
    <skos:editorialNote xml:lang="en">Getty AAT http://vocab.getty.edu/page/aat/300223948</skos:editorialNote>
    <skos:inScheme rdf:resource="https://w3id.org/crmrp#Archeometric_and_Diagnostic_Analysis"/>
    <rdfs:label xml:lang="en">Gas chromatography (GC)</rdfs:label>
    <skos:prefLabel xml:lang="it">Gas cromatografia (GC)</skos:prefLabel>
    <skos:exactMatch rdf:resource="http://vocab.getty.edu/page/aat/300223948"/>
    <rdf:type rdf:resource="http://www.w3.org/2004/02/skos/core#Concept"/>
    <skos:broader rdf:resource="https://w3id.org/crmrp#c_2d5cde83"/>
    <rdf:type rdf:resource="http://www.w3.org/2002/07/owl#NamedIndividual"/>
    <skos:prefLabel xml:lang="en">Gas chromatography (GC)</skos:prefLabel>
    <skos:topConceptOf rdf:resource="https://w3id.org/crmrp#Archeometric_and_Diagnostic_Analysis"/>
  </rdf:Description>
  <rdf:Description rdf:about="https://w3id.org/crmrp#c_98f7091c">
    <skos:definition xml:lang="en">Refers to an enhanced technique of liquid chromatography developed in the late 1960s in which stationary phase particles are smaller and packed more densely than in traditional liquid chromatography. The mobile phase solvent is then forced through the dense adsorbent by means of a pump. The technique was initially known as high pressure liquid chromatography (HPLC). The acronym remains but with a shift in emphasis to the high performance the method attains.</skos:definition>
    <skos:exactMatch rdf:resource="http://vocab.getty.edu/page/aat/300379487"/>
    <skos:inScheme rdf:resource="https://w3id.org/crmrp#Archeometric_and_Diagnostic_Analysis"/>
    <skos:topConceptOf rdf:resource="https://w3id.org/crmrp#Archeometric_and_Diagnostic_Analysis"/>
    <rdf:type rdf:resource="http://www.w3.org/2002/07/owl#NamedIndividual"/>
    <rdfs:label xml:lang="en">High performance liquid chromatography (HPLC)</rdfs:label>
    <skos:prefLabel xml:lang="it">Cromatografia liquida ad alta pressione (HPLC)</skos:prefLabel>
    <skos:prefLabel xml:lang="en">High performance liquid chromatography (HPLC)</skos:prefLabel>
    <rdf:type rdf:resource="http://www.w3.org/2004/02/skos/core#Concept"/>
    <skos:broader rdf:resource="https://w3id.org/crmrp#c_2d5cde83"/>
    <skos:editorialNote xml:lang="en">Getty AAT http://vocab.getty.edu/page/aat/300379487</skos:editorialNote>
  </rdf:Description>
  <rdf:Description rdf:about="https://w3id.org/crmrp#RP4_is_pre-restoration">
    <rdfs:label xml:lang="en">is pre-restoration</rdfs:label>
    <rdfs:comment xml:lang="en">This property links Invasive archaeometric and diagnostic analysis and Non-invasive achaeometric and diagnostic analysis to Restoration Project.
Indeed, some archaeometric and diagnostic analyses are sometimes repeated before and after the restoration.</rdfs:comment>
    <rdfs:range rdf:resource="https://w3id.org/crmrp#R7_Restoration_Project"/>
    <rdfs:domain rdf:resource="https://w3id.org/crmrp#R12_Invasive_archaeometric_and_diagnostic_analysis"/>
    <rdfs:domain rdf:resource="https://w3id.org/crmrp#R11_Non-invasive_archaeometric_and_diagnostic_analysis"/>
    <rdf:type rdf:resource="http://www.w3.org/2002/07/owl#ObjectProperty"/>
  </rdf:Description>
  <rdf:Description rdf:about="http://www.cidoc-crm.org/cidoc-crm/P165_incorporates">
    <rdfs:range rdf:resource="http://www.cidoc-crm.org/cidoc-crm/E73_Information_Object"/>
    <rdfs:domain rdf:resource="https://w3id.org/crmrp#R6_Video_Documentation"/>
    <rdfs:domain rdf:resource="https://w3id.org/crmrp#R5_Source_and_Document"/>
    <rdfs:domain rdf:resource="https://w3id.org/crmrp#R4_Photographic_Documentation"/>
    <rdfs:domain rdf:resource="https://w3id.org/crmrp#R3_Graphic_Documentation"/>
    <rdfs:domain rdf:resource="https://w3id.org/crmrp#R2_Audio_Documentation"/>
  </rdf:Description>
  <rdf:Description rdf:about="https://w3id.org/crmrp#c_17157ccd">
    <skos:prefLabel xml:lang="it">Tecnica di fonderia</skos:prefLabel>
    <skos:prefLabel xml:lang="en">Moulding / Casting technique</skos:prefLabel>
    <skos:editorialNote xml:lang="it">A.Giuffredi, “Formatura e fonderia”, Alinea editrice, Firenze, 2010</skos:editorialNote>
    <skos:definition xml:lang="en">Giving form to something by use of a mold; usually refers to pressing a material into the mold, as distinct from pouring liquid material into the mold, for which prefer casting.</skos:definition>
    <skos:closeMatch rdf:resource="http://vocab.getty.edu/page/aat/300053134"/>
    <skos:editorialNote xml:lang="en">Getty AAT http://vocab.getty.edu/page/aat/300053104</skos:editorialNote>
    <skos:inScheme rdf:resource="https://w3id.org/crmrp#Execution_Technique"/>
    <skos:topConceptOf rdf:resource="https://w3id.org/crmrp#Execution_Technique"/>
    <rdfs:label xml:lang="en">Moulding / Casting technique</rdfs:label>
    <skos:closeMatch rdf:resource="http://vocab.getty.edu/page/aat/300053104"/>
    <rdf:type rdf:resource="http://www.w3.org/2002/07/owl#NamedIndividual"/>
    <skos:definition xml:lang="en">The act or process of making casts or of shaping in a mold; usually refers to pouring liquid material into a mold, as distinguished from pressing a material into a mold, for which prefer molding.</skos:definition>
    <rdf:type rdf:resource="http://www.w3.org/2004/02/skos/core#Concept"/>
    <skos:editorialNote xml:lang="en">Getty AAT http://vocab.getty.edu/page/aat/300053134</skos:editorialNote>
  </rdf:Description>
  <rdf:Description rdf:about="https://w3id.org/crmrp#c_c41a962a">
    <skos:definition xml:lang="en">Some varieties of enamels and inks need to be applied while the metal surface is hot.</skos:definition>
    <rdfs:label xml:lang="en">Hot-foil patinatura</rdfs:label>
    <skos:broader rdf:resource="https://w3id.org/crmrp#c_e5a56926"/>
    <skos:topConceptOf rdf:resource="https://w3id.org/crmrp#Execution_Technique"/>
    <skos:editorialNote xml:lang="it">A.Giuffredi, “Formatura e fonderia”, Alinea editrice, Firenze</skos:editorialNote>
    <rdf:type rdf:resource="http://www.w3.org/2002/07/owl#NamedIndividual"/>
    <skos:note xml:lang="en">International references could not be found</skos:note>
    <skos:inScheme rdf:resource="https://w3id.org/crmrp#Execution_Technique"/>
    <rdf:type rdf:resource="http://www.w3.org/2004/02/skos/core#Concept"/>
    <skos:prefLabel xml:lang="it">Patinatura dipinta a caldo</skos:prefLabel>
    <skos:prefLabel xml:lang="en">Hot-foil patinatura</skos:prefLabel>
  </rdf:Description>
  <rdf:Description rdf:about="https://w3id.org/crmrp#c_05163919">
    <skos:definition xml:lang="en">Crafted instruments used for scientific purposes and research, in all branches of science.</skos:definition>
    <skos:editorialNote xml:lang="en">Getty AAT http://vocab.getty.edu/page/aat/300122283</skos:editorialNote>
    <rdf:type rdf:resource="http://www.w3.org/2004/02/skos/core#Concept"/>
    <skos:exactMatch rdf:resource="http://vocab.getty.edu/page/aat/300122283"/>
    <skos:prefLabel xml:lang="en">Scientific instruments</skos:prefLabel>
    <rdfs:label xml:lang="en">Scientific instruments</rdfs:label>
    <rdf:type rdf:resource="http://www.w3.org/2002/07/owl#NamedIndividual"/>
    <skos:prefLabel xml:lang="it">Scientifico-tecnologico</skos:prefLabel>
    <skos:topConceptOf rdf:resource="https://w3id.org/crmrp#Restoration_Object"/>
    <skos:inScheme rdf:resource="https://w3id.org/crmrp#Restoration_Object"/>
  </rdf:Description>
  <rdf:Description rdf:about="https://w3id.org/crmrp#c_3b7b721f">
    <skos:topConceptOf rdf:resource="https://w3id.org/crmrp#Intervention"/>
    <skos:prefLabel xml:lang="en">Tonal adjustment</skos:prefLabel>
    <rdfs:label xml:lang="en">Tonal adjustment</rdfs:label>
    <skos:prefLabel xml:lang="it">Abbassamento tonale</skos:prefLabel>
    <skos:definition xml:lang="en">Small losses in the paint layer, in the preparatory layer or in the final layer, caused by wear/use, abrasion or other damage, are reintegrated by means of reducing the tone with transparent glazes (applied using watercolours or any other compatible and adequate binding media).</skos:definition>
    <skos:altLabel xml:lang="en">Glazing</skos:altLabel>
    <skos:broader rdf:resource="https://w3id.org/crmrp#c_326da7e4"/>
    <rdf:type rdf:resource="http://www.w3.org/2002/07/owl#NamedIndividual"/>
    <skos:inScheme rdf:resource="https://w3id.org/crmrp#Intervention"/>
    <skos:editorialNote xml:lang="en">A. Weyer et al., “EwaGlos - European Illustrated Glossary of conservation terms for wall paintings and architectural surfaces”, Michael Imhof Verlag, Petersberg, Germany</skos:editorialNote>
    <rdf:type rdf:resource="http://www.w3.org/2004/02/skos/core#Concept"/>
  </rdf:Description>
  <rdf:Description rdf:about="https://w3id.org/crmrp#c_717419a3">
    <skos:definition xml:lang="en">Protective and/or decorative coat which is applied to architectural surfaces. It is also used for moulding and casting decorative elements.</skos:definition>
    <skos:inScheme rdf:resource="https://w3id.org/crmrp#Material"/>
    <rdf:type rdf:resource="http://www.w3.org/2004/02/skos/core#Concept"/>
    <skos:topConceptOf rdf:resource="https://w3id.org/crmrp#Material"/>
    <rdfs:label xml:lang="en">Plaster</rdfs:label>
    <rdf:type rdf:resource="http://www.w3.org/2002/07/owl#NamedIndividual"/>
    <skos:broader rdf:resource="https://w3id.org/crmrp#c_34d8fe56"/>
    <skos:prefLabel xml:lang="it">Intonaco</skos:prefLabel>
    <skos:prefLabel xml:lang="en">Plaster</skos:prefLabel>
    <skos:editorialNote xml:lang="en">A. Weyer et al., “EwaGlos - European Illustrated Glossary of conservation terms for wall paintings and architectural surfaces”, Michael Imhof Verlag, Petersberg, Germany</skos:editorialNote>
  </rdf:Description>
  <rdf:Description rdf:about="https://w3id.org/crmrp#c_13f3ce9e">
    <skos:exactMatch rdf:resource="http://vocab.getty.edu/page/aat/300072976"/>
    <skos:editorialNote xml:lang="en">A. Weyer et al., “EwaGlos - European Illustrated Glossary of conservation terms for wall paintings and architectural surfaces”, Michael Imhof Verlag, Petersberg, Germany</skos:editorialNote>
    <rdfs:label xml:lang="en">Deformation</rdfs:label>
    <rdf:type rdf:resource="http://www.w3.org/2002/07/owl#NamedIndividual"/>
    <skos:prefLabel xml:lang="it">Deformazione</skos:prefLabel>
    <skos:editorialNote xml:lang="en">Getty AAT http://vocab.getty.edu/page/aat/300072976</skos:editorialNote>
    <skos:prefLabel xml:lang="en">Deformation</skos:prefLabel>
    <skos:note xml:lang="en">The preferred editorial note and the definition closest to the meaning is Uni Cen/Ts 17135:2021</skos:note>
    <skos:topConceptOf rdf:resource="https://w3id.org/crmrp#Alteration"/>
    <skos:definition xml:lang="en">Change, without a break, of the form and/or dimensions of an object</skos:definition>
    <rdf:type rdf:resource="http://www.w3.org/2004/02/skos/core#Concept"/>
    <skos:inScheme rdf:resource="https://w3id.org/crmrp#Alteration"/>
    <skos:editorialNote xml:lang="en">Uni Cen/Ts 17135:2021 - Conservation of cultural heritage. General terms and definitions</skos:editorialNote>
  </rdf:Description>
  <rdf:Description rdf:about="https://w3id.org/crmrp#c_8e940120">
    <rdfs:label xml:lang="en">Mercury porosimetry</rdfs:label>
    <skos:prefLabel xml:lang="en">Mercury porosimetry</skos:prefLabel>
    <skos:exactMatch rdf:resource="http://vocab.getty.edu/page/aat/300379676"/>
    <rdf:type rdf:resource="http://www.w3.org/2004/02/skos/core#Concept"/>
    <skos:prefLabel xml:lang="it">Porosimetria al mercurio</skos:prefLabel>
    <skos:definition xml:lang="en">Porosimetry which uses mercury as the non-wetting liquid pressed into the pores of a material by the porosimeter.</skos:definition>
    <skos:editorialNote xml:lang="en">Getty AAT http://vocab.getty.edu/page/aat/300379676</skos:editorialNote>
    <skos:inScheme rdf:resource="https://w3id.org/crmrp#Archeometric_and_Diagnostic_Analysis"/>
    <skos:topConceptOf rdf:resource="https://w3id.org/crmrp#Archeometric_and_Diagnostic_Analysis"/>
    <skos:broader rdf:resource="https://w3id.org/crmrp#c_abed88a5"/>
    <rdf:type rdf:resource="http://www.w3.org/2002/07/owl#NamedIndividual"/>
  </rdf:Description>
  <rdf:Description rdf:about="https://w3id.org/crmrp#c_df05cb61">
    <skos:inScheme rdf:resource="https://w3id.org/crmrp#Alteration"/>
    <skos:prefLabel xml:lang="it">Alterazione cromatica</skos:prefLabel>
    <skos:editorialNote xml:lang="en">Verg`es-Belmin et al., ICOMOS-ISCS: Illustrated glossary on stone deterioration patterns, vol. XV. Icomos International Council on Monuments and Sites, 2008</skos:editorialNote>
    <skos:editorialNote xml:lang="en">Getty Conservation Institute “Illustrated Glossary - Definitions of terms used for the graphic documentation of in situ floor mosaics”, “Mosaics In Situ Project”, Los Angeles, 2003</skos:editorialNote>
    <skos:topConceptOf rdf:resource="https://w3id.org/crmrp#Alteration"/>
    <skos:altLabel xml:lang="en">Discolouration</skos:altLabel>
    <skos:note xml:lang="en">The preferred editorial note and the definition closest to the meaning is Uni Cen/Ts 17135:2021</skos:note>
    <skos:prefLabel xml:lang="en">Colour alteration</skos:prefLabel>
    <rdfs:label xml:lang="en">Colour alteration</rdfs:label>
    <skos:definition xml:lang="en">Change in at least one of the three colour parameters hue, lightness and chroma.</skos:definition>
    <skos:exactMatch rdf:resource="http://vocab.getty.edu/page/aat/300053045"/>
    <rdf:type rdf:resource="http://www.w3.org/2002/07/owl#NamedIndividual"/>
    <rdf:type rdf:resource="http://www.w3.org/2004/02/skos/core#Concept"/>
    <skos:editorialNote xml:lang="en">Uni Cen/Ts 17135:2021 - Conservation of cultural heritage. General terms and definitions</skos:editorialNote>
    <skos:editorialNote xml:lang="en">Getty AAT http://vocab.getty.edu/page/aat/300053045</skos:editorialNote>
  </rdf:Description>
  <rdf:Description rdf:about="https://w3id.org/crmrp#c_0a9f4d42">
    <skos:editorialNote xml:lang="en">Getty AAT http://vocab.getty.edu/page/aat/300054038</skos:editorialNote>
    <skos:topConceptOf rdf:resource="https://w3id.org/crmrp#Execution_Technique"/>
    <skos:prefLabel xml:lang="it">Tecnica di fonderia</skos:prefLabel>
    <skos:inScheme rdf:resource="https://w3id.org/crmrp#Execution_Technique"/>
    <rdf:type rdf:resource="http://www.w3.org/2004/02/skos/core#Concept"/>
    <rdf:type rdf:resource="http://www.w3.org/2002/07/owl#NamedIndividual"/>
    <skos:closeMatch rdf:resource="http://vocab.getty.edu/page/aat/300054038"/>
    <skos:definition xml:lang="en">Process of melting and pouring materials, such as metal or glass, into a mold; for glass also includes fusing.</skos:definition>
    <skos:prefLabel xml:lang="en">Founding</skos:prefLabel>
    <rdfs:label xml:lang="en">Founding</rdfs:label>
    <skos:editorialNote xml:lang="it">A.Giuffredi “Formatura e fonderia”, Alinea editrice, Firenze, 2010</skos:editorialNote>
  </rdf:Description>
  <rdf:Description rdf:about="https://w3id.org/crmrp#c_06f56dce">
    <skos:editorialNote xml:lang="en">A. Weyer et al., “EwaGlos - European Illustrated Glossary of conservation terms for wall paintings and architectural surfaces”, Michael Imhof Verlag, Petersberg, Germany</skos:editorialNote>
    <skos:topConceptOf rdf:resource="https://w3id.org/crmrp#Alteration"/>
    <rdfs:label xml:lang="en">Rising damp</rdfs:label>
    <skos:prefLabel xml:lang="en">Rising damp</skos:prefLabel>
    <skos:note xml:lang="en">The preferred editorial note and the definition closest to the meaning is EwaGlos - European Illustrated Glossary of conservation terms for wall paintings and architectural surfaces</skos:note>
    <skos:definition xml:lang="en">Dampness in the lower part of buildings resulting from capillary rise of ground water.</skos:definition>
    <skos:prefLabel xml:lang="it">Risalita</skos:prefLabel>
    <rdf:type rdf:resource="http://www.w3.org/2004/02/skos/core#Concept"/>
    <skos:broader rdf:resource="https://w3id.org/crmrp#c_61d92422"/>
    <skos:exactMatch rdf:resource="http://vocab.getty.edu/page/aat/300220162"/>
    <skos:inScheme rdf:resource="https://w3id.org/crmrp#Alteration"/>
    <skos:editorialNote xml:lang="en">Getty AAT http://vocab.getty.edu/page/aat/30022016</skos:editorialNote>
    <rdf:type rdf:resource="http://www.w3.org/2002/07/owl#NamedIndividual"/>
  </rdf:Description>
  <rdf:Description rdf:about="https://w3id.org/crmrp#c_4cd02f85">
    <skos:prefLabel xml:lang="it">Microscopia elettronica a scansione (SEM) corredata di microsonda elettronica (EDS)</skos:prefLabel>
    <skos:editorialNote xml:lang="en">Getty AAT http://vocab.getty.edu/page/aat/300343819</skos:editorialNote>
    <skos:definition xml:lang="en">Electron microscopes designed for directly studying the surfaces of solid objects, utilizing a beam of focused electrons of relatively low energy as an electron probe that is scanned in a regular manner over the specimen. An electrical signal is obtained by collecting and amplifying secondary electrons emitted by the specimen and is applied to a cathode-ray tube scanned in synchronism with the electron beam.</skos:definition>
    <skos:prefLabel xml:lang="en">Scanning electronic microscope (SEM) equipped with electronic micro wave (EDS)</skos:prefLabel>
    <skos:closeMatch rdf:resource="http://vocab.getty.edu/page/aat/300343819"/>
    <rdf:type rdf:resource="http://www.w3.org/2002/07/owl#NamedIndividual"/>
    <skos:topConceptOf rdf:resource="https://w3id.org/crmrp#Archeometric_and_Diagnostic_Analysis"/>
    <rdf:type rdf:resource="http://www.w3.org/2004/02/skos/core#Concept"/>
    <skos:broader rdf:resource="https://w3id.org/crmrp#c_7ee727f3"/>
    <skos:inScheme rdf:resource="https://w3id.org/crmrp#Archeometric_and_Diagnostic_Analysis"/>
    <rdfs:label xml:lang="en">Scanning electronic microscope (SEM) equipped with electronic micro wave (EDS)</rdfs:label>
  </rdf:Description>
  <rdf:Description rdf:about="https://w3id.org/crmrp#c_5a83cd16">
    <rdfs:label xml:lang="en">Chemical cleaning</rdfs:label>
    <rdf:type rdf:resource="http://www.w3.org/2004/02/skos/core#Concept"/>
    <skos:broader rdf:resource="https://w3id.org/crmrp#c_830e6744"/>
    <skos:topConceptOf rdf:resource="https://w3id.org/crmrp#Intervention"/>
    <skos:prefLabel xml:lang="en">Chemical cleaning</skos:prefLabel>
    <skos:editorialNote xml:lang="en">Getty Conservation Institute “Illustrated Glossary - Technician Training for the Maintenance of In Situ Mosaics”, Los Angeles, 2013</skos:editorialNote>
    <rdf:type rdf:resource="http://www.w3.org/2002/07/owl#NamedIndividual"/>
    <skos:prefLabel xml:lang="it">Pulitura chimico-fisica</skos:prefLabel>
    <skos:inScheme rdf:resource="https://w3id.org/crmrp#Intervention"/>
    <skos:definition xml:lang="en">Physico-chemical cleaning aims to dissolve the materials to be removed by means of organic solvents, water and/or chemical reagents.</skos:definition>
  </rdf:Description>
  <rdf:Description rdf:about="https://w3id.org/crmrp#c_227577b2">
    <skos:editorialNote xml:lang="en">Getty AAT http://vocab.getty.edu/page/aat/300053048</skos:editorialNote>
    <skos:note xml:lang="en">The preferred editorial note and the definition closest to the meaning is Uni Cen/Ts 17135:2021</skos:note>
    <rdf:type rdf:resource="http://www.w3.org/2004/02/skos/core#Concept"/>
    <rdf:type rdf:resource="http://www.w3.org/2002/07/owl#NamedIndividual"/>
    <rdfs:label xml:lang="en">Faded</rdfs:label>
    <skos:closeMatch rdf:resource="http://vocab.getty.edu/page/aat/300053048"/>
    <skos:topConceptOf rdf:resource="https://w3id.org/crmrp#Alteration"/>
    <skos:editorialNote xml:lang="en">Uni Cen/Ts 17135:2021 - Conservation of cultural heritage. General terms and definitions</skos:editorialNote>
    <skos:prefLabel xml:lang="it">Sbiadimento</skos:prefLabel>
    <skos:broader rdf:resource="https://w3id.org/crmrp#c_df05cb61"/>
    <skos:prefLabel xml:lang="en">Faded</skos:prefLabel>
    <skos:editorialNote xml:lang="en">A. Weyer et al., “EwaGlos - European Illustrated Glossary of conservation terms for wall paintings and architectural surfaces”, Michael Imhof Verlag, Petersberg, Germany</skos:editorialNote>
    <skos:inScheme rdf:resource="https://w3id.org/crmrp#Alteration"/>
    <skos:definition xml:lang="en">Exhibiting reduced chroma</skos:definition>
  </rdf:Description>
  <rdf:Description rdf:about="https://w3id.org/crmrp#c_c8704394">
    <rdf:type rdf:resource="http://www.w3.org/2002/07/owl#NamedIndividual"/>
    <skos:inScheme rdf:resource="https://w3id.org/crmrp#Intervention"/>
    <skos:editorialNote xml:lang="en">A. Weyer et al., “EwaGlos - European Illustrated Glossary of conservation terms for wall paintings and architectural surfaces”, Michael Imhof Verlag, Petersberg, Germany</skos:editorialNote>
    <skos:broader rdf:resource="https://w3id.org/crmrp#c_326da7e4"/>
    <rdfs:label xml:lang="en">Astrazione cromatica</rdfs:label>
    <skos:definition xml:lang="en">Using four pure colours on a light background applied with short hatched lines, an abstract structure is created. This structure merges optically with the contiguous original.</skos:definition>
    <skos:prefLabel xml:lang="en">Astrazione cromatica</skos:prefLabel>
    <skos:prefLabel xml:lang="it">Astrazione cromatica</skos:prefLabel>
    <skos:topConceptOf rdf:resource="https://w3id.org/crmrp#Intervention"/>
    <rdf:type rdf:resource="http://www.w3.org/2004/02/skos/core#Concept"/>
  </rdf:Description>
  <rdf:Description rdf:about="https://w3id.org/crmrp#c_00c8100f">
    <rdf:type rdf:resource="http://www.w3.org/2004/02/skos/core#Concept"/>
    <skos:prefLabel xml:lang="en">Crust</skos:prefLabel>
    <skos:editorialNote xml:lang="en">Getty AAT http://vocab.getty.edu/page/aat/300220976</skos:editorialNote>
    <skos:inScheme rdf:resource="https://w3id.org/crmrp#Alteration"/>
    <skos:definition xml:lang="en">Distinct outer layer more or less adherent to the surface of an object</skos:definition>
    <skos:closeMatch rdf:resource="http://vocab.getty.edu/page/aat/300220976"/>
    <skos:editorialNote xml:lang="en">Verg`es-Belmin et al., ICOMOS-ISCS: Illustrated glossary on stone deterioration patterns, vol. XV. Icomos International Council on Monuments and Sites, 2008</skos:editorialNote>
    <skos:editorialNote xml:lang="en">Uni Cen/Ts 17135:2021 - Conservation of cultural heritage. General terms and definitions</skos:editorialNote>
    <rdf:type rdf:resource="http://www.w3.org/2002/07/owl#NamedIndividual"/>
    <skos:note xml:lang="en">The preferred editorial note and the definition closest to the meaning is Uni Cen/Ts 17135:2021</skos:note>
    <rdfs:label xml:lang="en">Crust</rdfs:label>
    <skos:topConceptOf rdf:resource="https://w3id.org/crmrp#Alteration"/>
    <skos:prefLabel xml:lang="it">Crosta</skos:prefLabel>
  </rdf:Description>
  <rdf:Description rdf:about="https://w3id.org/crmrp#c_801d2563">
    <skos:inScheme rdf:resource="https://w3id.org/crmrp#Execution_Technique"/>
    <skos:definition xml:lang="en">Pencils with a lead made of graphite.</skos:definition>
    <skos:topConceptOf rdf:resource="https://w3id.org/crmrp#Execution_Technique"/>
    <skos:prefLabel xml:lang="en">Graphite pencils</skos:prefLabel>
    <rdf:type rdf:resource="http://www.w3.org/2004/02/skos/core#Concept"/>
    <skos:exactMatch rdf:resource="http://vocab.getty.edu/page/aat/300022443"/>
    <skos:broader rdf:resource="https://w3id.org/crmrp#c_044b6056"/>
    <rdf:type rdf:resource="http://www.w3.org/2002/07/owl#NamedIndividual"/>
    <skos:editorialNote xml:lang="en">Getty AAT http://vocab.getty.edu/page/aat/300022443</skos:editorialNote>
    <rdfs:label xml:lang="en">Graphite pencils</rdfs:label>
    <skos:prefLabel xml:lang="it">Grafite</skos:prefLabel>
  </rdf:Description>
  <rdf:Description rdf:about="https://w3id.org/crmrp#c_7988bd54">
    <skos:definition xml:lang="en"> The bioluminometer measures the light generated, indicating the level of contamination of a surface.</skos:definition>
    <skos:note xml:lang="en">International references could not be found</skos:note>
    <rdf:type rdf:resource="http://www.w3.org/2004/02/skos/core#Concept"/>
    <skos:inScheme rdf:resource="https://w3id.org/crmrp#Archeometric_and_Diagnostic_Analysis"/>
    <skos:topConceptOf rdf:resource="https://w3id.org/crmrp#Archeometric_and_Diagnostic_Analysis"/>
    <rdf:type rdf:resource="http://www.w3.org/2002/07/owl#NamedIndividual"/>
    <skos:broader rdf:resource="https://w3id.org/crmrp#c_1fd6102e"/>
    <skos:prefLabel xml:lang="en">Bioluminometric analysis</skos:prefLabel>
    <skos:prefLabel xml:lang="it">Analisi bioluminometrica</skos:prefLabel>
    <rdfs:label xml:lang="en">Bioluminometric analysis</rdfs:label>
  </rdf:Description>
  <rdf:Description rdf:about="https://w3id.org/crmrp#c_a08009f4">
    <skos:editorialNote xml:lang="en">Getty AAT http://vocab.getty.edu/page/aat/300078735</skos:editorialNote>
    <rdf:type rdf:resource="http://www.w3.org/2002/07/owl#NamedIndividual"/>
    <skos:definition xml:lang="en">The process by which a fresco is detached from a wall, used when the plaster on which it is painted has greatly deteriorated; the color layer is removed by a strong glue without removing excessive amounts of plaster.</skos:definition>
    <rdf:type rdf:resource="http://www.w3.org/2004/02/skos/core#Concept"/>
    <skos:inScheme rdf:resource="https://w3id.org/crmrp#Intervention"/>
    <rdfs:label xml:lang="en">Strappo</rdfs:label>
    <skos:broader rdf:resource="https://w3id.org/crmrp#c_4fe4d308"/>
    <skos:exactMatch rdf:resource="http://vocab.getty.edu/page/aat/300078735"/>
    <skos:prefLabel xml:lang="en">Strappo</skos:prefLabel>
    <skos:topConceptOf rdf:resource="https://w3id.org/crmrp#Intervention"/>
    <skos:note xml:lang="en">The preferred editorial note and the definition closest to the meaning is Getty AAT</skos:note>
    <skos:editorialNote xml:lang="en">A. Weyer et al., “EwaGlos - European Illustrated Glossary of conservation terms for wall paintings and architectural surfaces”, Michael Imhof Verlag, Petersberg, Germany</skos:editorialNote>
  </rdf:Description>
  <rdf:Description rdf:about="https://w3id.org/crmrp#c_f1e8854b">
    <skos:definition xml:lang="en">A method of casting metal or glass in a mold, the cavity of which, or the positive of the form to be made, is formed with wax which is then melted or burned off, and displaced by molten metal or glass.</skos:definition>
    <skos:broader rdf:resource="https://w3id.org/crmrp#c_0a9f4d42"/>
    <skos:inScheme rdf:resource="https://w3id.org/crmrp#Execution_Technique"/>
    <rdfs:label xml:lang="en">Lost wax process</rdfs:label>
    <skos:prefLabel xml:lang="en">Lost wax process</skos:prefLabel>
    <rdf:type rdf:resource="http://www.w3.org/2002/07/owl#NamedIndividual"/>
    <rdf:type rdf:resource="http://www.w3.org/2004/02/skos/core#Concept"/>
    <skos:exactMatch rdf:resource="http://vocab.getty.edu/page/aat/300053113"/>
    <skos:prefLabel xml:lang="it">Fusione a cera persa</skos:prefLabel>
    <skos:editorialNote xml:lang="en">Getty AAT http://vocab.getty.edu/page/aat/300053113</skos:editorialNote>
    <skos:topConceptOf rdf:resource="https://w3id.org/crmrp#Execution_Technique"/>
  </rdf:Description>
  <rdf:Description rdf:about="https://w3id.org/crmrp#c_e8592f3b">
    <skos:note xml:lang="en">International references could not be found</skos:note>
    <skos:prefLabel xml:lang="en">Support restoration</skos:prefLabel>
    <skos:definition xml:lang="en">Restoration work on a wooden support involving the replacement of degraded parts with additions. The lemma is also used in a more general sense to indicate direct interventions on the artistic artefact aimed at eliminating phenomena of degradation that jeopardise its conservation (disinfestation, dehumidification, desalinisation).</skos:definition>
    <skos:topConceptOf rdf:resource="https://w3id.org/crmrp#Intervention"/>
    <skos:prefLabel xml:lang="it">Risanamento del supporto</skos:prefLabel>
    <rdfs:label xml:lang="en">Support restoration</rdfs:label>
    <rdf:type rdf:resource="http://www.w3.org/2002/07/owl#NamedIndividual"/>
    <skos:inScheme rdf:resource="https://w3id.org/crmrp#Intervention"/>
    <rdf:type rdf:resource="http://www.w3.org/2004/02/skos/core#Concept"/>
    <skos:editorialNote xml:lang="it">C. Giannini, “Dizionario del restauro - Tecniche diagnostica conservazione”, Nardini Editore, Firenze, 2010</skos:editorialNote>
  </rdf:Description>
  <rdf:Description rdf:about="https://w3id.org/crmrp#c_6626f18c">
    <skos:topConceptOf rdf:resource="https://w3id.org/crmrp#Execution_Technique"/>
    <skos:prefLabel xml:lang="it">Tecnica dipinto murale</skos:prefLabel>
    <skos:prefLabel xml:lang="en">Wall painting</skos:prefLabel>
    <skos:note xml:lang="en">International references could not be found</skos:note>
    <skos:inScheme rdf:resource="https://w3id.org/crmrp#Execution_Technique"/>
    <skos:editorialNote xml:lang="en">A. Weyer et al., “EwaGlos - European Illustrated Glossary of conservation terms for wall paintings and architectural surfaces”, Michael Imhof Verlag, Petersberg, Germany</skos:editorialNote>
    <rdfs:label xml:lang="en">Wall painting</rdfs:label>
    <rdf:type rdf:resource="http://www.w3.org/2004/02/skos/core#Concept"/>
    <rdf:type rdf:resource="http://www.w3.org/2002/07/owl#NamedIndividual"/>
  </rdf:Description>
  <rdf:Description rdf:about="https://w3id.org/crmrp#c_342e7fe6">
    <skos:note xml:lang="en">International references could not be found</skos:note>
    <skos:editorialNote xml:lang="it">C. Giannini, “Dizionario del restauro - Tecniche diagnostica conservazione”, Nardini Editore, Firenze, 2010</skos:editorialNote>
    <skos:definition xml:lang="en">Deformation of tapestries, canvases and large paper supports due to the prolonged action of their own weight.</skos:definition>
    <rdf:type rdf:resource="http://www.w3.org/2004/02/skos/core#Concept"/>
    <rdfs:label xml:lang="en">Sagging</rdfs:label>
    <skos:prefLabel xml:lang="en">Sagging</skos:prefLabel>
    <skos:topConceptOf rdf:resource="https://w3id.org/crmrp#Alteration"/>
    <skos:inScheme rdf:resource="https://w3id.org/crmrp#Alteration"/>
    <skos:prefLabel xml:lang="it">Afflosciamento</skos:prefLabel>
    <skos:broader rdf:resource="https://w3id.org/crmrp#c_13f3ce9e"/>
    <rdf:type rdf:resource="http://www.w3.org/2002/07/owl#NamedIndividual"/>
  </rdf:Description>
  <rdf:Description rdf:about="https://w3id.org/crmrp#c_c202f020">
    <skos:inScheme rdf:resource="https://w3id.org/crmrp#Archeometric_and_Diagnostic_Analysis"/>
    <skos:prefLabel xml:lang="en">Stratigraphic investigation</skos:prefLabel>
    <rdf:type rdf:resource="http://www.w3.org/2004/02/skos/core#Concept"/>
    <rdf:type rdf:resource="http://www.w3.org/2002/07/owl#NamedIndividual"/>
    <skos:editorialNote xml:lang="en">A. Weyer et al., “EwaGlos - European Illustrated Glossary of conservation terms for wall paintings and architectural surfaces”, Michael Imhof Verlag, Petersberg, Germany</skos:editorialNote>
    <skos:topConceptOf rdf:resource="https://w3id.org/crmrp#Archeometric_and_Diagnostic_Analysis"/>
    <skos:definition xml:lang="en">The stepwise removal of covering paint layers for analysis and determination of the chronological order of successive paint layers.</skos:definition>
    <skos:prefLabel xml:lang="it">Saggio stratigrafico</skos:prefLabel>
    <rdfs:label xml:lang="en">Stratigraphic investigation</rdfs:label>
    <skos:broader rdf:resource="https://w3id.org/crmrp#c_abed88a5"/>
  </rdf:Description>
  <rdf:Description rdf:about="https://w3id.org/crmrp#c_773e0829">
    <skos:note xml:lang="en">International references could not be found</skos:note>
    <skos:prefLabel xml:lang="it">Documentazione fotografica</skos:prefLabel>
    <skos:altLabel xml:lang="en">Photodocumentation</skos:altLabel>
    <rdf:type rdf:resource="http://www.w3.org/2002/07/owl#NamedIndividual"/>
    <rdf:type rdf:resource="http://www.w3.org/2004/02/skos/core#Concept"/>
    <skos:topConceptOf rdf:resource="https://w3id.org/crmrp#Documentation"/>
    <skos:inScheme rdf:resource="https://w3id.org/crmrp#Documentation"/>
    <skos:definition xml:lang="en">The collection of all photographs concerning the work of art in question</skos:definition>
    <skos:prefLabel xml:lang="en">Photo documentation</skos:prefLabel>
    <rdfs:label xml:lang="en">Photo documentation</rdfs:label>
  </rdf:Description>
  <rdf:Description rdf:about="https://w3id.org/crmrp#c_77acfccf">
    <rdf:type rdf:resource="http://www.w3.org/2004/02/skos/core#Concept"/>
    <skos:broader rdf:resource="https://w3id.org/crmrp#c_143349b9"/>
    <rdfs:label xml:lang="en">Tempera</rdfs:label>
    <skos:editorialNote xml:lang="en">Getty AAT http://vocab.getty.edu/page/aat/300015062</skos:editorialNote>
    <skos:broader rdf:resource="https://w3id.org/crmrp#c_051209b3"/>
    <skos:prefLabel xml:lang="it">Tempera</skos:prefLabel>
    <skos:prefLabel xml:lang="en">Tempera</skos:prefLabel>
    <rdf:type rdf:resource="http://www.w3.org/2002/07/owl#NamedIndividual"/>
    <skos:topConceptOf rdf:resource="https://w3id.org/crmrp#Execution_Technique"/>
    <skos:broader rdf:resource="https://w3id.org/crmrp#c_044b6056"/>
    <skos:exactMatch rdf:resource="http://vocab.getty.edu/page/aat/300015062"/>
    <skos:definition xml:lang="en">Paint formed of an emulsion of fatty and watery constituents. The standard emulsion is usually created with egg yolk and water, with variants of man-made emulsions created with whole egg, linseed oil, casein glue, gum, or wax.</skos:definition>
    <skos:inScheme rdf:resource="https://w3id.org/crmrp#Execution_Technique"/>
  </rdf:Description>
  <rdf:Description rdf:about="https://w3id.org/crmrp#c_01fedc05">
    <skos:inScheme rdf:resource="https://w3id.org/crmrp#Material"/>
    <skos:prefLabel xml:lang="en">Bronze</skos:prefLabel>
    <rdf:type rdf:resource="http://www.w3.org/2002/07/owl#NamedIndividual"/>
    <rdfs:label xml:lang="en">Bronze</rdfs:label>
    <skos:exactMatch rdf:resource="http://vocab.getty.edu/page/aat/300010957"/>
    <skos:topConceptOf rdf:resource="https://w3id.org/crmrp#Material"/>
    <skos:prefLabel xml:lang="it">Bronzo</skos:prefLabel>
    <skos:definition xml:lang="en">Refers to a broad range of alloys of copper, specifically any non-ferrous alloy of copper, tin, and zinc or other trace metals. Bronze was made before 3,000 BCE -- possibly as early as 10,000 BCE, although its common use in tools and decorative items is dated only in later artifacts. The proportions of copper and tin vary widely, from 70 to 95 percent copper in surviving ancient artifacts. Because of the copper base, bronze may be very malleable and easy to work. By the Middle Ages in Europe, it was recognized that using the metals in certain proportions could yield specific properties. Some modern bronzes contain no tin at all, substituting other metals such as aluminum, manganese, and even zinc. Historically, the term was used interchangeably with latten. U.S. standard bronze is composed of 90% copper, 7% tin and 3% zinc. Ancient bronze alloys sometimes contained up to 14% tin. </skos:definition>
    <rdf:type rdf:resource="http://www.w3.org/2004/02/skos/core#Concept"/>
    <skos:broader rdf:resource="https://w3id.org/crmrp#c_6407466f"/>
    <skos:editorialNote xml:lang="en">Getty AAT http://vocab.getty.edu/page/aat/300010957</skos:editorialNote>
  </rdf:Description>
  <rdf:Description rdf:about="https://w3id.org/crmrp#Intervention">
    <skos:altLabel xml:lang="it">Restauro</skos:altLabel>
    <skos:altLabel xml:lang="en">Restoration</skos:altLabel>
    <skos:prefLabel xml:lang="it">Intervento</skos:prefLabel>
    <skos:prefLabel xml:lang="en">Intervention</skos:prefLabel>
    <skos:note xml:lang="en">International references could not be found</skos:note>
    <skos:editorialNote xml:lang="en">Uni En 15898:2019 Conservazione del patrimonio culturale - Termini generali e definizioni</skos:editorialNote>
    <skos:definition xml:lang="en">Actions performed on an object under stable or stabilised conditions, aimed at improving its appreciation, understanding and/or enjoyment, respecting and/or highlighting its cultural relevance, materials and techniques used.</skos:definition>
    <rdf:type rdf:resource="http://www.w3.org/2004/02/skos/core#ConceptScheme"/>
    <rdf:type rdf:resource="http://www.w3.org/2002/07/owl#NamedIndividual"/>
  </rdf:Description>
  <rdf:Description rdf:about="https://w3id.org/crmrp#c_6278f32b">
    <rdf:type rdf:resource="http://www.w3.org/2004/02/skos/core#Concept"/>
    <skos:inScheme rdf:resource="https://w3id.org/crmrp#Archeometric_and_Diagnostic_Analysis"/>
    <skos:prefLabel xml:lang="it">Radiografia</skos:prefLabel>
    <rdfs:label xml:lang="en">Radiography</rdfs:label>
    <rdf:type rdf:resource="http://www.w3.org/2002/07/owl#NamedIndividual"/>
    <skos:definition xml:lang="en">The making of radiographs, images produced on photographic film by a radiation other than light, especially x-rays or gamma rays. Modern radiography systems are moving away from x-ray sensitive film to produce these images, with a digital plate replacing film.</skos:definition>
    <skos:editorialNote xml:lang="en">Getty AAT http://vocab.getty.edu/page/aat/300053450</skos:editorialNote>
    <skos:topConceptOf rdf:resource="https://w3id.org/crmrp#Archeometric_and_Diagnostic_Analysis"/>
    <skos:broader rdf:resource="https://w3id.org/crmrp#c_1fd6102e"/>
    <skos:exactMatch rdf:resource="http://vocab.getty.edu/page/aat/300053450"/>
    <skos:prefLabel xml:lang="en">Radiography</skos:prefLabel>
  </rdf:Description>
  <rdf:Description rdf:about="https://w3id.org/crmrp#c_ff5d2cf3">
    <skos:definition xml:lang="en">Paint with a base that is polymer, which is compound formed by the combination of two or more molecules of the same substance to produce a new compound with the same empirical formula but with higher molecular weight. It is typically made from pigments in an acrylic resin or vinyl resin, which are polymers, or a combination of both resins. It is water based, spreads out in a layer, and forms a continuous, flexible, and waterproof film of plastic when the water evaporates.</skos:definition>
    <skos:exactMatch rdf:resource="http://vocab.getty.edu/page/aat/300015055"/>
    <skos:topConceptOf rdf:resource="https://w3id.org/crmrp#Execution_Technique"/>
    <rdf:type rdf:resource="http://www.w3.org/2004/02/skos/core#Concept"/>
    <skos:broader rdf:resource="https://w3id.org/crmrp#c_044b6056"/>
    <skos:inScheme rdf:resource="https://w3id.org/crmrp#Execution_Technique"/>
    <skos:editorialNote xml:lang="en">Getty AAT http://vocab.getty.edu/page/aat/300015055</skos:editorialNote>
    <rdfs:label xml:lang="en">Polymer paint</rdfs:label>
    <skos:prefLabel xml:lang="it">Polimero sintetico</skos:prefLabel>
    <rdf:type rdf:resource="http://www.w3.org/2002/07/owl#NamedIndividual"/>
    <skos:prefLabel xml:lang="en">Polymer paint</skos:prefLabel>
  </rdf:Description>
  <rdf:Description rdf:about="https://w3id.org/crmrp#c_aee6a805">
    <rdfs:label xml:lang="en">Etching technique</rdfs:label>
    <skos:closeMatch rdf:resource="http://vocab.getty.edu/page/aat/300053241"/>
    <rdf:type rdf:resource="http://www.w3.org/2004/02/skos/core#Concept"/>
    <skos:topConceptOf rdf:resource="https://w3id.org/crmrp#Execution_Technique"/>
    <skos:inScheme rdf:resource="https://w3id.org/crmrp#Execution_Technique"/>
    <skos:prefLabel xml:lang="it">Tecnica incisione</skos:prefLabel>
    <skos:definition xml:lang="en">Intaglio process in which the design is worked into an acid-resistant substance coating the metal printing plate; the plate is then exposed to acid, which etches the plate where the metal is exposed, to create lines and dark areas. For the single step of exposing the plate to acid, use biting.</skos:definition>
    <skos:editorialNote xml:lang="en">Getty AAT http://vocab.getty.edu/page/aat/300053241</skos:editorialNote>
    <rdf:type rdf:resource="http://www.w3.org/2002/07/owl#NamedIndividual"/>
    <skos:prefLabel xml:lang="en">Etching technique</skos:prefLabel>
  </rdf:Description>
  <rdf:Description rdf:about="https://w3id.org/crmrp#c_6920ec3f">
    <skos:topConceptOf rdf:resource="https://w3id.org/crmrp#Execution_Technique"/>
    <skos:prefLabel xml:lang="it">Tempera grassa</skos:prefLabel>
    <skos:inScheme rdf:resource="https://w3id.org/crmrp#Execution_Technique"/>
    <skos:prefLabel xml:lang="en">Tempera grassa</skos:prefLabel>
    <skos:editorialNote xml:lang="it">C. Giannini, “Dizionario del restauro - Tecniche diagnostica conservazione”, Nardini Editore, Firenze, 2010</skos:editorialNote>
    <rdf:type rdf:resource="http://www.w3.org/2004/02/skos/core#Concept"/>
    <skos:definition xml:lang="en">Tempera grassa is produced by mixing egg yolk with linseed oil. Used extensively in the 15th century with the emergence of the first paintings on canvas following Flemish influence.</skos:definition>
    <rdfs:label xml:lang="en">Tempera grassa</rdfs:label>
    <skos:note xml:lang="en">It was decided not to proceed with the English translation in order to avoid possible lexical errors and misunderstandings.</skos:note>
    <skos:broader rdf:resource="https://w3id.org/crmrp#c_77acfccf"/>
    <rdf:type rdf:resource="http://www.w3.org/2002/07/owl#NamedIndividual"/>
  </rdf:Description>
  <rdf:Description rdf:about="https://w3id.org/crmrp#c_ae6d1fdc">
    <skos:broader rdf:resource="https://w3id.org/crmrp#c_e5a56926"/>
    <skos:editorialNote xml:lang="it">A.Giuffredi, “Formatura e fonderia”, Alinea editrice, Firenze</skos:editorialNote>
    <skos:prefLabel xml:lang="en">Cold patinatura</skos:prefLabel>
    <skos:definition xml:lang="en">Some varieties of enamels and inks need to be applied while the metal surface is hot.</skos:definition>
    <rdf:type rdf:resource="http://www.w3.org/2002/07/owl#NamedIndividual"/>
    <skos:note xml:lang="en">International references could not be found</skos:note>
    <rdfs:label xml:lang="en">Cold patinatura</rdfs:label>
    <skos:inScheme rdf:resource="https://w3id.org/crmrp#Execution_Technique"/>
    <skos:prefLabel xml:lang="it">Patinatura dipinta a freddo</skos:prefLabel>
    <skos:topConceptOf rdf:resource="https://w3id.org/crmrp#Execution_Technique"/>
    <rdf:type rdf:resource="http://www.w3.org/2004/02/skos/core#Concept"/>
  </rdf:Description>
  <rdf:Description rdf:about="https://w3id.org/crmrp#c_41624a1a">
    <rdf:type rdf:resource="http://www.w3.org/2004/02/skos/core#Concept"/>
    <skos:topConceptOf rdf:resource="https://w3id.org/crmrp#Restoration_Object"/>
    <skos:prefLabel xml:lang="it">Paleontologico</skos:prefLabel>
    <skos:closeMatch rdf:resource="http://vocab.getty.edu/page/aat/300265420"/>
    <skos:editorialNote xml:lang="en">Getty AAT http://vocab.getty.edu/page/aat/300265420</skos:editorialNote>
    <rdfs:label xml:lang="en">Palaentological</rdfs:label>
    <skos:definition xml:lang="en">Materials or items left of a thing or things after other parts have been removed, used, or destroyed. Examples include substances of organic origin that are entirely or partially preserved, often in the earth, in a conserved or fossilized condition, including what is left of a person or animal when life is extinct. May also include artifacts, ruins, and other remanants of a person or civilization.</skos:definition>
    <skos:altLabel xml:lang="en">remains (object genre)</skos:altLabel>
    <skos:prefLabel xml:lang="en">Palaentological</skos:prefLabel>
    <rdf:type rdf:resource="http://www.w3.org/2002/07/owl#NamedIndividual"/>
    <skos:inScheme rdf:resource="https://w3id.org/crmrp#Restoration_Object"/>
  </rdf:Description>
  <rdf:Description rdf:about="https://w3id.org/crmrp#R12_Invasive_archaeometric_and_diagnostic_analysis">
    <rdfs:label xml:lang="en">Invasive archaeometric and diagnostic analysis</rdfs:label>
    <rdfs:comment xml:lang="en">This class describes the invasive investigations.
To get very specific results, it is sometimes necessary to choose invasive invesstigations.</rdfs:comment>
    <rdfs:subClassOf rdf:resource="http://www.cidoc-crm.org/extensions/crmsci/S3_Measurement_by_Sampling"/>
    <rdf:type rdf:resource="http://www.w3.org/2002/07/owl#Class"/>
  </rdf:Description>
  <rdf:Description rdf:about="https://w3id.org/crmrp#c_1b40d0c6">
    <skos:prefLabel xml:lang="en">Relief</skos:prefLabel>
    <skos:closeMatch rdf:resource="http://vocab.getty.edu/page/aat/300053622"/>
    <skos:inScheme rdf:resource="https://w3id.org/crmrp#Restoration_Object"/>
    <skos:topConceptOf rdf:resource="https://w3id.org/crmrp#Restoration_Object"/>
    <skos:editorialNote xml:lang="en">Getty AAT http://vocab.getty.edu/page/aat/300053622</skos:editorialNote>
    <skos:definition xml:lang="en">Use to describe a surface that has been carved, molded, or stamped so that an image or design projects from or is sunk into a continuous surface.</skos:definition>
    <skos:broader rdf:resource="https://w3id.org/crmrp#c_160c713a"/>
    <rdf:type rdf:resource="http://www.w3.org/2002/07/owl#NamedIndividual"/>
    <rdfs:label xml:lang="en">Relief</rdfs:label>
    <rdf:type rdf:resource="http://www.w3.org/2004/02/skos/core#Concept"/>
    <skos:prefLabel xml:lang="it">Rilievo</skos:prefLabel>
  </rdf:Description>
  <rdf:Description rdf:about="https://w3id.org/crmrp#c_b1c12a4d">
    <skos:definition xml:lang="en">General term for various combinations of ground, powdery pigment and aqueous binder that are used in drawing and dry painting, delivered via a crayon or stick. Pastel as a material is soft and blendable. For the crayons or sticks containing the pigment and binder, use pastels (crayons).</skos:definition>
    <skos:prefLabel xml:lang="en">Pastel</skos:prefLabel>
    <skos:inScheme rdf:resource="https://w3id.org/crmrp#Execution_Technique"/>
    <rdf:type rdf:resource="http://www.w3.org/2004/02/skos/core#Concept"/>
    <skos:prefLabel xml:lang="it">Pastello</skos:prefLabel>
    <skos:exactMatch rdf:resource="http://vocab.getty.edu/page/aat/300404632"/>
    <skos:broader rdf:resource="https://w3id.org/crmrp#c_044b6056"/>
    <rdfs:label xml:lang="en">Pastel</rdfs:label>
    <rdf:type rdf:resource="http://www.w3.org/2002/07/owl#NamedIndividual"/>
    <skos:topConceptOf rdf:resource="https://w3id.org/crmrp#Execution_Technique"/>
    <skos:editorialNote xml:lang="en">Getty AAT http://vocab.getty.edu/page/aat/300404632</skos:editorialNote>
  </rdf:Description>
  <rdf:Description rdf:about="https://w3id.org/crmrp#c_86abb308">
    <rdf:type rdf:resource="http://www.w3.org/2002/07/owl#NamedIndividual"/>
    <skos:inScheme rdf:resource="https://w3id.org/crmrp#Material"/>
    <skos:topConceptOf rdf:resource="https://w3id.org/crmrp#Material"/>
    <skos:prefLabel xml:lang="it">Ferro</skos:prefLabel>
    <skos:exactMatch rdf:resource="http://vocab.getty.edu/page/aat/300011002"/>
    <skos:prefLabel xml:lang="en">Iron</skos:prefLabel>
    <skos:editorialNote xml:lang="en">Getty AAT http://vocab.getty.edu/page/aat/300011002</skos:editorialNote>
    <skos:broader rdf:resource="https://w3id.org/crmrp#c_6407466f"/>
    <rdfs:label xml:lang="en">Iron</rdfs:label>
    <skos:definition xml:lang="en">Pure metallic element having symbol Fe and atomic number 26; metallic iron is silvery in color, lustrous, soft, ductile, malleable, and slightly magnetic; it rusts when exposed to moist air. It is rarely found as a native metal (telluric iron) except in meteorites (meteoric iron). Iron is most often found throughout the world as iron oxides (hematite, magnetite, limonite, and siderite) mixed with other ores.</skos:definition>
    <rdf:type rdf:resource="http://www.w3.org/2004/02/skos/core#Concept"/>
  </rdf:Description>
  <rdf:Description rdf:about="https://w3id.org/crmrp#c_7548d8b4">
    <rdf:type rdf:resource="http://www.w3.org/2004/02/skos/core#Concept"/>
    <skos:topConceptOf rdf:resource="https://w3id.org/crmrp#Material"/>
    <skos:inScheme rdf:resource="https://w3id.org/crmrp#Material"/>
    <skos:prefLabel xml:lang="en">Synthetic polymer</skos:prefLabel>
    <skos:definition xml:lang="en">High molecular weight compounds formed by the combination of one or more monomers, formed by the multiplication of molecules of the same species to produce a new compound with the same empirical formula but with higher molecular weight. Use copolymers for materials that combine molecules of differing chemical compounds.</skos:definition>
    <skos:closeMatch rdf:resource="http://vocab.getty.edu/page/aat/300218300"/>
    <rdf:type rdf:resource="http://www.w3.org/2002/07/owl#NamedIndividual"/>
    <skos:editorialNote xml:lang="en">Getty AAT http://vocab.getty.edu/page/aat/300218300</skos:editorialNote>
    <skos:prefLabel xml:lang="it">Polimero sintetico</skos:prefLabel>
    <skos:altLabel xml:lang="en">Polymers</skos:altLabel>
    <rdfs:label xml:lang="en">Synthetic polymer</rdfs:label>
  </rdf:Description>
  <rdf:Description rdf:about="https://w3id.org/crmrp#c_cbe3d99a">
    <skos:definition xml:lang="en">Fracturing of a stone along planes of weakness such as microcracks or clay/silt layers, in case where the structural elements are orientated vertically. For instance, a column may split into several parts along bedding planes if the load above it is too high</skos:definition>
    <skos:editorialNote xml:lang="en">Verg`es-Belmin et al., ICOMOS-ISCS: Illustrated glossary on stone deterioration patterns, vol. XV. Icomos International Council on Monuments and Sites, 2008</skos:editorialNote>
    <skos:prefLabel xml:lang="en">Splitting</skos:prefLabel>
    <skos:topConceptOf rdf:resource="https://w3id.org/crmrp#Alteration"/>
    <rdf:type rdf:resource="http://www.w3.org/2004/02/skos/core#Concept"/>
    <rdfs:label xml:lang="en">Splitting</rdfs:label>
    <skos:prefLabel xml:lang="it">Fenditura</skos:prefLabel>
    <skos:inScheme rdf:resource="https://w3id.org/crmrp#Alteration"/>
    <skos:broader rdf:resource="https://w3id.org/crmrp#c_8c762c3e"/>
    <rdf:type rdf:resource="http://www.w3.org/2002/07/owl#NamedIndividual"/>
  </rdf:Description>
  <rdf:Description rdf:about="https://w3id.org/crmrp">
    <owl:imports rdf:resource="http://www.cidoc-crm.org/extensions/crmdig/"/>
    <owl:imports rdf:resource="http://www.cidoc-crm.org/extensions/crmsci/"/>
    <owl:imports rdf:resource="http://www.cidoc-crm.org/cidoc-crm/"/>
    <rdf:type rdf:resource="http://www.w3.org/2002/07/owl#Ontology"/>
  </rdf:Description>
  <rdf:Description rdf:about="https://w3id.org/crmrp#c_707c9e81">
    <skos:exactMatch rdf:resource="http://vocab.getty.edu/page/aat/300378932"/>
    <skos:broader rdf:resource="https://w3id.org/crmrp#c_3ef20257"/>
    <skos:prefLabel xml:lang="it">Muffa</skos:prefLabel>
    <rdf:type rdf:resource="http://www.w3.org/2004/02/skos/core#Concept"/>
    <rdfs:label xml:lang="en">Mould</rdfs:label>
    <skos:topConceptOf rdf:resource="https://w3id.org/crmrp#Alteration"/>
    <skos:note xml:lang="en">The preferred editorial note and the definition closest to the meaning is ICOMOS-ISCS: Illustrated glossary on stone deterioration patterns</skos:note>
    <skos:editorialNote xml:lang="en">Getty AAT http://vocab.getty.edu/page/aat/300378932</skos:editorialNote>
    <skos:definition xml:lang="en">Microscopic fungus which colonies, to the naked eye, look like a downy film or a network or star-like millimetric patches of filaments of diverse colours (white, grey, black).</skos:definition>
    <skos:editorialNote xml:lang="en">Verg`es-Belmin et al., ICOMOS-ISCS: Illustrated glossary on stone deterioration patterns, vol. XV. Icomos International Council on Monuments and Sites, 2008</skos:editorialNote>
    <skos:inScheme rdf:resource="https://w3id.org/crmrp#Alteration"/>
    <rdf:type rdf:resource="http://www.w3.org/2002/07/owl#NamedIndividual"/>
    <skos:prefLabel xml:lang="en">Mould</skos:prefLabel>
  </rdf:Description>
  <rdf:Description rdf:about="https://w3id.org/crmrp#c_8c553ab1">
    <rdfs:label xml:lang="en">Dry-rot</rdfs:label>
    <skos:definition xml:lang="en">Refers to a type of decomposition of timber by fungi.</skos:definition>
    <skos:prefLabel xml:lang="en">Dry-rot</skos:prefLabel>
    <skos:exactMatch rdf:resource="http://vocab.getty.edu/page/aat/300188725"/>
    <skos:prefLabel xml:lang="it">Carie</skos:prefLabel>
    <skos:editorialNote xml:lang="en">Getty AAT http://vocab.getty.edu/page/aat/300188725</skos:editorialNote>
    <rdf:type rdf:resource="http://www.w3.org/2004/02/skos/core#Concept"/>
    <skos:inScheme rdf:resource="https://w3id.org/crmrp#Alteration"/>
    <rdf:type rdf:resource="http://www.w3.org/2002/07/owl#NamedIndividual"/>
    <skos:broader rdf:resource="https://w3id.org/crmrp#c_3ef20257"/>
    <skos:topConceptOf rdf:resource="https://w3id.org/crmrp#Alteration"/>
  </rdf:Description>
  <rdf:Description rdf:about="https://w3id.org/crmrp#c_83de0482">
    <rdf:type rdf:resource="http://www.w3.org/2002/07/owl#NamedIndividual"/>
    <skos:prefLabel xml:lang="en">Lime paint</skos:prefLabel>
    <skos:broader rdf:resource="https://w3id.org/crmrp#c_6626f18c"/>
    <skos:topConceptOf rdf:resource="https://w3id.org/crmrp#Execution_Technique"/>
    <rdfs:label xml:lang="en">Lime paint</rdfs:label>
    <skos:prefLabel xml:lang="it">A calce</skos:prefLabel>
    <skos:definition xml:lang="en">Mural painting technique used as an alternative and at the same time as ‘buon fresco'; pigments were diluted in milk of lime instead of water and spread even several times over a coat of lime, generally already carboborn and smoothed. This is an opaque paint recognisable by the body of the brushstroke.</skos:definition>
    <skos:editorialNote xml:lang="it">C. Giannini, “Dizionario del restauro - Tecniche diagnostica conservazione”, Nardini Editore, Firenze, 2010</skos:editorialNote>
    <rdf:type rdf:resource="http://www.w3.org/2004/02/skos/core#Concept"/>
    <skos:inScheme rdf:resource="https://w3id.org/crmrp#Execution_Technique"/>
    <skos:note xml:lang="en">International references could not be found</skos:note>
  </rdf:Description>
  <rdf:Description rdf:about="https://w3id.org/crmrp#Documentation">
    <skos:prefLabel xml:lang="it">Documentazione</skos:prefLabel>
    <skos:prefLabel xml:lang="en">Documentation</skos:prefLabel>
    <skos:note xml:lang="en">International references could not be found</skos:note>
    <skos:editorialNote xml:lang="en">Uni En 15898:2019 Conservazione del patrimonio culturale - Termini generali e definizioni</skos:editorialNote>
    <skos:definition xml:lang="en">Set of information recorded, created, collected, stored and updated for the purpose of facilitating present and future preservation. Is as reference material. Examples: X-rays, drawings, photographs, written reports, digital files, photogrammetry, laser scans, etc.</skos:definition>
    <rdf:type rdf:resource="http://www.w3.org/2004/02/skos/core#ConceptScheme"/>
    <rdf:type rdf:resource="http://www.w3.org/2002/07/owl#NamedIndividual"/>
  </rdf:Description>
  <rdf:Description rdf:about="https://w3id.org/crmrp#c_8dcb0eb4">
    <skos:editorialNote xml:lang="en">Getty AAT http://vocab.getty.edu/page/aat/300041273</skos:editorialNote>
    <skos:inScheme rdf:resource="https://w3id.org/crmrp#Restoration_Object"/>
    <skos:prefLabel xml:lang="it">Stampa</skos:prefLabel>
    <rdf:type rdf:resource="http://www.w3.org/2004/02/skos/core#Concept"/>
    <rdfs:label xml:lang="en">Print</rdfs:label>
    <skos:prefLabel xml:lang="en">Prints</skos:prefLabel>
    <skos:definition xml:lang="en">Pictorial works produced by transferring images by means of a matrix such as a plate, block, or screen, using any of various printing processes. When emphasizing the individual printed image, use impressions. Avoid the controversial expression original prints, except in reference to discussions of the expression's use. If prints are neither reproductive prints nor popular prints, use the simple term prints. With regard to photographs, prefer photographic prints; for types of reproductions of technical drawings and documents, see terms found under reprographic copies.</skos:definition>
    <skos:topConceptOf rdf:resource="https://w3id.org/crmrp#Restoration_Object"/>
    <rdf:type rdf:resource="http://www.w3.org/2002/07/owl#NamedIndividual"/>
    <skos:exactMatch rdf:resource="http://vocab.getty.edu/page/aat/300041273"/>
  </rdf:Description>
  <rdf:Description rdf:about="https://w3id.org/crmrp#c_4973d8ba">
    <skos:topConceptOf rdf:resource="https://w3id.org/crmrp#Alteration"/>
    <skos:editorialNote xml:lang="en">Uni Cen/Ts 17135:2021 - Conservation of cultural heritage. General terms and definitions</skos:editorialNote>
    <skos:broader rdf:resource="https://w3id.org/crmrp#c_3ef20257"/>
    <rdf:type rdf:resource="http://www.w3.org/2004/02/skos/core#Concept"/>
    <skos:prefLabel xml:lang="it">Biofilm</skos:prefLabel>
    <skos:prefLabel xml:lang="en">Biofilm</skos:prefLabel>
    <skos:note xml:lang="en">The preferred editorial note and the definition closest to the meaning is Uni Cen/Ts 17135:2021</skos:note>
    <skos:exactMatch rdf:resource="http://vocab.getty.edu/page/aat/300379570"/>
    <skos:editorialNote xml:lang="en">Getty AAT http://vocab.getty.edu/page/aat/300379570</skos:editorialNote>
    <rdf:type rdf:resource="http://www.w3.org/2002/07/owl#NamedIndividual"/>
    <skos:definition xml:lang="en">Film consisting of an aggregation of microorganisms adhering to a surface.</skos:definition>
    <rdfs:label xml:lang="en">Biofilm</rdfs:label>
    <skos:inScheme rdf:resource="https://w3id.org/crmrp#Alteration"/>
  </rdf:Description>
  <rdf:Description rdf:about="https://w3id.org/crmrp#c_575a314b">
    <skos:prefLabel xml:lang="en">Drawing</skos:prefLabel>
    <skos:editorialNote xml:lang="en">Getty AAT http://vocab.getty.edu/page/aat/300033973</skos:editorialNote>
    <rdf:type rdf:resource="http://www.w3.org/2004/02/skos/core#Concept"/>
    <skos:definition xml:lang="en">Visual works produced by drawing, which is the application of lines on a surface, often paper, by using a pencil, pen, chalk, or some other tracing instrument to focus on the delineation of form rather than the application of color. This term is often defined broadly to refer to computer-generated images as well.</skos:definition>
    <skos:exactMatch rdf:resource="http://vocab.getty.edu/page/aat/300033973"/>
    <rdf:type rdf:resource="http://www.w3.org/2002/07/owl#NamedIndividual"/>
    <skos:prefLabel xml:lang="it">Disegno</skos:prefLabel>
    <skos:topConceptOf rdf:resource="https://w3id.org/crmrp#Restoration_Object"/>
    <rdfs:label xml:lang="en">Drawing</rdfs:label>
    <skos:inScheme rdf:resource="https://w3id.org/crmrp#Restoration_Object"/>
  </rdf:Description>
  <rdf:Description rdf:about="https://w3id.org/crmrp#c_68cc67d0">
    <skos:prefLabel xml:lang="it">Microscopio ottico polarizzatore in luce trasmessa e riflessa</skos:prefLabel>
    <skos:editorialNote xml:lang="it">M.Ceroni, G.Elia, “Diagnostica per i beni culturali”, Alinea editrice, Firenze, 2008</skos:editorialNote>
    <skos:broader rdf:resource="https://w3id.org/crmrp#c_7ee727f3"/>
    <skos:definition xml:lang="en">A polarising microscope, or transmitted-light polarising optical microscope, also known as a petrography microscope, is an optical microscope modified to use polarised light for sample observation.</skos:definition>
    <rdfs:label xml:lang="en">Polarising optical microscope in reflected and transmitted light</rdfs:label>
    <rdf:type rdf:resource="http://www.w3.org/2002/07/owl#NamedIndividual"/>
    <skos:inScheme rdf:resource="https://w3id.org/crmrp#Archeometric_and_Diagnostic_Analysis"/>
    <skos:prefLabel xml:lang="en">Polarising optical microscope in reflected and transmitted light</skos:prefLabel>
    <skos:topConceptOf rdf:resource="https://w3id.org/crmrp#Archeometric_and_Diagnostic_Analysis"/>
    <rdf:type rdf:resource="http://www.w3.org/2004/02/skos/core#Concept"/>
  </rdf:Description>
  <rdf:Description rdf:about="https://w3id.org/crmrp#c_8fe789e5">
    <skos:editorialNote xml:lang="en">A. Weyer et al., “EwaGlos - European Illustrated Glossary of conservation terms for wall paintings and architectural surfaces”, Michael Imhof Verlag, Petersberg, Germany</skos:editorialNote>
    <skos:broader rdf:resource="https://w3id.org/crmrp#c_bd34e984"/>
    <rdfs:label xml:lang="en">Terracotta</rdfs:label>
    <rdf:type rdf:resource="http://www.w3.org/2002/07/owl#NamedIndividual"/>
    <skos:inScheme rdf:resource="https://w3id.org/crmrp#Material"/>
    <skos:topConceptOf rdf:resource="https://w3id.org/crmrp#Material"/>
    <rdf:type rdf:resource="http://www.w3.org/2004/02/skos/core#Concept"/>
    <skos:definition xml:lang="en">A glazed or unglazed product made with clay and mixed with fillers (grog – calcinated clay, chamotte, brick dust or pot clay) and natural binders which are then baked at a high temperature (above 600 °C). Any kind of baked or semi-fired clay used to create utilitarian or decorative objects, or structural forms such as: floor tiles, roof tiles or decorative architectural elements</skos:definition>
    <skos:prefLabel xml:lang="en">Terracotta</skos:prefLabel>
    <skos:prefLabel xml:lang="it">Terracotta</skos:prefLabel>
  </rdf:Description>
  <rdf:Description rdf:about="https://w3id.org/crmrp#c_e3781f70">
    <skos:broader rdf:resource="https://w3id.org/crmrp#c_1fd6102e"/>
    <skos:closeMatch rdf:resource="http://vocab.getty.edu/page/aat/300053463"/>
    <skos:inScheme rdf:resource="https://w3id.org/crmrp#Archeometric_and_Diagnostic_Analysis"/>
    <rdfs:label xml:lang="en">Infrared photography</rdfs:label>
    <skos:topConceptOf rdf:resource="https://w3id.org/crmrp#Archeometric_and_Diagnostic_Analysis"/>
    <skos:prefLabel xml:lang="it">Infrarosso fotografico</skos:prefLabel>
    <skos:definition xml:lang="en"> Technique using film sensitive to both some visible light waves and to wavelengths generated by the infrared segment of the electromagnetic spectum.</skos:definition>
    <rdf:type rdf:resource="http://www.w3.org/2004/02/skos/core#Concept"/>
    <rdf:type rdf:resource="http://www.w3.org/2002/07/owl#NamedIndividual"/>
    <skos:prefLabel xml:lang="en">Infrared photography</skos:prefLabel>
    <skos:editorialNote xml:lang="en">Getty AAT http://vocab.getty.edu/page/aat/300053463</skos:editorialNote>
  </rdf:Description>
  <rdf:Description rdf:about="https://w3id.org/crmrp#c_a75330d3">
    <skos:prefLabel xml:lang="en">Tratteggio</skos:prefLabel>
    <skos:prefLabel xml:lang="it">Tratteggio</skos:prefLabel>
    <skos:definition xml:lang="en">Based on the conservation/restoration theory of Cesare Brandi, the shape and colour of a damaged area are reconstructed using short vertical lines.</skos:definition>
    <rdfs:label xml:lang="en">Tratteggio</rdfs:label>
    <rdf:type rdf:resource="http://www.w3.org/2004/02/skos/core#Concept"/>
    <skos:inScheme rdf:resource="https://w3id.org/crmrp#Intervention"/>
    <skos:broader rdf:resource="https://w3id.org/crmrp#c_326da7e4"/>
    <rdf:type rdf:resource="http://www.w3.org/2002/07/owl#NamedIndividual"/>
    <skos:topConceptOf rdf:resource="https://w3id.org/crmrp#Intervention"/>
    <skos:editorialNote xml:lang="en">A. Weyer et al., “EwaGlos - European Illustrated Glossary of conservation terms for wall paintings and architectural surfaces”, Michael Imhof Verlag, Petersberg, Germany</skos:editorialNote>
  </rdf:Description>
  <rdf:Description rdf:about="https://w3id.org/crmrp#c_0ddda1a6">
    <skos:broader rdf:resource="https://w3id.org/crmrp#c_6626f18c"/>
    <rdf:type rdf:resource="http://www.w3.org/2002/07/owl#NamedIndividual"/>
    <rdf:type rdf:resource="http://www.w3.org/2004/02/skos/core#Concept"/>
    <skos:note xml:lang="en">The preferred editorial note and the most complete definition is in EwaGlos - European Illustrated Glossary of conservation terms for wall paintings and architectural surfaces</skos:note>
    <skos:definition xml:lang="en">Technique where the painting is executed on a lime plaster surface which is in a state of advanced carbonation.</skos:definition>
    <skos:exactMatch rdf:resource="http://vocab.getty.edu/page/aat/300053364"/>
    <skos:inScheme rdf:resource="https://w3id.org/crmrp#Execution_Technique"/>
    <skos:editorialNote xml:lang="en">Getty AAT http://vocab.getty.edu/page/aat/300053364</skos:editorialNote>
    <skos:editorialNote xml:lang="en">A. Weyer et al., “EwaGlos - European Illustrated Glossary of conservation terms for wall paintings and architectural surfaces”, Michael Imhof Verlag, Petersberg, Germany</skos:editorialNote>
    <skos:prefLabel xml:lang="it">Mezzo fresco</skos:prefLabel>
    <skos:prefLabel xml:lang="en">Mezzo fresco</skos:prefLabel>
    <rdfs:label xml:lang="en">Mezzo fresco</rdfs:label>
    <skos:topConceptOf rdf:resource="https://w3id.org/crmrp#Execution_Technique"/>
  </rdf:Description>
  <rdf:Description rdf:about="https://w3id.org/crmrp#c_101f9b20">
    <rdf:type rdf:resource="http://www.w3.org/2004/02/skos/core#Concept"/>
    <skos:prefLabel xml:lang="it">Arcuatura</skos:prefLabel>
    <skos:prefLabel xml:lang="en">Arching</skos:prefLabel>
    <rdfs:label xml:lang="en">Arching</rdfs:label>
    <skos:editorialNote xml:lang="en">C. Giannini, “Dizionario del restauro - Tecniche diagnostica conservazione”, Nardini Editore, Firenze, 2010</skos:editorialNote>
    <skos:broader rdf:resource="https://w3id.org/crmrp#c_13f3ce9e"/>
    <skos:definition xml:lang="en">Deformation of sawn wood. In panel paintings, it causes movement or disruption in the overlying imprimitura and colour.</skos:definition>
    <skos:inScheme rdf:resource="https://w3id.org/crmrp#Alteration"/>
    <rdf:type rdf:resource="http://www.w3.org/2002/07/owl#NamedIndividual"/>
    <skos:note xml:lang="en">International references could not be found</skos:note>
    <skos:topConceptOf rdf:resource="https://w3id.org/crmrp#Alteration"/>
  </rdf:Description>
  <rdf:Description rdf:about="https://w3id.org/crmrp#c_aea2f21f">
    <skos:prefLabel xml:lang="it">Ultrasuoni</skos:prefLabel>
    <rdf:type rdf:resource="http://www.w3.org/2002/07/owl#NamedIndividual"/>
    <skos:topConceptOf rdf:resource="https://w3id.org/crmrp#Archeometric_and_Diagnostic_Analysis"/>
    <skos:inScheme rdf:resource="https://w3id.org/crmrp#Archeometric_and_Diagnostic_Analysis"/>
    <skos:note xml:lang="en">International references could not be found, but the preferred editorial note and the definition closest to the meaning is Dizionario del restauro - Tecniche diagnostica conservazione</skos:note>
    <skos:broader rdf:resource="https://w3id.org/crmrp#c_1fd6102e"/>
    <skos:definition xml:lang="en">Determining the propagation speed of ultrasonic pulses. In diagnostic applications in the field restoration and conservation, ultrasounds are used to identify discontinuities in materials by their propagation within them</skos:definition>
    <skos:editorialNote xml:lang="it">M.Ceroni, G.Elia, “Diagnostica per i beni culturali”, Alinea editrice, Firenze, 2008</skos:editorialNote>
    <skos:editorialNote xml:lang="it">C. Giannini, “Dizionario del restauro - Tecniche diagnostica conservazione”, Nardini Editore, Firenze, 2010</skos:editorialNote>
    <skos:prefLabel xml:lang="en">Ultrasound</skos:prefLabel>
    <rdfs:label xml:lang="en">Ultrasound</rdfs:label>
    <rdf:type rdf:resource="http://www.w3.org/2004/02/skos/core#Concept"/>
  </rdf:Description>
  <rdf:Description rdf:about="https://w3id.org/crmrp#c_5b7fce15">
    <skos:topConceptOf rdf:resource="https://w3id.org/crmrp#Documentation"/>
    <skos:prefLabel xml:lang="it">Fonti e documenti</skos:prefLabel>
    <skos:prefLabel xml:lang="en">Sources and documents</skos:prefLabel>
    <skos:note xml:lang="en">International references could not be found</skos:note>
    <skos:inScheme rdf:resource="https://w3id.org/crmrp#Documentation"/>
    <skos:definition xml:lang="en">It comprise technical and scientific reports produced before and after each restoration. Moreover, restoration is a moment of recognition and in-depth study of an artwork, so it is not uncommon to review additional resources to broaden the knowledge of it, from historical and conservation perspective.</skos:definition>
    <rdfs:label xml:lang="en">Sources and documents</rdfs:label>
    <rdf:type rdf:resource="http://www.w3.org/2004/02/skos/core#Concept"/>
    <rdf:type rdf:resource="http://www.w3.org/2002/07/owl#NamedIndividual"/>
  </rdf:Description>
  <rdf:Description rdf:about="https://w3id.org/crmrp#c_1fd6102e">
    <skos:editorialNote xml:lang="en">A. Weyer et al., “EwaGlos - European Illustrated Glossary of conservation terms for wall paintings and architectural surfaces”, Michael Imhof Verlag, Petersberg, Germany</skos:editorialNote>
    <skos:topConceptOf rdf:resource="https://w3id.org/crmrp#Archeometric_and_Diagnostic_Analysis"/>
    <skos:inScheme rdf:resource="https://w3id.org/crmrp#Archeometric_and_Diagnostic_Analysis"/>
    <skos:editorialNote xml:lang="en">Getty AAT http://vocab.getty.edu/page/aat/300389952</skos:editorialNote>
    <skos:altLabel xml:lang="en">Noninvasive testing</skos:altLabel>
    <skos:exactMatch rdf:resource="http://vocab.getty.edu/page/aat/300389952"/>
    <rdf:type rdf:resource="http://www.w3.org/2002/07/owl#NamedIndividual"/>
    <skos:definition xml:lang="en">The gathering of information on site using techniques that do not modify or damage the material at the contact point between the instrument or the beam emitted by the instrument and the object surface.</skos:definition>
    <skos:prefLabel xml:lang="it">Indagine non invasiva</skos:prefLabel>
    <skos:prefLabel xml:lang="en">Non-invasive investigation</skos:prefLabel>
    <skos:note xml:lang="en">The preferred editorial note and the definition closest to the meaning is EwaGlos - European Illustrated Glossary of conservation terms for wall paintings and architectural surfaces</skos:note>
    <rdf:type rdf:resource="http://www.w3.org/2004/02/skos/core#Concept"/>
    <rdfs:label xml:lang="en">Non-invasive investigation</rdfs:label>
  </rdf:Description>
  <rdf:Description rdf:about="https://w3id.org/crmrp#c_af82711f">
    <skos:exactMatch rdf:resource="http://vocab.getty.edu/page/aat/300015055"/>
    <rdf:type rdf:resource="http://www.w3.org/2004/02/skos/core#Concept"/>
    <skos:definition xml:lang="en">Paint with a base that is polymer, which is compound formed by the combination of two or more molecules of the same substance to produce a new compound with the same empirical formula but with higher molecular weight. It is typically made from pigments in an acrylic resin or vinyl resin, which are polymers, or a combination of both resins. It is water based, spreads out in a layer, and forms a continuous, flexible, and waterproof film of plastic when the water evaporates.</skos:definition>
    <skos:broader rdf:resource="https://w3id.org/crmrp#c_051209b3"/>
    <skos:topConceptOf rdf:resource="https://w3id.org/crmrp#Execution_Technique"/>
    <rdf:type rdf:resource="http://www.w3.org/2002/07/owl#NamedIndividual"/>
    <skos:prefLabel xml:lang="it">Polimero sintetico</skos:prefLabel>
    <skos:prefLabel xml:lang="en">Polymer paint</skos:prefLabel>
    <skos:inScheme rdf:resource="https://w3id.org/crmrp#Execution_Technique"/>
    <skos:editorialNote xml:lang="en">Getty AAT http://vocab.getty.edu/page/aat/300015055</skos:editorialNote>
    <rdfs:label xml:lang="en">Polymer paint</rdfs:label>
  </rdf:Description>
  <rdf:Description rdf:about="https://w3id.org/crmrp#c_cf65605c">
    <rdf:type rdf:resource="http://www.w3.org/2002/07/owl#NamedIndividual"/>
    <skos:broader rdf:resource="https://w3id.org/crmrp#c_bd34e984"/>
    <rdfs:label xml:lang="en">Glazed decoration</rdfs:label>
    <skos:definition xml:lang="en">Façade and interior wall ornaments made with polychrome and glazed bricks or terracotta tiles.</skos:definition>
    <skos:inScheme rdf:resource="https://w3id.org/crmrp#Material"/>
    <skos:closeMatch xml:lang="en">Glazed decoration</skos:closeMatch>
    <skos:editorialNote xml:lang="en">A. Weyer et al., “EwaGlos - European Illustrated Glossary of conservation terms for wall paintings and architectural surfaces”, Michael Imhof Verlag, Petersberg, Germany</skos:editorialNote>
    <skos:prefLabel xml:lang="it">Maiolica</skos:prefLabel>
    <skos:topConceptOf rdf:resource="https://w3id.org/crmrp#Material"/>
    <skos:prefLabel xml:lang="en">Glazed decoration</skos:prefLabel>
    <rdf:type rdf:resource="http://www.w3.org/2004/02/skos/core#Concept"/>
  </rdf:Description>
  <rdf:Description rdf:about="https://w3id.org/crmrp#c_0be4284c">
    <rdf:type rdf:resource="http://www.w3.org/2002/07/owl#NamedIndividual"/>
    <skos:topConceptOf rdf:resource="https://w3id.org/crmrp#Alteration"/>
    <skos:broader rdf:resource="https://w3id.org/crmrp#c_df05cb61"/>
    <skos:inScheme rdf:resource="https://w3id.org/crmrp#Alteration"/>
    <skos:note xml:lang="en">The preferred editorial note and the definition closest to the meaning is Uni Cen/Ts 17135:2021</skos:note>
    <skos:prefLabel xml:lang="en">Yellowed</skos:prefLabel>
    <rdfs:label xml:lang="en">Yellowed</rdfs:label>
    <skos:prefLabel xml:lang="it">Ingiallimento</skos:prefLabel>
    <skos:editorialNote xml:lang="en">A. Weyer et al., “EwaGlos - European Illustrated Glossary of conservation terms for wall paintings and architectural surfaces”, Michael Imhof Verlag, Petersberg, Germany</skos:editorialNote>
    <skos:editorialNote xml:lang="en">Uni Cen/Ts 17135:2021 - Conservation of cultural heritage. General terms and definitions</skos:editorialNote>
    <rdf:type rdf:resource="http://www.w3.org/2004/02/skos/core#Concept"/>
  </rdf:Description>
  <rdf:Description rdf:about="https://w3id.org/crmrp#c_f8f782c5">
    <skos:prefLabel xml:lang="it">Foxing</skos:prefLabel>
    <skos:prefLabel xml:lang="en">Foxing</skos:prefLabel>
    <skos:definition xml:lang="en">Multiple spots on paper or textile</skos:definition>
    <rdf:type rdf:resource="http://www.w3.org/2002/07/owl#NamedIndividual"/>
    <skos:closeMatch rdf:resource="http://vocab.getty.edu/page/aat/300078853"/>
    <skos:topConceptOf rdf:resource="https://w3id.org/crmrp#Alteration"/>
    <rdf:type rdf:resource="http://www.w3.org/2004/02/skos/core#Concept"/>
    <skos:note xml:lang="en">The preferred editorial note and the definition closest to the meaning is Uni Cen/Ts 17135:2021</skos:note>
    <skos:editorialNote xml:lang="en">Getty AAT http://vocab.getty.edu/page/aat/300078853</skos:editorialNote>
    <skos:editorialNote xml:lang="en">Uni Cen/Ts 17135:2021 - Conservation of cultural heritage. General terms and definitions</skos:editorialNote>
    <skos:broader rdf:resource="https://w3id.org/crmrp#c_df05cb61"/>
    <rdfs:label xml:lang="en">Foxing</rdfs:label>
    <skos:inScheme rdf:resource="https://w3id.org/crmrp#Alteration"/>
  </rdf:Description>
  <rdf:Description rdf:about="https://w3id.org/crmrp#c_94b88ed9">
    <skos:inScheme rdf:resource="https://w3id.org/crmrp#Archeometric_and_Diagnostic_Analysis"/>
    <rdf:type rdf:resource="http://www.w3.org/2002/07/owl#NamedIndividual"/>
    <skos:definition xml:lang="en">With UV reflectography, a work is illuminated with UV light and the resulting image is photographed with a camera using a UV lens filter. Since different materials will have different levels of opacity under UV than under visible or infrared light, this technique can provide clues to the material composition of pigments. Furthermore, it is a good choice for analysing roughness and surface details.</skos:definition>
    <rdf:type rdf:resource="http://www.w3.org/2004/02/skos/core#Concept"/>
    <skos:note xml:lang="it">Riflettografia ultravioletta</skos:note>
    <skos:prefLabel xml:lang="en">Ultraviolet reflectography</skos:prefLabel>
    <rdfs:label xml:lang="en">Ultraviolet reflectography</rdfs:label>
    <skos:broader rdf:resource="https://w3id.org/crmrp#c_1285fa71"/>
    <skos:prefLabel xml:lang="it">Riflettografia ultravioletta</skos:prefLabel>
    <skos:topConceptOf rdf:resource="https://w3id.org/crmrp#Archeometric_and_Diagnostic_Analysis"/>
    <skos:note xml:lang="en">International references could not be found</skos:note>
  </rdf:Description>
  <rdf:Description rdf:about="https://w3id.org/crmrp#c_251b286b">
    <skos:inScheme rdf:resource="https://w3id.org/crmrp#Execution_Technique"/>
    <skos:definition xml:lang="en">Use with regard to specialized procedures related to how a photograph is taken or composed, or is manipulated during or after processing. Use photographic processes for the procedures by which light-sensitive materials are made to produce an image.</skos:definition>
    <skos:prefLabel xml:lang="en">Photographic technique</skos:prefLabel>
    <skos:editorialNote xml:lang="en">Getty AAT http://vocab.getty.edu/page/aat/300134334</skos:editorialNote>
    <rdf:type rdf:resource="http://www.w3.org/2002/07/owl#NamedIndividual"/>
    <skos:prefLabel xml:lang="it">Tecnica fotografica</skos:prefLabel>
    <rdfs:label xml:lang="en">Photographic technique</rdfs:label>
    <skos:topConceptOf rdf:resource="https://w3id.org/crmrp#Execution_Technique"/>
    <skos:closeMatch rdf:resource="http://vocab.getty.edu/page/aat/300134334"/>
    <rdf:type rdf:resource="http://www.w3.org/2004/02/skos/core#Concept"/>
  </rdf:Description>
  <rdf:Description rdf:about="https://w3id.org/crmrp#c_18fdda7b">
    <skos:closeMatch rdf:resource="http://vocab.getty.edu/page/aat/300053271"/>
    <skos:prefLabel xml:lang="en">Lithography</skos:prefLabel>
    <skos:editorialNote xml:lang="en">Getty AAT http://vocab.getty.edu/page/aat/300053271</skos:editorialNote>
    <rdf:type rdf:resource="http://www.w3.org/2004/02/skos/core#Concept"/>
    <skos:definition xml:lang="en">Planographic printing process in which a design is deposited on a stone or plate with a greasy substance and the surface is chemically treated to accept ink only in the greasy areas.</skos:definition>
    <skos:topConceptOf rdf:resource="https://w3id.org/crmrp#Execution_Technique"/>
    <skos:broader rdf:resource="https://w3id.org/crmrp#c_aee6a805"/>
    <skos:inScheme rdf:resource="https://w3id.org/crmrp#Execution_Technique"/>
    <skos:prefLabel xml:lang="it">Litografia</skos:prefLabel>
    <rdfs:label xml:lang="en">Lithography</rdfs:label>
    <rdf:type rdf:resource="http://www.w3.org/2002/07/owl#NamedIndividual"/>
  </rdf:Description>
  <rdf:Description rdf:about="https://w3id.org/crmrp#c_ef9ea44a">
    <skos:exactMatch rdf:resource="http://vocab.getty.edu/page/aat/300053123"/>
    <skos:definition xml:lang="en">The distortion of an object originally linear or planar so that it is curved or coiled in shape.</skos:definition>
    <rdf:type rdf:resource="http://www.w3.org/2002/07/owl#NamedIndividual"/>
    <skos:broader rdf:resource="https://w3id.org/crmrp#c_13f3ce9e"/>
    <rdfs:label xml:lang="en">Curling</rdfs:label>
    <skos:inScheme rdf:resource="https://w3id.org/crmrp#Alteration"/>
    <skos:prefLabel xml:lang="en">Curling</skos:prefLabel>
    <skos:editorialNote xml:lang="en">Getty AAT http://vocab.getty.edu/page/aat/300053123</skos:editorialNote>
    <skos:prefLabel xml:lang="it">Accartocciamento</skos:prefLabel>
    <skos:topConceptOf rdf:resource="https://w3id.org/crmrp#Alteration"/>
    <rdf:type rdf:resource="http://www.w3.org/2004/02/skos/core#Concept"/>
  </rdf:Description>
  <rdf:Description rdf:about="http://www.w3.org/2004/02/skos/core#altLabel">
    <rdfs:subPropertyOf rdf:resource="http://www.w3.org/2000/01/rdf-schema#label"/>
    <rdf:type rdf:resource="http://www.w3.org/2002/07/owl#AnnotationProperty"/>
  </rdf:Description>
  <rdf:Description rdf:about="https://w3id.org/crmrp#c_bbb3b219">
    <rdfs:label xml:lang="en">Drying oil</rdfs:label>
    <skos:inScheme rdf:resource="https://w3id.org/crmrp#Execution_Technique"/>
    <skos:prefLabel xml:lang="en">Drying oil</skos:prefLabel>
    <skos:broader rdf:resource="https://w3id.org/crmrp#c_143349b9"/>
    <skos:prefLabel xml:lang="it">Olio</skos:prefLabel>
    <skos:topConceptOf rdf:resource="https://w3id.org/crmrp#Execution_Technique"/>
    <rdf:type rdf:resource="http://www.w3.org/2002/07/owl#NamedIndividual"/>
    <skos:editorialNote xml:lang="en">A. Weyer et al., “EwaGlos - European Illustrated Glossary of conservation terms for wall paintings and architectural surfaces”, Michael Imhof Verlag, Petersberg, Germany</skos:editorialNote>
    <skos:definition xml:lang="en">Vegetable oils which form a solid, elastic film after a period of exposure to the air.</skos:definition>
    <rdf:type rdf:resource="http://www.w3.org/2004/02/skos/core#Concept"/>
  </rdf:Description>
  <rdf:Description rdf:about="http://www.w3.org/2004/02/skos/core#defintion">
    <rdf:type rdf:resource="http://www.w3.org/2002/07/owl#AnnotationProperty"/>
  </rdf:Description>
  <rdf:Description rdf:about="https://w3id.org/crmrp#c_813d8e86">
    <skos:topConceptOf rdf:resource="https://w3id.org/crmrp#Execution_Technique"/>
    <rdfs:label xml:lang="en">Enamel paint</rdfs:label>
    <skos:prefLabel xml:lang="en">Enamel paint</skos:prefLabel>
    <skos:inScheme rdf:resource="https://w3id.org/crmrp#Execution_Technique"/>
    <skos:prefLabel xml:lang="it">Smalto</skos:prefLabel>
    <skos:editorialNote xml:lang="en">Getty AAT http://vocab.getty.edu/page/aat/300147678</skos:editorialNote>
    <rdf:type rdf:resource="http://www.w3.org/2004/02/skos/core#Concept"/>
    <skos:definition xml:lang="en">Paint made from oil, resin, varnish, or a combination of these, mixed with finely ground pigment; usually giving a glossy finish, but sometimes giving a semigloss or flat finish</skos:definition>
    <skos:broader rdf:resource="https://w3id.org/crmrp#c_143349b9"/>
    <rdf:type rdf:resource="http://www.w3.org/2002/07/owl#NamedIndividual"/>
    <skos:closeMatch rdf:resource="http://vocab.getty.edu/page/aat/300147678"/>
  </rdf:Description>
  <rdf:Description rdf:about="https://w3id.org/crmrp#c_fdaf0926">
    <skos:definition xml:lang="en">Method for the removal of wall paintings involving the removal of the arriccio together with the wall support.</skos:definition>
    <rdfs:label xml:lang="en">Stacco a massello</rdfs:label>
    <skos:topConceptOf rdf:resource="https://w3id.org/crmrp#Intervention"/>
    <skos:exactMatch rdf:resource="http://vocab.getty.edu/page/aat/300266091"/>
    <skos:inScheme rdf:resource="https://w3id.org/crmrp#Intervention"/>
    <rdf:type rdf:resource="http://www.w3.org/2004/02/skos/core#Concept"/>
    <rdf:type rdf:resource="http://www.w3.org/2002/07/owl#NamedIndividual"/>
    <skos:broader rdf:resource="https://w3id.org/crmrp#c_4fe4d308"/>
    <skos:prefLabel xml:lang="it">Stacco a massello</skos:prefLabel>
    <skos:prefLabel xml:lang="en">Stacco a massello</skos:prefLabel>
    <skos:editorialNote xml:lang="en">Getty AAT http://vocab.getty.edu/page/aat/300266091</skos:editorialNote>
  </rdf:Description>
  <rdf:Description rdf:about="http://www.w3.org/2004/02/skos/core#closeMatch">
    <rdf:type rdf:resource="http://www.w3.org/2002/07/owl#AnnotationProperty"/>
  </rdf:Description>
  <rdf:Description rdf:about="https://w3id.org/crmrp#c_bd37c76d">
    <skos:note xml:lang="en">International references could not be found</skos:note>
    <skos:inScheme rdf:resource="https://w3id.org/crmrp#Execution_Technique"/>
    <rdf:type rdf:resource="http://www.w3.org/2004/02/skos/core#Concept"/>
    <skos:broader rdf:resource="https://w3id.org/crmrp#c_757ed6ec"/>
    <rdf:type rdf:resource="http://www.w3.org/2002/07/owl#NamedIndividual"/>
    <rdfs:label xml:lang="en">Graffito</rdfs:label>
    <skos:topConceptOf rdf:resource="https://w3id.org/crmrp#Execution_Technique"/>
    <skos:prefLabel xml:lang="it">Graffito</skos:prefLabel>
    <skos:prefLabel xml:lang="en">Graffito</skos:prefLabel>
    <skos:editorialNote xml:lang="it">G. Pignolo, “Effetti d’oro - Storia e tecnica della doratura nell’arte”, Editrice Compositori, Bologna, 2002</skos:editorialNote>
    <skos:definition xml:lang="en">The technique derives from the way gold leaf is treated in wall decoration. </skos:definition>
  </rdf:Description>
  <rdf:Description rdf:about="https://w3id.org/crmrp#c_fc8da886">
    <skos:inScheme rdf:resource="https://w3id.org/crmrp#Intervention"/>
    <skos:note xml:lang="en">It was decided not to proceed with the English translation in order to avoid possible lexical errors and misunderstandings.</skos:note>
    <rdf:type rdf:resource="http://www.w3.org/2004/02/skos/core#Concept"/>
    <skos:broader rdf:resource="https://w3id.org/crmrp#c_326da7e4"/>
    <rdfs:label xml:lang="en">Rigatino</rdfs:label>
    <skos:editorialNote xml:lang="it">C. Giannini, “Dizionario del restauro - Tecniche diagnostica conservazione”, Nardini Editore, Firenze, 2010</skos:editorialNote>
    <skos:prefLabel xml:lang="it">Rigatino</skos:prefLabel>
    <skos:prefLabel xml:lang="en">Rigatino</skos:prefLabel>
    <skos:definition xml:lang="en">Type of pictorial integration that allows the gap to be identified. It is called also called ‘righettino’ and is carried out by means of vertical hatching in harmony with local chromatic values; at a distance, the intervention is imperceptible, while it is visible at close range, in accordance with the principle of recognisability.</skos:definition>
    <skos:topConceptOf rdf:resource="https://w3id.org/crmrp#Intervention"/>
    <rdf:type rdf:resource="http://www.w3.org/2002/07/owl#NamedIndividual"/>
  </rdf:Description>
  <rdf:Description rdf:about="https://w3id.org/crmrp#Material">
    <skos:prefLabel xml:lang="it">Materia</skos:prefLabel>
    <skos:prefLabel xml:lang="en">Material</skos:prefLabel>
    <skos:note xml:lang="en">International references could not be found</skos:note>
    <rdf:type rdf:resource="http://www.w3.org/2004/02/skos/core#ConceptScheme"/>
    <rdf:type rdf:resource="http://www.w3.org/2002/07/owl#NamedIndividual"/>
  </rdf:Description>
  <rdf:Description rdf:about="https://w3id.org/crmrp#c_eb357ebb">
    <skos:topConceptOf rdf:resource="https://w3id.org/crmrp#Execution_Technique"/>
    <skos:prefLabel xml:lang="it">Tecnica delle arti contemporanee</skos:prefLabel>
    <skos:prefLabel xml:lang="en">Technique of contemporary arts</skos:prefLabel>
    <skos:note xml:lang="en">International references could not be found</skos:note>
    <skos:inScheme rdf:resource="https://w3id.org/crmrp#Execution_Technique"/>
    <skos:definition xml:lang="en">Any execution technique of works created from the 1960s onwards, which does not correspond to traditional artistic techniques.</skos:definition>
    <rdfs:label xml:lang="en">Technique of contemporary arts</rdfs:label>
    <rdf:type rdf:resource="http://www.w3.org/2004/02/skos/core#Concept"/>
    <rdf:type rdf:resource="http://www.w3.org/2002/07/owl#NamedIndividual"/>
  </rdf:Description>
  <rdf:Description rdf:about="https://w3id.org/crmrp#c_c2349eb7">
    <skos:altLabel xml:lang="en">Securing</skos:altLabel>
    <rdf:type rdf:resource="http://www.w3.org/2004/02/skos/core#Concept"/>
    <skos:definition xml:lang="en">Treatments that aim to temporarily halt active deterioration and preserve a part of or the entire artwork.</skos:definition>
    <skos:prefLabel xml:lang="en">Emergency measure</skos:prefLabel>
    <rdf:type rdf:resource="http://www.w3.org/2002/07/owl#NamedIndividual"/>
    <skos:inScheme rdf:resource="https://w3id.org/crmrp#Intervention"/>
    <rdfs:label xml:lang="en">Emergency measure</rdfs:label>
    <skos:prefLabel xml:lang="it">Messa in sicurezza</skos:prefLabel>
    <skos:editorialNote xml:lang="en">A. Weyer et al., “EwaGlos - European Illustrated Glossary of conservation terms for wall paintings and architectural surfaces”, Michael Imhof Verlag, Petersberg, Germany</skos:editorialNote>
    <skos:topConceptOf rdf:resource="https://w3id.org/crmrp#Intervention"/>
  </rdf:Description>
  <rdf:Description rdf:about="https://w3id.org/crmrp#RP1_intervents_on">
    <rdfs:label xml:lang="en">intervents on</rdfs:label>
    <rdfs:comment>This property links R1 Restoration Object and R7 Restoration Project
This property RP1 intervents on (needed intervention) allows you to indicate which artwork the restoration project refers to.</rdfs:comment>
    <rdfs:range rdf:resource="https://w3id.org/crmrp#R1_Restoration_Object"/>
    <rdfs:range rdf:resource="http://www.cidoc-crm.org/extensions/crmsci/S18_Alteration"/>
    <rdfs:domain rdf:resource="https://w3id.org/crmrp#R8_Intervention"/>
    <rdfs:domain rdf:resource="https://w3id.org/crmrp#R7_Restoration_Project"/>
    <owl:inverseOf rdf:resource="https://w3id.org/crmrp#RP1i_needed_intervention"/>
    <rdf:type rdf:resource="http://www.w3.org/2002/07/owl#ObjectProperty"/>
  </rdf:Description>
  <rdf:Description rdf:about="http://www.w3.org/2004/02/skos/core#prefLabel">
    <rdfs:subPropertyOf rdf:resource="http://www.w3.org/2000/01/rdf-schema#label"/>
    <rdf:type rdf:resource="http://www.w3.org/2002/07/owl#AnnotationProperty"/>
  </rdf:Description>
  <rdf:Description rdf:about="https://w3id.org/crmrp#c_41bb39c8">
    <skos:topConceptOf rdf:resource="https://w3id.org/crmrp#Documentation"/>
    <skos:broader rdf:resource="https://w3id.org/crmrp#c_5b7fce15"/>
    <skos:prefLabel xml:lang="en">Authorisation</skos:prefLabel>
    <skos:definition xml:lang="en">Confirmation by the competent state bodies of the relevance of projects, reports or work carried out directly on works of art.</skos:definition>
    <rdfs:label xml:lang="en">Authorisation</rdfs:label>
    <skos:note xml:lang="en">International references could not be found</skos:note>
    <skos:prefLabel xml:lang="it">Autorizzazione</skos:prefLabel>
    <rdf:type rdf:resource="http://www.w3.org/2002/07/owl#NamedIndividual"/>
    <skos:inScheme rdf:resource="https://w3id.org/crmrp#Documentation"/>
    <rdf:type rdf:resource="http://www.w3.org/2004/02/skos/core#Concept"/>
  </rdf:Description>
  <rdf:Description rdf:about="https://w3id.org/crmrp#c_ec7e0a6f">
    <skos:inScheme rdf:resource="https://w3id.org/crmrp#Execution_Technique"/>
    <skos:prefLabel xml:lang="it">Olio</skos:prefLabel>
    <skos:editorialNote xml:lang="en">A. Weyer et al., “EwaGlos - European Illustrated Glossary of conservation terms for wall paintings and architectural surfaces”, Michael Imhof Verlag, Petersberg, Germany</skos:editorialNote>
    <rdf:type rdf:resource="http://www.w3.org/2004/02/skos/core#Concept"/>
    <rdf:type rdf:resource="http://www.w3.org/2002/07/owl#NamedIndividual"/>
    <skos:prefLabel xml:lang="en">Drying oil</skos:prefLabel>
    <skos:broader rdf:resource="https://w3id.org/crmrp#c_051209b3"/>
    <rdfs:label xml:lang="en">Drying oil</rdfs:label>
    <skos:topConceptOf rdf:resource="https://w3id.org/crmrp#Execution_Technique"/>
    <skos:definition xml:lang="en">Vegetable oils which form a solid, elastic film after a period of exposure to the air.</skos:definition>
  </rdf:Description>
  <rdf:Description rdf:about="https://w3id.org/crmrp#c_11153277">
    <skos:broader rdf:resource="https://w3id.org/crmrp#c_1fd6102e"/>
    <rdfs:label xml:lang="en">Infrared thermography</rdfs:label>
    <rdf:type rdf:resource="http://www.w3.org/2002/07/owl#NamedIndividual"/>
    <skos:definition xml:lang="en">A technique that measures variations in temperature of an area, object, or organism by creating infrared images (thermograms) to detect discontinuities such as voids in solid structures, deteriorations in frescoes, biotic infestations of a surface, or tumors in human tissue.</skos:definition>
    <skos:topConceptOf rdf:resource="https://w3id.org/crmrp#Archeometric_and_Diagnostic_Analysis"/>
    <skos:prefLabel xml:lang="it">Termografia</skos:prefLabel>
    <skos:inScheme rdf:resource="https://w3id.org/crmrp#Archeometric_and_Diagnostic_Analysis"/>
    <skos:closeMatch rdf:resource="http://vocab.getty.edu/page/aat/300379531"/>
    <rdf:type rdf:resource="http://www.w3.org/2004/02/skos/core#Concept"/>
    <skos:editorialNote xml:lang="en">Getty AAT http://vocab.getty.edu/page/aat/300379531</skos:editorialNote>
    <skos:prefLabel xml:lang="en">Infrared thermography</skos:prefLabel>
  </rdf:Description>
  <rdf:Description rdf:about="https://w3id.org/crmrp#c_d68fd470">
    <skos:inScheme rdf:resource="https://w3id.org/crmrp#Execution_Technique"/>
    <rdf:type rdf:resource="http://www.w3.org/2002/07/owl#NamedIndividual"/>
    <skos:definition xml:lang="en">Decorative wood process in which the design or pattern is made by assembling small pieces of veneer in various shapes. The term, which derives from 15th-century Italy, is commonly used to describe both marquetry, in which the entire surface is veneered, and wood inlay, in which the pattern pieces are laid into a solid ground. The term may also be used to refer to similar works of stone, glass, or another material. Distinguished from mosaics, as pieces in intarsia work are precision-cut to tightly fit together</skos:definition>
    <rdf:type rdf:resource="http://www.w3.org/2004/02/skos/core#Concept"/>
    <skos:broader rdf:resource="https://w3id.org/crmrp#c_051209b3"/>
    <skos:note xml:lang="en">The preferred editorial note and the definition closest to the meaning is Getty AAT</skos:note>
    <skos:editorialNote xml:lang="en">The Getty Conservation Institute, “The structural conservation of panel paintings”, Proceedings of a Symposium at the J. Paul Getty Museum, 24 - 28 April 1995</skos:editorialNote>
    <skos:topConceptOf rdf:resource="https://w3id.org/crmrp#Execution_Technique"/>
    <skos:closeMatch rdf:resource="http://vocab.getty.edu/page/aat/300053852"/>
    <skos:prefLabel xml:lang="en">Intarsia</skos:prefLabel>
    <rdfs:label xml:lang="en">Intarsia</rdfs:label>
    <skos:prefLabel xml:lang="it">Intarsio</skos:prefLabel>
    <skos:editorialNote xml:lang="en">Getty AAT http://vocab.getty.edu/page/aat/300053852</skos:editorialNote>
  </rdf:Description>
  <rdf:Description rdf:about="https://w3id.org/crmrp#c_003d58ac">
    <skos:prefLabel xml:lang="en">Secco</skos:prefLabel>
    <skos:editorialNote xml:lang="en">Getty AAT http://vocab.getty.edu/page/aat/300053374</skos:editorialNote>
    <rdf:type rdf:resource="http://www.w3.org/2002/07/owl#NamedIndividual"/>
    <skos:inScheme rdf:resource="https://w3id.org/crmrp#Execution_Technique"/>
    <skos:altLabel xml:lang="en">Fresco secco</skos:altLabel>
    <skos:closeMatch rdf:resource="http://vocab.getty.edu/page/aat/300053374"/>
    <skos:note xml:lang="en">The preferred editorial note and the definition closest to the meaning is EwaGlos - European Illustrated Glossary of conservation terms for wall paintings and architectural surfaces</skos:note>
    <skos:editorialNote xml:lang="en">A. Weyer et al., “EwaGlos - European Illustrated Glossary of conservation terms for wall paintings and architectural surfaces”, Michael Imhof Verlag, Petersberg, Germany</skos:editorialNote>
    <skos:definition xml:lang="en">A wall painting technique where pigments mixed with an organic binder and /or lime are applied onto a dry plaster.</skos:definition>
    <rdfs:label xml:lang="en">Secco</rdfs:label>
    <skos:prefLabel xml:lang="it">A secco</skos:prefLabel>
    <rdf:type rdf:resource="http://www.w3.org/2004/02/skos/core#Concept"/>
    <skos:broader rdf:resource="https://w3id.org/crmrp#c_6626f18c"/>
    <skos:topConceptOf rdf:resource="https://w3id.org/crmrp#Execution_Technique"/>
  </rdf:Description>
  <rdf:Description rdf:about="https://w3id.org/crmrp#c_d9bb34c7">
    <skos:editorialNote xml:lang="en">Getty AAT http://vocab.getty.edu/page/aat/300435419</skos:editorialNote>
    <rdf:type rdf:resource="http://www.w3.org/2004/02/skos/core#Concept"/>
    <skos:inScheme rdf:resource="https://w3id.org/crmrp#Documentation"/>
    <skos:definition xml:lang="en">List, note, or other recording of the bibliography for a work or other entity's documentation.</skos:definition>
    <skos:exactMatch rdf:resource="http://vocab.getty.edu/page/aat/300435419"/>
    <skos:prefLabel xml:lang="en">Bibliography</skos:prefLabel>
    <rdf:type rdf:resource="http://www.w3.org/2002/07/owl#NamedIndividual"/>
    <rdfs:label xml:lang="en">Bibliography</rdfs:label>
    <skos:topConceptOf rdf:resource="https://w3id.org/crmrp#Documentation"/>
    <skos:prefLabel xml:lang="it">Bibliografia</skos:prefLabel>
    <skos:broader rdf:resource="https://w3id.org/crmrp#c_5b7fce15"/>
  </rdf:Description>
  <rdf:Description rdf:about="https://w3id.org/crmrp#c_6aacbe2f">
    <skos:editorialNote xml:lang="en">A. Weyer et al., “EwaGlos - European Illustrated Glossary of conservation terms for wall paintings and architectural surfaces”, Michael Imhof Verlag, Petersberg, Germany</skos:editorialNote>
    <skos:altLabel xml:lang="it">Delaminazione</skos:altLabel>
    <skos:altLabel xml:lang="en">Peeling</skos:altLabel>
    <rdf:type rdf:resource="http://www.w3.org/2002/07/owl#NamedIndividual"/>
    <skos:editorialNote xml:lang="en">Verg`es-Belmin et al., ICOMOS-ISCS: Illustrated glossary on stone deterioration patterns, vol. XV. Icomos International Council on Monuments and Sites, 2008</skos:editorialNote>
    <skos:topConceptOf rdf:resource="https://w3id.org/crmrp#Alteration"/>
    <rdfs:label xml:lang="en">Exfoliation</rdfs:label>
    <skos:altLabel xml:lang="en">Delamination</skos:altLabel>
    <skos:editorialNote xml:lang="en">Uni Cen/Ts 17135:2021 - Conservation of cultural heritage. General terms and definitions</skos:editorialNote>
    <skos:definition xml:lang="en">Separation into layers</skos:definition>
    <skos:prefLabel xml:lang="it">Esfoliazione</skos:prefLabel>
    <skos:prefLabel xml:lang="en">Exfoliation</skos:prefLabel>
    <skos:editorialNote xml:lang="en">Getty Conservation Institute “Illustrated Glossary - Definitions of terms used for the graphic documentation of in situ floor mosaics”, “Mosaics In Situ Project”, Los Angeles, 2003</skos:editorialNote>
    <skos:inScheme rdf:resource="https://w3id.org/crmrp#Alteration"/>
    <rdf:type rdf:resource="http://www.w3.org/2004/02/skos/core#Concept"/>
  </rdf:Description>
  <rdf:Description rdf:about="https://w3id.org/crmrp#c_ae321441">
    <skos:note xml:lang="en">The preferred editorial note and the definition closest to the meaning is Uni Cen/Ts 17135:2021</skos:note>
    <skos:inScheme rdf:resource="https://w3id.org/crmrp#Alteration"/>
    <rdf:type rdf:resource="http://www.w3.org/2002/07/owl#NamedIndividual"/>
    <skos:prefLabel xml:lang="en">Corroded</skos:prefLabel>
    <skos:topConceptOf rdf:resource="https://w3id.org/crmrp#Alteration"/>
    <skos:editorialNote xml:lang="en"> A. Weyer et al., “EwaGlos - European Illustrated Glossary of conservation terms for wall paintings and architectural surfaces”, Michael Imhof Verlag, Petersberg, Germany</skos:editorialNote>
    <skos:editorialNote xml:lang="en">Uni Cen/Ts 17135:2021 - Conservation of cultural heritage. General terms and definitions</skos:editorialNote>
    <skos:exactMatch rdf:resource="http://vocab.getty.edu/page/aat/300054107"/>
    <skos:editorialNote xml:lang="en">Getty AAT http://vocab.getty.edu/page/aat/300054107</skos:editorialNote>
    <rdfs:label xml:lang="en">Corroded</rdfs:label>
    <skos:altLabel xml:lang="en">Corrosion</skos:altLabel>
    <skos:prefLabel xml:lang="it">Corrosione</skos:prefLabel>
    <skos:definition xml:lang="en">Exhibiting transformation by chemical reaction with the environment.</skos:definition>
    <rdf:type rdf:resource="http://www.w3.org/2004/02/skos/core#Concept"/>
  </rdf:Description>
  <rdf:Description rdf:about="https://w3id.org/crmrp#Restoration_Object">
    <skos:prefLabel xml:lang="it">Bene (culturale)</skos:prefLabel>
    <skos:prefLabel xml:lang="en">Restoration object</skos:prefLabel>
    <skos:note xml:lang="en">International references could not be found</skos:note>
    <rdf:type rdf:resource="http://www.w3.org/2004/02/skos/core#ConceptScheme"/>
    <rdf:type rdf:resource="http://www.w3.org/2002/07/owl#NamedIndividual"/>
  </rdf:Description>
  <rdf:Description rdf:about="https://w3id.org/crmrp#c_694546c0">
    <rdf:type rdf:resource="http://www.w3.org/2002/07/owl#NamedIndividual"/>
    <rdf:type rdf:resource="http://www.w3.org/2004/02/skos/core#Concept"/>
    <skos:editorialNote xml:lang="en">Getty AAT http://vocab.getty.edu/page/aat/300193147</skos:editorialNote>
    <skos:inScheme rdf:resource="https://w3id.org/crmrp#Execution_Technique"/>
    <skos:closeMatch rdf:resource="http://vocab.getty.edu/page/aat/300193147"/>
    <skos:prefLabel xml:lang="it">Bulino</skos:prefLabel>
    <skos:topConceptOf rdf:resource="https://w3id.org/crmrp#Execution_Technique"/>
    <skos:broader rdf:resource="https://w3id.org/crmrp#c_aee6a805"/>
    <skos:definition xml:lang="en">Tools used in printmaking for engraving metal plates or end-grain wood blocks, consisting of a small steel rod, of square or lozenge section, with a sharpened point, and having a half-round wood handle that fits in the palm of the hand. In the context of archaeology, a specialized flake or blade with a chisel edge; used to carve or engrave softer materials such as bone, wood, or antler. For various tools for chasing or engraving metal or wood, use gravers.</skos:definition>
    <rdfs:label xml:lang="en">Burins</rdfs:label>
    <skos:prefLabel xml:lang="en">Burins</skos:prefLabel>
  </rdf:Description>
  <rdf:Description rdf:about="https://w3id.org/crmrp#c_52e9c866">
    <skos:prefLabel xml:lang="it">Pastiglia</skos:prefLabel>
    <skos:inScheme rdf:resource="https://w3id.org/crmrp#Execution_Technique"/>
    <rdfs:label xml:lang="en">Pastille gilding</rdfs:label>
    <rdf:type rdf:resource="http://www.w3.org/2004/02/skos/core#Concept"/>
    <skos:definition xml:lang="en">A technique used by ancient decorators to reproduce friezes and high reliefs on different supports. The mixture consists of plaster, scagliola and starch glue.</skos:definition>
    <skos:note xml:lang="en">International references could not be found</skos:note>
    <skos:editorialNote xml:lang="it">C. Giannini, “Dizionario del restauro - Tecniche diagnostica conservazione”, Nardini Editore, Firenze, 2010</skos:editorialNote>
    <rdf:type rdf:resource="http://www.w3.org/2002/07/owl#NamedIndividual"/>
    <skos:topConceptOf rdf:resource="https://w3id.org/crmrp#Execution_Technique"/>
    <skos:prefLabel xml:lang="en">Pastille gilding</skos:prefLabel>
    <skos:broader rdf:resource="https://w3id.org/crmrp#c_4d471b17"/>
    <skos:editorialNote xml:lang="it">G. Pignolo, “Effetti d’oro - Storia e tecnica della doratura nell’arte”, Editrice Compositori, Bologna, 2002</skos:editorialNote>
  </rdf:Description>
  <rdf:Description rdf:about="https://w3id.org/crmrp#c_fa940954">
    <rdfs:label xml:lang="en">Consumption</rdfs:label>
    <skos:note xml:lang="en">International references could not be found</skos:note>
    <rdf:type rdf:resource="http://www.w3.org/2004/02/skos/core#Concept"/>
    <skos:editorialNote xml:lang="it">C. Giannini, “Dizionario del restauro - Tecniche diagnostica conservazione”, Nardini Editore, Firenze, 2010</skos:editorialNote>
    <rdf:type rdf:resource="http://www.w3.org/2002/07/owl#NamedIndividual"/>
    <skos:prefLabel xml:lang="en">Consumption</skos:prefLabel>
    <skos:inScheme rdf:resource="https://w3id.org/crmrp#Alteration"/>
    <skos:topConceptOf rdf:resource="https://w3id.org/crmrp#Alteration"/>
    <skos:definition xml:lang="en">Form of degradation by rubbing to which floors with mosaic, stone, ceramic etc. decorations are subjected due to continuous trampling; it can lead to the total loss of the coating. The term is also used in relation to the state of conservation of paintings or to indicate the alteration of a work, linked to a particular religious cult, subjected to the touch or continuous rubbing of the faithful on one or more points of the surface. It may refer more generally to the wear and tear of objects of artistic value as a consequence of the use that was originally made of them.</skos:definition>
    <skos:prefLabel xml:lang="it">Consunzione</skos:prefLabel>
  </rdf:Description>
  <rdf:Description rdf:about="https://w3id.org/crmrp#RP3_has_intervention">
    <rdfs:label xml:lang="en">has intervention</rdfs:label>
    <rdfs:comment>This property links R7 Restoration Project to R8 Intervention.
This property allows you to specify which operations (or interventions) were performed during the restoration.</rdfs:comment>
    <rdfs:range rdf:resource="https://w3id.org/crmrp#R8_Intervention"/>
    <rdfs:domain rdf:resource="https://w3id.org/crmrp#R7_Restoration_Project"/>
    <rdf:type rdf:resource="http://www.w3.org/2002/07/owl#ObjectProperty"/>
  </rdf:Description>
  <rdf:Description rdf:about="https://w3id.org/crmrp#c_088ec8d4">
    <skos:closeMatch rdf:resource="http://vocab.getty.edu/page/aat/300010662"/>
    <skos:definition xml:lang="en">Pottery with a porous body, fired below 1200 degrees Centigrade. It is not vitrified, and must be glazed to render it nonporous</skos:definition>
    <skos:prefLabel xml:lang="en">Earthenware</skos:prefLabel>
    <skos:broader rdf:resource="https://w3id.org/crmrp#c_bd34e984"/>
    <rdf:type rdf:resource="http://www.w3.org/2002/07/owl#NamedIndividual"/>
    <rdf:type rdf:resource="http://www.w3.org/2004/02/skos/core#Concept"/>
    <skos:prefLabel xml:lang="it">Terraglia</skos:prefLabel>
    <skos:inScheme rdf:resource="https://w3id.org/crmrp#Material"/>
    <skos:editorialNote xml:lang="en">Getty AAT http://vocab.getty.edu/page/aat/300010662</skos:editorialNote>
    <rdfs:label xml:lang="en">Earthenware</rdfs:label>
    <skos:topConceptOf rdf:resource="https://w3id.org/crmrp#Material"/>
  </rdf:Description>
  <rdf:Description rdf:about="https://w3id.org/crmrp#c_49988b8d">
    <skos:inScheme rdf:resource="https://w3id.org/crmrp#Alteration"/>
    <skos:topConceptOf rdf:resource="https://w3id.org/crmrp#Alteration"/>
    <skos:prefLabel xml:lang="en">Xylophagous attack</skos:prefLabel>
    <rdfs:label xml:lang="en">Xylophagous attack</rdfs:label>
    <skos:prefLabel xml:lang="it">Attacco xilofago</skos:prefLabel>
    <rdf:type rdf:resource="http://www.w3.org/2002/07/owl#NamedIndividual"/>
    <skos:broader rdf:resource="https://w3id.org/crmrp#c_3ef20257"/>
    <rdf:type rdf:resource="http://www.w3.org/2004/02/skos/core#Concept"/>
    <skos:note xml:lang="en">International references could not be found</skos:note>
    <skos:definition xml:lang="en">A category of insects belonging to numerous orders and families (Lepidoptera Cossidae, Bostricidae beetles, Scolytidae, Cerambidae, Buprestidae, Hymenoptera Siricidae); they feed on wood even after the plant has been felled and are one of the causes of the degradation of the substrates of wooden artefacts, in which they dig tunnels tunnels that make the material porous and fragile, destructuring it.</skos:definition>
  </rdf:Description>
  <rdf:Description rdf:about="https://w3id.org/crmrp#c_945b8f77">
    <rdf:type rdf:resource="http://www.w3.org/2002/07/owl#NamedIndividual"/>
    <rdf:type rdf:resource="http://www.w3.org/2004/02/skos/core#Concept"/>
    <rdfs:label xml:lang="en">Copper</rdfs:label>
    <skos:prefLabel xml:lang="it">Rame</skos:prefLabel>
    <skos:prefLabel xml:lang="en">Copper</skos:prefLabel>
    <skos:topConceptOf rdf:resource="https://w3id.org/crmrp#Material"/>
    <skos:definition xml:lang="en">Pure metallic element having the symbol Cu and atomic number 29; a reddish brown, ductile metal that is present in the earth's crust, occurring as a native metal and as ores of sulfide, sulfate and carbonate (azurite, malachite, etc.). It was the first metal used by humans, probably from about 8000 BCE, in the regions of Mesopotamia and India. By about 3800 BCE copper was made into bronze for weapons and knives. Today, copper is one of the most widely used metals because it has high electrical and thermal conductivity, can be easily fabricated, is ductile and polishes well. In moist air, copper forms a protective green film of basic carbonate. Metallic copper combines well with other metals to form alloys, most commonly brass and bronze. Copper and its alloys are used for wire, electrical devices, pipes, cooking vessels, ammunition, ornamental trim, roofing, grillwork, coins, musical instruments, jewelry, and sculptures.</skos:definition>
    <skos:exactMatch rdf:resource="http://vocab.getty.edu/page/aat/300011020"/>
    <skos:source xml:lang="en">Getty AAT http://vocab.getty.edu/page/aat/300011020</skos:source>
    <skos:broader rdf:resource="https://w3id.org/crmrp#c_6407466f"/>
    <skos:inScheme rdf:resource="https://w3id.org/crmrp#Material"/>
  </rdf:Description>
  <rdf:Description rdf:about="https://w3id.org/crmrp#c_4064717d">
    <skos:prefLabel xml:lang="it">Stereomicroscopio</skos:prefLabel>
    <skos:editorialNote xml:lang="en">M.Ceroni, G.Elia, “Diagnostica per i beni culturali”, Alinea editrice, Firenze, 2008</skos:editorialNote>
    <skos:inScheme rdf:resource="https://w3id.org/crmrp#Archeometric_and_Diagnostic_Analysis"/>
    <rdf:type rdf:resource="http://www.w3.org/2002/07/owl#NamedIndividual"/>
    <rdf:type rdf:resource="http://www.w3.org/2004/02/skos/core#Concept"/>
    <skos:prefLabel xml:lang="en">Stereomicroscope</skos:prefLabel>
    <skos:topConceptOf rdf:resource="https://w3id.org/crmrp#Archeometric_and_Diagnostic_Analysis"/>
    <rdfs:label xml:lang="en">Stereomicroscope</rdfs:label>
    <skos:broader rdf:resource="https://w3id.org/crmrp#c_abed88a5"/>
    <skos:definition xml:lang="en">The stereoscopic microscope, also known as stereomicroscope, microstereoscope or dissector, is a type of optical microscope designed to produce a stereoscopic view of an object.</skos:definition>
    <skos:note xml:lang="en">International references could not be found</skos:note>
  </rdf:Description>
  <rdf:Description rdf:about="https://w3id.org/crmrp#c_e7a46f25">
    <rdf:type rdf:resource="http://www.w3.org/2004/02/skos/core#Concept"/>
    <rdfs:label xml:lang="en">Radiocarbon dating</rdfs:label>
    <skos:topConceptOf rdf:resource="https://w3id.org/crmrp#Archeometric_and_Diagnostic_Analysis"/>
    <skos:prefLabel xml:lang="it">Radiocarbonio</skos:prefLabel>
    <skos:prefLabel xml:lang="en">Radiocarbon dating</skos:prefLabel>
    <skos:inScheme rdf:resource="https://w3id.org/crmrp#Archeometric_and_Diagnostic_Analysis"/>
    <rdf:type rdf:resource="http://www.w3.org/2002/07/owl#NamedIndividual"/>
    <skos:editorialNote xml:lang="en">Getty AAT http://vocab.getty.edu/page/aat/300054717</skos:editorialNote>
    <skos:definition xml:lang="en">Method of dating, based on the known half-life of carbon-14, by measuring the amount of low-level radioactivity of carbon remaining in ancient and dead material of organic origin and thus determining when a plant or animal had died.</skos:definition>
    <skos:broader rdf:resource="https://w3id.org/crmrp#c_abed88a5"/>
    <skos:exactMatch rdf:resource="http://vocab.getty.edu/page/aat/300054717"/>
  </rdf:Description>
  <rdf:Description rdf:about="http://www.w3.org/2004/02/skos/core#broader">
    <rdf:type rdf:resource="http://www.w3.org/2002/07/owl#AnnotationProperty"/>
  </rdf:Description>
  <rdf:Description rdf:about="https://w3id.org/crmrp#c_ba5a5776">
    <skos:topConceptOf rdf:resource="https://w3id.org/crmrp#Documentation"/>
    <skos:prefLabel xml:lang="it">Documentazione video-cinematografica</skos:prefLabel>
    <skos:prefLabel xml:lang="en">Video documentation</skos:prefLabel>
    <skos:note xml:lang="en">International references could not be found</skos:note>
    <skos:inScheme rdf:resource="https://w3id.org/crmrp#Documentation"/>
    <skos:definition xml:lang="en">Any video of an object that testifies its history or the way it was made, especially interesting for contemporary art, where the artist is sometimes shown at work.</skos:definition>
    <rdfs:label xml:lang="en">Video documentation</rdfs:label>
    <rdf:type rdf:resource="http://www.w3.org/2004/02/skos/core#Concept"/>
    <rdf:type rdf:resource="http://www.w3.org/2002/07/owl#NamedIndividual"/>
  </rdf:Description>
  <rdf:Description rdf:about="http://www.cidoc-crm.org/cidoc-crm/P70i_is_documented_in">
    <rdfs:range rdf:resource="http://www.cidoc-crm.org/cidoc-crm/E31_Document"/>
    <rdfs:domain rdf:resource="https://w3id.org/crmrp#R7_Restoration_Project"/>
  </rdf:Description>
  <rdf:Description rdf:about="https://w3id.org/crmrp#c_8c762c3e">
    <rdfs:label xml:lang="en">Crack</rdfs:label>
    <skos:topConceptOf rdf:resource="https://w3id.org/crmrp#Alteration"/>
    <skos:altLabel xml:lang="it">Fratturazione</skos:altLabel>
    <skos:editorialNote xml:lang="en">Uni Cen/Ts 17135:2021 - Conservation of cultural heritage. General terms and definitions</skos:editorialNote>
    <skos:editorialNote xml:lang="en">Getty Conservation Institute “Illustrated Glossary - Definitions of terms used for the graphic documentation of in situ floor mosaics”, “Mosaics In Situ Project”, Los Angeles, 2003</skos:editorialNote>
    <skos:altLabel xml:lang="en">Fracture</skos:altLabel>
    <skos:definition xml:lang="en">Separation of a solid material without breaking apart.</skos:definition>
    <skos:note xml:lang="en">The preferred editorial note and the definition closest to the meaning is Uni Cen/Ts 17135:2021</skos:note>
    <skos:prefLabel xml:lang="it">Fessurazione</skos:prefLabel>
    <skos:editorialNote xml:lang="en">Verg`es-Belmin et al., ICOMOS-ISCS: Illustrated glossary on stone deterioration patterns, vol. XV. Icomos International Council on Monuments and Sites, 2008</skos:editorialNote>
    <rdf:type rdf:resource="http://www.w3.org/2002/07/owl#NamedIndividual"/>
    <skos:editorialNote xml:lang="en">A. Weyer et al., “EwaGlos - European Illustrated Glossary of conservation terms for wall paintings and architectural surfaces”, Michael Imhof Verlag, Petersberg, Germany</skos:editorialNote>
    <skos:prefLabel xml:lang="en">Crack</skos:prefLabel>
    <skos:inScheme rdf:resource="https://w3id.org/crmrp#Alteration"/>
    <rdf:type rdf:resource="http://www.w3.org/2004/02/skos/core#Concept"/>
  </rdf:Description>
  <rdf:Description rdf:about="https://w3id.org/crmrp#c_b7c4df2f">
    <skos:broader rdf:resource="https://w3id.org/crmrp#c_bd34e984"/>
    <rdf:type rdf:resource="http://www.w3.org/2002/07/owl#NamedIndividual"/>
    <skos:prefLabel xml:lang="it">Grés</skos:prefLabel>
    <skos:prefLabel xml:lang="en">Grés</skos:prefLabel>
    <rdfs:label xml:lang="en">Grés</rdfs:label>
    <rdf:type rdf:resource="http://www.w3.org/2004/02/skos/core#Concept"/>
    <skos:definition xml:lang="en">A type of pottery midway between earthenware and porcelain being made of clay and a fusible stone. It is fired to a point where partial vitrification renders it impervious to liquids, but, unlike porcelain, it is very seldom more than faintly translucent. The vitrification makes it unnecessary to add a glaze, but for reasons of utility and appearance decorative glazes are sometimes used, such as salt glaze and lead glaze.</skos:definition>
    <skos:inScheme rdf:resource="https://w3id.org/crmrp#Material"/>
    <skos:topConceptOf rdf:resource="https://w3id.org/crmrp#Material"/>
    <skos:closeMatch rdf:resource="http://vocab.getty.edu/page/aat/300010672"/>
    <skos:editorialNote xml:lang="en">Getty AAT http://vocab.getty.edu/page/aat/300010672</skos:editorialNote>
  </rdf:Description>
  <rdf:Description rdf:about="https://w3id.org/crmrp#c_7cb6da0e">
    <skos:editorialNote xml:lang="en">Verg`es-Belmin et al., ICOMOS-ISCS: Illustrated glossary on stone deterioration patterns, vol. XV. Icomos International Council on Monuments and Sites, 2008</skos:editorialNote>
    <skos:definition xml:lang="en">Human exèressions by engraving, scratching, addition of paint, link or other material applied to the surface of an object.</skos:definition>
    <skos:prefLabel xml:lang="it">Graffito</skos:prefLabel>
    <skos:prefLabel xml:lang="en">Graffiti</skos:prefLabel>
    <skos:topConceptOf rdf:resource="https://w3id.org/crmrp#Alteration"/>
    <skos:note xml:lang="en">The preferred editorial note and the definition closest to the meaning is Uni Cen/Ts 17135:2021</skos:note>
    <rdf:type rdf:resource="http://www.w3.org/2004/02/skos/core#Concept"/>
    <rdf:type rdf:resource="http://www.w3.org/2002/07/owl#NamedIndividual"/>
    <skos:altLabel xml:lang="en">Anthropically induced deterioration</skos:altLabel>
    <skos:inScheme rdf:resource="https://w3id.org/crmrp#Alteration"/>
    <rdfs:label xml:lang="en">Graffiti</rdfs:label>
    <skos:editorialNote xml:lang="en">A. Weyer et al., “EwaGlos - European Illustrated Glossary of conservation terms for wall paintings and architectural surfaces”, Michael Imhof Verlag, Petersberg, Germany</skos:editorialNote>
    <skos:editorialNote xml:lang="en">Uni Cen/Ts 17135:2021 - Conservation of cultural heritage. General terms and definitions</skos:editorialNote>
  </rdf:Description>
  <rdf:Description rdf:about="https://w3id.org/crmrp#c_6407466f">
    <skos:prefLabel xml:lang="it">Metallo</skos:prefLabel>
    <rdf:type rdf:resource="http://www.w3.org/2004/02/skos/core#Concept"/>
    <skos:inScheme rdf:resource="https://w3id.org/crmrp#Material"/>
    <rdfs:label xml:lang="en">Metal</rdfs:label>
    <skos:editorialNote xml:lang="en">Getty AAT http://vocab.getty.edu/page/aat/300010900</skos:editorialNote>
    <rdf:type rdf:resource="http://www.w3.org/2002/07/owl#NamedIndividual"/>
    <skos:closeMatch rdf:resource="http://vocab.getty.edu/page/aat/300010900"/>
    <skos:definition xml:lang="en">Any of a large group of substances that typically show a characteristic luster, are good conductors of electricity and heat, are opaque, can be fused, and are usually malleable or ductile.</skos:definition>
    <skos:topConceptOf rdf:resource="https://w3id.org/crmrp#Material"/>
    <skos:prefLabel xml:lang="en">Metal</skos:prefLabel>
  </rdf:Description>
  <rdf:Description rdf:about="https://w3id.org/crmrp#c_49aa1adb">
    <skos:prefLabel xml:lang="it">Dosaggio sali solubili</skos:prefLabel>
    <rdfs:label xml:lang="en">Dosing of soluble salts</rdfs:label>
    <skos:defintion xml:lang="en">The test is conducted in order to determine the presence of specific soluble salts (qualitative analysis) and to detect a range within which the concentration of the detected salts can be found</skos:defintion>
    <rdf:type rdf:resource="http://www.w3.org/2004/02/skos/core#Concept"/>
    <skos:topConceptOf rdf:resource="https://w3id.org/crmrp#Archeometric_and_Diagnostic_Analysis"/>
    <rdf:type rdf:resource="http://www.w3.org/2002/07/owl#NamedIndividual"/>
    <skos:note xml:lang="en">International references could not be found</skos:note>
    <skos:inScheme rdf:resource="https://w3id.org/crmrp#Archeometric_and_Diagnostic_Analysis"/>
    <skos:editorialNote xml:lang="it">UNI 11087:2003 Beni culturali - Materiali lapidei naturali ed artificiali - Determinazione del contenuto di sali solubili</skos:editorialNote>
    <skos:broader rdf:resource="https://w3id.org/crmrp#c_abed88a5"/>
    <skos:prefLabel xml:lang="en">Dosing of soluble salts</skos:prefLabel>
  </rdf:Description>
  <rdf:Description rdf:about="https://w3id.org/crmrp#c_3523110e">
    <rdf:type rdf:resource="http://www.w3.org/2002/07/owl#NamedIndividual"/>
    <rdfs:label xml:lang="en">Low pressure karsten tube</rdfs:label>
    <rdf:type rdf:resource="http://www.w3.org/2004/02/skos/core#Concept"/>
    <skos:editorialNote xml:lang="it">UNI EN 16302:2013 Conservazione dei Beni Culturali - Metodi di prova - Misura dell'assorbimento di acqua con il metodo della pipetta</skos:editorialNote>
    <skos:prefLabel xml:lang="it">Misura dell'assorbimento di acqua con il metodo della pipetta</skos:prefLabel>
    <skos:inScheme rdf:resource="https://w3id.org/crmrp#Archeometric_and_Diagnostic_Analysis"/>
    <skos:prefLabel xml:lang="en">Low pressure karsten tube</skos:prefLabel>
    <skos:definition xml:lang="en">The low-pressure water absorption method is performed to determine the volume of water absorbed at low pressure by a given surface of material, after a set time.</skos:definition>
    <skos:note xml:lang="en">International references could not be found</skos:note>
    <skos:broader rdf:resource="https://w3id.org/crmrp#c_1fd6102e"/>
    <skos:topConceptOf rdf:resource="https://w3id.org/crmrp#Archeometric_and_Diagnostic_Analysis"/>
  </rdf:Description>
  <rdf:Description rdf:about="https://w3id.org/crmrp#c_4a72d11e">
    <skos:editorialNote xml:lang="en"> A. Weyer et al., “EwaGlos - European Illustrated Glossary of conservation terms for wall paintings and architectural surfaces”, Michael Imhof Verlag, Petersberg, Germany</skos:editorialNote>
    <skos:prefLabel xml:lang="en">Abrasion</skos:prefLabel>
    <skos:exactMatch rdf:resource="http://vocab.getty.edu/page/aat/300053077"/>
    <skos:editorialNote xml:lang="en">Verg`es-Belmin et al., ICOMOS-ISCS: Illustrated glossary on stone deterioration patterns, vol. XV. Icomos International Council on Monuments and Sites, 2008</skos:editorialNote>
    <rdf:type rdf:resource="http://www.w3.org/2004/02/skos/core#Concept"/>
    <skos:topConceptOf rdf:resource="https://w3id.org/crmrp#Alteration"/>
    <skos:definition xml:lang="en">loss of material from a surface due to frictional forces.</skos:definition>
    <rdf:type rdf:resource="http://www.w3.org/2002/07/owl#NamedIndividual"/>
    <skos:editorialNote xml:lang="en">Uni Cen/Ts 17135:2021 - Conservation of cultural heritage. General terms and definitions</skos:editorialNote>
    <skos:prefLabel xml:lang="it">Abrasione</skos:prefLabel>
    <skos:editorialNote xml:lang="en">Getty AAT http://vocab.getty.edu/page/aat/300053077</skos:editorialNote>
    <skos:inScheme rdf:resource="https://w3id.org/crmrp#Alteration"/>
    <skos:note xml:lang="en">The preferred editorial note and the definition closest to the meaning is Uni Cen/Ts 17135:2021</skos:note>
    <rdfs:label xml:lang="en">Abrasion</rdfs:label>
  </rdf:Description>
  <rdf:Description rdf:about="https://w3id.org/crmrp#c_1285fa71">
    <skos:definition xml:lang="en">It is a non-invasive technique that does not damage the works and allows the underlying layers of paintings on canvas, panel or paper to be revealed</skos:definition>
    <skos:note xml:lang="en">International references could not be found</skos:note>
    <rdf:type rdf:resource="http://www.w3.org/2004/02/skos/core#Concept"/>
    <skos:prefLabel xml:lang="it">Riflettografia</skos:prefLabel>
    <skos:topConceptOf rdf:resource="https://w3id.org/crmrp#Archeometric_and_Diagnostic_Analysis"/>
    <skos:editorialNote xml:lang="it">C. Giannini, “Dizionario del restauro - Tecniche diagnostica conservazione”, Nardini Editore, Firenze, 2010</skos:editorialNote>
    <skos:broader rdf:resource="https://w3id.org/crmrp#c_1fd6102e"/>
    <skos:inScheme rdf:resource="https://w3id.org/crmrp#Archeometric_and_Diagnostic_Analysis"/>
    <skos:prefLabel xml:lang="en">Reflectography</skos:prefLabel>
    <rdfs:label xml:lang="en">Reflectography</rdfs:label>
    <rdf:type rdf:resource="http://www.w3.org/2002/07/owl#NamedIndividual"/>
  </rdf:Description>
  <rdf:Description rdf:about="https://w3id.org/crmrp#c_062492de">
    <skos:prefLabel xml:lang="en">Pointillism</skos:prefLabel>
    <skos:prefLabel xml:lang="it">Punteggiato</skos:prefLabel>
    <rdfs:label xml:lang="en">Pointillism</rdfs:label>
    <skos:definition xml:lang="en">The colour – and not necessarily the shape – of the damage or lacuna is reconstructed using a dense application of dots (wherever possible in pure colours).</skos:definition>
    <rdf:type rdf:resource="http://www.w3.org/2004/02/skos/core#Concept"/>
    <skos:broader rdf:resource="https://w3id.org/crmrp#c_326da7e4"/>
    <rdf:type rdf:resource="http://www.w3.org/2002/07/owl#NamedIndividual"/>
    <skos:topConceptOf rdf:resource="https://w3id.org/crmrp#Intervention"/>
    <skos:inScheme rdf:resource="https://w3id.org/crmrp#Intervention"/>
    <skos:editorialNote xml:lang="en">A. Weyer et al., “EwaGlos - European Illustrated Glossary of conservation terms for wall paintings and architectural surfaces”, Michael Imhof Verlag, Petersberg, Germany</skos:editorialNote>
  </rdf:Description>
  <rdf:Description rdf:about="http://www.w3.org/2004/02/skos/core#definition">
    <rdfs:subPropertyOf rdf:resource="http://www.w3.org/2000/01/rdf-schema#label"/>
    <rdf:type rdf:resource="http://www.w3.org/2002/07/owl#AnnotationProperty"/>
  </rdf:Description>
  <rdf:Description rdf:about="https://w3id.org/crmrp#c_1381790a">
    <skos:editorialNote xml:lang="en">Getty AAT http://vocab.getty.edu/page/aat/300265183</skos:editorialNote>
    <rdfs:label xml:lang="en">Faience</rdfs:label>
    <skos:inScheme rdf:resource="https://w3id.org/crmrp#Material"/>
    <skos:closeMatch rdf:resource="http://vocab.getty.edu/page/aat/30026518"/>
    <skos:broader rdf:resource="https://w3id.org/crmrp#c_bd34e984"/>
    <skos:prefLabel xml:lang="it">Faience</skos:prefLabel>
    <skos:prefLabel xml:lang="en">Faience</skos:prefLabel>
    <rdf:type rdf:resource="http://www.w3.org/2004/02/skos/core#Concept"/>
    <rdf:type rdf:resource="http://www.w3.org/2002/07/owl#NamedIndividual"/>
    <skos:definition xml:lang="en">A composite material consisting of a body of sintered quartz coupled with an alkaline glaze surface, and used for decorating beads, amulets, figurines, and other small objects. It was invented in Mesopotamia or Iran ca. 4500 BCE, and produced through the mid-7th century CE.</skos:definition>
    <skos:topConceptOf rdf:resource="https://w3id.org/crmrp#Material"/>
  </rdf:Description>
  <rdf:Description rdf:about="http://www.w3.org/2004/02/skos/core#closeMatc">
    <rdf:type rdf:resource="http://www.w3.org/2002/07/owl#AnnotationProperty"/>
  </rdf:Description>
  <rdf:Description rdf:about="https://w3id.org/crmrp#c_49fed917">
    <skos:broader rdf:resource="https://w3id.org/crmrp#c_044b6056"/>
    <skos:prefLabel xml:lang="it">Acquerello</skos:prefLabel>
    <skos:topConceptOf rdf:resource="https://w3id.org/crmrp#Execution_Technique"/>
    <rdf:type rdf:resource="http://www.w3.org/2002/07/owl#NamedIndividual"/>
    <rdf:type rdf:resource="http://www.w3.org/2004/02/skos/core#Concept"/>
    <skos:altLabel xml:lang="en">Watercolour</skos:altLabel>
    <skos:inScheme rdf:resource="https://w3id.org/crmrp#Execution_Technique"/>
    <skos:definition xml:lang="en">Watercolor painting done in transparent washes of color as distinguished from the opaque method using gouache</skos:definition>
    <skos:exactMatch rdf:resource="http://vocab.getty.edu/page/aat/300053363"/>
    <skos:prefLabel xml:lang="en">Aquarelle</skos:prefLabel>
    <skos:editorialNote xml:lang="en">Getty AAT http://vocab.getty.edu/page/aat/300053363</skos:editorialNote>
    <rdfs:label xml:lang="en">Aquarelle</rdfs:label>
  </rdf:Description>
  <rdf:Description rdf:about="https://w3id.org/crmrp#c_5ca7c66b">
    <skos:topConceptOf rdf:resource="https://w3id.org/crmrp#Intervention"/>
    <skos:inScheme rdf:resource="https://w3id.org/crmrp#Intervention"/>
    <rdfs:label xml:lang="en">Surface active agent</rdfs:label>
    <skos:broader rdf:resource="https://w3id.org/crmrp#c_5a83cd16"/>
    <rdf:type rdf:resource="http://www.w3.org/2004/02/skos/core#Concept"/>
    <rdf:type rdf:resource="http://www.w3.org/2002/07/owl#NamedIndividual"/>
    <skos:exactMatch rdf:resource="http://vocab.getty.edu/page/aat/300015321"/>
    <skos:prefLabel xml:lang="en">Surface active agent</skos:prefLabel>
    <skos:editorialNote xml:lang="en">Getty AAT http://vocab.getty.edu/page/aat/300015321</skos:editorialNote>
    <skos:prefLabel xml:lang="it">Tensioattivo</skos:prefLabel>
    <skos:definition xml:lang="en">Compound able to reduce the surface tension of liquid to which it is added.</skos:definition>
  </rdf:Description>
  <rdf:Description rdf:about="https://w3id.org/crmrp#c_777a4068">
    <skos:note xml:lang="en">The preferred editorial note and the definition closest to the meaning is Uni Cen/Ts 17135:2021</skos:note>
    <skos:editorialNote xml:lang="en">Getty AAT http://vocab.getty.edu/page/aat/300263354</skos:editorialNote>
    <skos:inScheme rdf:resource="https://w3id.org/crmrp#Alteration"/>
    <skos:topConceptOf rdf:resource="https://w3id.org/crmrp#Alteration"/>
    <rdf:type rdf:resource="http://www.w3.org/2004/02/skos/core#Concept"/>
    <skos:editorialNote xml:lang="en">Verg`es-Belmin et al., ICOMOS-ISCS: Illustrated glossary on stone deterioration patterns, vol. XV. Icomos International Council on Monuments and Sites, 2008</skos:editorialNote>
    <rdfs:label xml:lang="en">Lacuna</rdfs:label>
    <skos:prefLabel xml:lang="it">Lacuna</skos:prefLabel>
    <skos:prefLabel xml:lang="en">Lacuna</skos:prefLabel>
    <skos:editorialNote xml:lang="en">Uni Cen/Ts 17135:2021 - Conservation of cultural heritage. General terms and definitions</skos:editorialNote>
    <skos:altLabel xml:lang="en">Lacunae</skos:altLabel>
    <skos:closeMatch rdf:resource="http://vocab.getty.edu/page/aat/300263354"/>
    <skos:editorialNote xml:lang="en">A. Weyer et al., “EwaGlos - European Illustrated Glossary of conservation terms for wall paintings and architectural surfaces”, Michael Imhof Verlag, Petersberg, Germany</skos:editorialNote>
    <skos:definition xml:lang="en">Loss with a form defined by its relation to the rest of the object.</skos:definition>
    <rdf:type rdf:resource="http://www.w3.org/2002/07/owl#NamedIndividual"/>
  </rdf:Description>
  <rdf:Description rdf:about="https://w3id.org/crmrp#c_767414bb">
    <rdf:type rdf:resource="http://www.w3.org/2002/07/owl#NamedIndividual"/>
    <skos:broader rdf:resource="https://w3id.org/crmrp#c_49988b8d"/>
    <skos:note xml:lang="en">International references could not be found</skos:note>
    <skos:topConceptOf rdf:resource="https://w3id.org/crmrp#Alteration"/>
    <rdf:type rdf:resource="http://www.w3.org/2004/02/skos/core#Concept"/>
    <skos:inScheme rdf:resource="https://w3id.org/crmrp#Alteration"/>
    <skos:prefLabel xml:lang="en">Inactive xylophagous attack</skos:prefLabel>
    <skos:prefLabel xml:lang="it">Attacco xilofago inattivo</skos:prefLabel>
    <skos:definition xml:lang="en">an inactive xylophagus attack.</skos:definition>
    <rdfs:label xml:lang="en">Inactive xylophagous attack</rdfs:label>
  </rdf:Description>
  <rdf:Description rdf:about="https://w3id.org/crmrp#c_f80c2aa3">
    <skos:note xml:lang="en">The preferred editorial note and the definition closest to the meaning is ICOMOS-ISCS: Illustrated glossary on stone deterioration patterns</skos:note>
    <skos:prefLabel xml:lang="it">Presenza di vegetazione</skos:prefLabel>
    <skos:prefLabel xml:lang="en">Plant</skos:prefLabel>
    <rdf:type rdf:resource="http://www.w3.org/2002/07/owl#NamedIndividual"/>
    <skos:editorialNote xml:lang="en">Verg`es-Belmin et al., ICOMOS-ISCS: Illustrated glossary on stone deterioration patterns, vol. XV. Icomos International Council on Monuments and Sites, 2008</skos:editorialNote>
    <skos:broader rdf:resource="https://w3id.org/crmrp#c_3ef20257"/>
    <skos:topConceptOf rdf:resource="https://w3id.org/crmrp#Alteration"/>
    <skos:inScheme rdf:resource="https://w3id.org/crmrp#Alteration"/>
    <rdfs:label xml:lang="en">Plant</rdfs:label>
    <skos:altLabel xml:lang="en">Plant intrusion</skos:altLabel>
    <skos:definition xml:lang="en">Vegetal living being, having, when complete, root, stem, and leaves, though consisting sometimes only of a single leafy expansion (e.g. Tree, fern, herb).</skos:definition>
    <skos:editorialNote xml:lang="en">Getty Conservation Institute “Illustrated Glossary - Definitions of terms used for the graphic documentation of in situ floor mosaics”, “Mosaics In Situ Project”, Los Angeles, 2003</skos:editorialNote>
    <rdf:type rdf:resource="http://www.w3.org/2004/02/skos/core#Concept"/>
  </rdf:Description>
  <rdf:Description rdf:about="https://w3id.org/crmrp#c_1931dc9b">
    <skos:prefLabel xml:lang="it">Forma persa</skos:prefLabel>
    <skos:prefLabel xml:lang="en">Forma persa</skos:prefLabel>
    <skos:topConceptOf rdf:resource="https://w3id.org/crmrp#Execution_Technique"/>
    <skos:definition xml:lang="en">Plaster mould made on clay, plasticine or wax models that makes it possible to obtain a single plaster model, as for its extraction the form must be destroyed</skos:definition>
    <skos:editorialNote xml:lang="it">P. Clérin, “Manuale di scultura - Tecniche, materiali, realizzazioni”, Sovera editore, Roma, 1995</skos:editorialNote>
    <skos:broader rdf:resource="https://w3id.org/crmrp#c_17157ccd"/>
    <rdf:type rdf:resource="http://www.w3.org/2004/02/skos/core#Concept"/>
    <rdfs:label xml:lang="en">Forma persa</rdfs:label>
    <skos:note xml:lang="en">It was decided not to proceed with the English translation in order to avoid possible lexical errors and misunderstandings.</skos:note>
    <skos:inScheme rdf:resource="https://w3id.org/crmrp#Execution_Technique"/>
    <rdf:type rdf:resource="http://www.w3.org/2002/07/owl#NamedIndividual"/>
  </rdf:Description>
  <rdf:Description rdf:about="https://w3id.org/crmrp#c_fd858a66">
    <skos:definition xml:lang="en">Pavement usually made of same-sized rectangular ceramic fragments, inserted on their smaller side and assembled together in groups of a few elements. The orientation of adjacent groups is alternated so that their juxtaposition creates the visual impression of a basket weave pattern.</skos:definition>
    <skos:editorialNote xml:lang="en">Getty Conservation Institute “Illustrated Glossary - Technician Training for the Maintenance of In Situ Mosaics”, Los Angeles, 2013</skos:editorialNote>
    <rdf:type rdf:resource="http://www.w3.org/2002/07/owl#NamedIndividual"/>
    <skos:prefLabel xml:lang="it">Opus signinum</skos:prefLabel>
    <skos:prefLabel xml:lang="en">Opus signinum</skos:prefLabel>
    <skos:editorialNote xml:lang="it">C. Fiori “Teoria e tecniche per la conservazione del mosaico”, Il Prato, Padova, 2002</skos:editorialNote>
    <skos:broader rdf:resource="https://w3id.org/crmrp#c_b9a6a1c8"/>
    <skos:topConceptOf rdf:resource="https://w3id.org/crmrp#Execution_Technique"/>
    <rdf:type rdf:resource="http://www.w3.org/2004/02/skos/core#Concept"/>
    <skos:inScheme rdf:resource="https://w3id.org/crmrp#Execution_Technique"/>
    <rdfs:label xml:lang="en">Opus signinum</rdfs:label>
  </rdf:Description>
  <rdf:Description rdf:about="http://www.cidoc-crm.org/cidoc-crm/P108i_was_produced_by">
    <rdfs:range rdf:resource="http://www.cidoc-crm.org/cidoc-crm/E73_Exectution_Technique"/>
    <rdfs:domain rdf:resource="https://w3id.org/crmrp#R1_Restoration_Object"/>
  </rdf:Description>
  <rdf:Description rdf:about="https://w3id.org/crmrp#c_584a7943">
    <skos:topConceptOf rdf:resource="https://w3id.org/crmrp#Archeometric_and_Diagnostic_Analysis"/>
    <skos:editorialNote xml:lang="en">Getty AAT http://vocab.getty.edu/page/aat/300024594</skos:editorialNote>
    <skos:inScheme rdf:resource="https://w3id.org/crmrp#Archeometric_and_Diagnostic_Analysis"/>
    <skos:closeMatch rdf:resource="http://vocab.getty.edu/page/aat/300024594"/>
    <rdfs:label xml:lang="en">Microscopes</rdfs:label>
    <skos:prefLabel xml:lang="en">Microscopes</skos:prefLabel>
    <skos:broader rdf:resource="https://w3id.org/crmrp#c_1fd6102e"/>
    <rdf:type rdf:resource="http://www.w3.org/2004/02/skos/core#Concept"/>
    <rdf:type rdf:resource="http://www.w3.org/2002/07/owl#NamedIndividual"/>
    <skos:definition xml:lang="en">Optical instruments consisting of a lens or combination of lenses that allow the viewing of objects that are too small to be seen with the naked, unaided eye. The term may also be used for various types of instruments that use a stream of electrons (electron microscope), electromagnetic radiation (x-ray microscope), or other means other than light and lenses to magnify images of small objects.</skos:definition>
    <skos:prefLabel xml:lang="it">Microscopia</skos:prefLabel>
  </rdf:Description>
  <rdf:Description rdf:about="https://w3id.org/crmrp#c_dd7e90e1">
    <rdf:type rdf:resource="http://www.w3.org/2002/07/owl#NamedIndividual"/>
    <skos:editorialNote xml:lang="it">G. Pignolo, “Effetti d’oro - Storia e tecnica della doratura nell’arte”, Editrice Compositori, Bologna, 2002</skos:editorialNote>
    <skos:broader rdf:resource="https://w3id.org/crmrp#c_4d471b17"/>
    <rdf:type rdf:resource="http://www.w3.org/2004/02/skos/core#Concept"/>
    <rdfs:label xml:lang="en">Haze</rdfs:label>
    <skos:prefLabel xml:lang="it">Velatura</skos:prefLabel>
    <skos:inScheme rdf:resource="https://w3id.org/crmrp#Execution_Technique"/>
    <skos:note xml:lang="en">International references could not be found</skos:note>
    <skos:definition xml:lang="en">Gold foil residues are removed with brushes or cotton to make the glaze opaque</skos:definition>
    <skos:topConceptOf rdf:resource="https://w3id.org/crmrp#Execution_Technique"/>
    <skos:prefLabel xml:lang="en">Haze</skos:prefLabel>
  </rdf:Description>
  <rdf:Description rdf:about="https://w3id.org/crmrp#c_a90ef012">
    <skos:exactMatch rdf:resource="http://vocab.getty.edu/page/aat/300263579"/>
    <skos:prefLabel xml:lang="it">A conchiglia</skos:prefLabel>
    <skos:editorialNote xml:lang="en">Getty AAT http://vocab.getty.edu/page/aat/300263579</skos:editorialNote>
    <rdf:type rdf:resource="http://www.w3.org/2004/02/skos/core#Concept"/>
    <skos:broader rdf:resource="https://w3id.org/crmrp#c_8af455cd"/>
    <rdfs:label xml:lang="en">Shell gold</rdfs:label>
    <skos:prefLabel xml:lang="en">Shell gold</skos:prefLabel>
    <skos:definition xml:lang="en">Gold leaf ground into a powder and mixed with honey or other binder, used to produce powdered effects on leather bindings, to repair or restore gold tooling, and to gild manuscripts. Originally packaged in mussel shells, more recently it is sold in plastic containers shaped like mussel shells or in tablet or small block form.</skos:definition>
    <skos:inScheme rdf:resource="https://w3id.org/crmrp#Execution_Technique"/>
    <rdf:type rdf:resource="http://www.w3.org/2002/07/owl#NamedIndividual"/>
    <skos:topConceptOf rdf:resource="https://w3id.org/crmrp#Execution_Technique"/>
  </rdf:Description>
  <rdf:Description rdf:about="https://w3id.org/crmrp#R7_Restoration_Project">
    <rdfs:label xml:lang="en">Restoration Project</rdfs:label>
    <rdfs:comment xml:lang="en">This class is about the overall view of a restoration project.
It refers to the entire restoration process, including the various operations that have taken place in an artwork. The purpose of this class is not only to group a series of operations, but also to be able to indicate the time frame required to complete each operation and the entire restoration site.</rdfs:comment>
    <rdfs:subClassOf rdf:resource="http://www.cidoc-crm.org/cidoc-crm/E5_Event"/>
    <rdf:type rdf:resource="http://www.w3.org/2002/07/owl#Class"/>
  </rdf:Description>
  <rdf:Description rdf:about="https://w3id.org/crmrp#c_b86776d0">
    <skos:prefLabel xml:lang="it">Consolidamento</skos:prefLabel>
    <skos:topConceptOf rdf:resource="https://w3id.org/crmrp#Intervention"/>
    <skos:editorialNote xml:lang="en">Getty Conservation Institute “Illustrated Glossary - Definitions of terms used for the graphic documentation of in situ floor mosaics”, “Mosaics In Situ Project”, Los Angeles, 2003</skos:editorialNote>
    <skos:editorialNote xml:lang="it">Uni En 15898:2019 Conservazione del patrimonio culturale - Termini generali e definizioni</skos:editorialNote>
    <skos:prefLabel xml:lang="en">Consolidation</skos:prefLabel>
    <skos:editorialNote xml:lang="en">Getty AAT http://vocab.getty.edu/page/aat/300219960</skos:editorialNote>
    <rdf:type rdf:resource="http://www.w3.org/2004/02/skos/core#Concept"/>
    <rdfs:label xml:lang="en">Consolidation</rdfs:label>
    <skos:inScheme rdf:resource="https://w3id.org/crmrp#Intervention"/>
    <skos:editorialNote xml:lang="en">A. Weyer et al., “EwaGlos - European Illustrated Glossary of conservation terms for wall paintings and architectural surfaces”, Michael Imhof Verlag, Petersberg, Germany</skos:editorialNote>
    <rdf:type rdf:resource="http://www.w3.org/2002/07/owl#NamedIndividual"/>
    <skos:note xml:lang="en">The preferred editorial note and the definition closest to the meaning is Uni En 15898:2019</skos:note>
    <skos:closeMatch rdf:resource="http://vocab.getty.edu/page/aat/300219960"/>
    <skos:definition xml:lang="en">Improvement of internal cohesion or mechanical stability, usually by adding material</skos:definition>
  </rdf:Description>
  <rdf:Description rdf:about="http://www.cidoc-crm.org/extensions/crmsci/O16_observed_value">
    <rdfs:domain rdf:resource="https://w3id.org/crmrp#R12_Invasive_archaeometric_and_diagnostic_analysis"/>
    <rdfs:domain rdf:resource="https://w3id.org/crmrp#R11_Non-invasive_archaeometric_and_diagnostic_analysis"/>
    <rdfs:range rdf:resource="http://www.cidoc-crm.org/cidoc-crm/E73_Information_Object"/>
    <rdfs:range rdf:resource="http://www.cidoc-crm.org/cidoc-crm/E54_Dimension"/>
  </rdf:Description>
  <rdf:Description rdf:about="https://w3id.org/crmrp#c_5b39b8a8">
    <rdf:type rdf:resource="http://www.w3.org/2002/07/owl#NamedIndividual"/>
    <skos:prefLabel xml:lang="it">Meccatura</skos:prefLabel>
    <skos:editorialNote xml:lang="it">C. Giannini, “Dizionario del restauro - Tecniche diagnostica conservazione”, Nardini Editore, Firenze, 2010</skos:editorialNote>
    <skos:prefLabel xml:lang="en">Mecca gilding</skos:prefLabel>
    <skos:inScheme rdf:resource="https://w3id.org/crmrp#Execution_Technique"/>
    <skos:definition xml:lang="en">Technique of applying paint known as mecha on tin or silver surfaces to achieve an optical effect similar to gilding</skos:definition>
    <skos:broader rdf:resource="https://w3id.org/crmrp#c_757ed6ec"/>
    <skos:topConceptOf rdf:resource="https://w3id.org/crmrp#Execution_Technique"/>
    <rdf:type rdf:resource="http://www.w3.org/2004/02/skos/core#Concept"/>
    <skos:note xml:lang="en">International references could not be found</skos:note>
    <rdfs:label xml:lang="en">Mecca gilding</rdfs:label>
  </rdf:Description>
  <rdf:Description rdf:about="https://w3id.org/crmrp#c_7621b79d">
    <skos:prefLabel xml:lang="en">Painting</skos:prefLabel>
    <rdf:type rdf:resource="http://www.w3.org/2002/07/owl#NamedIndividual"/>
    <rdfs:label xml:lang="en">Paintings</rdfs:label>
    <skos:exactMatch rdf:resource="http://vocab.getty.edu/page/aat/300033618"/>
    <rdf:type rdf:resource="http://www.w3.org/2004/02/skos/core#Concept"/>
    <skos:definition xml:lang="en">Unique works in which images are formed primarily by the direct application of pigments suspended in oil, water, egg yolk, molten wax, or other liquid, arranged in masses of color, onto a generally two-dimensional surface.</skos:definition>
    <skos:prefLabel xml:lang="it">Dipinto</skos:prefLabel>
    <skos:inScheme rdf:resource="https://w3id.org/crmrp#Restoration_Object"/>
    <skos:editorialNote xml:lang="en">Getty AAT http://vocab.getty.edu/page/aat/300033618</skos:editorialNote>
    <skos:topConceptOf rdf:resource="https://w3id.org/crmrp#Restoration_Object"/>
  </rdf:Description>
  <rdf:Description rdf:about="https://w3id.org/crmrp#c_3fa9cd31">
    <skos:prefLabel xml:lang="en">Polymer paint</skos:prefLabel>
    <skos:exactMatch rdf:resource="http://vocab.getty.edu/page/aat/300147678"/>
    <skos:inScheme rdf:resource="https://w3id.org/crmrp#Execution_Technique"/>
    <skos:editorialNote xml:lang="en">Getty AAT http://vocab.getty.edu/page/aat/300015055</skos:editorialNote>
    <skos:prefLabel xml:lang="it">Polimero sintetico</skos:prefLabel>
    <skos:definition xml:lang="en">Paint with a base that is polymer, which is compound formed by the combination of two or more molecules of the same substance to produce a new compound with the same empirical formula but with higher molecular weight. It is typically made from pigments in an acrylic resin or vinyl resin, which are polymers, or a combination of both resins. It is water based, spreads out in a layer, and forms a continuous, flexible, and waterproof film of plastic when the water evaporates.</skos:definition>
    <rdfs:label xml:lang="en">Polymer paint</rdfs:label>
    <rdf:type rdf:resource="http://www.w3.org/2002/07/owl#NamedIndividual"/>
    <rdf:type rdf:resource="http://www.w3.org/2004/02/skos/core#Concept"/>
    <skos:topConceptOf rdf:resource="https://w3id.org/crmrp#Execution_Technique"/>
    <skos:broader rdf:resource="https://w3id.org/crmrp#c_143349b9"/>
  </rdf:Description>
  <rdf:Description rdf:about="https://w3id.org/crmrp#c_6671d452">
    <skos:prefLabel xml:lang="en">Silver</skos:prefLabel>
    <rdf:type rdf:resource="http://www.w3.org/2002/07/owl#NamedIndividual"/>
    <skos:broader rdf:resource="https://w3id.org/crmrp#c_6407466f"/>
    <skos:prefLabel xml:lang="it">Argento</skos:prefLabel>
    <skos:inScheme rdf:resource="https://w3id.org/crmrp#Material"/>
    <skos:definition xml:lang="en">Pure metallic element having symbol Ag and atomic number 47; a malleable, ductile, white metal with characteristic sheen, considered a precious metal. Silver is widely distributed throughout the world, occurring rarely as metallic silver (in Peru, Norway) but more often as silver-gold alloys and silver ore. Today silver is obtained as a byproduct in the refinement of gold, lead, copper, or zinc ores. Silver was smelted from the ore galena as early as 3800 BCE. As a pure metal, silver is second to gold in malleability and ductility, can be polished to a highly reflective surface, and used -- typically in an alloy -- in jewelry, coinage, photography, mirrors, electrical contacts, and tableware.</skos:definition>
    <skos:topConceptOf rdf:resource="https://w3id.org/crmrp#Material"/>
    <rdf:type rdf:resource="http://www.w3.org/2004/02/skos/core#Concept"/>
    <skos:exactMatch rdf:resource="http://vocab.getty.edu/page/aat/30001102"/>
    <rdfs:label xml:lang="en">Silver</rdfs:label>
    <skos:editorialNote xml:lang="en">Getty AAT http://vocab.getty.edu/page/aat/300011029</skos:editorialNote>
  </rdf:Description>
  <rdf:Description rdf:about="https://w3id.org/crmrp#c_602a357d">
    <skos:prefLabel xml:lang="en">Visible diffuse light</skos:prefLabel>
    <skos:inScheme rdf:resource="https://w3id.org/crmrp#Archeometric_and_Diagnostic_Analysis"/>
    <skos:topConceptOf rdf:resource="https://w3id.org/crmrp#Archeometric_and_Diagnostic_Analysis"/>
    <skos:definition xml:lang="en">Photographs obtained by recreating, even artificially, lighting conditions that make the composition and its colour values most readable.</skos:definition>
    <skos:prefLabel xml:lang="it">Fotografia a luce diffusa</skos:prefLabel>
    <skos:editorialNote xml:lang="it">V. Marcovaz, “Indagine e diagnostica fotografica per i beni culturali”, Isiaurbino, Trieste, 2016</skos:editorialNote>
    <rdf:type rdf:resource="http://www.w3.org/2004/02/skos/core#Concept"/>
    <skos:editorialNote xml:lang="it">A. Aldrovandi, M. Picollo “Metodi di documentazione indagini non invasive sui dipinti”, Il Prato, Padova, 1999</skos:editorialNote>
    <rdfs:label xml:lang="en">Visible diffuse light</rdfs:label>
    <rdf:type rdf:resource="http://www.w3.org/2002/07/owl#NamedIndividual"/>
    <skos:broader rdf:resource="https://w3id.org/crmrp#c_1fd6102e"/>
  </rdf:Description>
  <rdf:Description rdf:about="https://w3id.org/crmrp#Execution_Technique">
    <skos:prefLabel xml:lang="it">Tecnica esecutiva</skos:prefLabel>
    <skos:prefLabel xml:lang="en">Execution Technique</skos:prefLabel>
    <rdf:type rdf:resource="http://www.w3.org/2004/02/skos/core#ConceptScheme"/>
    <rdf:type rdf:resource="http://www.w3.org/2002/07/owl#NamedIndividual"/>
  </rdf:Description>
  <rdf:Description rdf:about="https://w3id.org/crmrp#c_6a6dc187">
    <skos:definition xml:lang="en">Type of sectional mosaic in which elements are cut with great precision and juxtaposed with each other so that the com almost invisible. The stones are chosen in so as to exploit the material's own colour material to achieve effects of chiaroscuro, shadows and shading.</skos:definition>
    <skos:prefLabel xml:lang="en">Intarsia</skos:prefLabel>
    <skos:broader rdf:resource="https://w3id.org/crmrp#c_b9a6a1c8"/>
    <skos:editorialNote xml:lang="it">C. Fiori “Teoria e tecniche per la conservazione del mosaico”, Il Prato, Padova, 2002</skos:editorialNote>
    <skos:editorialNote xml:lang="en">The Getty Conservation Institute, “The structural conservation of panel paintings”, Proceedings of a Symposium at the J. Paul Getty Museum, 24 - 28 April 1995</skos:editorialNote>
    <skos:prefLabel xml:lang="it">Commesso/Intarsio</skos:prefLabel>
    <rdf:type rdf:resource="http://www.w3.org/2004/02/skos/core#Concept"/>
    <skos:inScheme rdf:resource="https://w3id.org/crmrp#Execution_Technique"/>
    <rdf:type rdf:resource="http://www.w3.org/2002/07/owl#NamedIndividual"/>
    <rdfs:label xml:lang="en">Intarsia</rdfs:label>
    <skos:editorialNote xml:lang="it">C. Giannini, “Dizionario del restauro - Tecniche diagnostica conservazione”, Nardini Editore, Firenze, 2010</skos:editorialNote>
    <skos:topConceptOf rdf:resource="https://w3id.org/crmrp#Execution_Technique"/>
  </rdf:Description>
  <rdf:Description rdf:about="https://w3id.org/crmrp#c_fd0e78d4">
    <skos:broader rdf:resource="https://w3id.org/crmrp#c_34d8fe56"/>
    <skos:closeMatch rdf:resource="http://vocab.getty.edu/page/aat/300011176"/>
    <skos:prefLabel xml:lang="en">Rock</skos:prefLabel>
    <rdf:type rdf:resource="http://www.w3.org/2004/02/skos/core#Concept"/>
    <rdfs:label xml:lang="en">Rock</rdfs:label>
    <skos:prefLabel xml:lang="it">Pietra</skos:prefLabel>
    <skos:topConceptOf rdf:resource="https://w3id.org/crmrp#Material"/>
    <skos:inScheme rdf:resource="https://w3id.org/crmrp#Material"/>
    <skos:editorialNote xml:lang="en">Getty AAT http://vocab.getty.edu/page/aat/300011176</skos:editorialNote>
    <skos:definition xml:lang="en">Naturally formed aggregate of one or more minerals. For processed or dressed rock use stone.</skos:definition>
    <rdf:type rdf:resource="http://www.w3.org/2002/07/owl#NamedIndividual"/>
  </rdf:Description>
  <rdf:Description rdf:about="https://w3id.org/crmrp#c_160c713a">
    <skos:prefLabel xml:lang="en">Sculpture</skos:prefLabel>
    <rdf:type rdf:resource="http://www.w3.org/2004/02/skos/core#Concept"/>
    <rdf:type rdf:resource="http://www.w3.org/2002/07/owl#NamedIndividual"/>
    <skos:topConceptOf rdf:resource="https://w3id.org/crmrp#Restoration_Object"/>
    <skos:exactMatch rdf:resource="http://vocab.getty.edu/page/aat/300047090"/>
    <skos:editorialNote xml:lang="en">Getty AAT http://vocab.getty.edu/page/aat/300047090</skos:editorialNote>
    <skos:inScheme rdf:resource="https://w3id.org/crmrp#Restoration_Object"/>
    <skos:prefLabel xml:lang="it">Scultura</skos:prefLabel>
    <skos:definition xml:lang="en">Three-dimensional works of art in which images and forms are produced in relief, in intaglio, or in the round. The term refers particularly to art works created by carving or engraving a hard material, by molding or casting a malleable material (which usually then hardens), or by assembling parts to create a three-dimensional object. It is typically used to refer to large or medium-sized objects made of stone, wood, bronze, or another metal.</skos:definition>
    <rdfs:label xml:lang="en">Sculpture</rdfs:label>
  </rdf:Description>
  <rdf:Description rdf:about="https://w3id.org/crmrp#c_9ff50f5a">
    <skos:note xml:lang="en">The preferred editorial note and the definition closest to the meaning is Uni Cen/Ts 17135:2021</skos:note>
    <rdfs:label xml:lang="en">Concretion</rdfs:label>
    <skos:definition xml:lang="en">Hard adherent accumulation and coalescence of a deposit</skos:definition>
    <skos:topConceptOf rdf:resource="https://w3id.org/crmrp#Alteration"/>
    <skos:prefLabel xml:lang="it">Concrezione</skos:prefLabel>
    <skos:editorialNote xml:lang="en">Getty AAT http://vocab.getty.edu/page/aat/300379825</skos:editorialNote>
    <skos:editorialNote xml:lang="en">Uni Cen/Ts 17135:2021 - Conservation of cultural heritage. General terms and definitions</skos:editorialNote>
    <skos:inScheme rdf:resource="https://w3id.org/crmrp#Alteration"/>
    <rdf:type rdf:resource="http://www.w3.org/2004/02/skos/core#Concept"/>
    <rdf:type rdf:resource="http://www.w3.org/2002/07/owl#NamedIndividual"/>
    <skos:editorialNote xml:lang="en">Verg`es-Belmin et al., ICOMOS-ISCS: Illustrated glossary on stone deterioration patterns, vol. XV. Icomos International Council on Monuments and Sites, 2008</skos:editorialNote>
    <skos:prefLabel xml:lang="en">Concretion</skos:prefLabel>
    <skos:closeMatch rdf:resource="http://vocab.getty.edu/page/aat/300379825"/>
  </rdf:Description>
  <rdf:Description rdf:about="https://w3id.org/crmrp#c_18e54874">
    <skos:note xml:lang="en">International references could not be found</skos:note>
    <rdfs:label xml:lang="en">Mechanical cleaning</rdfs:label>
    <skos:topConceptOf rdf:resource="https://w3id.org/crmrp#Intervention"/>
    <skos:prefLabel xml:lang="it">Pulitura meccanica</skos:prefLabel>
    <skos:editorialNote xml:lang="en">G. Botticelli, “Lezioni di restauro - Le pitture murali”, Centro Di Editore, Firenze, 2012</skos:editorialNote>
    <rdf:type rdf:resource="http://www.w3.org/2002/07/owl#NamedIndividual"/>
    <skos:inScheme rdf:resource="https://w3id.org/crmrp#Intervention"/>
    <skos:prefLabel xml:lang="en">Mechanical cleaning</skos:prefLabel>
    <rdf:type rdf:resource="http://www.w3.org/2004/02/skos/core#Concept"/>
    <skos:broader rdf:resource="https://w3id.org/crmrp#c_830e6744"/>
    <skos:definition xml:lang="en">Removal of all surface impurities (dust, insect droppings, micro-organism spores, etc.) using brushes, scalpels. laser and/or soft rubbers, often without the use of water or other solvents. This term comprises the dry cleaning techniques.</skos:definition>
  </rdf:Description>
  <rdf:Description rdf:about="https://w3id.org/crmrp#c_ada0bb45">
    <skos:prefLabel xml:lang="it">Ritorsione</skos:prefLabel>
    <skos:prefLabel xml:lang="en">Twisted</skos:prefLabel>
    <rdf:type rdf:resource="http://www.w3.org/2004/02/skos/core#Concept"/>
    <rdfs:label xml:lang="en">Twisted</rdfs:label>
    <skos:broader rdf:resource="https://w3id.org/crmrp#c_13f3ce9e"/>
    <skos:editorialNote xml:lang="en">Uni Cen/Ts 17135:2021 - Conservation of cultural heritage. General terms and definitions</skos:editorialNote>
    <skos:inScheme rdf:resource="https://w3id.org/crmrp#Alteration"/>
    <rdf:type rdf:resource="http://www.w3.org/2002/07/owl#NamedIndividual"/>
    <skos:topConceptOf rdf:resource="https://w3id.org/crmrp#Alteration"/>
    <skos:definition xml:lang="en">Exhibiting deformation around a single axis.</skos:definition>
  </rdf:Description>
  <rdf:Description rdf:about="https://w3id.org/crmrp#c_cc85125b">
    <skos:editorialNote xml:lang="en">Getty AAT http://vocab.getty.edu/page/aat/300053281</skos:editorialNote>
    <skos:inScheme rdf:resource="https://w3id.org/crmrp#Execution_Technique"/>
    <skos:definition xml:lang="en">Stencil technique of printing in which ink or dye is forced through a mesh, traditionally silk, on which a design has been formed by stopping out certain areas.</skos:definition>
    <skos:closeMatch rdf:resource="http://vocab.getty.edu/page/aat/300053281"/>
    <skos:prefLabel xml:lang="en">Screen printing</skos:prefLabel>
    <skos:topConceptOf rdf:resource="https://w3id.org/crmrp#Execution_Technique"/>
    <rdf:type rdf:resource="http://www.w3.org/2004/02/skos/core#Concept"/>
    <rdfs:label xml:lang="en">Screen printing</rdfs:label>
    <skos:prefLabel xml:lang="it">Serigrafia</skos:prefLabel>
    <skos:broader rdf:resource="https://w3id.org/crmrp#c_aee6a805"/>
    <rdf:type rdf:resource="http://www.w3.org/2002/07/owl#NamedIndividual"/>
  </rdf:Description>
  <rdf:Description rdf:about="https://w3id.org/crmrp#c_33147d64">
    <rdf:type rdf:resource="http://www.w3.org/2002/07/owl#NamedIndividual"/>
    <skos:prefLabel xml:lang="en">Miniature</skos:prefLabel>
    <skos:altLabel xml:lang="en">Illuminations</skos:altLabel>
    <skos:broader rdf:resource="https://w3id.org/crmrp#c_044b6056"/>
    <skos:editorialNote xml:lang="en">Getty AAT http://vocab.getty.edu/page/aat/300033936</skos:editorialNote>
    <skos:inScheme rdf:resource="https://w3id.org/crmrp#Execution_Technique"/>
    <rdfs:label xml:lang="en">Miniature</rdfs:label>
    <skos:definition xml:lang="en">Paintings on a very small scale. The term is often applied specifically to small scenes in illuminated manuscripts or to portraits on vellum or ivory that were popular in Europe and America from the Renaissance into the 19th century. For paintings in manuscripts, the term illuminations may also be appropriate.</skos:definition>
    <skos:topConceptOf rdf:resource="https://w3id.org/crmrp#Execution_Technique"/>
    <skos:closeMatch rdf:resource="http://vocab.getty.edu/page/aat/300033936"/>
    <rdf:type rdf:resource="http://www.w3.org/2004/02/skos/core#Concept"/>
    <skos:prefLabel xml:lang="it">Miniatura</skos:prefLabel>
  </rdf:Description>
  <rdf:Description rdf:about="https://w3id.org/crmrp#c_78efb0c7">
    <skos:topConceptOf rdf:resource="https://w3id.org/crmrp#Execution_Technique"/>
    <skos:prefLabel xml:lang="en">Fresco</skos:prefLabel>
    <skos:note xml:lang="en">The preferred editorial note and the definition closest to the meaning is EwaGlos - European Illustrated Glossary of conservation terms for wall paintings and architectural surfaces</skos:note>
    <skos:editorialNote xml:lang="en">A. Weyer et al., “EwaGlos - European Illustrated Glossary of conservation terms for wall paintings and architectural surfaces”, Michael Imhof Verlag, Petersberg, Germany</skos:editorialNote>
    <skos:prefLabel xml:lang="it">Affresco</skos:prefLabel>
    <skos:broader rdf:resource="https://w3id.org/crmrp#c_6626f18c"/>
    <rdfs:label xml:lang="en">Fresco</rdfs:label>
    <skos:editorialNote xml:lang="en">Getty AAT http://vocab.getty.edu/page/aat/300177433</skos:editorialNote>
    <rdf:type rdf:resource="http://www.w3.org/2004/02/skos/core#Concept"/>
    <skos:definition xml:lang="en">A wall painting technique in which pigments are mixed with clear water and applied to a fresh and still damp lime plaster (intonaco); pigments are fixed inside a thin layer of calcium carbonate formed on the plaster surface (carbonation).</skos:definition>
    <rdf:type rdf:resource="http://www.w3.org/2002/07/owl#NamedIndividual"/>
    <skos:exactMatch rdf:resource="http://vocab.getty.edu/page/aat/300177433"/>
    <skos:inScheme rdf:resource="https://w3id.org/crmrp#Execution_Technique"/>
  </rdf:Description>
  <rdf:Description rdf:about="https://w3id.org/crmrp#RP5_is_post-restoration">
    <rdfs:label xml:lang="en">is post-restoration</rdfs:label>
    <rdfs:comment xml:lang="en">This property links Invasive archaeometric and diagnostic analysis and Non-invasive achaeometric and diagnostic analysis to Restoration Project.
Indeed, some archaeometric and diagnostic analyses are sometimes repeated before and after the restoration.</rdfs:comment>
    <rdfs:range rdf:resource="https://w3id.org/crmrp#R7_Restoration_Project"/>
    <rdfs:domain rdf:resource="https://w3id.org/crmrp#R12_Invasive_archaeometric_and_diagnostic_analysis"/>
    <rdfs:domain rdf:resource="https://w3id.org/crmrp#R11_Non-invasive_archaeometric_and_diagnostic_analysis"/>
    <rdf:type rdf:resource="http://www.w3.org/2002/07/owl#ObjectProperty"/>
  </rdf:Description>
  <rdf:Description rdf:about="https://w3id.org/crmrp#c_3639e649">
    <skos:topConceptOf rdf:resource="https://w3id.org/crmrp#Alteration"/>
    <skos:note xml:lang="en">The preferred editorial note and the closest definition  to the meaning is Uni Cen/Ts 17135:2021</skos:note>
    <skos:altLabel xml:lang="en">Cut</skos:altLabel>
    <skos:inScheme rdf:resource="https://w3id.org/crmrp#Alteration"/>
    <skos:prefLabel xml:lang="it">Graffio</skos:prefLabel>
    <skos:definition xml:lang="en">Line of loss or displacement of material caused by sharp edge.</skos:definition>
    <rdfs:label xml:lang="en">Scratch</rdfs:label>
    <skos:prefLabel xml:lang="en">Scratch</skos:prefLabel>
    <rdf:type rdf:resource="http://www.w3.org/2004/02/skos/core#Concept"/>
    <skos:editorialNote xml:lang="en">Verg`es-Belmin et al., ICOMOS-ISCS: Illustrated glossary on stone deterioration patterns, vol. XV. Icomos International Council on Monuments and Sites, 2008</skos:editorialNote>
    <rdf:type rdf:resource="http://www.w3.org/2002/07/owl#NamedIndividual"/>
    <skos:editorialNote xml:lang="en">Uni Cen/Ts 17135:2021 - Conservation of cultural heritage. General terms and definitions</skos:editorialNote>
  </rdf:Description>
  <rdf:Description rdf:about="https://w3id.org/crmrp#c_d54b0be2">
    <skos:prefLabel xml:lang="en">Detachment</skos:prefLabel>
    <skos:definition xml:lang="en">Break in continuity between layers of a plaster, both between them and in relation to the substrate, which generally preludes the fall of the layers themselves.</skos:definition>
    <skos:inScheme rdf:resource="https://w3id.org/crmrp#Alteration"/>
    <rdf:type rdf:resource="http://www.w3.org/2002/07/owl#NamedIndividual"/>
    <rdf:type rdf:resource="http://www.w3.org/2004/02/skos/core#Concept"/>
    <skos:prefLabel xml:lang="it">Distacco</skos:prefLabel>
    <skos:editorialNote xml:lang="en">Verg`es-Belmin et al., ICOMOS-ISCS: Illustrated glossary on stone deterioration patterns, vol. XV. Icomos International Council on Monuments and Sites, 2008</skos:editorialNote>
    <skos:topConceptOf rdf:resource="https://w3id.org/crmrp#Alteration"/>
    <skos:editorialNote xml:lang="it">Uni 11182:2006 - Materiali lapidei naturali ed artificiali. Descrizione della forma di alterazione - Termini e definizioni</skos:editorialNote>
    <rdfs:label xml:lang="en">Detachment</rdfs:label>
  </rdf:Description>
  <rdf:Description rdf:about="https://w3id.org/crmrp#c_8590c59f">
    <skos:inScheme rdf:resource="https://w3id.org/crmrp#Execution_Technique"/>
    <rdf:type rdf:resource="http://www.w3.org/2002/07/owl#NamedIndividual"/>
    <skos:prefLabel xml:lang="it">Olio</skos:prefLabel>
    <rdf:type rdf:resource="http://www.w3.org/2004/02/skos/core#Concept"/>
    <skos:prefLabel xml:lang="en">Drying oil</skos:prefLabel>
    <rdfs:label xml:lang="en">Drying oil</rdfs:label>
    <skos:definition xml:lang="en">Vegetable oils which form a solid, elastic film after a period of exposure to the air.</skos:definition>
    <skos:broader rdf:resource="https://w3id.org/crmrp#c_044b6056"/>
    <skos:topConceptOf rdf:resource="https://w3id.org/crmrp#Execution_Technique"/>
    <skos:editorialNote xml:lang="en">A. Weyer et al., “EwaGlos - European Illustrated Glossary of conservation terms for wall paintings and architectural surfaces”, Michael Imhof Verlag, Petersberg, Germany</skos:editorialNote>
  </rdf:Description>
  <rdf:Description rdf:about="https://w3id.org/crmrp#c_c006ffaa">
    <skos:prefLabel xml:lang="it">Riproduzione fotografica da fonte archivistica</skos:prefLabel>
    <rdfs:label xml:lang="en">Photographic reproduction from archival sources</rdfs:label>
    <rdf:type rdf:resource="http://www.w3.org/2004/02/skos/core#Concept"/>
    <skos:topConceptOf rdf:resource="https://w3id.org/crmrp#Documentation"/>
    <skos:inScheme rdf:resource="https://w3id.org/crmrp#Documentation"/>
    <skos:prefLabel xml:lang="en">Photographic reproduction from archival sources</skos:prefLabel>
    <skos:note xml:lang="en">International references could not be found</skos:note>
    <skos:definition xml:lang="en">Photographic document showing how the artwork looked in the past</skos:definition>
    <skos:broader rdf:resource="https://w3id.org/crmrp#c_773e0829"/>
    <rdf:type rdf:resource="http://www.w3.org/2002/07/owl#NamedIndividual"/>
  </rdf:Description>
  <rdf:Description rdf:about="https://w3id.org/crmrp#c_21ebd5c7">
    <skos:inScheme rdf:resource="https://w3id.org/crmrp#Intervention"/>
    <skos:prefLabel xml:lang="it">Solvente</skos:prefLabel>
    <rdfs:label xml:lang="en">Solvent</rdfs:label>
    <skos:definition xml:lang="en">Any material, usually liquid, having the power of dissolving another material.</skos:definition>
    <skos:topConceptOf rdf:resource="https://w3id.org/crmrp#Intervention"/>
    <skos:prefLabel xml:lang="en">Solvent</skos:prefLabel>
    <skos:broader rdf:resource="https://w3id.org/crmrp#c_5a83cd16"/>
    <skos:editorialNote xml:lang="en">Getty AAT http://vocab.getty.edu/page/aat/300015217</skos:editorialNote>
    <rdf:type rdf:resource="http://www.w3.org/2004/02/skos/core#Concept"/>
    <rdf:type rdf:resource="http://www.w3.org/2002/07/owl#NamedIndividual"/>
    <skos:exactMatch rdf:resource="http://vocab.getty.edu/page/aat/300015217"/>
  </rdf:Description>
  <rdf:Description rdf:about="https://w3id.org/crmrp#c_2a4faa96">
    <skos:inScheme rdf:resource="https://w3id.org/crmrp#Execution_Technique"/>
    <skos:prefLabel xml:lang="it">Opus scutulatum</skos:prefLabel>
    <skos:prefLabel xml:lang="en">Opus scutulatum</skos:prefLabel>
    <skos:topConceptOf rdf:resource="https://w3id.org/crmrp#Execution_Technique"/>
    <skos:broader rdf:resource="https://w3id.org/crmrp#c_b9a6a1c8"/>
    <rdf:type rdf:resource="http://www.w3.org/2002/07/owl#NamedIndividual"/>
    <skos:definition xml:lang="en">Pavement combining an opus tessellatum background, frequently monochrome, and small stone slabs, often in fragments, generally aligned in rows. The slabs are of different forms, colors, and dimensions.</skos:definition>
    <rdfs:label xml:lang="en">Opus scutulatum</rdfs:label>
    <skos:editorialNote xml:lang="en">Getty Conservation Institute “Illustrated Glossary - Technician Training for the Maintenance of In Situ Mosaics”, Los Angeles, 2013</skos:editorialNote>
    <skos:editorialNote xml:lang="it">C. Fiori “Teoria e tecniche per la conservazione del mosaico”, Il Prato, Padova, 2002</skos:editorialNote>
    <rdf:type rdf:resource="http://www.w3.org/2004/02/skos/core#Concept"/>
  </rdf:Description>
  <rdf:Description rdf:about="https://w3id.org/crmrp#c_54648e63">
    <rdf:type rdf:resource="http://www.w3.org/2004/02/skos/core#Concept"/>
    <rdf:type rdf:resource="http://www.w3.org/2002/07/owl#NamedIndividual"/>
    <skos:broader rdf:resource="https://w3id.org/crmrp#c_1fd6102e"/>
    <skos:prefLabel xml:lang="it">Analisi colorimetrica</skos:prefLabel>
    <skos:prefLabel xml:lang="en">Colorimetry</skos:prefLabel>
    <skos:inScheme rdf:resource="https://w3id.org/crmrp#Archeometric_and_Diagnostic_Analysis"/>
    <skos:defintion xml:lang="en">The process of determining and specifying colors.</skos:defintion>
    <skos:editorialNote xml:lang="en">Getty AAT http://vocab.getty.edu/page/aat/300053579</skos:editorialNote>
    <skos:closeMatch rdf:resource="http://vocab.getty.edu/page/aat/300053579"/>
    <skos:topConceptOf rdf:resource="https://w3id.org/crmrp#Archeometric_and_Diagnostic_Analysis"/>
    <rdfs:label xml:lang="en">Colorimetry</rdfs:label>
  </rdf:Description>
  <rdf:Description rdf:about="https://w3id.org/crmrp#c_3de3f55a">
    <skos:definition xml:lang="en">Metallisation is a fundamental process in surface finishing, especially of steel and iron. This metal coating protects the underlying material from oxidation and corrosion, extending durability and strength over time.</skos:definition>
    <skos:prefLabel xml:lang="en">Metallisation</skos:prefLabel>
    <rdfs:label xml:lang="en">Metallisation</rdfs:label>
    <rdf:type rdf:resource="http://www.w3.org/2002/07/owl#NamedIndividual"/>
    <skos:note xml:lang="en">International references could not be found</skos:note>
    <skos:inScheme rdf:resource="https://w3id.org/crmrp#Execution_Technique"/>
    <skos:editorialNote xml:lang="it">T. Turco, “Il doratore”, Hoepli, Milano, 2017</skos:editorialNote>
    <skos:broader rdf:resource="https://w3id.org/crmrp#c_f1c689bb"/>
    <skos:topConceptOf rdf:resource="https://w3id.org/crmrp#Execution_Technique"/>
    <rdf:type rdf:resource="http://www.w3.org/2004/02/skos/core#Concept"/>
    <skos:prefLabel xml:lang="it">Metalizzazione</skos:prefLabel>
    <skos:editorialNote xml:lang="it">C. Giannini, “Dizionario del restauro - Tecniche diagnostica conservazione”, Nardini Editore, Firenze, 2010</skos:editorialNote>
  </rdf:Description>
  <rdf:Description rdf:about="https://w3id.org/crmrp#c_abed88a5">
    <rdfs:label xml:lang="en">Microinvasive testing</rdfs:label>
    <skos:exactMatch rdf:resource="http://vocab.getty.edu/page/aat/300448614"/>
    <skos:prefLabel xml:lang="en">Microinvasive testing</skos:prefLabel>
    <skos:editorialNote xml:lang="en">Getty AAT http://vocab.getty.edu/page/aat/300448614</skos:editorialNote>
    <skos:topConceptOf rdf:resource="https://w3id.org/crmrp#Archeometric_and_Diagnostic_Analysis"/>
    <skos:prefLabel xml:lang="it">Indagine invasiva/microinvasiva</skos:prefLabel>
    <rdf:type rdf:resource="http://www.w3.org/2004/02/skos/core#Concept"/>
    <rdf:type rdf:resource="http://www.w3.org/2002/07/owl#NamedIndividual"/>
    <skos:definition xml:lang="en">Testing techniques that penetrate or alter the sample at a microscopic level.</skos:definition>
    <skos:inScheme rdf:resource="https://w3id.org/crmrp#Archeometric_and_Diagnostic_Analysis"/>
  </rdf:Description>
  <rdf:Description rdf:about="https://w3id.org/crmrp#c_269dfecc">
    <skos:closeMatch rdf:resource="http://vocab.getty.edu/page/aat/300195853"/>
    <rdf:type rdf:resource="http://www.w3.org/2004/02/skos/core#Concept"/>
    <rdfs:label xml:lang="en">Typography</rdfs:label>
    <skos:prefLabel xml:lang="it">Tipografia</skos:prefLabel>
    <rdf:type rdf:resource="http://www.w3.org/2002/07/owl#NamedIndividual"/>
    <skos:definition xml:lang="en">Various processes performed with type and typefaces, including setting type and creating layouts with type for printing. For the process of designing type used in the practice of typography, use type design.</skos:definition>
    <skos:editorialNote xml:lang="en">Getty AAT http://vocab.getty.edu/page/aat/300195853</skos:editorialNote>
    <skos:inScheme rdf:resource="https://w3id.org/crmrp#Execution_Technique"/>
    <skos:topConceptOf rdf:resource="https://w3id.org/crmrp#Execution_Technique"/>
    <skos:prefLabel xml:lang="en">Typography</skos:prefLabel>
    <skos:broader rdf:resource="https://w3id.org/crmrp#c_aee6a805"/>
  </rdf:Description>
  <rdf:Description rdf:about="https://w3id.org/crmrp#c_17ef6a5b">
    <skos:defintion xml:lang="en">Infrared photography technique commonly applied to a variety of techniques including aerial photography and art examination. False color infrared is preferred for vegetative and hydrologic studies. False color infrared film is sensitive to ultraviolet, visible and infrared radiation to approximately 900 nm. When the film is exposed with a yellow filter, the emulsion layers become sensitive to only green, red and infrared wavelengths. Blue radiation is absorbed by the filter; hence, the greater haze penetration ability of infrared film. In art conservation, the resulting false color images can be used as a noninvasive means of identifying the pigments that have been used in a painting or underdrawing.</skos:defintion>
    <skos:exactMatch rdf:resource="http://vocab.getty.edu/page/aat/300391245"/>
    <skos:inScheme rdf:resource="https://w3id.org/crmrp#Archeometric_and_Diagnostic_Analysis"/>
    <skos:prefLabel xml:lang="en">False-colour infrared photography</skos:prefLabel>
    <rdf:type rdf:resource="http://www.w3.org/2004/02/skos/core#Concept"/>
    <skos:editorialNote xml:lang="en">Getty AAT http://vocab.getty.edu/page/aat/300391245</skos:editorialNote>
    <skos:broader rdf:resource="https://w3id.org/crmrp#c_1fd6102e"/>
    <skos:topConceptOf rdf:resource="https://w3id.org/crmrp#Archeometric_and_Diagnostic_Analysis"/>
    <rdf:type rdf:resource="http://www.w3.org/2002/07/owl#NamedIndividual"/>
    <rdfs:label xml:lang="en">False-colour infrared photography</rdfs:label>
    <skos:prefLabel xml:lang="it">Falso colore</skos:prefLabel>
  </rdf:Description>
  <rdf:Description rdf:about="https://w3id.org/crmrp#c_bcebc1fb">
    <skos:closeMatch rdf:resource="http://vocab.getty.edu/page/aat/300053353"/>
    <rdfs:label xml:lang="en">Encausto</rdfs:label>
    <rdf:type rdf:resource="http://www.w3.org/2002/07/owl#NamedIndividual"/>
    <skos:prefLabel xml:lang="it">Encausto</skos:prefLabel>
    <skos:prefLabel xml:lang="en">Encausto</skos:prefLabel>
    <skos:editorialNote xml:lang="en">A. Weyer et al., “EwaGlos - European Illustrated Glossary of conservation terms for wall paintings and architectural surfaces”, Michael Imhof Verlag, Petersberg, Germany</skos:editorialNote>
    <skos:note xml:lang="en">The preferred editorial note and the definition closest to the meaning is EwaGlos - European Illustrated Glossary of conservation terms for wall paintings and architectural surfaces</skos:note>
    <skos:altLabel xml:lang="en">Encaustic painting</skos:altLabel>
    <skos:broader rdf:resource="https://w3id.org/crmrp#c_6626f18c"/>
    <rdf:type rdf:resource="http://www.w3.org/2004/02/skos/core#Concept"/>
    <skos:topConceptOf rdf:resource="https://w3id.org/crmrp#Execution_Technique"/>
    <skos:inScheme rdf:resource="https://w3id.org/crmrp#Execution_Technique"/>
    <skos:definition xml:lang="en">Painting technique using a heated mixture of pigments, molten wax and resin.</skos:definition>
    <skos:editorialNote xml:lang="en">AAT Getty http://vocab.getty.edu/page/aat/300053353</skos:editorialNote>
  </rdf:Description>
  <rdf:Description rdf:about="https://w3id.org/crmrp#c_4b4e8dc7">
    <skos:topConceptOf rdf:resource="https://w3id.org/crmrp#Archeometric_and_Diagnostic_Analysis"/>
    <rdf:type rdf:resource="http://www.w3.org/2002/07/owl#NamedIndividual"/>
    <skos:definition xml:lang="en">Specular light is light reflected from a surface on which a single ray is reflected in a single direction.</skos:definition>
    <skos:broader rdf:resource="https://w3id.org/crmrp#c_1fd6102e"/>
    <skos:prefLabel xml:lang="en">Specular light</skos:prefLabel>
    <rdf:type rdf:resource="http://www.w3.org/2004/02/skos/core#Concept"/>
    <skos:inScheme rdf:resource="https://w3id.org/crmrp#Archeometric_and_Diagnostic_Analysis"/>
    <skos:note xml:lang="en">International references could not be found</skos:note>
    <rdfs:label xml:lang="en">Specular light</rdfs:label>
    <skos:prefLabel xml:lang="it">Fotografia a luce speculare</skos:prefLabel>
  </rdf:Description>
  <rdf:Description rdf:about="http://www.w3.org/2004/02/skos/core#exactMatch">
    <rdf:type rdf:resource="http://www.w3.org/2002/07/owl#AnnotationProperty"/>
  </rdf:Description>
  <rdf:Description rdf:about="https://w3id.org/crmrp#c_46fa5a86">
    <skos:definition xml:lang="en">An iron alloy containing about 2 to 4% carbon and 1 to 3% silicon, having a high compressive strength but low tensile strength. Cast iron is manufactured by melting scrap iron or pig iron in a cupola that is in contact with the coal fuel, then casting the molten iron into a mold. A large range of building and decorative items are made of cast iron by pouring the molten metal into sand molds and then machining. It is inexpensive and easy to make. It was made in China by at least the 3rd century BCE; the technique for its production did not reach Europe until medieval times.</skos:definition>
    <skos:closeMatch rdf:resource="http://vocab.getty.edu/page/aat/300011004"/>
    <skos:topConceptOf rdf:resource="https://w3id.org/crmrp#Material"/>
    <skos:broader rdf:resource="https://w3id.org/crmrp#c_6407466f"/>
    <rdf:type rdf:resource="http://www.w3.org/2004/02/skos/core#Concept"/>
    <skos:inScheme rdf:resource="https://w3id.org/crmrp#Material"/>
    <rdfs:label xml:lang="en">Cast iron</rdfs:label>
    <rdf:type rdf:resource="http://www.w3.org/2002/07/owl#NamedIndividual"/>
    <skos:prefLabel xml:lang="it">Ghisa</skos:prefLabel>
    <skos:source xml:lang="en">Getty AAT http://vocab.getty.edu/page/aat/300011004</skos:source>
    <skos:prefLabel xml:lang="en">Cast iron</skos:prefLabel>
  </rdf:Description>
  <rdf:Description rdf:about="http://www.w3.org/2004/02/skos/core#inScheme">
    <rdf:type rdf:resource="http://www.w3.org/2002/07/owl#AnnotationProperty"/>
  </rdf:Description>
  <rdf:Description rdf:about="https://w3id.org/crmrp#c_f1c689bb">
    <rdf:type rdf:resource="http://www.w3.org/2004/02/skos/core#Concept"/>
    <rdfs:label xml:lang="en">Patinatura</rdfs:label>
    <skos:definition xml:lang="en">Any process by which an attempt is made to artificially impart a patina to objects, especially metal objects.</skos:definition>
    <skos:editorialNote xml:lang="it">A.Giuffredi “Formatura e fonderia”, Alinea editrice, Firenze, 2010</skos:editorialNote>
    <skos:note xml:lang="en">It was decided not to proceed with the English translation in order to avoid possible lexical errors and misunderstandings.The preferred editorial note and the definition closest to the meaning is Formatura e fonderia</skos:note>
    <skos:topConceptOf rdf:resource="https://w3id.org/crmrp#Execution_Technique"/>
    <rdf:type rdf:resource="http://www.w3.org/2002/07/owl#NamedIndividual"/>
    <skos:prefLabel xml:lang="it">Patinatura</skos:prefLabel>
    <skos:prefLabel xml:lang="en">Patinatura</skos:prefLabel>
    <skos:inScheme rdf:resource="https://w3id.org/crmrp#Execution_Technique"/>
    <skos:editorialNote xml:lang="it">C. Giannini, “Dizionario del restauro - Tecniche diagnostica conservazione”, Nardini Editore, Firenze, 2010</skos:editorialNote>
  </rdf:Description>
  <rdf:Description rdf:about="https://w3id.org/crmrp#R5_Source_and_Document">
    <rdfs:label xml:lang="en">Source and Document</rdfs:label>
    <rdfs:comment xml:lang="en">This class represents source and document related to an object.
Every restoration is accompanied by a huge amount of documents, such as projects or reports. Most of these are required by the Superintendencies to evaluate if the restoration works has been carried out with the respect for the artifacts and their history.
These documents can also help future restorers to know how restorations were carried out in the past or to understand how to operate on artworks with similar characteristics (such as materials or execution techniques).</rdfs:comment>
    <rdfs:subClassOf rdf:resource="http://www.cidoc-crm.org/cidoc-crm/E31_Document"/>
    <rdf:type rdf:resource="http://www.w3.org/2002/07/owl#Class"/>
  </rdf:Description>
  <rdf:Description rdf:about="https://w3id.org/crmrp#c_446c8061">
    <skos:prefLabel xml:lang="en">Stain</skos:prefLabel>
    <skos:note xml:lang="en">The preferred editorial note and the definition closest to the meaning is Uni Cen/Ts 17135:2021</skos:note>
    <skos:definition xml:lang="en">Area of change of colour.</skos:definition>
    <skos:closeMatch rdf:resource="http://vocab.getty.edu/page/aat/300379497"/>
    <skos:prefLabel xml:lang="it">Macchia</skos:prefLabel>
    <skos:editorialNote xml:lang="en">Getty AAT http://vocab.getty.edu/page/aat/300379497</skos:editorialNote>
    <skos:topConceptOf rdf:resource="https://w3id.org/crmrp#Alteration"/>
    <rdf:type rdf:resource="http://www.w3.org/2002/07/owl#NamedIndividual"/>
    <skos:editorialNote xml:lang="en">Uni Cen/Ts 17135:2021 - Conservation of cultural heritage. General terms and definitions</skos:editorialNote>
    <rdfs:label xml:lang="en">Stain</rdfs:label>
    <rdf:type rdf:resource="http://www.w3.org/2004/02/skos/core#Concept"/>
    <skos:inScheme rdf:resource="https://w3id.org/crmrp#Alteration"/>
  </rdf:Description>
  <rdf:Description rdf:about="https://w3id.org/crmrp#c_d342102c">
    <skos:topConceptOf rdf:resource="https://w3id.org/crmrp#Intervention"/>
    <skos:prefLabel xml:lang="it">Protezione</skos:prefLabel>
    <skos:prefLabel xml:lang="en">Protection</skos:prefLabel>
    <skos:inScheme rdf:resource="https://w3id.org/crmrp#Intervention"/>
    <skos:editorialNote xml:lang="it">C. Giannini, “Dizionario del restauro - Tecniche diagnostica conservazione”, Nardini Editore, Firenze, 2010</skos:editorialNote>
    <skos:definition xml:lang="en">Action involving the application of a film-forming substance applied in fluid form to the surface of an item; its task is to preserve the surface from contact with the environment.</skos:definition>
    <rdfs:label xml:lang="en">Protection</rdfs:label>
    <rdf:type rdf:resource="http://www.w3.org/2004/02/skos/core#Concept"/>
    <rdf:type rdf:resource="http://www.w3.org/2002/07/owl#NamedIndividual"/>
  </rdf:Description>
  <rdf:Description rdf:about="https://w3id.org/crmrp#c_aa16888d">
    <skos:inScheme rdf:resource="https://w3id.org/crmrp#Execution_Technique"/>
    <skos:broader rdf:resource="https://w3id.org/crmrp#c_77acfccf"/>
    <skos:prefLabel xml:lang="it">Tempera magra</skos:prefLabel>
    <skos:prefLabel xml:lang="en">Tempera magra</skos:prefLabel>
    <skos:editorialNote xml:lang="it">C. Giannini, “Dizionario del restauro - Tecniche diagnostica conservazione”, Nardini Editore, Firenze, 2010</skos:editorialNote>
    <rdf:type rdf:resource="http://www.w3.org/2002/07/owl#NamedIndividual"/>
    <skos:topConceptOf rdf:resource="https://w3id.org/crmrp#Execution_Technique"/>
    <rdfs:label xml:lang="en">Tempera magra</rdfs:label>
    <skos:note xml:lang="en">It was decided not to proceed with the English translation in order to avoid possible lexical errors and misunderstandings.</skos:note>
    <skos:definition xml:lang="en">Lean tempera is made from egg white, vegetable glues or substances derived from casein, and was used for painting without preparation. It is very sensitive to the aqueous medium.</skos:definition>
    <rdf:type rdf:resource="http://www.w3.org/2004/02/skos/core#Concept"/>
  </rdf:Description>
  <rdf:Description rdf:about="https://w3id.org/crmrp#c_b9a6a1c8">
    <skos:topConceptOf rdf:resource="https://w3id.org/crmrp#Execution_Technique"/>
    <skos:prefLabel xml:lang="it">Opus musivo</skos:prefLabel>
    <skos:prefLabel xml:lang="en">Mosaic technique</skos:prefLabel>
    <skos:note xml:lang="en">International references could not be found</skos:note>
    <skos:inScheme rdf:resource="https://w3id.org/crmrp#Execution_Technique"/>
    <skos:definition xml:lang="en">The different techniques to produce a mosaic, which vary according to the shape and size of the tiles.</skos:definition>
    <rdfs:label xml:lang="en">Mosaic technique</rdfs:label>
    <rdf:type rdf:resource="http://www.w3.org/2004/02/skos/core#Concept"/>
    <rdf:type rdf:resource="http://www.w3.org/2002/07/owl#NamedIndividual"/>
  </rdf:Description>
  <rdf:Description rdf:about="https://w3id.org/crmrp#c_e763e25d">
    <skos:prefLabel xml:lang="en">Efflorescence</skos:prefLabel>
    <skos:editorialNote xml:lang="en">A. Weyer et al., “EwaGlos - European Illustrated Glossary of conservation terms for wall paintings and architectural surfaces”, Michael Imhof Verlag, Petersberg, Germany</skos:editorialNote>
    <skos:inScheme rdf:resource="https://w3id.org/crmrp#Alteration"/>
    <skos:exactMatch rdf:resource="http://vocab.getty.edu/page/aat/300214748"/>
    <skos:editorialNote xml:lang="en">Getty Conservation Institute “Illustrated Glossary - Definitions of terms used for the graphic documentation of in situ floor mosaics”, “Mosaics In Situ Project”, Los Angeles, 2003</skos:editorialNote>
    <skos:definition xml:lang="en">Accumulation of salt crystals on the surface of an object</skos:definition>
    <skos:editorialNote xml:lang="en">Verg`es-Belmin et al., ICOMOS-ISCS: Illustrated glossary on stone deterioration patterns, vol. XV. Icomos International Council on Monuments and Sites, 2008</skos:editorialNote>
    <skos:topConceptOf rdf:resource="https://w3id.org/crmrp#Alteration"/>
    <rdfs:label xml:lang="en">Efflorescence</rdfs:label>
    <skos:editorialNote xml:lang="en">Getty AAT http://vocab.getty.edu/page/aat/300214748</skos:editorialNote>
    <skos:editorialNote xml:lang="en">Uni Cen/Ts 17135:2021 - Conservation of cultural heritage. General terms and definitions</skos:editorialNote>
    <skos:note xml:lang="en">The preferred editorial note and the definition closest to the meaning is Uni Cen/Ts 17135:2021</skos:note>
    <rdf:type rdf:resource="http://www.w3.org/2004/02/skos/core#Concept"/>
    <skos:prefLabel xml:lang="it">Efflorescenza</skos:prefLabel>
    <rdf:type rdf:resource="http://www.w3.org/2002/07/owl#NamedIndividual"/>
  </rdf:Description>
  <rdf:Description rdf:about="https://w3id.org/crmrp#c_00213896">
    <rdf:type rdf:resource="http://www.w3.org/2004/02/skos/core#Concept"/>
    <skos:inScheme rdf:resource="https://w3id.org/crmrp#Execution_Technique"/>
    <skos:prefLabel xml:lang="en">Satin finishing</skos:prefLabel>
    <rdfs:label xml:lang="en">Satin finishing</rdfs:label>
    <skos:note xml:lang="en">International references could not be found</skos:note>
    <skos:definition xml:lang="en">The final appearance is half-veined and can be achieved by passing the agate stone over the bolus before the leaf is applied.</skos:definition>
    <skos:broader rdf:resource="https://w3id.org/crmrp#c_757ed6ec"/>
    <skos:topConceptOf rdf:resource="https://w3id.org/crmrp#Execution_Technique"/>
    <skos:editorialNote xml:lang="it">G. Pignolo, “Effetti d’oro - Storia e tecnica della doratura nell’arte”, Editrice Compositori, Bologna, 2002</skos:editorialNote>
    <skos:prefLabel xml:lang="it">Satinatura</skos:prefLabel>
    <rdf:type rdf:resource="http://www.w3.org/2002/07/owl#NamedIndividual"/>
  </rdf:Description>
  <rdf:Description rdf:about="https://w3id.org/crmrp#c_5e406e4a">
    <skos:broader rdf:resource="https://w3id.org/crmrp#c_044b6056"/>
    <skos:prefLabel xml:lang="en">Charcoal</skos:prefLabel>
    <rdfs:label xml:lang="en">Charcoal</rdfs:label>
    <skos:closeMatch rdf:resource="http://vocab.getty.edu/page/aat/300012862"/>
    <skos:inScheme rdf:resource="https://w3id.org/crmrp#Execution_Technique"/>
    <skos:editorialNote xml:lang="en">Getty AAt http://vocab.getty.edu/page/aat/300012862</skos:editorialNote>
    <skos:topConceptOf rdf:resource="https://w3id.org/crmrp#Execution_Technique"/>
    <skos:definition xml:lang="en">A black, porous carbonaceous material comprising the carbon-containing residue from burned wood (e.g., willow, maple, beech, linden or plum) or other organic containing materials such as bone, plants or animals. It is used as a drawing material, for filtering liquids or air, and for other purposes.</skos:definition>
    <rdf:type rdf:resource="http://www.w3.org/2002/07/owl#NamedIndividual"/>
    <skos:prefLabel xml:lang="it">Carboncino</skos:prefLabel>
    <rdf:type rdf:resource="http://www.w3.org/2004/02/skos/core#Concept"/>
  </rdf:Description>
  <rdf:Description rdf:about="https://w3id.org/crmrp#c_f1966944">
    <rdf:type rdf:resource="http://www.w3.org/2004/02/skos/core#Concept"/>
    <skos:inScheme rdf:resource="https://w3id.org/crmrp#Intervention"/>
    <skos:definition xml:lang="en">Consolidation intervention involving the surface layers (the substrate) of the artwork.</skos:definition>
    <skos:broader rdf:resource="https://w3id.org/crmrp#c_b86776d0"/>
    <skos:topConceptOf rdf:resource="https://w3id.org/crmrp#Intervention"/>
    <rdfs:label xml:lang="en">Superficial consolidation</rdfs:label>
    <skos:prefLabel xml:lang="en">Superficial consolidation</skos:prefLabel>
    <skos:note xml:lang="en">International references could not be found</skos:note>
    <rdf:type rdf:resource="http://www.w3.org/2002/07/owl#NamedIndividual"/>
    <skos:prefLabel xml:lang="it">Consolidamento superficiale</skos:prefLabel>
  </rdf:Description>
  <rdf:Description rdf:about="https://w3id.org/crmrp#c_7db77b32">
    <skos:inScheme rdf:resource="https://w3id.org/crmrp#Archeometric_and_Diagnostic_Analysis"/>
    <rdf:type rdf:resource="http://www.w3.org/2002/07/owl#NamedIndividual"/>
    <skos:definition xml:lang="en">Techniques to photograph subjects that can be viewed only with the aid of a microscope or other magnifier</skos:definition>
    <rdf:type rdf:resource="http://www.w3.org/2004/02/skos/core#Concept"/>
    <skos:editorialNote xml:lang="en">Getty AAT http://vocab.getty.edu/page/aat/300053550</skos:editorialNote>
    <skos:closeMatch rdf:resource="http://vocab.getty.edu/page/aat/300053550"/>
    <skos:prefLabel xml:lang="en">Microphotography</skos:prefLabel>
    <skos:prefLabel xml:lang="it">Microfotografia</skos:prefLabel>
    <skos:broader rdf:resource="https://w3id.org/crmrp#c_1fd6102e"/>
    <skos:topConceptOf rdf:resource="https://w3id.org/crmrp#Archeometric_and_Diagnostic_Analysis"/>
    <rdfs:label xml:lang="en">Microphotography</rdfs:label>
  </rdf:Description>
  <rdf:Description rdf:about="https://w3id.org/crmrp#c_d999bf3e">
    <skos:prefLabel xml:lang="en">Analytical techniques of Fourier transform infrared spectroscopy (FTIR)</skos:prefLabel>
    <skos:definition xml:lang="en">Fourier transform infrared spectroscopy adapted for selective analysis of components of heterogeneous samples on a micrometer scale.</skos:definition>
    <skos:editorialNote xml:lang="en">Getty AAT http://vocab.getty.edu/page/aat/300391288</skos:editorialNote>
    <skos:broader rdf:resource="https://w3id.org/crmrp#c_789c3e32"/>
    <skos:topConceptOf rdf:resource="https://w3id.org/crmrp#Archeometric_and_Diagnostic_Analysis"/>
    <rdfs:label xml:lang="en">Analytical techniques of Fourier transform infrared spectroscopy (FTIR)</rdfs:label>
    <skos:inScheme rdf:resource="https://w3id.org/crmrp#Archeometric_and_Diagnostic_Analysis"/>
    <skos:closeMatch rdf:resource="http://vocab.getty.edu/page/aat/300391288"/>
    <rdf:type rdf:resource="http://www.w3.org/2004/02/skos/core#Concept"/>
    <rdf:type rdf:resource="http://www.w3.org/2002/07/owl#NamedIndividual"/>
    <skos:prefLabel xml:lang="it">Spettrofotometria infrarossa in trasformata di Fuorier (FTIR)</skos:prefLabel>
  </rdf:Description>
  <rdf:Description rdf:about="https://w3id.org/crmrp#c_847b008d">
    <skos:topConceptOf rdf:resource="https://w3id.org/crmrp#Intervention"/>
    <skos:prefLabel xml:lang="it">Applicazione su nuovo supporto</skos:prefLabel>
    <skos:prefLabel xml:lang="en">Transfer</skos:prefLabel>
    <skos:inScheme rdf:resource="https://w3id.org/crmrp#Intervention"/>
    <skos:editorialNote xml:lang="en">A. Weyer et al., “EwaGlos - European Illustrated Glossary of conservation terms for wall paintings and architectural surfaces”, Michael Imhof Verlag, Petersberg, Germany</skos:editorialNote>
    <skos:definition xml:lang="en">Adhesion of a detached wall painting or mosaic or painting to a new support replacing the original.</skos:definition>
    <rdfs:label xml:lang="en">Transfer</rdfs:label>
    <rdf:type rdf:resource="http://www.w3.org/2004/02/skos/core#Concept"/>
    <rdf:type rdf:resource="http://www.w3.org/2002/07/owl#NamedIndividual"/>
  </rdf:Description>
  <rdf:Description rdf:about="https://w3id.org/crmrp#c_40a6d4b1">
    <rdfs:label xml:lang="en">Steel</rdfs:label>
    <rdf:type rdf:resource="http://www.w3.org/2004/02/skos/core#Concept"/>
    <skos:prefLabel xml:lang="en">Steel</skos:prefLabel>
    <skos:inScheme rdf:resource="https://w3id.org/crmrp#Material"/>
    <skos:closeMatch rdf:resource="http://vocab.getty.edu/page/aat/300133751"/>
    <skos:topConceptOf rdf:resource="https://w3id.org/crmrp#Material"/>
    <rdf:type rdf:resource="http://www.w3.org/2002/07/owl#NamedIndividual"/>
    <skos:prefLabel xml:lang="it">Acciao</skos:prefLabel>
    <skos:editorialNote xml:lang="en">Getty AAT http://vocab.getty.edu/page/aat/300133751</skos:editorialNote>
    <skos:broader rdf:resource="https://w3id.org/crmrp#c_6407466f"/>
    <skos:definition xml:lang="en">Any of various hard, strong, durable, malleable alloys of iron and carbon, often with other elements such as manganese, chromium, nickel, molybdenum, copper, tungsten, cobalt, or silicon; widely used as a structural material.</skos:definition>
  </rdf:Description>
  <rdf:Description rdf:about="https://w3id.org/crmrp#c_977962bd">
    <rdf:type rdf:resource="http://www.w3.org/2004/02/skos/core#Concept"/>
    <skos:topConceptOf rdf:resource="https://w3id.org/crmrp#Material"/>
    <skos:exactMatch rdf:resource="http://vocab.getty.edu/page/aat/300133751"/>
    <rdfs:label xml:lang="en">Tin</rdfs:label>
    <skos:definition xml:lang="en">Pure metallic element having symbol Sn and atomic number 50; a soft, pliable, silvery white metal. Use also for this metal as processed and formed, usually in combination with other substances, to make various objects and materials.</skos:definition>
    <rdf:type rdf:resource="http://www.w3.org/2002/07/owl#NamedIndividual"/>
    <skos:broader rdf:resource="https://w3id.org/crmrp#c_6407466f"/>
    <skos:inScheme rdf:resource="https://w3id.org/crmrp#Material"/>
    <skos:prefLabel xml:lang="it">Stagno</skos:prefLabel>
    <skos:prefLabel xml:lang="en">Tin</skos:prefLabel>
    <skos:editorialNote xml:lang="en">Getty AAT http://vocab.getty.edu/page/aat/300133751</skos:editorialNote>
  </rdf:Description>
  <rdf:Description rdf:about="https://w3id.org/crmrp#c_789c3e32">
    <skos:prefLabel xml:lang="it">Spettroscopia</skos:prefLabel>
    <skos:topConceptOf rdf:resource="https://w3id.org/crmrp#Archeometric_and_Diagnostic_Analysis"/>
    <skos:closeMatch rdf:resource="http://vocab.getty.edu/page/aat/300179535"/>
    <rdf:type rdf:resource="http://www.w3.org/2004/02/skos/core#Concept"/>
    <skos:editorialNote xml:lang="en">Getty AAT http://vocab.getty.edu/page/aat/300179535</skos:editorialNote>
    <skos:definition xml:lang="en">Means of observing the way a substance transmits, emits, or responds to various wavelengths in the electromagnetic energy spectrum.</skos:definition>
    <skos:broader rdf:resource="https://w3id.org/crmrp#c_abed88a5"/>
    <skos:inScheme rdf:resource="https://w3id.org/crmrp#Archeometric_and_Diagnostic_Analysis"/>
    <skos:prefLabel xml:lang="en">Spectroscopy</skos:prefLabel>
    <rdf:type rdf:resource="http://www.w3.org/2002/07/owl#NamedIndividual"/>
    <rdfs:label xml:lang="en">Spectroscopy</rdfs:label>
  </rdf:Description>
  <rdf:Description rdf:about="https://w3id.org/crmrp#c_e7949d93">
    <skos:inScheme rdf:resource="https://w3id.org/crmrp#Material"/>
    <skos:definition xml:lang="en">A material comprising white clay, or kaolin, and a feldspathic rock, that react when fired so the clay serves to hold the shape of the object and the rock fuses into a natural glass. In China, it includes any such ware that is highly fired enough to produce a ringing sound when struck. In Europe, it is limited to hard-fired ceramic that is translucent.</skos:definition>
    <rdf:type rdf:resource="http://www.w3.org/2004/02/skos/core#Concept"/>
    <rdf:type rdf:resource="http://www.w3.org/2002/07/owl#NamedIndividual"/>
    <skos:prefLabel xml:lang="en">Porcelain</skos:prefLabel>
    <skos:editorialNote xml:lang="en">Getty AAT http://vocab.getty.edu/page/aat/300010662</skos:editorialNote>
    <skos:closeMatch rdf:resource="http://vocab.getty.edu/page/aat/300010662"/>
    <skos:topConceptOf rdf:resource="https://w3id.org/crmrp#Material"/>
    <skos:broader rdf:resource="https://w3id.org/crmrp#c_bd34e984"/>
    <rdfs:label xml:lang="en">Porcelain</rdfs:label>
    <skos:prefLabel xml:lang="it">Porcellana</skos:prefLabel>
  </rdf:Description>
  <rdf:Description rdf:about="https://w3id.org/crmrp#c_bd34e984">
    <skos:topConceptOf rdf:resource="https://w3id.org/crmrp#Material"/>
    <skos:prefLabel xml:lang="it">Ceramica</skos:prefLabel>
    <skos:prefLabel xml:lang="en">Ceramic</skos:prefLabel>
    <skos:inScheme rdf:resource="https://w3id.org/crmrp#Material"/>
    <skos:editorialNote xml:lang="en">A. Weyer et al., “EwaGlos - European Illustrated Glossary of conservation terms for wall paintings and architectural surfaces”, Michael Imhof Verlag, Petersberg, Germany</skos:editorialNote>
    <skos:definition xml:lang="en">A hard and brittle, heat- and corrosion-resistant material, made by shaping clay or similar earth materials and subsequently firing them at high temperatures.</skos:definition>
    <rdfs:label xml:lang="en">Ceramic</rdfs:label>
    <rdf:type rdf:resource="http://www.w3.org/2004/02/skos/core#Concept"/>
    <rdf:type rdf:resource="http://www.w3.org/2002/07/owl#NamedIndividual"/>
  </rdf:Description>
  <rdf:Description rdf:about="https://w3id.org/crmrp#c_3ef20257">
    <skos:closeMatch rdf:resource="http://vocab.getty.edu/page/aat/300219639"/>
    <skos:closeMatch rdf:resource="http://vocab.getty.edu/page/aat/300419379"/>
    <skos:altLabel xml:lang="en">Biodegradation</skos:altLabel>
    <rdf:type rdf:resource="http://www.w3.org/2002/07/owl#NamedIndividual"/>
    <skos:altLabel xml:lang="en">Microbiological organisms</skos:altLabel>
    <skos:editorialNote xml:lang="en">Getty Conservation Institute “Illustrated Glossary - Definitions of terms used for the graphic documentation of in situ floor mosaics”, “Mosaics In Situ Project”, Los Angeles, 2003</skos:editorialNote>
    <skos:prefLabel xml:lang="en">Biological colonisation</skos:prefLabel>
    <skos:editorialNote xml:lang="en"> A. Weyer et al., “EwaGlos - European Illustrated Glossary of conservation terms for wall paintings and architectural surfaces”, Michael Imhof Verlag, Petersberg, Germany</skos:editorialNote>
    <skos:editorialNote xml:lang="en">Getty AAT http://vocab.getty.edu/page/aat/300219639</skos:editorialNote>
    <skos:editorialNote xml:lang="en">Uni Cen/Ts 17135:2021 - Conservation of cultural heritage. General terms and definitions</skos:editorialNote>
    <rdf:type rdf:resource="http://www.w3.org/2004/02/skos/core#Concept"/>
    <skos:note xml:lang="en">The preferred editorial note and the definition closest to the meaning is Uni Cen/Ts 17135:2021</skos:note>
    <skos:prefLabel xml:lang="it">Colonizzazione biologica</skos:prefLabel>
    <rdfs:label xml:lang="en">Biological colonisation</rdfs:label>
    <skos:altLabel xml:lang="en">Biological growth</skos:altLabel>
    <skos:definition xml:lang="en">Growth of organisms on or within an object. Example: lichen, moss, plant, animals, microorganisms.</skos:definition>
    <skos:topConceptOf rdf:resource="https://w3id.org/crmrp#Alteration"/>
    <skos:altLabel xml:lang="en">Biodeterioration</skos:altLabel>
    <skos:inScheme rdf:resource="https://w3id.org/crmrp#Alteration"/>
    <skos:editorialNote xml:lang="en">Getty AAT http://vocab.getty.edu/page/aat/300419379</skos:editorialNote>
    <skos:editorialNote xml:lang="en">Verg`es-Belmin et al., ICOMOS-ISCS: Illustrated glossary on stone deterioration patterns, vol. XV. Icomos International Council on Monuments and Sites, 2008</skos:editorialNote>
  </rdf:Description>
  <rdf:Description rdf:about="https://w3id.org/crmrp#R8_Intervention">
    <rdfs:label xml:lang="en">Intervention</rdfs:label>
    <rdfs:comment xml:lang="en">This class indicates the individual intervention of restoration.</rdfs:comment>
    <rdfs:subClassOf rdf:resource="http://www.cidoc-crm.org/cidoc-crm/E7_Activity"/>
    <rdf:type rdf:resource="http://www.w3.org/2002/07/owl#Class"/>
  </rdf:Description>
  <rdf:Description rdf:about="https://w3id.org/crmrp#c_34d8fe56">
    <skos:prefLabel xml:lang="en">Stone</skos:prefLabel>
    <skos:topConceptOf rdf:resource="https://w3id.org/crmrp#Material"/>
    <skos:prefLabel xml:lang="it">Lapideo</skos:prefLabel>
    <rdfs:label xml:lang="en">Stone</rdfs:label>
    <skos:closeMatch rdf:resource="http://vocab.getty.edu/page/aat/300011176"/>
    <rdf:type rdf:resource="http://www.w3.org/2004/02/skos/core#Concept"/>
    <rdf:type rdf:resource="http://www.w3.org/2002/07/owl#NamedIndividual"/>
    <skos:inScheme rdf:resource="https://w3id.org/crmrp#Material"/>
    <skos:definition xml:lang="en">General term for rock that has been cut, shaped, crushed, or otherwise formed for use in construction or other purposes. Includes the specific archaeological and anthropological sense of individual stones which may be decorated or ornamented and which may be used in ritual contexts. These are usually not carved or dressed, and so differ from sculptures made from stone.</skos:definition>
    <skos:editorialNote xml:lang="en">Getty AAT http://vocab.getty.edu/page/aat/300011176</skos:editorialNote>
  </rdf:Description>
  <rdf:Description rdf:about="https://w3id.org/crmrp#c_66314288">
    <skos:definition xml:lang="en">A mould that allows multiple copies to be made because it does not need to be broken or modified during demoulding</skos:definition>
    <rdfs:label xml:lang="en">Stampo a buona forma</rdfs:label>
    <skos:prefLabel xml:lang="it">Stampo a buona forma</skos:prefLabel>
    <skos:prefLabel xml:lang="en">Stampo a buona forma</skos:prefLabel>
    <skos:editorialNote xml:lang="it">C. Giannini, “Dizionario del restauro - Tecniche diagnostica conservazione”, Nardini Editore, Firenze, 2010</skos:editorialNote>
    <rdf:type rdf:resource="http://www.w3.org/2004/02/skos/core#Concept"/>
    <rdf:type rdf:resource="http://www.w3.org/2002/07/owl#NamedIndividual"/>
    <skos:inScheme rdf:resource="https://w3id.org/crmrp#Execution_Technique"/>
    <skos:topConceptOf rdf:resource="https://w3id.org/crmrp#Execution_Technique"/>
    <skos:broader rdf:resource="https://w3id.org/crmrp#c_17157ccd"/>
    <skos:note xml:lang="en">It was decided not to proceed with the English translation in order to avoid possible lexical errors and misunderstandings.</skos:note>
    <skos:editorialNote xml:lang="it">P. Clérin, “Manuale di scultura - Tecniche, materiali, realizzazioni”, Sovera editore, Roma, 1995</skos:editorialNote>
  </rdf:Description>
  <rdf:Description rdf:about="https://w3id.org/crmrp#c_4ad9e448">
    <rdfs:label xml:lang="en">Incision</rdfs:label>
    <rdf:type rdf:resource="http://www.w3.org/2004/02/skos/core#Concept"/>
    <skos:prefLabel xml:lang="it">Incisione</skos:prefLabel>
    <rdf:type rdf:resource="http://www.w3.org/2002/07/owl#NamedIndividual"/>
    <skos:prefLabel xml:lang="en">Incision</skos:prefLabel>
    <skos:topConceptOf rdf:resource="https://w3id.org/crmrp#Alteration"/>
    <skos:definition xml:lang="en">Separation with sharply defined edges limited to a part of the thickness of the material</skos:definition>
    <skos:editorialNote xml:lang="en">Uni Cen/Ts 17135:2021 - Conservation of cultural heritage. General terms and definitions</skos:editorialNote>
    <skos:inScheme rdf:resource="https://w3id.org/crmrp#Alteration"/>
    <skos:altLabel xml:lang="en">Engraving</skos:altLabel>
    <skos:note xml:lang="en">The preferred editorial note and the definition closest to the meaning is Uni Cen/Ts 17135:2021</skos:note>
    <skos:editorialNote xml:lang="en">Verg`es-Belmin et al., ICOMOS-ISCS: Illustrated glossary on stone deterioration patterns, vol. XV. Icomos International Council on Monuments and Sites, 2008</skos:editorialNote>
  </rdf:Description>
  <rdf:Description rdf:about="https://w3id.org/crmrp#c_0b943779">
    <skos:topConceptOf rdf:resource="https://w3id.org/crmrp#Execution_Technique"/>
    <skos:definition xml:lang="en">Pavement made of ceramic elements, usually of the same size and rectangular shape, arranged in a herringbone pattern.</skos:definition>
    <rdf:type rdf:resource="http://www.w3.org/2004/02/skos/core#Concept"/>
    <rdfs:label xml:lang="en">Opus spicatum</rdfs:label>
    <skos:prefLabel xml:lang="en">Opus spicatum</skos:prefLabel>
    <rdf:type rdf:resource="http://www.w3.org/2002/07/owl#NamedIndividual"/>
    <skos:prefLabel xml:lang="it">Opus spicatum</skos:prefLabel>
    <skos:editorialNote xml:lang="en">Getty Conservation Institute “Illustrated Glossary - Technician Training for the Maintenance of In Situ Mosaics”, Los Angeles, 2013</skos:editorialNote>
    <skos:broader rdf:resource="https://w3id.org/crmrp#c_b9a6a1c8"/>
    <skos:inScheme rdf:resource="https://w3id.org/crmrp#Execution_Technique"/>
  </rdf:Description>
</rdf:RDF>
